@prefix rdf: <http://www.w3.org/1999/02/22-rdf-syntax-ns#> .
@prefix dc: <http://purl.org/dc/elements/1.1/> .
@prefix foaf: <http://xmlns.com/foaf/0.1/> .
@prefix owl: <http://www.w3.org/2002/07/owl#> .
@prefix rdfs: <http://www.w3.org/2000/01/rdf-schema#> .
@prefix reg: <http://metadataregistry.org/uri/profile/regap/> .
@prefix skos: <http://www.w3.org/2004/02/skos/core#> .

<http://metadataregistry.org/uri/RegStatus/1001>
    a skos:Concept ;
    skos:prefLabel "Published"@en .

<http://metadataregistry.org/uri/RegStatus/1008>
    a skos:Concept ;
    skos:prefLabel "Deprecated"@en .

<http://rdaregistry.info/Elements/u/>
    dc:title "RDA Unconstrained properties"@en ;
    skos:note "Properties derived from RDA elements and relationship designators without specific or implicit restrictions to RDA entities."@en ;
    foaf:homepage <http://www.rdaregistry.info/Elements/u/> .

<http://rdaregistry.info/Elements/u/P60001>
    reg:hasSubproperty <http://rdaregistry.info/Elements/a/P50001> ;
    reg:lexicalAlias <http://rdaregistry.info/Elements/u/respondentOf.en> ;
    reg:name "respondentOf"@en ;
    reg:status <http://metadataregistry.org/uri/RegStatus/1001> ;
    a rdf:Property ;
    rdfs:isDefinedBy <http://rdaregistry.info/Elements/u/> ;
    rdfs:label "is respondent of"@en ;
    rdfs:subPropertyOf <http://rdaregistry.info/Elements/u/P60672> ;
    owl:inverseOf <http://rdaregistry.info/Elements/u/P60045> ;
    skos:definition "Relates a candidate for a degree who defends or opposes a thesis provided by the praeses in an academic disputation to the resource."@en .

<http://rdaregistry.info/Elements/u/P60002>
    reg:hasSubproperty <http://rdaregistry.info/Elements/a/P50003> ;
    reg:lexicalAlias <http://rdaregistry.info/Elements/u/degreeGrantingInstitutionOf.en> ;
    reg:name "degreeGrantingInstitutionOf"@en ;
    reg:status <http://metadataregistry.org/uri/RegStatus/1001> ;
    a rdf:Property ;
    rdfs:isDefinedBy <http://rdaregistry.info/Elements/u/> ;
    rdfs:label "is degree granting institution of"@en ;
    rdfs:subPropertyOf <http://rdaregistry.info/Elements/u/P60602> ;
    owl:inverseOf <http://rdaregistry.info/Elements/u/P60060> ;
    skos:definition "Relates a corporate body granting an academic degree to the resource."@en .

<http://rdaregistry.info/Elements/u/P60003>
    reg:hasSubproperty <http://rdaregistry.info/Elements/a/P50004> ;
    reg:lexicalAlias <http://rdaregistry.info/Elements/u/hostInstitutionOf.en> ;
    reg:name "hostInstitutionOf"@en ;
    reg:status <http://metadataregistry.org/uri/RegStatus/1001> ;
    a rdf:Property ;
    rdfs:isDefinedBy <http://rdaregistry.info/Elements/u/> ;
    rdfs:label "is host institution of"@en ;
    rdfs:subPropertyOf <http://rdaregistry.info/Elements/u/P60602> ;
    owl:inverseOf <http://rdaregistry.info/Elements/u/P60061> ;
    skos:definition "Relates a corporate body hosting the event, exhibit, conference, etc., which gave rise to a resource, but having little or no responsibility for the content of the resource to the resource."@en .

<http://rdaregistry.info/Elements/u/P60004>
    reg:hasSubproperty <http://rdaregistry.info/Elements/a/P50005> ;
    reg:lexicalAlias <http://rdaregistry.info/Elements/u/productionCompanyOf.en> ;
    reg:name "productionCompanyOf"@en ;
    reg:status <http://metadataregistry.org/uri/RegStatus/1001> ;
    a rdf:Property ;
    rdfs:isDefinedBy <http://rdaregistry.info/Elements/u/> ;
    rdfs:label "is production company of"@en ;
    rdfs:subPropertyOf <http://rdaregistry.info/Elements/u/P60602> ;
    owl:inverseOf <http://rdaregistry.info/Elements/u/P60062> ;
    skos:definition "Relates a corporate body that is responsible for financial, technical, and organizational management of a production for stage, screen, sound recording, television, webcast, etc. to the resource."@en .

<http://rdaregistry.info/Elements/u/P60005>
    reg:hasSubproperty <http://rdaregistry.info/Elements/a/P50044> ;
    reg:lexicalAlias <http://rdaregistry.info/Elements/u/courtGovernedOf.en> ;
    reg:name "courtGovernedOf"@en ;
    reg:status <http://metadataregistry.org/uri/RegStatus/1001> ;
    a rdf:Property ;
    rdfs:isDefinedBy <http://rdaregistry.info/Elements/u/> ;
    rdfs:label "is court governed of"@en ;
    rdfs:subPropertyOf <http://rdaregistry.info/Elements/u/P60602> ;
    owl:inverseOf <http://rdaregistry.info/Elements/u/P60065> ;
    skos:definition "Relates a court governed by court rules, regardless of their official nature (e.g., laws, administrative regulations) to the resource."@en .

<http://rdaregistry.info/Elements/u/P60006>
    reg:hasSubproperty <http://rdaregistry.info/Elements/a/P50045> ;
    reg:lexicalAlias <http://rdaregistry.info/Elements/u/collectorOf.en> ;
    reg:name "collectorOf"@en ;
    reg:status <http://metadataregistry.org/uri/RegStatus/1001> ;
    a rdf:Property ;
    rdfs:isDefinedBy <http://rdaregistry.info/Elements/u/> ;
    rdfs:label "is collector of"@en ;
    rdfs:subPropertyOf <http://rdaregistry.info/Elements/u/P60604> ;
    owl:inverseOf <http://rdaregistry.info/Elements/u/P60066> ;
    skos:definition "Relates a curator who brings together resources from various sources that are then arranged, described, and cataloged as a collection to the resource."@en .

<http://rdaregistry.info/Elements/u/P60007>
    reg:hasSubproperty <http://rdaregistry.info/Elements/a/P50046> ;
    reg:lexicalAlias <http://rdaregistry.info/Elements/u/collectionRegistrarOf.en> ;
    reg:name "collectionRegistrarOf"@en ;
    reg:status <http://metadataregistry.org/uri/RegStatus/1001> ;
    a rdf:Property ;
    rdfs:isDefinedBy <http://rdaregistry.info/Elements/u/> ;
    rdfs:label "is collection registrar of"@en ;
    rdfs:subPropertyOf <http://rdaregistry.info/Elements/u/P60604> ;
    owl:inverseOf <http://rdaregistry.info/Elements/u/P60067> ;
    skos:definition "Relates a curator who lists or inventories the items in an aggregate resource such as a collection of items or resources to the resource."@en .

<http://rdaregistry.info/Elements/u/P60008>
    reg:hasSubproperty <http://rdaregistry.info/Elements/a/P50047> ;
    reg:lexicalAlias <http://rdaregistry.info/Elements/u/depositorOf.en> ;
    reg:name "depositorOf"@en ;
    reg:status <http://metadataregistry.org/uri/RegStatus/1001> ;
    a rdf:Property ;
    rdfs:isDefinedBy <http://rdaregistry.info/Elements/u/> ;
    rdfs:label "is depositor of"@en ;
    rdfs:subPropertyOf <http://rdaregistry.info/Elements/u/P60628> ;
    owl:inverseOf <http://rdaregistry.info/Elements/u/P60068> ;
    skos:definition "Relates a current owner of a resource who deposited the resource into the custody of another person, family, or corporate body, while still retaining ownership to the resource."@en .

<http://rdaregistry.info/Elements/u/P60009>
    reg:hasSubproperty <http://rdaregistry.info/Elements/a/P50048> ;
    reg:lexicalAlias <http://rdaregistry.info/Elements/u/filmDirectorOf.en> ;
    reg:name "filmDirectorOf"@en ;
    reg:status <http://metadataregistry.org/uri/RegStatus/1001> ;
    a rdf:Property ;
    rdfs:isDefinedBy <http://rdaregistry.info/Elements/u/> ;
    rdfs:label "is film director of"@en ;
    rdfs:subPropertyOf <http://rdaregistry.info/Elements/u/P60673> ;
    owl:inverseOf <http://rdaregistry.info/Elements/u/P60084> ;
    skos:definition "Relates a director responsible for the general management and supervision of a filmed performance to the resource."@en .

<http://rdaregistry.info/Elements/u/P60010>
    reg:hasSubproperty <http://rdaregistry.info/Elements/a/P50049> ;
    reg:lexicalAlias <http://rdaregistry.info/Elements/u/radioDirectorOf.en> ;
    reg:name "radioDirectorOf"@en ;
    reg:status <http://metadataregistry.org/uri/RegStatus/1001> ;
    a rdf:Property ;
    rdfs:isDefinedBy <http://rdaregistry.info/Elements/u/> ;
    rdfs:label "is radio director of"@en ;
    rdfs:subPropertyOf <http://rdaregistry.info/Elements/u/P60673> ;
    owl:inverseOf <http://rdaregistry.info/Elements/u/P60085> ;
    skos:definition "Relates a director responsible for the general management and supervision of a radio program to the resource."@en .

<http://rdaregistry.info/Elements/u/P60011>
    reg:hasSubproperty <http://rdaregistry.info/Elements/a/P50050> ;
    reg:lexicalAlias <http://rdaregistry.info/Elements/u/televisionDirectorOf.en> ;
    reg:name "televisionDirectorOf"@en ;
    reg:status <http://metadataregistry.org/uri/RegStatus/1001> ;
    a rdf:Property ;
    rdfs:isDefinedBy <http://rdaregistry.info/Elements/u/> ;
    rdfs:label "is television director of"@en ;
    rdfs:subPropertyOf <http://rdaregistry.info/Elements/u/P60673> ;
    owl:inverseOf <http://rdaregistry.info/Elements/u/P60086> ;
    skos:definition "Relates a director responsible for the general management and supervision of a television program to the resource."@en .

<http://rdaregistry.info/Elements/u/P60012>
    reg:hasSubproperty <http://rdaregistry.info/Elements/a/P50066> ;
    reg:lexicalAlias <http://rdaregistry.info/Elements/u/donorOf.en> ;
    reg:name "donorOf"@en ;
    reg:status <http://metadataregistry.org/uri/RegStatus/1001> ;
    a rdf:Property ;
    rdfs:isDefinedBy <http://rdaregistry.info/Elements/u/> ;
    rdfs:label "is donor of"@en ;
    rdfs:subPropertyOf <http://rdaregistry.info/Elements/u/P60630> ;
    owl:inverseOf <http://rdaregistry.info/Elements/u/P60091> ;
    skos:definition "Relates a former owner of a resource who donated that resource to another owner to the resource."@en .

<http://rdaregistry.info/Elements/u/P60013>
    reg:hasSubproperty <http://rdaregistry.info/Elements/a/P50067> ;
    reg:lexicalAlias <http://rdaregistry.info/Elements/u/sellerOf.en> ;
    reg:name "sellerOf"@en ;
    reg:status <http://metadataregistry.org/uri/RegStatus/1001> ;
    a rdf:Property ;
    rdfs:isDefinedBy <http://rdaregistry.info/Elements/u/> ;
    rdfs:label "is seller of"@en ;
    rdfs:subPropertyOf <http://rdaregistry.info/Elements/u/P60630> ;
    owl:inverseOf <http://rdaregistry.info/Elements/u/P60092> ;
    skos:definition "Relates a former owner of a resource who sold that resource to another owner to the resource."@en .

<http://rdaregistry.info/Elements/u/P60014>
    reg:hasSubproperty <http://rdaregistry.info/Elements/a/P50068> ;
    reg:lexicalAlias <http://rdaregistry.info/Elements/u/enactingJurisdictionOf.en> ;
    reg:name "enactingJurisdictionOf"@en ;
    reg:status <http://metadataregistry.org/uri/RegStatus/1001> ;
    a rdf:Property ;
    rdfs:isDefinedBy <http://rdaregistry.info/Elements/u/> ;
    rdfs:label "is enacting jurisdiction of"@en ;
    rdfs:subPropertyOf <http://rdaregistry.info/Elements/u/P60672> ;
    owl:inverseOf <http://rdaregistry.info/Elements/u/P60096> ;
    skos:definition "Relates a jurisdiction enacting a law, regulation, constitution, court rule, etc. to the resource."@en .

<http://rdaregistry.info/Elements/u/P60015>
    reg:hasSubproperty <http://rdaregistry.info/Elements/a/P50069> ;
    reg:lexicalAlias <http://rdaregistry.info/Elements/u/jurisdictionGovernedOf.en> ;
    reg:name "jurisdictionGovernedOf"@en ;
    reg:status <http://metadataregistry.org/uri/RegStatus/1001> ;
    a rdf:Property ;
    rdfs:isDefinedBy <http://rdaregistry.info/Elements/u/> ;
    rdfs:label "is jurisdiction governed of"@en ;
    rdfs:subPropertyOf <http://rdaregistry.info/Elements/u/P60602> ;
    owl:inverseOf <http://rdaregistry.info/Elements/u/P60097> ;
    skos:definition "Relates a jurisdiction governed by a law, regulation, etc., that was enacted by another jurisdiction to the resource."@en .

<http://rdaregistry.info/Elements/u/P60016>
    reg:hasSubproperty <http://rdaregistry.info/Elements/a/P50070>, <http://rdaregistry.info/Elements/u/P60843>, <http://rdaregistry.info/Elements/u/P60845> ;
    reg:lexicalAlias <http://rdaregistry.info/Elements/u/conductorOf.en> ;
    reg:name "conductorOf"@en ;
    reg:status <http://metadataregistry.org/uri/RegStatus/1001> ;
    a rdf:Property ;
    rdfs:isDefinedBy <http://rdaregistry.info/Elements/u/> ;
    rdfs:label "is conductor of"@en ;
    rdfs:subPropertyOf <http://rdaregistry.info/Elements/u/P60615> ;
    owl:inverseOf <http://rdaregistry.info/Elements/u/P60141> ;
    skos:definition "Relates a performer contributing to a musical resource by leading a performing group (orchestra, chorus, opera, etc.) in a musical or dramatic presentation, etc. to the resource."@en .

<http://rdaregistry.info/Elements/u/P60017>
    reg:hasSubproperty <http://rdaregistry.info/Elements/a/P50071>, <http://rdaregistry.info/Elements/u/P60027> ;
    reg:lexicalAlias <http://rdaregistry.info/Elements/u/actorOf.en> ;
    reg:name "actorOf"@en ;
    reg:status <http://metadataregistry.org/uri/RegStatus/1001> ;
    a rdf:Property ;
    rdfs:isDefinedBy <http://rdaregistry.info/Elements/u/> ;
    rdfs:label "is actor of"@en ;
    rdfs:subPropertyOf <http://rdaregistry.info/Elements/u/P60615> ;
    owl:inverseOf <http://rdaregistry.info/Elements/u/P60142> ;
    skos:definition "Relates a performer contributing to a resource by acting as a cast member or player in a musical or dramatic presentation, etc. to the resource."@en .

<http://rdaregistry.info/Elements/u/P60018>
    reg:hasSubproperty <http://rdaregistry.info/Elements/a/P50072> ;
    reg:lexicalAlias <http://rdaregistry.info/Elements/u/onScreenPresenterOf.en> ;
    reg:name "onScreenPresenterOf"@en ;
    reg:status <http://metadataregistry.org/uri/RegStatus/1001> ;
    a rdf:Property ;
    rdfs:isDefinedBy <http://rdaregistry.info/Elements/u/> ;
    rdfs:label "is on-screen presenter of"@en ;
    rdfs:subPropertyOf <http://rdaregistry.info/Elements/u/P60615> ;
    owl:inverseOf <http://rdaregistry.info/Elements/u/P60143> ;
    skos:definition "Relates a performer contributing to a resource by appearing on screen to provide contextual or background information. an on-screen presenter may appear in nonfiction moving image materials or in introductions to fiction moving image materials to the resource."@en .

<http://rdaregistry.info/Elements/u/P60019>
    reg:hasSubproperty <http://rdaregistry.info/Elements/a/P50073> ;
    reg:lexicalAlias <http://rdaregistry.info/Elements/u/dancerOf.en> ;
    reg:name "dancerOf"@en ;
    reg:status <http://metadataregistry.org/uri/RegStatus/1001> ;
    a rdf:Property ;
    rdfs:isDefinedBy <http://rdaregistry.info/Elements/u/> ;
    rdfs:label "is dancer of"@en ;
    rdfs:subPropertyOf <http://rdaregistry.info/Elements/u/P60615> ;
    owl:inverseOf <http://rdaregistry.info/Elements/u/P60144> ;
    skos:definition "Relates a performer contributing to a resource by dancing in a musical, dramatic, etc., presentation to the resource."@en .

<http://rdaregistry.info/Elements/u/P60020>
    reg:hasSubproperty <http://rdaregistry.info/Elements/a/P50074> ;
    reg:lexicalAlias <http://rdaregistry.info/Elements/u/teacherOf.en> ;
    reg:name "teacherOf"@en ;
    reg:status <http://metadataregistry.org/uri/RegStatus/1001> ;
    a rdf:Property ;
    rdfs:isDefinedBy <http://rdaregistry.info/Elements/u/> ;
    rdfs:label "is teacher of"@en ;
    rdfs:subPropertyOf <http://rdaregistry.info/Elements/u/P60615> ;
    owl:inverseOf <http://rdaregistry.info/Elements/u/P60145> ;
    skos:definition "Relates a performer contributing to a resource by giving instruction or providing a demonstration to the resource."@en .

<http://rdaregistry.info/Elements/u/P60021>
    reg:hasSubproperty <http://rdaregistry.info/Elements/a/P50075> ;
    reg:lexicalAlias <http://rdaregistry.info/Elements/u/hostOf.en> ;
    reg:name "hostOf"@en ;
    reg:status <http://metadataregistry.org/uri/RegStatus/1001> ;
    a rdf:Property ;
    rdfs:isDefinedBy <http://rdaregistry.info/Elements/u/> ;
    rdfs:label "is host of"@en ;
    rdfs:subPropertyOf <http://rdaregistry.info/Elements/u/P60615> ;
    owl:inverseOf <http://rdaregistry.info/Elements/u/P60146> ;
    skos:definition "Relates a performer contributing to a resource by leading a program (often broadcast) that includes other guests, performers, etc. (e.g., talk show host) to the resource."@en .

<http://rdaregistry.info/Elements/u/P60022>
    reg:hasSubproperty <http://rdaregistry.info/Elements/a/P50076> ;
    reg:lexicalAlias <http://rdaregistry.info/Elements/u/moderatorOf.en> ;
    reg:name "moderatorOf"@en ;
    reg:status <http://metadataregistry.org/uri/RegStatus/1001> ;
    a rdf:Property ;
    rdfs:isDefinedBy <http://rdaregistry.info/Elements/u/> ;
    rdfs:label "is moderator of"@en ;
    rdfs:subPropertyOf <http://rdaregistry.info/Elements/u/P60615> ;
    owl:inverseOf <http://rdaregistry.info/Elements/u/P60147> ;
    skos:definition "Relates a performer contributing to a resource by leading a program (often broadcast) where topics are discussed, usually with participation of experts in fields related to the discussion to the resource."@en .

<http://rdaregistry.info/Elements/u/P60023>
    reg:hasSubproperty <http://rdaregistry.info/Elements/a/P50077> ;
    reg:lexicalAlias <http://rdaregistry.info/Elements/u/puppeteerOf.en> ;
    reg:name "puppeteerOf"@en ;
    reg:status <http://metadataregistry.org/uri/RegStatus/1001> ;
    a rdf:Property ;
    rdfs:isDefinedBy <http://rdaregistry.info/Elements/u/> ;
    rdfs:label "is puppeteer of"@en ;
    rdfs:subPropertyOf <http://rdaregistry.info/Elements/u/P60615> ;
    owl:inverseOf <http://rdaregistry.info/Elements/u/P60148> ;
    skos:definition "Relates a performer contributing to a resource by manipulating, controlling, or directing puppets or marionettes in a moving image production or a musical or dramatic presentation or entertainment to the resource."@en .

<http://rdaregistry.info/Elements/u/P60024>
    reg:hasSubproperty <http://rdaregistry.info/Elements/a/P50078> ;
    reg:lexicalAlias <http://rdaregistry.info/Elements/u/panelistOf.en> ;
    reg:name "panelistOf"@en ;
    reg:status <http://metadataregistry.org/uri/RegStatus/1001> ;
    a rdf:Property ;
    rdfs:isDefinedBy <http://rdaregistry.info/Elements/u/> ;
    rdfs:label "is panelist of"@en ;
    rdfs:subPropertyOf <http://rdaregistry.info/Elements/u/P60615> ;
    owl:inverseOf <http://rdaregistry.info/Elements/u/P60149> ;
    skos:definition "Relates a performer contributing to a resource by participating in a program (often broadcast) where topics are discussed, usually with participation of experts in fields related to the discussion to the resource."@en .

<http://rdaregistry.info/Elements/u/P60025>
    reg:hasSubproperty <http://rdaregistry.info/Elements/a/P50079> ;
    reg:lexicalAlias <http://rdaregistry.info/Elements/u/instrumentalistOf.en> ;
    reg:name "instrumentalistOf"@en ;
    reg:status <http://metadataregistry.org/uri/RegStatus/1001> ;
    a rdf:Property ;
    rdfs:isDefinedBy <http://rdaregistry.info/Elements/u/> ;
    rdfs:label "is instrumentalist of"@en ;
    rdfs:subPropertyOf <http://rdaregistry.info/Elements/u/P60615> ;
    owl:inverseOf <http://rdaregistry.info/Elements/u/P60150> ;
    skos:definition "Relates a performer contributing to a resource by playing a musical instrument to the resource."@en .

<http://rdaregistry.info/Elements/u/P60026>
    reg:hasSubproperty <http://rdaregistry.info/Elements/a/P50080> ;
    reg:lexicalAlias <http://rdaregistry.info/Elements/u/commentatorOf.en> ;
    reg:name "commentatorOf"@en ;
    reg:status <http://metadataregistry.org/uri/RegStatus/1001> ;
    a rdf:Property ;
    rdfs:isDefinedBy <http://rdaregistry.info/Elements/u/> ;
    rdfs:label "is commentator of"@en ;
    rdfs:subPropertyOf <http://rdaregistry.info/Elements/u/P60615> ;
    owl:inverseOf <http://rdaregistry.info/Elements/u/P60151> ;
    skos:definition "Relates a performer contributing to a resource by providing interpretation, analysis, or a discussion of the subject matter on a recording, film, or other audiovisual medium to the resource."@en .

<http://rdaregistry.info/Elements/u/P60027>
    reg:hasSubproperty <http://rdaregistry.info/Elements/a/P50217> ;
    reg:lexicalAlias <http://rdaregistry.info/Elements/u/voiceActorOf.en> ;
    reg:name "voiceActorOf"@en ;
    reg:status <http://metadataregistry.org/uri/RegStatus/1001> ;
    a rdf:Property ;
    rdfs:isDefinedBy <http://rdaregistry.info/Elements/u/> ;
    rdfs:label "is voice actor of"@en ;
    rdfs:subPropertyOf <http://rdaregistry.info/Elements/u/P60017> ;
    owl:inverseOf <http://rdaregistry.info/Elements/u/P60152> ;
    skos:definition "Relates a performer contributing to a resource by providing the voice for characters in radio and audio productions and for animated characters in moving image resources as well as by providing voice-overs in radio and television commercials, dubbed resources, etc. to the resource."@en .

<http://rdaregistry.info/Elements/u/P60028>
    reg:hasSubproperty <http://rdaregistry.info/Elements/a/P50081> ;
    reg:lexicalAlias <http://rdaregistry.info/Elements/u/narratorOf.en> ;
    reg:name "narratorOf"@en ;
    reg:status <http://metadataregistry.org/uri/RegStatus/1001> ;
    a rdf:Property ;
    rdfs:isDefinedBy <http://rdaregistry.info/Elements/u/> ;
    rdfs:label "is narrator of"@en ;
    rdfs:subPropertyOf <http://rdaregistry.info/Elements/u/P60615> ;
    owl:inverseOf <http://rdaregistry.info/Elements/u/P60153> ;
    skos:definition "Relates a performer contributing to a resource by reading aloud or giving an account of an act, occurrence, course of events, etc. to the resource."@en .

<http://rdaregistry.info/Elements/u/P60029>
    reg:hasSubproperty <http://rdaregistry.info/Elements/a/P50082> ;
    reg:lexicalAlias <http://rdaregistry.info/Elements/u/storytellerOf.en> ;
    reg:name "storytellerOf"@en ;
    reg:status <http://metadataregistry.org/uri/RegStatus/1001> ;
    a rdf:Property ;
    rdfs:isDefinedBy <http://rdaregistry.info/Elements/u/> ;
    rdfs:label "is storyteller of"@en ;
    rdfs:subPropertyOf <http://rdaregistry.info/Elements/u/P60615> ;
    owl:inverseOf <http://rdaregistry.info/Elements/u/P60154> ;
    skos:definition "Relates a performer contributing to a resource by relaying a creator's original story with dramatic or theatrical interpretation to the resource."@en .

<http://rdaregistry.info/Elements/u/P60030>
    reg:hasSubproperty <http://rdaregistry.info/Elements/a/P50083> ;
    reg:lexicalAlias <http://rdaregistry.info/Elements/u/speakerOf.en> ;
    reg:name "speakerOf"@en ;
    reg:status <http://metadataregistry.org/uri/RegStatus/1001> ;
    a rdf:Property ;
    rdfs:isDefinedBy <http://rdaregistry.info/Elements/u/> ;
    rdfs:label "is speaker of"@en ;
    rdfs:subPropertyOf <http://rdaregistry.info/Elements/u/P60615> ;
    owl:inverseOf <http://rdaregistry.info/Elements/u/P60155> ;
    skos:definition "Relates a performer contributing to a resource by speaking words, such as a lecture, speech, etc. to the resource."@en .

<http://rdaregistry.info/Elements/u/P60031>
    reg:hasSubproperty <http://rdaregistry.info/Elements/a/P50084> ;
    reg:lexicalAlias <http://rdaregistry.info/Elements/u/singerOf.en> ;
    reg:name "singerOf"@en ;
    reg:status <http://metadataregistry.org/uri/RegStatus/1001> ;
    a rdf:Property ;
    rdfs:isDefinedBy <http://rdaregistry.info/Elements/u/> ;
    rdfs:label "is singer of"@en ;
    rdfs:subPropertyOf <http://rdaregistry.info/Elements/u/P60615> ;
    owl:inverseOf <http://rdaregistry.info/Elements/u/P60156> ;
    skos:definition "Relates a performer contributing to a resource by using his/her/their voice, with or without instrumental accompaniment, to produce music. a singer's performance may or may not include actual words to the resource."@en .

<http://rdaregistry.info/Elements/u/P60032>
    reg:hasSubproperty <http://rdaregistry.info/Elements/a/P50086> ;
    reg:lexicalAlias <http://rdaregistry.info/Elements/u/mediumOf.en> ;
    reg:name "mediumOf"@en ;
    reg:status <http://metadataregistry.org/uri/RegStatus/1001> ;
    a rdf:Property ;
    rdfs:isDefinedBy <http://rdaregistry.info/Elements/u/> ;
    rdfs:label "is medium of"@en ;
    rdfs:subPropertyOf <http://rdaregistry.info/Elements/u/P60602> ;
    owl:inverseOf <http://rdaregistry.info/Elements/u/P60157> ;
    skos:definition "Relates a person held to be a channel of communication between the earthly world and a world of spirits to the resource."@en .

<http://rdaregistry.info/Elements/u/P60033>
    reg:hasSubproperty <http://rdaregistry.info/Elements/a/P50213> ;
    reg:lexicalAlias <http://rdaregistry.info/Elements/u/filmProducerOf.en> ;
    reg:name "filmProducerOf"@en ;
    reg:status <http://metadataregistry.org/uri/RegStatus/1001> ;
    a rdf:Property ;
    rdfs:isDefinedBy <http://rdaregistry.info/Elements/u/> ;
    rdfs:label "is film producer of"@en ;
    rdfs:subPropertyOf <http://rdaregistry.info/Elements/u/P60668> ;
    owl:inverseOf <http://rdaregistry.info/Elements/u/P60169> ;
    skos:definition "Relates a producer responsible for most of the business aspects of a film to the resource."@en .

<http://rdaregistry.info/Elements/u/P60034>
    reg:hasSubproperty <http://rdaregistry.info/Elements/a/P50214> ;
    reg:lexicalAlias <http://rdaregistry.info/Elements/u/radioProducerOf.en> ;
    reg:name "radioProducerOf"@en ;
    reg:status <http://metadataregistry.org/uri/RegStatus/1001> ;
    a rdf:Property ;
    rdfs:isDefinedBy <http://rdaregistry.info/Elements/u/> ;
    rdfs:label "is radio producer of"@en ;
    rdfs:subPropertyOf <http://rdaregistry.info/Elements/u/P60668> ;
    owl:inverseOf <http://rdaregistry.info/Elements/u/P60170> ;
    skos:definition "Relates a producer responsible for most of the business aspects of a radio program to the resource."@en .

<http://rdaregistry.info/Elements/u/P60035>
    reg:hasSubproperty <http://rdaregistry.info/Elements/a/P50215> ;
    reg:lexicalAlias <http://rdaregistry.info/Elements/u/televisionProducerOf.en> ;
    reg:name "televisionProducerOf"@en ;
    reg:status <http://metadataregistry.org/uri/RegStatus/1001> ;
    a rdf:Property ;
    rdfs:isDefinedBy <http://rdaregistry.info/Elements/u/> ;
    rdfs:label "is television producer of"@en ;
    rdfs:subPropertyOf <http://rdaregistry.info/Elements/u/P60668> ;
    owl:inverseOf <http://rdaregistry.info/Elements/u/P60171> ;
    skos:definition "Relates a producer responsible for most of the business aspects of a television program to the resource."@en .

<http://rdaregistry.info/Elements/u/P60036>
    reg:hasSubproperty <http://rdaregistry.info/Elements/a/P50105> ;
    reg:lexicalAlias <http://rdaregistry.info/Elements/u/alternateIdentity.en> ;
    reg:name "alternateIdentity"@en ;
    reg:status <http://metadataregistry.org/uri/RegStatus/1001> ;
    a rdf:Property ;
    rdfs:isDefinedBy <http://rdaregistry.info/Elements/u/> ;
    rdfs:label "has alternate identity"@en ;
    owl:inverseOf <http://rdaregistry.info/Elements/u/P60037> ;
    skos:definition "Relates a pseudonymous or other identity assumed by the agent to the agent."@en .

<http://rdaregistry.info/Elements/u/P60037>
    reg:hasSubproperty <http://rdaregistry.info/Elements/a/P50106> ;
    reg:lexicalAlias <http://rdaregistry.info/Elements/u/realIdentity.en> ;
    reg:name "realIdentity"@en ;
    reg:status <http://metadataregistry.org/uri/RegStatus/1001> ;
    a rdf:Property ;
    rdfs:isDefinedBy <http://rdaregistry.info/Elements/u/> ;
    rdfs:label "has real identity"@en ;
    owl:inverseOf <http://rdaregistry.info/Elements/u/P60036> ;
    skos:definition "Relates a real agent who assumes the alternate identity to the agent."@en .

<http://rdaregistry.info/Elements/u/P60045>
    reg:lexicalAlias <http://rdaregistry.info/Elements/u/respondent.en> ;
    reg:name "respondent"@en ;
    reg:status <http://metadataregistry.org/uri/RegStatus/1001> ;
    a rdf:Property ;
    rdfs:isDefinedBy <http://rdaregistry.info/Elements/u/> ;
    rdfs:label "has respondent"@en ;
    rdfs:subPropertyOf <http://rdaregistry.info/Elements/u/P60447> ;
    owl:inverseOf <http://rdaregistry.info/Elements/u/P60001> ;
    skos:definition "Relates a resource to a candidate for a degree who defends or opposes a thesis provided by the praeses in an academic disputation."@en .

<http://rdaregistry.info/Elements/u/P60046>
    reg:hasSubproperty <http://rdaregistry.info/Elements/a/P50093> ;
    reg:lexicalAlias <http://rdaregistry.info/Elements/u/undifferentiatedNameIndicator.en> ;
    reg:name "undifferentiatedNameIndicator"@en ;
    reg:status <http://metadataregistry.org/uri/RegStatus/1001> ;
    a rdf:Property ;
    rdfs:isDefinedBy <http://rdaregistry.info/Elements/u/> ;
    rdfs:label "has undifferentiated name indicator"@en ;
    skos:definition "Relates a resource to a categorization indicating that the core elements recorded are insufficient to differentiate between two or more agents with the same name."@en .

<http://rdaregistry.info/Elements/u/P60047>
    reg:hasSubproperty <http://rdaregistry.info/Elements/a/P50051>, <http://rdaregistry.info/Elements/a/P50237>, <http://rdaregistry.info/Elements/a/P50238> ;
    reg:lexicalAlias <http://rdaregistry.info/Elements/u/typeOfAgent.en> ;
    reg:name "typeOfAgent"@en ;
    reg:status <http://metadataregistry.org/uri/RegStatus/1001> ;
    a rdf:Property ;
    rdfs:isDefinedBy <http://rdaregistry.info/Elements/u/> ;
    rdfs:label "has type of agent"@en ;
    skos:definition "Relates a resource to a categorization or generic descriptor for the type of agent."@en .

<http://rdaregistry.info/Elements/u/P60048>
    reg:hasSubproperty <http://rdaregistry.info/Elements/m/P30001> ;
    reg:lexicalAlias <http://rdaregistry.info/Elements/u/carrierType.en> ;
    reg:name "carrierType"@en ;
    reg:status <http://metadataregistry.org/uri/RegStatus/1001> ;
    a rdf:Property ;
    rdfs:isDefinedBy <http://rdaregistry.info/Elements/u/> ;
    rdfs:label "has carrier type"@en ;
    skos:definition "Relates a resource to a categorization reflecting the format of the storage medium and housing of a carrier in combination with the type of intermediation device required to view, play, run, etc., the content of a resource."@en .

<http://rdaregistry.info/Elements/u/P60049>
    reg:hasSubproperty <http://rdaregistry.info/Elements/e/P20001> ;
    reg:lexicalAlias <http://rdaregistry.info/Elements/u/contentType.en> ;
    reg:name "contentType"@en ;
    reg:status <http://metadataregistry.org/uri/RegStatus/1001> ;
    a rdf:Property ;
    rdfs:isDefinedBy <http://rdaregistry.info/Elements/u/> ;
    rdfs:label "has content type"@en ;
    skos:definition "Relates a resource to a categorization reflecting the fundamental form of communication in which the content is expressed and the human sense through which it is intended to be perceived."@en .

<http://rdaregistry.info/Elements/u/P60050>
    reg:hasSubproperty <http://rdaregistry.info/Elements/m/P30002> ;
    reg:lexicalAlias <http://rdaregistry.info/Elements/u/mediaType.en> ;
    reg:name "mediaType"@en ;
    reg:status <http://metadataregistry.org/uri/RegStatus/1001> ;
    a rdf:Property ;
    rdfs:isDefinedBy <http://rdaregistry.info/Elements/u/> ;
    rdfs:label "has media type"@en ;
    skos:definition "Relates a resource to a categorization reflecting the general type of intermediation device required to view, play, run, etc., the content of a resource."@en .

<http://rdaregistry.info/Elements/u/P60051>
    reg:hasSubproperty <http://rdaregistry.info/Elements/m/P30003> ;
    reg:lexicalAlias <http://rdaregistry.info/Elements/u/modeOfIssuance.en> ;
    reg:name "modeOfIssuance"@en ;
    reg:status <http://metadataregistry.org/uri/RegStatus/1001> ;
    a rdf:Property ;
    rdfs:isDefinedBy <http://rdaregistry.info/Elements/u/> ;
    rdfs:label "has mode of issuance"@en ;
    skos:definition "Relates a resource to a categorization reflecting whether a resource is issued in one or more parts, the way it is updated, and its intended termination."@en .

<http://rdaregistry.info/Elements/u/P60052>
    reg:hasSubproperty <http://rdaregistry.info/Elements/e/P20002>, <http://rdaregistry.info/Elements/i/P40001>, <http://rdaregistry.info/Elements/m/P30004>, <http://rdaregistry.info/Elements/u/P60139>, <http://rdaregistry.info/Elements/u/P60140> ;
    reg:lexicalAlias <http://rdaregistry.info/Elements/u/identifierForTheResource.en> ;
    reg:name "identifierForTheResource"@en ;
    reg:status <http://metadataregistry.org/uri/RegStatus/1001> ;
    a rdf:Property ;
    rdfs:isDefinedBy <http://rdaregistry.info/Elements/u/> ;
    rdfs:label "has identifier for the resource"@en ;
    skos:definition "Relates a resource to a character string associated with a resource that serves to differentiate that resource from other resources."@en .

<http://rdaregistry.info/Elements/u/P60053>
    reg:hasSubproperty <http://rdaregistry.info/Elements/a/P50006>, <http://rdaregistry.info/Elements/a/P50052>, <http://rdaregistry.info/Elements/a/P50094> ;
    reg:lexicalAlias <http://rdaregistry.info/Elements/u/identifierForTheAgent.en> ;
    reg:name "identifierForTheAgent"@en ;
    reg:status <http://metadataregistry.org/uri/RegStatus/1001> ;
    a rdf:Property ;
    rdfs:isDefinedBy <http://rdaregistry.info/Elements/u/> ;
    rdfs:label "has identifier for the agent"@en ;
    skos:definition "Relates a resource to a character string uniquely associated with an agent, or with a surrogate for an agent (e.g., an authority record)."@en .

<http://rdaregistry.info/Elements/u/P60054>
    reg:hasSubproperty <http://rdaregistry.info/Elements/e/P20003> ;
    reg:lexicalAlias <http://rdaregistry.info/Elements/u/otherDistinguishingCharacteristicOfTheResource.en> ;
    reg:name "otherDistinguishingCharacteristicOfTheResource"@en ;
    reg:status <http://metadataregistry.org/uri/RegStatus/1001> ;
    a rdf:Property ;
    rdfs:isDefinedBy <http://rdaregistry.info/Elements/u/> ;
    rdfs:label "has other distinguishing characteristic of the resource"@en ;
    skos:definition "Relates a resource to a characteristic other than content type, language of resource, date of resource, form of resource, or place of origin of the resource."@en .

<http://rdaregistry.info/Elements/u/P60055>
    reg:status <http://metadataregistry.org/uri/RegStatus/1008> ;
    rdfs:isDefinedBy <http://rdaregistry.info/Elements/u/> .

<http://rdaregistry.info/Elements/u/P60056>
    reg:hasSubproperty <http://rdaregistry.info/Elements/i/P40003>, <http://rdaregistry.info/Elements/u/P60055> ;
    reg:lexicalAlias <http://rdaregistry.info/Elements/u/noteOnResourceSpecificCarrierCharacteristic.en> ;
    reg:name "noteOnResourceSpecificCarrierCharacteristic"@en ;
    reg:status <http://metadataregistry.org/uri/RegStatus/1001> ;
    a rdf:Property ;
    rdfs:isDefinedBy <http://rdaregistry.info/Elements/u/> ;
    rdfs:label "has note on resource-specific carrier characteristic"@en ;
    skos:definition "Relates a resource to a note providing information about additional characteristics that are specific to the resource being described and are assumed not to apply to other resources exemplifying the same resource."@en .

<http://rdaregistry.info/Elements/u/P60057>
    reg:hasSubproperty <http://rdaregistry.info/Elements/m/P30005> ;
    reg:lexicalAlias <http://rdaregistry.info/Elements/u/preferredCitation.en> ;
    reg:name "preferredCitation"@en ;
    reg:status <http://metadataregistry.org/uri/RegStatus/1001> ;
    a rdf:Property ;
    rdfs:isDefinedBy <http://rdaregistry.info/Elements/u/> ;
    rdfs:label "has preferred citation"@en ;
    skos:definition "Relates a resource to a citation for a resource in the form preferred by a creator, publisher, custodian, indexing or abstracting service, etc."@en .

<http://rdaregistry.info/Elements/u/P60058>
    reg:lexicalAlias <http://rdaregistry.info/Elements/u/formOfResource.en> ;
    reg:name "formOfResource"@en ;
    reg:status <http://metadataregistry.org/uri/RegStatus/1001> ;
    a rdf:Property ;
    rdfs:isDefinedBy <http://rdaregistry.info/Elements/u/> ;
    rdfs:label "has form of resource"@en ;
    skos:definition "Relates a resource to a class or genre to which a resource belongs."@en .

<http://rdaregistry.info/Elements/u/P60059>
    reg:hasSubproperty <http://rdaregistry.info/Elements/m/P30006> ;
    reg:lexicalAlias <http://rdaregistry.info/Elements/u/regionalEncoding.en> ;
    reg:name "regionalEncoding"@en ;
    reg:status <http://metadataregistry.org/uri/RegStatus/1001> ;
    a rdf:Property ;
    rdfs:isDefinedBy <http://rdaregistry.info/Elements/u/> ;
    rdfs:label "has regional encoding"@en ;
    rdfs:subPropertyOf <http://rdaregistry.info/Elements/u/P60350> ;
    skos:definition "Relates a resource to a code identifying the region of the world for which a videodisc has been encoded and preventing the disc from being played on a player sold in a different region."@en .

<http://rdaregistry.info/Elements/u/P60060>
    reg:lexicalAlias <http://rdaregistry.info/Elements/u/degreeGrantingInstitution.en> ;
    reg:name "degreeGrantingInstitution"@en ;
    reg:status <http://metadataregistry.org/uri/RegStatus/1001> ;
    a rdf:Property ;
    rdfs:isDefinedBy <http://rdaregistry.info/Elements/u/> ;
    rdfs:label "has degree granting institution"@en ;
    rdfs:subPropertyOf <http://rdaregistry.info/Elements/u/P60374> ;
    owl:inverseOf <http://rdaregistry.info/Elements/u/P60002> ;
    skos:definition "Relates a resource to a corporate body granting an academic degree."@en .

<http://rdaregistry.info/Elements/u/P60061>
    reg:lexicalAlias <http://rdaregistry.info/Elements/u/hostInstitution.en> ;
    reg:name "host institution"@en ;
    reg:status <http://metadataregistry.org/uri/RegStatus/1001> ;
    a rdf:Property ;
    rdfs:isDefinedBy <http://rdaregistry.info/Elements/u/> ;
    rdfs:label "has host institution"@en ;
    rdfs:subPropertyOf <http://rdaregistry.info/Elements/u/P60374> ;
    owl:inverseOf <http://rdaregistry.info/Elements/u/P60003> ;
    skos:definition "Relates a resource to a corporate body hosting the event, exhibit, conference, etc., which gave rise to a resource, but having little or no responsibility for the content of the resource."@en .

<http://rdaregistry.info/Elements/u/P60062>
    reg:lexicalAlias <http://rdaregistry.info/Elements/u/productionCompany.en> ;
    reg:name "productionCompany"@en ;
    reg:status <http://metadataregistry.org/uri/RegStatus/1001> ;
    a rdf:Property ;
    rdfs:isDefinedBy <http://rdaregistry.info/Elements/u/> ;
    rdfs:label "has production company"@en ;
    rdfs:subPropertyOf <http://rdaregistry.info/Elements/u/P60374> ;
    owl:inverseOf <http://rdaregistry.info/Elements/u/P60004> ;
    skos:definition "Relates a resource to a corporate body that is responsible for financial, technical, and organizational management of a production for stage, screen, sound recording, television, webcast, etc."@en .

<http://rdaregistry.info/Elements/u/P60063>
    reg:hasSubproperty <http://rdaregistry.info/Elements/a/P50097> ;
    reg:lexicalAlias <http://rdaregistry.info/Elements/u/countryAssociatedWithThePerson.en> ;
    reg:name "countryAssociatedWithTheAgent"@en ;
    reg:status <http://metadataregistry.org/uri/RegStatus/1001> ;
    a rdf:Property ;
    rdfs:isDefinedBy <http://rdaregistry.info/Elements/u/> ;
    rdfs:label "has country associated with the agent"@en ;
    skos:definition "Relates a resource to a country with which an agent is identified."@en .

<http://rdaregistry.info/Elements/u/P60064>
    reg:lexicalAlias <http://rdaregistry.info/Elements/u/locationOfHeadquarters.en> ;
    reg:name "locationOfHeadquarters"@en ;
    reg:status <http://metadataregistry.org/uri/RegStatus/1008> ;
    a rdf:Property ;
    rdfs:isDefinedBy <http://rdaregistry.info/Elements/u/> ;
    rdfs:subPropertyOf <http://rdaregistry.info/Elements/u/P60325> .

<http://rdaregistry.info/Elements/u/P60065>
    reg:lexicalAlias <http://rdaregistry.info/Elements/u/courtGoverned.en> ;
    reg:name "courtGoverned"@en ;
    reg:status <http://metadataregistry.org/uri/RegStatus/1001> ;
    a rdf:Property ;
    rdfs:isDefinedBy <http://rdaregistry.info/Elements/u/> ;
    rdfs:label "has court governed"@en ;
    rdfs:subPropertyOf <http://rdaregistry.info/Elements/u/P60374> ;
    owl:inverseOf <http://rdaregistry.info/Elements/u/P60005> ;
    skos:definition "Relates a resource to a court governed by court rules, regardless of their official nature (e.g., laws, administrative regulations)."@en .

<http://rdaregistry.info/Elements/u/P60066>
    reg:hasSubproperty <http://rdaregistry.info/Elements/i/P40004> ;
    reg:lexicalAlias <http://rdaregistry.info/Elements/u/collector.en> ;
    reg:name "collector"@en ;
    reg:status <http://metadataregistry.org/uri/RegStatus/1001> ;
    a rdf:Property ;
    rdfs:isDefinedBy <http://rdaregistry.info/Elements/u/> ;
    rdfs:label "has collector"@en ;
    rdfs:subPropertyOf <http://rdaregistry.info/Elements/u/P60376> ;
    owl:inverseOf <http://rdaregistry.info/Elements/u/P60006> ;
    skos:definition "Relates a resource to a curator who brings together resources from various sources that are then arranged, described, and cataloged as a collection."@en .

<http://rdaregistry.info/Elements/u/P60067>
    reg:hasSubproperty <http://rdaregistry.info/Elements/i/P40005> ;
    reg:lexicalAlias <http://rdaregistry.info/Elements/u/collectionRegistrar.en> ;
    reg:name "collectionRegistrar"@en ;
    reg:status <http://metadataregistry.org/uri/RegStatus/1001> ;
    a rdf:Property ;
    rdfs:isDefinedBy <http://rdaregistry.info/Elements/u/> ;
    rdfs:label "has collection registrar"@en ;
    rdfs:subPropertyOf <http://rdaregistry.info/Elements/u/P60376> ;
    owl:inverseOf <http://rdaregistry.info/Elements/u/P60007> ;
    skos:definition "Relates a resource to a curator who lists or inventories the items in an aggregate resource such as a collection of items or resources."@en .

<http://rdaregistry.info/Elements/u/P60068>
    reg:hasSubproperty <http://rdaregistry.info/Elements/i/P40006> ;
    reg:lexicalAlias <http://rdaregistry.info/Elements/u/depositor.en> ;
    reg:name "depositor"@en ;
    reg:status <http://metadataregistry.org/uri/RegStatus/1001> ;
    a rdf:Property ;
    rdfs:isDefinedBy <http://rdaregistry.info/Elements/u/> ;
    rdfs:label "has depositor"@en ;
    rdfs:subPropertyOf <http://rdaregistry.info/Elements/u/P60400> ;
    owl:inverseOf <http://rdaregistry.info/Elements/u/P60008> ;
    skos:definition "Relates a resource to a current owner of a resource who deposited the resource into the custody of another person, family, or corporate body, while still retaining ownership."@en .

<http://rdaregistry.info/Elements/u/P60069>
    reg:hasSubproperty <http://rdaregistry.info/Elements/m/P30007> ;
    reg:lexicalAlias <http://rdaregistry.info/Elements/u/copyrightDate.en> ;
    reg:name "copyrightDate"@en ;
    reg:status <http://metadataregistry.org/uri/RegStatus/1001> ;
    a rdf:Property ;
    rdfs:isDefinedBy <http://rdaregistry.info/Elements/u/> ;
    rdfs:label "has copyright date"@en ;
    skos:definition "Relates a resource to a date associated with a claim of protection under copyright or a similar regime."@en .

<http://rdaregistry.info/Elements/u/P60070>
    reg:hasSubproperty <http://rdaregistry.info/Elements/m/P30008> ;
    reg:lexicalAlias <http://rdaregistry.info/Elements/u/dateOfDistribution.en> ;
    reg:name "dateOfDistribution"@en ;
    reg:status <http://metadataregistry.org/uri/RegStatus/1001> ;
    a rdf:Property ;
    rdfs:isDefinedBy <http://rdaregistry.info/Elements/u/> ;
    rdfs:label "has date of distribution"@en ;
    skos:definition "Relates a resource to a date associated with the distribution of a resource in a published form."@en .

<http://rdaregistry.info/Elements/u/P60071>
    reg:hasSubproperty <http://rdaregistry.info/Elements/m/P30009> ;
    reg:lexicalAlias <http://rdaregistry.info/Elements/u/dateOfProduction.en> ;
    reg:name "dateOfProduction"@en ;
    reg:status <http://metadataregistry.org/uri/RegStatus/1001> ;
    a rdf:Property ;
    rdfs:isDefinedBy <http://rdaregistry.info/Elements/u/> ;
    rdfs:label "has date of production"@en ;
    skos:definition "Relates a resource to a date associated with the inscription, fabrication, construction, etc., of a resource in an unpublished form."@en .

<http://rdaregistry.info/Elements/u/P60072>
    reg:hasSubproperty <http://rdaregistry.info/Elements/m/P30010> ;
    reg:lexicalAlias <http://rdaregistry.info/Elements/u/dateOfManufacture.en> ;
    reg:name "dateOfManufacture"@en ;
    reg:status <http://metadataregistry.org/uri/RegStatus/1001> ;
    a rdf:Property ;
    rdfs:isDefinedBy <http://rdaregistry.info/Elements/u/> ;
    rdfs:label "has date of manufacture"@en ;
    skos:definition "Relates a resource to a date associated with the printing, duplicating, casting, etc., of a resource in a published form."@en .

<http://rdaregistry.info/Elements/u/P60073>
    reg:hasSubproperty <http://rdaregistry.info/Elements/m/P30011> ;
    reg:lexicalAlias <http://rdaregistry.info/Elements/u/dateOfPublication.en> ;
    reg:name "dateOfPublication"@en ;
    reg:status <http://metadataregistry.org/uri/RegStatus/1001> ;
    a rdf:Property ;
    rdfs:isDefinedBy <http://rdaregistry.info/Elements/u/> ;
    rdfs:label "has date of publication"@en ;
    skos:definition "Relates a resource to a date associated with the publication, release, or issuing of a resource."@en .

<http://rdaregistry.info/Elements/u/P60074>
    reg:hasSubproperty <http://rdaregistry.info/Elements/e/P20004> ;
    reg:lexicalAlias <http://rdaregistry.info/Elements/u/dateOfCapture.en> ;
    reg:name "dateOfCapture"@en ;
    reg:status <http://metadataregistry.org/uri/RegStatus/1001> ;
    a rdf:Property ;
    rdfs:isDefinedBy <http://rdaregistry.info/Elements/u/> ;
    rdfs:label "has date of capture"@en ;
    skos:definition "Relates a resource to a date or range of dates associated with the capture (i.e., recording, filming, etc.) of the content of a resource."@en .

<http://rdaregistry.info/Elements/u/P60075>
    reg:lexicalAlias <http://rdaregistry.info/Elements/u/dateOfUsage.en> ;
    reg:name "dateOfUsage"@en ;
    reg:status <http://metadataregistry.org/uri/RegStatus/1001> ;
    a rdf:Property ;
    rdfs:isDefinedBy <http://rdaregistry.info/Elements/u/> ;
    rdfs:label "has date of usage"@en ;
    skos:definition "Relates a name to a date or range of dates associated with the use of the name chosen as the preferred name for an agent."@en .

<http://rdaregistry.info/Elements/u/P60076>
    reg:hasSubproperty <http://rdaregistry.info/Elements/a/P50098>, <http://rdaregistry.info/Elements/a/P50236> ;
    reg:lexicalAlias <http://rdaregistry.info/Elements/u/periodOfActivityOfTheAgent.en> ;
    reg:name "periodOfActivityOfTheAgent"@en ;
    reg:status <http://metadataregistry.org/uri/RegStatus/1001> ;
    a rdf:Property ;
    rdfs:isDefinedBy <http://rdaregistry.info/Elements/u/> ;
    rdfs:label "has period of activity of the agent"@en ;
    rdfs:subPropertyOf <http://rdaregistry.info/Elements/u/P60324> ;
    skos:definition "Relates a resource to a date or range of dates indicative of the period in which an agent was active in his or her primary field of endeavour."@en .

<http://rdaregistry.info/Elements/u/P60077>
    reg:hasSubproperty <http://rdaregistry.info/Elements/m/P30012> ;
    reg:lexicalAlias <http://rdaregistry.info/Elements/u/parallelDesignationOfANamedRevisionOfAnEdition.en> ;
    reg:name "parallelDesignationOfANamedRevisionOfAnEdition"@en ;
    reg:status <http://metadataregistry.org/uri/RegStatus/1001> ;
    a rdf:Property ;
    rdfs:isDefinedBy <http://rdaregistry.info/Elements/u/> ;
    rdfs:label "has parallel designation of a named revision of an edition"@en ;
    skos:definition "Relates a resource to a designation of a named revision of an edition in a language and/or script that differs from that recorded in the designation of a named revision of an edition element."@en .

<http://rdaregistry.info/Elements/u/P60078>
    reg:hasSubproperty <http://rdaregistry.info/Elements/m/P30013> ;
    reg:lexicalAlias <http://rdaregistry.info/Elements/u/parallelDesignationOfEdition.en> ;
    reg:name "parallelDesignationOfEdition"@en ;
    reg:status <http://metadataregistry.org/uri/RegStatus/1001> ;
    a rdf:Property ;
    rdfs:isDefinedBy <http://rdaregistry.info/Elements/u/> ;
    rdfs:label "has parallel designation of edition"@en ;
    skos:definition "Relates a resource to a designation of edition in a language and/or script that differs from that recorded in the designation of edition element."@en .

<http://rdaregistry.info/Elements/u/P60079>
    reg:hasSubproperty <http://rdaregistry.info/Elements/a/P50019> ;
    reg:lexicalAlias <http://rdaregistry.info/Elements/u/numberOfAConferenceEtc.en> ;
    reg:name "numberOfAConferenceEtc"@en ;
    reg:status <http://metadataregistry.org/uri/RegStatus/1001> ;
    a rdf:Property ;
    rdfs:isDefinedBy <http://rdaregistry.info/Elements/u/> ;
    rdfs:label "has number of a conference, etc."@en ;
    skos:definition "Relates a resource to a designation of the sequencing of a conference, etc., within a series of conferences, etc."@en .

<http://rdaregistry.info/Elements/u/P60080>
    reg:lexicalAlias <http://rdaregistry.info/Elements/u/numberingOfPart.en> ;
    reg:name "numberingOfPart"@en ;
    reg:status <http://metadataregistry.org/uri/RegStatus/1001> ;
    a rdf:Property ;
    rdfs:isDefinedBy <http://rdaregistry.info/Elements/u/> ;
    rdfs:label "has numbering of part"@en ;
    skos:definition "Relates a resource to a designation of the sequencing of a part or parts within a larger resource."@en .

<http://rdaregistry.info/Elements/u/P60081>
    reg:hasSubproperty <http://rdaregistry.info/Elements/m/P30014> ;
    reg:lexicalAlias <http://rdaregistry.info/Elements/u/numberingWithinSeries.en> ;
    reg:name "numberingWithinSeries"@en ;
    reg:status <http://metadataregistry.org/uri/RegStatus/1001> ;
    a rdf:Property ;
    rdfs:isDefinedBy <http://rdaregistry.info/Elements/u/> ;
    rdfs:label "has numbering within series"@en ;
    skos:definition "Relates a resource to a designation of the sequencing of a part or parts within a series."@en .

<http://rdaregistry.info/Elements/u/P60082>
    reg:hasSubproperty <http://rdaregistry.info/Elements/m/P30015> ;
    reg:lexicalAlias <http://rdaregistry.info/Elements/u/numberingWithinSubseries.en> ;
    reg:name "numberingWithinSubseries"@en ;
    reg:status <http://metadataregistry.org/uri/RegStatus/1001> ;
    a rdf:Property ;
    rdfs:isDefinedBy <http://rdaregistry.info/Elements/u/> ;
    rdfs:label "has numbering within subseries"@en ;
    skos:definition "Relates a resource to a designation of the sequencing of a part or parts within a subseries."@en .

<http://rdaregistry.info/Elements/u/P60083>
    reg:hasSubproperty <http://rdaregistry.info/Elements/i/P40057>, <http://rdaregistry.info/Elements/m/P30016> ;
    reg:lexicalAlias <http://rdaregistry.info/Elements/u/electronicReproduction.en> ;
    reg:name "electronicReproduction"@en ;
    reg:status <http://metadataregistry.org/uri/RegStatus/1001> ;
    a rdf:Property ;
    rdfs:isDefinedBy <http://rdaregistry.info/Elements/u/> ;
    rdfs:label "has electronic reproduction"@en ;
    rdfs:subPropertyOf <http://rdaregistry.info/Elements/u/P60272> ;
    owl:inverseOf <http://rdaregistry.info/Elements/u/P60469> ;
    skos:definition "Relates a resource to a resource in a digital format that is the result of the transfer of a resource in an analog format."@en .

<http://rdaregistry.info/Elements/u/P60084>
    reg:lexicalAlias <http://rdaregistry.info/Elements/u/filmDirector.en> ;
    reg:name "filmDirector"@en ;
    reg:status <http://metadataregistry.org/uri/RegStatus/1001> ;
    a rdf:Property ;
    rdfs:isDefinedBy <http://rdaregistry.info/Elements/u/> ;
    rdfs:label "has film director"@en ;
    rdfs:subPropertyOf <http://rdaregistry.info/Elements/u/P60449> ;
    owl:inverseOf <http://rdaregistry.info/Elements/u/P60009> ;
    skos:definition "Relates a resource to a director responsible for the general management and supervision of a filmed performance."@en .

<http://rdaregistry.info/Elements/u/P60085>
    reg:lexicalAlias <http://rdaregistry.info/Elements/u/radioDirector.en> ;
    reg:name "radioDirector"@en ;
    reg:status <http://metadataregistry.org/uri/RegStatus/1001> ;
    a rdf:Property ;
    rdfs:isDefinedBy <http://rdaregistry.info/Elements/u/> ;
    rdfs:label "has radio director"@en ;
    rdfs:subPropertyOf <http://rdaregistry.info/Elements/u/P60449> ;
    owl:inverseOf <http://rdaregistry.info/Elements/u/P60010> ;
    skos:definition "Relates a resource to a director responsible for the general management and supervision of a radio program."@en .

<http://rdaregistry.info/Elements/u/P60086>
    reg:lexicalAlias <http://rdaregistry.info/Elements/u/televisionDirector.en> ;
    reg:name "televisionDirector"@en ;
    reg:status <http://metadataregistry.org/uri/RegStatus/1001> ;
    a rdf:Property ;
    rdfs:isDefinedBy <http://rdaregistry.info/Elements/u/> ;
    rdfs:label "has television director"@en ;
    rdfs:subPropertyOf <http://rdaregistry.info/Elements/u/P60449> ;
    owl:inverseOf <http://rdaregistry.info/Elements/u/P60011> ;
    skos:definition "Relates a resource to a director responsible for the general management and supervision of a television program."@en .

<http://rdaregistry.info/Elements/u/P60087>
    reg:hasSubproperty <http://rdaregistry.info/Elements/m/P30017> ;
    reg:lexicalAlias <http://rdaregistry.info/Elements/u/parallelDistributorsName.en> ;
    reg:name "parallelDistributorsName"@en ;
    reg:status <http://metadataregistry.org/uri/RegStatus/1001> ;
    a rdf:Property ;
    rdfs:isDefinedBy <http://rdaregistry.info/Elements/u/> ;
    rdfs:label "has parallel distributor’s name"@en ;
    skos:definition "Relates a resource to a distributor's name in a language and/or script that differs from that recorded in the distributor's name element."@en .

<http://rdaregistry.info/Elements/u/P60088>
    reg:hasSubproperty <http://rdaregistry.info/Elements/e/P20073> ;
    reg:lexicalAlias <http://rdaregistry.info/Elements/u/dramatizedAs.en> ;
    reg:name "dramatizedAs"@en ;
    reg:status <http://metadataregistry.org/uri/RegStatus/1001> ;
    a rdf:Property ;
    rdfs:isDefinedBy <http://rdaregistry.info/Elements/u/> ;
    rdfs:label "is dramatized as"@en ;
    rdfs:subPropertyOf <http://rdaregistry.info/Elements/u/P60260> ;
    owl:inverseOf <http://rdaregistry.info/Elements/u/P60225> ;
    skos:definition "Relates a resource to a dramatic resource adapted from the source resource."@en .

<http://rdaregistry.info/Elements/u/P60089>
    reg:hasSubproperty <http://rdaregistry.info/Elements/a/P50022>, <http://rdaregistry.info/Elements/a/P50100> ;
    reg:lexicalAlias <http://rdaregistry.info/Elements/u/fieldOfActivity.en> ;
    reg:name "fieldOfActivity"@en ;
    reg:status <http://metadataregistry.org/uri/RegStatus/1001> ;
    a rdf:Property ;
    rdfs:isDefinedBy <http://rdaregistry.info/Elements/u/> ;
    rdfs:label "has field of activity of the agent"@en ;
    skos:definition "Relates a resource to a field of endeavour, area of expertise, competence, responsibility, jurisdiction etc., in which an agent is engaged or was engaged."@en .

<http://rdaregistry.info/Elements/u/P60090>
    reg:hasSubproperty <http://rdaregistry.info/Elements/e/P20005> ;
    reg:lexicalAlias <http://rdaregistry.info/Elements/u/award.en> ;
    reg:name "award"@en ;
    reg:status <http://metadataregistry.org/uri/RegStatus/1001> ;
    a rdf:Property ;
    rdfs:isDefinedBy <http://rdaregistry.info/Elements/u/> ;
    rdfs:label "has award"@en ;
    skos:definition "Relates a resource to a formal recognition of excellence, etc., given by an award- or prize-granting body, for the content of a resource."@en .

<http://rdaregistry.info/Elements/u/P60091>
    reg:hasSubproperty <http://rdaregistry.info/Elements/i/P40007> ;
    reg:lexicalAlias <http://rdaregistry.info/Elements/u/donor.en> ;
    reg:name "donor"@en ;
    reg:status <http://metadataregistry.org/uri/RegStatus/1001> ;
    a rdf:Property ;
    rdfs:isDefinedBy <http://rdaregistry.info/Elements/u/> ;
    rdfs:label "has donor"@en ;
    rdfs:subPropertyOf <http://rdaregistry.info/Elements/u/P60401> ;
    owl:inverseOf <http://rdaregistry.info/Elements/u/P60012> ;
    skos:definition "Relates a resource to a former owner of a resource who donated that resource to another owner."@en .

<http://rdaregistry.info/Elements/u/P60092>
    reg:hasSubproperty <http://rdaregistry.info/Elements/i/P40008> ;
    reg:lexicalAlias <http://rdaregistry.info/Elements/u/seller.en> ;
    reg:name "seller"@en ;
    reg:status <http://metadataregistry.org/uri/RegStatus/1001> ;
    a rdf:Property ;
    rdfs:isDefinedBy <http://rdaregistry.info/Elements/u/> ;
    rdfs:label "has seller"@en ;
    rdfs:subPropertyOf <http://rdaregistry.info/Elements/u/P60401> ;
    owl:inverseOf <http://rdaregistry.info/Elements/u/P60013> ;
    skos:definition "Relates a resource to a former owner of a resource who sold that resource to another owner."@en .

<http://rdaregistry.info/Elements/u/P60093>
    reg:hasSubproperty <http://rdaregistry.info/Elements/m/P30018> ;
    reg:lexicalAlias <http://rdaregistry.info/Elements/u/fileType.en> ;
    reg:name "fileType"@en ;
    reg:status <http://metadataregistry.org/uri/RegStatus/1001> ;
    a rdf:Property ;
    rdfs:isDefinedBy <http://rdaregistry.info/Elements/u/> ;
    rdfs:label "has file type"@en ;
    rdfs:subPropertyOf <http://rdaregistry.info/Elements/u/P60350> ;
    skos:definition "Relates a resource to a general type of data content encoded in a computer file."@en .

<http://rdaregistry.info/Elements/u/P60095>
    reg:hasSubproperty <http://rdaregistry.info/Elements/a/P50101> ;
    reg:lexicalAlias <http://rdaregistry.info/Elements/u/affiliation.en> ;
    reg:name "affiliation"@en ;
    reg:status <http://metadataregistry.org/uri/RegStatus/1001> ;
    a rdf:Property ;
    rdfs:isDefinedBy <http://rdaregistry.info/Elements/u/> ;
    rdfs:label "has affiliation"@en ;
    skos:definition "Relates a resource to a group with which an agent is affiliated or has been affiliated through employment, membership, cultural identity, etc."@en .

<http://rdaregistry.info/Elements/u/P60096>
    reg:lexicalAlias <http://rdaregistry.info/Elements/u/enactingJurisdiction.en> ;
    reg:name "enactingJurisdiction"@en ;
    reg:status <http://metadataregistry.org/uri/RegStatus/1001> ;
    a rdf:Property ;
    rdfs:isDefinedBy <http://rdaregistry.info/Elements/u/> ;
    rdfs:label "has enacting jurisdiction"@en ;
    rdfs:subPropertyOf <http://rdaregistry.info/Elements/u/P60447> ;
    owl:inverseOf <http://rdaregistry.info/Elements/u/P60014> ;
    skos:definition "Relates a resource to a jurisdiction enacting a law, regulation, constitution, court rule, etc."@en .

<http://rdaregistry.info/Elements/u/P60097>
    reg:lexicalAlias <http://rdaregistry.info/Elements/u/jurisdictionGoverned.en> ;
    reg:name "jurisdictionGoverned"@en ;
    reg:status <http://metadataregistry.org/uri/RegStatus/1001> ;
    a rdf:Property ;
    rdfs:isDefinedBy <http://rdaregistry.info/Elements/u/> ;
    rdfs:label "has jurisdiction governed"@en ;
    rdfs:subPropertyOf <http://rdaregistry.info/Elements/u/P60374> ;
    owl:inverseOf <http://rdaregistry.info/Elements/u/P60015> ;
    skos:definition "Relates a resource to a jurisdiction governed by a law, regulation, etc., that was enacted by another jurisdiction."@en .

<http://rdaregistry.info/Elements/u/P60098>
    reg:hasSubproperty <http://rdaregistry.info/Elements/a/P50023>, <http://rdaregistry.info/Elements/a/P50102>, <http://rdaregistry.info/Elements/a/P50235> ;
    reg:lexicalAlias <http://rdaregistry.info/Elements/u/languageOfTheAgent.en> ;
    reg:name "languageOfTheAgent"@en ;
    reg:status <http://metadataregistry.org/uri/RegStatus/1001> ;
    a rdf:Property ;
    rdfs:isDefinedBy <http://rdaregistry.info/Elements/u/> ;
    rdfs:label "has language of the agent"@en ;
    skos:definition "Relates a resource to a language an agent uses in its communications, when writing for publication, broadcasting, etc."@en .

<http://rdaregistry.info/Elements/u/P60099>
    reg:hasSubproperty <http://rdaregistry.info/Elements/e/P20006>, <http://rdaregistry.info/Elements/e/P20007> ;
    reg:lexicalAlias <http://rdaregistry.info/Elements/u/languageOfTheContent.en> ;
    reg:name "languageOfTheContent"@en ;
    reg:status <http://metadataregistry.org/uri/RegStatus/1001> ;
    a rdf:Property ;
    rdfs:isDefinedBy <http://rdaregistry.info/Elements/u/> ;
    rdfs:label "has language of the content"@en ;
    skos:definition "Relates a resource to a language used to express the content of a resource."@en .

<http://rdaregistry.info/Elements/u/P60100>
    reg:hasSubproperty <http://rdaregistry.info/Elements/m/P30019> ;
    reg:lexicalAlias <http://rdaregistry.info/Elements/u/facsimileContainedIn.en> ;
    reg:name "facsimileContainedIn"@en ;
    reg:status <http://metadataregistry.org/uri/RegStatus/1001> ;
    a rdf:Property ;
    rdfs:isDefinedBy <http://rdaregistry.info/Elements/u/> ;
    rdfs:label "is facsimile contained in"@en ;
    rdfs:subPropertyOf <http://rdaregistry.info/Elements/u/P60101> ;
    owl:inverseOf <http://rdaregistry.info/Elements/u/P60300> ;
    skos:definition "Relates a resource to a larger resource of which a part is a discrete component that exactly reproduces another resource embodying the resource."@en .

<http://rdaregistry.info/Elements/u/P60101>
    reg:hasSubproperty <http://rdaregistry.info/Elements/e/P20074>, <http://rdaregistry.info/Elements/i/P40009>, <http://rdaregistry.info/Elements/m/P30020>, <http://rdaregistry.info/Elements/u/P60100>, <http://rdaregistry.info/Elements/u/P60192>, <http://rdaregistry.info/Elements/u/P60193>, <http://rdaregistry.info/Elements/u/P60194>, <http://rdaregistry.info/Elements/u/P60317> ;
    reg:lexicalAlias <http://rdaregistry.info/Elements/u/containedIn.en> ;
    reg:name "containedIn"@en ;
    reg:status <http://metadataregistry.org/uri/RegStatus/1001> ;
    a rdf:Property ;
    rdfs:isDefinedBy <http://rdaregistry.info/Elements/u/> ;
    rdfs:label "is contained in"@en ;
    rdfs:subPropertyOf <http://rdaregistry.info/Elements/u/P60714> ;
    owl:inverseOf <http://rdaregistry.info/Elements/u/P60249> ;
    skos:definition "Relates a resource to a larger resource of which a part is a discrete component."@en .

<http://rdaregistry.info/Elements/u/P60102>
    reg:lexicalAlias <http://rdaregistry.info/Elements/u/sequel.en> ;
    reg:name "sequel"@en ;
    reg:status <http://metadataregistry.org/uri/RegStatus/1001> ;
    a rdf:Property ;
    rdfs:isDefinedBy <http://rdaregistry.info/Elements/u/> ;
    rdfs:label "is sequel"@en ;
    rdfs:subPropertyOf <http://rdaregistry.info/Elements/u/P60278> ;
    owl:inverseOf <http://rdaregistry.info/Elements/u/P60577> ;
    skos:definition "Relates a resource to a later resource that continues the narrative of an earlier resource."@en .

<http://rdaregistry.info/Elements/u/P60103>
    reg:hasSubproperty <http://rdaregistry.info/Elements/e/P20075> ;
    reg:lexicalAlias <http://rdaregistry.info/Elements/u/replacedInPartBy.en> ;
    reg:name "replacedInPartBy"@en ;
    reg:status <http://metadataregistry.org/uri/RegStatus/1001> ;
    a rdf:Property ;
    rdfs:isDefinedBy <http://rdaregistry.info/Elements/u/> ;
    rdfs:label "is replaced in part by"@en ;
    rdfs:subPropertyOf <http://rdaregistry.info/Elements/u/P60278> ;
    owl:inverseOf <http://rdaregistry.info/Elements/u/P60479> ;
    skos:definition "Relates a resource to a later resource used in part in place of an earlier resource, usually because the later resource contains updated or new information that makes part of the earlier resource obsolete."@en .

<http://rdaregistry.info/Elements/u/P60104>
    reg:hasSubproperty <http://rdaregistry.info/Elements/e/P20076> ;
    reg:lexicalAlias <http://rdaregistry.info/Elements/u/replacedBy.en> ;
    reg:name "replacedBy"@en ;
    reg:status <http://metadataregistry.org/uri/RegStatus/1001> ;
    a rdf:Property ;
    rdfs:isDefinedBy <http://rdaregistry.info/Elements/u/> ;
    rdfs:label "is replaced by"@en ;
    rdfs:subPropertyOf <http://rdaregistry.info/Elements/u/P60278> ;
    owl:inverseOf <http://rdaregistry.info/Elements/u/P60480> ;
    skos:definition "Relates a resource to a later resource used in place of an earlier resource, usually because the later resource contains updated or new information that makes the earlier resource obsolete."@en .

<http://rdaregistry.info/Elements/u/P60105>
    reg:status <http://metadataregistry.org/uri/RegStatus/1008> ;
    rdfs:isDefinedBy <http://rdaregistry.info/Elements/u/> .

<http://rdaregistry.info/Elements/u/P60106>
    reg:hasSubproperty <http://rdaregistry.info/Elements/e/P20077> ;
    reg:lexicalAlias <http://rdaregistry.info/Elements/u/adaptedInVerseAs.en> ;
    reg:name "adaptedInVerseAs"@en ;
    reg:status <http://metadataregistry.org/uri/RegStatus/1001> ;
    a rdf:Property ;
    rdfs:isDefinedBy <http://rdaregistry.info/Elements/u/> ;
    rdfs:label "is adapted in verse as"@en ;
    rdfs:subPropertyOf <http://rdaregistry.info/Elements/u/P60260> ;
    owl:inverseOf <http://rdaregistry.info/Elements/u/P60226> ;
    skos:definition "Relates a resource to a literary composition in verse form adapted from the source resource."@en .

<http://rdaregistry.info/Elements/u/P60107>
    reg:hasSubproperty <http://rdaregistry.info/Elements/a/P50024> ;
    reg:lexicalAlias <http://rdaregistry.info/Elements/u/locationOfConferenceEtc.en> ;
    reg:name "locationOfConferenceEtc"@en ;
    reg:status <http://metadataregistry.org/uri/RegStatus/1001> ;
    a rdf:Property ;
    rdfs:isDefinedBy <http://rdaregistry.info/Elements/u/> ;
    rdfs:label "has location of conference, etc."@en ;
    rdfs:subPropertyOf <http://rdaregistry.info/Elements/u/P60325> ;
    skos:definition "Relates a resource to a local place in which a conference, congress, meeting, exhibition, fair, festival, etc., was held."@en .

<http://rdaregistry.info/Elements/u/P60108>
    reg:hasSubproperty <http://rdaregistry.info/Elements/m/P30049> ;
    reg:lexicalAlias <http://rdaregistry.info/Elements/u/parallelManufacturersName.en> ;
    reg:name "parallelManufacturersName"@en ;
    reg:status <http://metadataregistry.org/uri/RegStatus/1001> ;
    a rdf:Property ;
    rdfs:isDefinedBy <http://rdaregistry.info/Elements/u/> ;
    rdfs:label "has parallel manufacturer’s name"@en ;
    skos:definition "Relates a resource to a manufacturer's name in a language and/or script that differs from that recorded in the manufacturer's name element."@en .

<http://rdaregistry.info/Elements/u/P60109>
    reg:hasSubproperty <http://rdaregistry.info/Elements/u/P60345>, <http://rdaregistry.info/Elements/u/P60346>, <http://rdaregistry.info/Elements/u/P60347> ;
    reg:lexicalAlias <http://rdaregistry.info/Elements/u/coordinatesOfCartographicContent.en> ;
    reg:name "coordinatesOfCartographicContent"@en ;
    reg:status <http://metadataregistry.org/uri/RegStatus/1001> ;
    a rdf:Property ;
    rdfs:isDefinedBy <http://rdaregistry.info/Elements/u/> ;
    rdfs:label "has coordinates of cartographic content"@en ;
    skos:definition "Relates a resource to a mathematical system for identifying the area covered by the cartographic content of a resource."@en .

<http://rdaregistry.info/Elements/u/P60110>
    reg:hasSubproperty <http://rdaregistry.info/Elements/e/P20009> ;
    reg:lexicalAlias <http://rdaregistry.info/Elements/u/adaptedAsAMotionPicture.en> ;
    reg:name "adaptedAsAMotionPicture"@en ;
    reg:status <http://metadataregistry.org/uri/RegStatus/1001> ;
    a rdf:Property ;
    rdfs:isDefinedBy <http://rdaregistry.info/Elements/u/> ;
    rdfs:label "is adapted as motion picture"@en ;
    rdfs:subPropertyOf <http://rdaregistry.info/Elements/u/P60260> ;
    owl:inverseOf <http://rdaregistry.info/Elements/u/P60227> ;
    skos:definition "Relates a resource to a motion picture based on the source resource."@en .

<http://rdaregistry.info/Elements/u/P60111>
    reg:hasSubproperty <http://rdaregistry.info/Elements/e/P20078> ;
    reg:lexicalAlias <http://rdaregistry.info/Elements/u/dubbedVersionOf.en> ;
    reg:name "dubbedVersionOf"@en ;
    reg:status <http://metadataregistry.org/uri/RegStatus/1001> ;
    a rdf:Property ;
    rdfs:isDefinedBy <http://rdaregistry.info/Elements/u/> ;
    rdfs:label "is dubbed version of"@en ;
    rdfs:subPropertyOf <http://rdaregistry.info/Elements/u/P60244> ;
    owl:inverseOf <http://rdaregistry.info/Elements/u/P60112> ;
    skos:definition "Relates a resource to a moving image resource in which the spoken dialogue has been translated into a language different from that of the original resource."@en .

<http://rdaregistry.info/Elements/u/P60112>
    reg:hasSubproperty <http://rdaregistry.info/Elements/e/P20079> ;
    reg:lexicalAlias <http://rdaregistry.info/Elements/u/dubbedVersion.en> ;
    reg:name "dubbedVersion"@en ;
    reg:status <http://metadataregistry.org/uri/RegStatus/1001> ;
    a rdf:Property ;
    rdfs:isDefinedBy <http://rdaregistry.info/Elements/u/> ;
    rdfs:label "is dubbed version"@en ;
    rdfs:subPropertyOf <http://rdaregistry.info/Elements/u/P60280> ;
    owl:inverseOf <http://rdaregistry.info/Elements/u/P60111> ;
    skos:definition "Relates a resource to a moving image resource that translates the spoken dialogue of the original resource into a different language."@en .

<http://rdaregistry.info/Elements/u/P60113>
    reg:hasSubproperty <http://rdaregistry.info/Elements/e/P20080> ;
    reg:lexicalAlias <http://rdaregistry.info/Elements/u/cadenza.en> ;
    reg:name "cadenza"@en ;
    reg:status <http://metadataregistry.org/uri/RegStatus/1001> ;
    a rdf:Property ;
    rdfs:isDefinedBy <http://rdaregistry.info/Elements/u/> ;
    rdfs:label "is cadenza"@en ;
    rdfs:subPropertyOf <http://rdaregistry.info/Elements/u/P60204> ;
    owl:inverseOf <http://rdaregistry.info/Elements/u/P60116> ;
    skos:definition "Relates a resource to a musical resource consisting of an ornamental passage for a soloist, added to a musical resource such as a concerto, either by the same or a different composer."@en .

<http://rdaregistry.info/Elements/u/P60114>
    reg:hasSubproperty <http://rdaregistry.info/Elements/e/P20081> ;
    reg:lexicalAlias <http://rdaregistry.info/Elements/u/variationsBasedOn.en> ;
    reg:name "variationsBasedOn"@en ;
    reg:status <http://metadataregistry.org/uri/RegStatus/1001> ;
    a rdf:Property ;
    rdfs:isDefinedBy <http://rdaregistry.info/Elements/u/> ;
    rdfs:label "is variations based on"@en ;
    rdfs:subPropertyOf <http://rdaregistry.info/Elements/u/P60305> ;
    owl:inverseOf <http://rdaregistry.info/Elements/u/P60115> ;
    skos:definition "Relates a resource to a musical resource from which melodic, thematic, or harmonic material is taken to form a discrete theme, which is repeated one or more times with subsequent modifications."@en .

<http://rdaregistry.info/Elements/u/P60115>
    reg:hasSubproperty <http://rdaregistry.info/Elements/e/P20082> ;
    reg:lexicalAlias <http://rdaregistry.info/Elements/u/modifiedByVariationAs.en> ;
    reg:name "modifiedByVariationAs"@en ;
    reg:status <http://metadataregistry.org/uri/RegStatus/1001> ;
    a rdf:Property ;
    rdfs:isDefinedBy <http://rdaregistry.info/Elements/u/> ;
    rdfs:label "is modified by variation as"@en ;
    rdfs:subPropertyOf <http://rdaregistry.info/Elements/u/P60250> ;
    owl:inverseOf <http://rdaregistry.info/Elements/u/P60114> ;
    skos:definition "Relates a resource to a musical resource in which melodic, thematic, or harmonic material taken from the source resource forms a discrete theme, which is repeated one or more times with subsequent modifications."@en .

<http://rdaregistry.info/Elements/u/P60116>
    reg:hasSubproperty <http://rdaregistry.info/Elements/e/P20083> ;
    reg:lexicalAlias <http://rdaregistry.info/Elements/u/cadenzaComposedFor.en> ;
    reg:name "cadenzaComposedFor"@en ;
    reg:status <http://metadataregistry.org/uri/RegStatus/1001> ;
    a rdf:Property ;
    rdfs:isDefinedBy <http://rdaregistry.info/Elements/u/> ;
    rdfs:label "is cadenza composed for"@en ;
    rdfs:subPropertyOf <http://rdaregistry.info/Elements/u/P60307> ;
    owl:inverseOf <http://rdaregistry.info/Elements/u/P60113> ;
    skos:definition "Relates a resource to a musical resource such as a concerto for which an ornamental passage for a soloist has been composed, either by the same or a different composer."@en .

<http://rdaregistry.info/Elements/u/P60117>
    reg:hasSubproperty <http://rdaregistry.info/Elements/e/P20084> ;
    reg:lexicalAlias <http://rdaregistry.info/Elements/u/librettoFor.en> ;
    reg:name "librettoFor"@en ;
    reg:status <http://metadataregistry.org/uri/RegStatus/1001> ;
    a rdf:Property ;
    rdfs:isDefinedBy <http://rdaregistry.info/Elements/u/> ;
    rdfs:label "is libretto for"@en ;
    rdfs:subPropertyOf <http://rdaregistry.info/Elements/u/P60198> ;
    owl:inverseOf <http://rdaregistry.info/Elements/u/P60270> ;
    skos:definition "Relates a resource to a musical resource such as an opera or other resource for the musical stage, or an oratorio, that uses the text of the related resource as a libretto."@en .

<http://rdaregistry.info/Elements/u/P60118>
    reg:hasSubproperty <http://rdaregistry.info/Elements/e/P20085> ;
    reg:lexicalAlias <http://rdaregistry.info/Elements/u/incidentalMusic.en> ;
    reg:name "incidentalMusic"@en ;
    reg:status <http://metadataregistry.org/uri/RegStatus/1001> ;
    a rdf:Property ;
    rdfs:isDefinedBy <http://rdaregistry.info/Elements/u/> ;
    rdfs:label "is incidental music"@en ;
    rdfs:subPropertyOf <http://rdaregistry.info/Elements/u/P60723> ;
    owl:inverseOf <http://rdaregistry.info/Elements/u/P60202> ;
    skos:definition "Relates a resource to a musical resource that provides the incidental music for a play or other spoken work for the stage."@en .

<http://rdaregistry.info/Elements/u/P60119>
    reg:hasSubproperty <http://rdaregistry.info/Elements/a/P50025>, <http://rdaregistry.info/Elements/a/P50054>, <http://rdaregistry.info/Elements/a/P50103> ;
    reg:lexicalAlias <http://rdaregistry.info/Elements/u/variantNameForTheAgent.en> ;
    reg:name "variantNameForTheAgent"@en ;
    reg:status <http://metadataregistry.org/uri/RegStatus/1001> ;
    a rdf:Property ;
    rdfs:isDefinedBy <http://rdaregistry.info/Elements/u/> ;
    rdfs:label "has variant name for the agent"@en ;
    rdfs:subPropertyOf <http://rdaregistry.info/Elements/u/P60368> ;
    skos:definition "Relates a resource to a name or form of name by which an agent is known that differs from the name or form of name chosen as the preferred name."@en .

<http://rdaregistry.info/Elements/u/P60120>
    reg:hasSubproperty <http://rdaregistry.info/Elements/e/P20086> ;
    reg:lexicalAlias <http://rdaregistry.info/Elements/u/remadeAs.en> ;
    reg:name "remadeAs"@en ;
    reg:status <http://metadataregistry.org/uri/RegStatus/1001> ;
    a rdf:Property ;
    rdfs:isDefinedBy <http://rdaregistry.info/Elements/u/> ;
    rdfs:label "is remade as"@en ;
    rdfs:subPropertyOf <http://rdaregistry.info/Elements/u/P60250> ;
    owl:inverseOf <http://rdaregistry.info/Elements/u/P60295> ;
    skos:definition "Relates a resource to a new motion picture, radio program, television program, or video based on an earlier resource."@en .

<http://rdaregistry.info/Elements/u/P60121>
    reg:hasSubproperty <http://rdaregistry.info/Elements/e/P20087> ;
    reg:lexicalAlias <http://rdaregistry.info/Elements/u/setToMusicAs.en> ;
    reg:name "setToMusicAs"@en ;
    reg:status <http://metadataregistry.org/uri/RegStatus/1001> ;
    a rdf:Property ;
    rdfs:isDefinedBy <http://rdaregistry.info/Elements/u/> ;
    rdfs:label "is set to music as"@en ;
    rdfs:subPropertyOf <http://rdaregistry.info/Elements/u/P60250> ;
    owl:inverseOf <http://rdaregistry.info/Elements/u/P60266> ;
    skos:definition "Relates a resource to a non-dramatic musical resource, other than an oratorio, that uses the text of the source resource."@en .

<http://rdaregistry.info/Elements/u/P60122>
    reg:hasSubproperty <http://rdaregistry.info/Elements/m/P30050> ;
    reg:lexicalAlias <http://rdaregistry.info/Elements/u/noteOnIssuePartOrIterationUsedAsTheBasisForIdentificationOfTheResource.en> ;
    reg:name "noteOnIssuePartOrIterationUsedAsTheBasisForIdentificationOfTheResource"@en ;
    reg:status <http://metadataregistry.org/uri/RegStatus/1001> ;
    a rdf:Property ;
    rdfs:isDefinedBy <http://rdaregistry.info/Elements/u/> ;
    rdfs:label "has note on issue, part, or iteration used as the basis for identification of the resource"@en ;
    rdfs:subPropertyOf <http://rdaregistry.info/Elements/u/P60470> ;
    skos:definition "Relates a resource to a note identifying the issue or part of a multipart monograph or serial, or the iteration of an integrating resource that has been used as the basis for the identification of a resource."@en .

<http://rdaregistry.info/Elements/u/P60123>
    reg:hasSubproperty <http://rdaregistry.info/Elements/e/P20010> ;
    reg:lexicalAlias <http://rdaregistry.info/Elements/u/noteOnChangesInContentCharacteristics.en> ;
    reg:name "noteOnChangesInContentCharacteristics"@en ;
    reg:status <http://metadataregistry.org/uri/RegStatus/1001> ;
    a rdf:Property ;
    rdfs:isDefinedBy <http://rdaregistry.info/Elements/u/> ;
    rdfs:label "has note on changes in content characteristics"@en ;
    rdfs:subPropertyOf <http://rdaregistry.info/Elements/u/P60470> ;
    skos:definition "Relates a resource to a note on changes in content characteristics that occur in subsequent issues or parts of a resource issued in successive parts or between iterations of an integrating resource."@en .

<http://rdaregistry.info/Elements/u/P60124>
    reg:hasSubproperty <http://rdaregistry.info/Elements/m/P30051> ;
    reg:lexicalAlias <http://rdaregistry.info/Elements/u/noteOnChangesInCarrierCharacteristics.en> ;
    reg:name "noteOnChangesInCarrierCharacteristics"@en ;
    reg:status <http://metadataregistry.org/uri/RegStatus/1001> ;
    a rdf:Property ;
    rdfs:isDefinedBy <http://rdaregistry.info/Elements/u/> ;
    rdfs:label "has note on changes in carrier characteristics"@en ;
    rdfs:subPropertyOf <http://rdaregistry.info/Elements/u/P60470> ;
    skos:definition "Relates a resource to a note on changes in the characteristics of the carrier that occur in subsequent issues or parts of a resource issued in successive parts or between iterations of an integrating resource."@en .

<http://rdaregistry.info/Elements/u/P60125>
    reg:hasSubproperty <http://rdaregistry.info/Elements/m/P30052> ;
    reg:lexicalAlias <http://rdaregistry.info/Elements/u/noteOnDistributionStatement.en> ;
    reg:name "noteOnDistributionStatement"@en ;
    reg:status <http://metadataregistry.org/uri/RegStatus/1001> ;
    a rdf:Property ;
    rdfs:isDefinedBy <http://rdaregistry.info/Elements/u/> ;
    rdfs:label "has note on distribution statement"@en ;
    rdfs:subPropertyOf <http://rdaregistry.info/Elements/u/P60470> ;
    skos:definition "Relates a resource to a note providing details on place of distribution, distributor, or date of distribution, or information on changes in the place of distribution, distributor, or distributor’s name."@en .

<http://rdaregistry.info/Elements/u/P60126>
    reg:hasSubproperty <http://rdaregistry.info/Elements/m/P30053> ;
    reg:lexicalAlias <http://rdaregistry.info/Elements/u/noteOnManufactureStatement.en> ;
    reg:name "noteOnManufactureStatement"@en ;
    reg:status <http://metadataregistry.org/uri/RegStatus/1001> ;
    a rdf:Property ;
    rdfs:isDefinedBy <http://rdaregistry.info/Elements/u/> ;
    rdfs:label "has note on manufacture statement"@en ;
    rdfs:subPropertyOf <http://rdaregistry.info/Elements/u/P60470> ;
    skos:definition "Relates a resource to a note providing details on place of manufacture, manufacturer, or date of manufacture, or information on changes in the place of manufacture, manufacturer, or manufacturer’s name."@en .

<http://rdaregistry.info/Elements/u/P60127>
    reg:hasSubproperty <http://rdaregistry.info/Elements/m/P30054> ;
    reg:lexicalAlias <http://rdaregistry.info/Elements/u/noteOnProductionStatement.en> ;
    reg:name "noteOnProductionStatement"@en ;
    reg:status <http://metadataregistry.org/uri/RegStatus/1001> ;
    a rdf:Property ;
    rdfs:isDefinedBy <http://rdaregistry.info/Elements/u/> ;
    rdfs:label "has note on production statement"@en ;
    rdfs:subPropertyOf <http://rdaregistry.info/Elements/u/P60470> ;
    skos:definition "Relates a resource to a note providing details on place of production, producer, or date of production, or information on changes in the place of production, producer, or producer’s name."@en .

<http://rdaregistry.info/Elements/u/P60128>
    reg:hasSubproperty <http://rdaregistry.info/Elements/m/P30055> ;
    reg:lexicalAlias <http://rdaregistry.info/Elements/u/noteOnPublicationStatement.en> ;
    reg:name "noteOnPublicationStatement"@en ;
    reg:status <http://metadataregistry.org/uri/RegStatus/1001> ;
    a rdf:Property ;
    rdfs:isDefinedBy <http://rdaregistry.info/Elements/u/> ;
    rdfs:label "has note on publication statement"@en ;
    rdfs:subPropertyOf <http://rdaregistry.info/Elements/u/P60470> ;
    skos:definition "Relates a resource to a note providing details on place of publication, publisher, or date of publication, information on changes in the place of publication, publisher, or publisher’s name, or on suspension of publication."@en .

<http://rdaregistry.info/Elements/u/P60129>
    reg:hasSubproperty <http://rdaregistry.info/Elements/m/P30056> ;
    reg:lexicalAlias <http://rdaregistry.info/Elements/u/noteOnFrequency.en> ;
    reg:name "noteOnFrequency"@en ;
    reg:status <http://metadataregistry.org/uri/RegStatus/1001> ;
    a rdf:Property ;
    rdfs:isDefinedBy <http://rdaregistry.info/Elements/u/> ;
    rdfs:label "has note on frequency"@en ;
    rdfs:subPropertyOf <http://rdaregistry.info/Elements/u/P60470> ;
    skos:definition "Relates a resource to a note providing details on the currency of the contents, on the frequency of release of issues or parts of a serial or the frequency of updates to an integrating resource, or on changes in frequency."@en .

<http://rdaregistry.info/Elements/u/P60130>
    reg:hasSubproperty <http://rdaregistry.info/Elements/m/P30057> ;
    reg:lexicalAlias <http://rdaregistry.info/Elements/u/noteOnStatementOfResponsibility.en> ;
    reg:name "noteOnStatementOfResponsibility"@en ;
    reg:status <http://metadataregistry.org/uri/RegStatus/1001> ;
    a rdf:Property ;
    rdfs:isDefinedBy <http://rdaregistry.info/Elements/u/> ;
    rdfs:label "has note on statement of responsibility"@en ;
    rdfs:subPropertyOf <http://rdaregistry.info/Elements/u/P60470> ;
    skos:definition "Relates a resource to a note providing information on an agent not named in a statement of responsibility to whom responsibility for the intellectual or artistic content of the resource has been attributed, on variant forms of names appearing in the resource, on changes in statements of responsibility, or on other details relating to a statement of responsibility."@en .

<http://rdaregistry.info/Elements/u/P60131>
    reg:hasSubproperty <http://rdaregistry.info/Elements/m/P30058> ;
    reg:lexicalAlias <http://rdaregistry.info/Elements/u/noteOnSeriesStatement.en> ;
    reg:name "noteOnSeriesStatement"@en ;
    reg:status <http://metadataregistry.org/uri/RegStatus/1001> ;
    a rdf:Property ;
    rdfs:isDefinedBy <http://rdaregistry.info/Elements/u/> ;
    rdfs:label "has note on series statement"@en ;
    rdfs:subPropertyOf <http://rdaregistry.info/Elements/u/P60470> ;
    skos:definition "Relates a resource to a note providing information on complex series statements, incorrect numbering within series, or changes in series statements."@en .

<http://rdaregistry.info/Elements/u/P60132>
    reg:hasSubproperty <http://rdaregistry.info/Elements/m/P30059> ;
    reg:lexicalAlias <http://rdaregistry.info/Elements/u/noteOnCopyrightDate.en> ;
    reg:name "noteOnCopyrightDate"@en ;
    reg:status <http://metadataregistry.org/uri/RegStatus/1001> ;
    a rdf:Property ;
    rdfs:isDefinedBy <http://rdaregistry.info/Elements/u/> ;
    rdfs:label "has note on copyright date"@en ;
    rdfs:subPropertyOf <http://rdaregistry.info/Elements/u/P60470> ;
    skos:definition "Relates a resource to a note providing information on copyright dates not recorded as part of the copyright date element."@en .

<http://rdaregistry.info/Elements/u/P60133>
    reg:hasSubproperty <http://rdaregistry.info/Elements/i/P40010>, <http://rdaregistry.info/Elements/m/P30060> ;
    reg:lexicalAlias <http://rdaregistry.info/Elements/u/noteOnDimensionsOfResource.en> ;
    reg:name "noteOnDimensionsOfResource"@en ;
    reg:status <http://metadataregistry.org/uri/RegStatus/1001> ;
    a rdf:Property ;
    rdfs:isDefinedBy <http://rdaregistry.info/Elements/u/> ;
    rdfs:label "has note on dimensions of resource"@en ;
    rdfs:subPropertyOf <http://rdaregistry.info/Elements/u/P60470> ;
    skos:definition "Relates a resource to a note providing information on the dimensions of a resource that is not recorded as part of the dimensions element."@en .

<http://rdaregistry.info/Elements/u/P60134>
    reg:hasSubproperty <http://rdaregistry.info/Elements/i/P40011>, <http://rdaregistry.info/Elements/m/P30061> ;
    reg:lexicalAlias <http://rdaregistry.info/Elements/u/noteOnExtentOfResource.en> ;
    reg:name "noteOnExtentOfResource"@en ;
    reg:status <http://metadataregistry.org/uri/RegStatus/1001> ;
    a rdf:Property ;
    rdfs:isDefinedBy <http://rdaregistry.info/Elements/u/> ;
    rdfs:label "has note on extent of resource"@en ;
    rdfs:subPropertyOf <http://rdaregistry.info/Elements/u/P60470> ;
    skos:definition "Relates a resource to a note providing information on the extent of a resource that is not recorded as part of the extent element."@en .

<http://rdaregistry.info/Elements/u/P60135>
    reg:hasSubproperty <http://rdaregistry.info/Elements/m/P30062> ;
    reg:lexicalAlias <http://rdaregistry.info/Elements/u/noteOnNumberingOfSerials.en> ;
    reg:name "noteOnNumberingOfSerials"@en ;
    reg:status <http://metadataregistry.org/uri/RegStatus/1001> ;
    a rdf:Property ;
    rdfs:isDefinedBy <http://rdaregistry.info/Elements/u/> ;
    rdfs:label "has note on numbering of serials"@en ;
    rdfs:subPropertyOf <http://rdaregistry.info/Elements/u/P60470> ;
    skos:definition "Relates a resource to a note providing information on the numbering of the first and/or last issue or part, on complex or irregular numbering (including numbering errors), or on the period covered by a volume, issue, part, etc."@en .

<http://rdaregistry.info/Elements/u/P60136>
    reg:hasSubproperty <http://rdaregistry.info/Elements/m/P30063> ;
    reg:lexicalAlias <http://rdaregistry.info/Elements/u/noteOnTitle.en> ;
    reg:name "noteOnTitle"@en ;
    reg:status <http://metadataregistry.org/uri/RegStatus/1001> ;
    a rdf:Property ;
    rdfs:isDefinedBy <http://rdaregistry.info/Elements/u/> ;
    rdfs:label "has note on title"@en ;
    rdfs:subPropertyOf <http://rdaregistry.info/Elements/u/P60470> ;
    skos:definition "Relates a resource to a note providing information on the source from which a title was taken, the date the title was viewed, variations in titles, inaccuracies, deletions, etc., or other information relating to a title."@en .

<http://rdaregistry.info/Elements/u/P60137>
    reg:hasSubproperty <http://rdaregistry.info/Elements/m/P30064> ;
    reg:lexicalAlias <http://rdaregistry.info/Elements/u/noteOnEditionStatement.en> ;
    reg:name "noteOnEditionStatement"@en ;
    reg:status <http://metadataregistry.org/uri/RegStatus/1001> ;
    a rdf:Property ;
    rdfs:isDefinedBy <http://rdaregistry.info/Elements/u/> ;
    rdfs:label "has note on edition statement"@en ;
    rdfs:subPropertyOf <http://rdaregistry.info/Elements/u/P60470> ;
    skos:definition "Relates a resource to a note providing information on the source of an edition statement, on edition statements relating to issues, parts, etc., on changes in edition statements, or other information relating to an edition statement."@en .

<http://rdaregistry.info/Elements/u/P60138>
    reg:hasSubproperty <http://rdaregistry.info/Elements/e/P20088> ;
    reg:lexicalAlias <http://rdaregistry.info/Elements/u/adaptedAsNovel.en> ;
    reg:name "novelization"@en ;
    reg:status <http://metadataregistry.org/uri/RegStatus/1001> ;
    a rdf:Property ;
    rdfs:isDefinedBy <http://rdaregistry.info/Elements/u/> ;
    rdfs:label "is adapted as novel"@en ;
    rdfs:subPropertyOf <http://rdaregistry.info/Elements/u/P60260> ;
    owl:inverseOf <http://rdaregistry.info/Elements/u/P60228> ;
    skos:definition "Relates a resource to a novel adapted from the source resource."@en .

<http://rdaregistry.info/Elements/u/P60139>
    reg:hasSubproperty <http://rdaregistry.info/Elements/m/P30065> ;
    reg:lexicalAlias <http://rdaregistry.info/Elements/u/publishersNumberForMusic.en> ;
    reg:name "publishersNumberForMusic"@en ;
    reg:status <http://metadataregistry.org/uri/RegStatus/1001> ;
    a rdf:Property ;
    rdfs:isDefinedBy <http://rdaregistry.info/Elements/u/> ;
    rdfs:label "has publisher’s number for music"@en ;
    rdfs:subPropertyOf <http://rdaregistry.info/Elements/u/P60052> ;
    skos:definition "Relates a resource to a numbering designation assigned to a resource by a music publisher, appearing normally only on the title page, the cover, and/or the first page of music."@en .

<http://rdaregistry.info/Elements/u/P60140>
    reg:hasSubproperty <http://rdaregistry.info/Elements/m/P30066> ;
    reg:lexicalAlias <http://rdaregistry.info/Elements/u/plateNumberForMusic.en> ;
    reg:name "plateNumberForMusic"@en ;
    reg:status <http://metadataregistry.org/uri/RegStatus/1001> ;
    a rdf:Property ;
    rdfs:isDefinedBy <http://rdaregistry.info/Elements/u/> ;
    rdfs:label "has plate number for music"@en ;
    rdfs:subPropertyOf <http://rdaregistry.info/Elements/u/P60052> ;
    skos:definition "Relates a resource to a numbering designation assigned to a resource by a music publisher."@en .

<http://rdaregistry.info/Elements/u/P60141>
    reg:hasSubproperty <http://rdaregistry.info/Elements/e/P20011>, <http://rdaregistry.info/Elements/u/P60842>, <http://rdaregistry.info/Elements/u/P60844> ;
    reg:lexicalAlias <http://rdaregistry.info/Elements/u/conductor.en> ;
    reg:name "conductor"@en ;
    reg:status <http://metadataregistry.org/uri/RegStatus/1001> ;
    a rdf:Property ;
    rdfs:isDefinedBy <http://rdaregistry.info/Elements/u/> ;
    rdfs:label "has conductor"@en ;
    rdfs:subPropertyOf <http://rdaregistry.info/Elements/u/P60387> ;
    owl:inverseOf <http://rdaregistry.info/Elements/u/P60016> ;
    skos:definition "Relates a resource to a performer contributing to a musical resource by leading a performing group (orchestra, chorus, opera, etc.) in a musical or dramatic presentation, etc."@en .

<http://rdaregistry.info/Elements/u/P60142>
    reg:hasSubproperty <http://rdaregistry.info/Elements/e/P20012>, <http://rdaregistry.info/Elements/u/P60152> ;
    reg:lexicalAlias <http://rdaregistry.info/Elements/u/actor.en> ;
    reg:name "actor"@en ;
    reg:status <http://metadataregistry.org/uri/RegStatus/1001> ;
    a rdf:Property ;
    rdfs:isDefinedBy <http://rdaregistry.info/Elements/u/> ;
    rdfs:label "has actor"@en ;
    rdfs:subPropertyOf <http://rdaregistry.info/Elements/u/P60387> ;
    owl:inverseOf <http://rdaregistry.info/Elements/u/P60017> ;
    skos:definition "Relates a resource to a performer contributing to a resource by acting as a cast member or player in a musical or dramatic presentation, etc."@en .

<http://rdaregistry.info/Elements/u/P60143>
    reg:hasSubproperty <http://rdaregistry.info/Elements/e/P20013> ;
    reg:lexicalAlias <http://rdaregistry.info/Elements/u/onScreenPresenter.en> ;
    reg:name "onScreenPresenter"@en ;
    reg:status <http://metadataregistry.org/uri/RegStatus/1001> ;
    a rdf:Property ;
    rdfs:isDefinedBy <http://rdaregistry.info/Elements/u/> ;
    rdfs:label "has on-screen presenter"@en ;
    rdfs:subPropertyOf <http://rdaregistry.info/Elements/u/P60387> ;
    owl:inverseOf <http://rdaregistry.info/Elements/u/P60018> ;
    skos:definition "Relates a resource to a performer contributing to a resource by appearing on screen to provide contextual or background information. an on-screen presenter may appear in nonfiction moving image materials or in introductions to fiction moving image materials."@en .

<http://rdaregistry.info/Elements/u/P60144>
    reg:hasSubproperty <http://rdaregistry.info/Elements/e/P20014> ;
    reg:lexicalAlias <http://rdaregistry.info/Elements/u/dancer.en> ;
    reg:name "dancer"@en ;
    reg:status <http://metadataregistry.org/uri/RegStatus/1001> ;
    a rdf:Property ;
    rdfs:isDefinedBy <http://rdaregistry.info/Elements/u/> ;
    rdfs:label "has dancer"@en ;
    rdfs:subPropertyOf <http://rdaregistry.info/Elements/u/P60387> ;
    owl:inverseOf <http://rdaregistry.info/Elements/u/P60019> ;
    skos:definition "Relates a resource to a performer contributing to a resource by dancing in a musical, dramatic, etc., presentation."@en .

<http://rdaregistry.info/Elements/u/P60145>
    reg:hasSubproperty <http://rdaregistry.info/Elements/e/P20015> ;
    reg:lexicalAlias <http://rdaregistry.info/Elements/u/teacher.en> ;
    reg:name "teacher"@en ;
    reg:status <http://metadataregistry.org/uri/RegStatus/1001> ;
    a rdf:Property ;
    rdfs:isDefinedBy <http://rdaregistry.info/Elements/u/> ;
    rdfs:label "has teacher"@en ;
    rdfs:subPropertyOf <http://rdaregistry.info/Elements/u/P60387> ;
    owl:inverseOf <http://rdaregistry.info/Elements/u/P60020> ;
    skos:definition "Relates a resource to a performer contributing to a resource by giving instruction or providing a demonstration."@en .

<http://rdaregistry.info/Elements/u/P60146>
    reg:hasSubproperty <http://rdaregistry.info/Elements/e/P20016> ;
    reg:lexicalAlias <http://rdaregistry.info/Elements/u/host.en> ;
    reg:name "host"@en ;
    reg:status <http://metadataregistry.org/uri/RegStatus/1001> ;
    a rdf:Property ;
    rdfs:isDefinedBy <http://rdaregistry.info/Elements/u/> ;
    rdfs:label "has host"@en ;
    rdfs:subPropertyOf <http://rdaregistry.info/Elements/u/P60387> ;
    owl:inverseOf <http://rdaregistry.info/Elements/u/P60021> ;
    skos:definition "Relates a resource to a performer contributing to a resource by leading a program (often broadcast) that includes other guests, performers, etc. (e.g., talk show host)."@en .

<http://rdaregistry.info/Elements/u/P60147>
    reg:hasSubproperty <http://rdaregistry.info/Elements/e/P20017> ;
    reg:lexicalAlias <http://rdaregistry.info/Elements/u/moderator.en> ;
    reg:name "moderator"@en ;
    reg:status <http://metadataregistry.org/uri/RegStatus/1001> ;
    a rdf:Property ;
    rdfs:isDefinedBy <http://rdaregistry.info/Elements/u/> ;
    rdfs:label "has moderator"@en ;
    rdfs:subPropertyOf <http://rdaregistry.info/Elements/u/P60387> ;
    owl:inverseOf <http://rdaregistry.info/Elements/u/P60022> ;
    skos:definition "Relates a resource to a performer contributing to a resource by leading a program (often broadcast) where topics are discussed, usually with participation of experts in fields related to the discussion."@en .

<http://rdaregistry.info/Elements/u/P60148>
    reg:hasSubproperty <http://rdaregistry.info/Elements/e/P20018> ;
    reg:lexicalAlias <http://rdaregistry.info/Elements/u/puppeteer.en> ;
    reg:name "puppeteer"@en ;
    reg:status <http://metadataregistry.org/uri/RegStatus/1001> ;
    a rdf:Property ;
    rdfs:isDefinedBy <http://rdaregistry.info/Elements/u/> ;
    rdfs:label "has puppeteer"@en ;
    rdfs:subPropertyOf <http://rdaregistry.info/Elements/u/P60387> ;
    owl:inverseOf <http://rdaregistry.info/Elements/u/P60023> ;
    skos:definition "Relates a resource to a performer contributing to a resource by manipulating, controlling, or directing puppets or marionettes in a moving image production or a musical or dramatic presentation or entertainment."@en .

<http://rdaregistry.info/Elements/u/P60149>
    reg:hasSubproperty <http://rdaregistry.info/Elements/e/P20019> ;
    reg:lexicalAlias <http://rdaregistry.info/Elements/u/panelist.en> ;
    reg:name "panelist"@en ;
    reg:status <http://metadataregistry.org/uri/RegStatus/1001> ;
    a rdf:Property ;
    rdfs:isDefinedBy <http://rdaregistry.info/Elements/u/> ;
    rdfs:label "has panelist"@en ;
    rdfs:subPropertyOf <http://rdaregistry.info/Elements/u/P60387> ;
    owl:inverseOf <http://rdaregistry.info/Elements/u/P60024> ;
    skos:definition "Relates a resource to a performer contributing to a resource by participating in a program (often broadcast) where topics are discussed, usually with participation of experts in fields related to the discussion."@en .

<http://rdaregistry.info/Elements/u/P60150>
    reg:hasSubproperty <http://rdaregistry.info/Elements/e/P20020> ;
    reg:lexicalAlias <http://rdaregistry.info/Elements/u/instrumentalist.en> ;
    reg:name "instrumentalist"@en ;
    reg:status <http://metadataregistry.org/uri/RegStatus/1001> ;
    a rdf:Property ;
    rdfs:isDefinedBy <http://rdaregistry.info/Elements/u/> ;
    rdfs:label "has instrumentalist"@en ;
    rdfs:subPropertyOf <http://rdaregistry.info/Elements/u/P60387> ;
    owl:inverseOf <http://rdaregistry.info/Elements/u/P60025> ;
    skos:definition "Relates a resource to a performer contributing to a resource by playing a musical instrument."@en .

<http://rdaregistry.info/Elements/u/P60151>
    reg:hasSubproperty <http://rdaregistry.info/Elements/e/P20021> ;
    reg:lexicalAlias <http://rdaregistry.info/Elements/u/commentator.en> ;
    reg:name "commentator"@en ;
    reg:status <http://metadataregistry.org/uri/RegStatus/1001> ;
    a rdf:Property ;
    rdfs:isDefinedBy <http://rdaregistry.info/Elements/u/> ;
    rdfs:label "has commentator"@en ;
    rdfs:subPropertyOf <http://rdaregistry.info/Elements/u/P60387> ;
    owl:inverseOf <http://rdaregistry.info/Elements/u/P60026> ;
    skos:definition "Relates a resource to a performer contributing to a resource by providing interpretation, analysis, or a discussion of the subject matter on a recording, film, or other audiovisual medium."@en .

<http://rdaregistry.info/Elements/u/P60152>
    reg:hasSubproperty <http://rdaregistry.info/Elements/e/P20070> ;
    reg:lexicalAlias <http://rdaregistry.info/Elements/u/voiceActor.en> ;
    reg:name "voiceActor"@en ;
    reg:status <http://metadataregistry.org/uri/RegStatus/1001> ;
    a rdf:Property ;
    rdfs:isDefinedBy <http://rdaregistry.info/Elements/u/> ;
    rdfs:label "has voice actor"@en ;
    rdfs:subPropertyOf <http://rdaregistry.info/Elements/u/P60142> ;
    owl:inverseOf <http://rdaregistry.info/Elements/u/P60027> ;
    skos:definition "Relates a resource to a performer contributing to a resource by providing the voice for characters in radio and audio productions and for animated characters in moving image resources as well as by providing voice-overs in radio and television commercials, dubbed resources, etc."@en .

<http://rdaregistry.info/Elements/u/P60153>
    reg:hasSubproperty <http://rdaregistry.info/Elements/e/P20022> ;
    reg:lexicalAlias <http://rdaregistry.info/Elements/u/narrator.en> ;
    reg:name "narrator"@en ;
    reg:status <http://metadataregistry.org/uri/RegStatus/1001> ;
    a rdf:Property ;
    rdfs:isDefinedBy <http://rdaregistry.info/Elements/u/> ;
    rdfs:label "has narrator"@en ;
    rdfs:subPropertyOf <http://rdaregistry.info/Elements/u/P60387> ;
    owl:inverseOf <http://rdaregistry.info/Elements/u/P60028> ;
    skos:definition "Relates a resource to a performer contributing to a resource by reading aloud or giving an account of an act, occurrence, course of events, etc."@en .

<http://rdaregistry.info/Elements/u/P60154>
    reg:hasSubproperty <http://rdaregistry.info/Elements/e/P20023> ;
    reg:lexicalAlias <http://rdaregistry.info/Elements/u/storyteller.en> ;
    reg:name "storyteller"@en ;
    reg:status <http://metadataregistry.org/uri/RegStatus/1001> ;
    a rdf:Property ;
    rdfs:isDefinedBy <http://rdaregistry.info/Elements/u/> ;
    rdfs:label "has storyteller"@en ;
    rdfs:subPropertyOf <http://rdaregistry.info/Elements/u/P60387> ;
    owl:inverseOf <http://rdaregistry.info/Elements/u/P60029> ;
    skos:definition "Relates a resource to a performer contributing to a resource by relaying a creator's original story with dramatic or theatrical interpretation."@en .

<http://rdaregistry.info/Elements/u/P60155>
    reg:hasSubproperty <http://rdaregistry.info/Elements/e/P20024> ;
    reg:lexicalAlias <http://rdaregistry.info/Elements/u/speaker.en> ;
    reg:name "speaker"@en ;
    reg:status <http://metadataregistry.org/uri/RegStatus/1001> ;
    a rdf:Property ;
    rdfs:isDefinedBy <http://rdaregistry.info/Elements/u/> ;
    rdfs:label "has speaker"@en ;
    rdfs:subPropertyOf <http://rdaregistry.info/Elements/u/P60387> ;
    owl:inverseOf <http://rdaregistry.info/Elements/u/P60030> ;
    skos:definition "Relates a resource to a performer contributing to a resource by speaking words, such as a lecture, speech, etc."@en .

<http://rdaregistry.info/Elements/u/P60156>
    reg:hasSubproperty <http://rdaregistry.info/Elements/e/P20025> ;
    reg:lexicalAlias <http://rdaregistry.info/Elements/u/singer.en> ;
    reg:name "singer"@en ;
    reg:status <http://metadataregistry.org/uri/RegStatus/1001> ;
    a rdf:Property ;
    rdfs:isDefinedBy <http://rdaregistry.info/Elements/u/> ;
    rdfs:label "has singer"@en ;
    rdfs:subPropertyOf <http://rdaregistry.info/Elements/u/P60387> ;
    owl:inverseOf <http://rdaregistry.info/Elements/u/P60031> ;
    skos:definition "Relates a resource to a performer contributing to a resource by using his/her/their voice, with or without instrumental accompaniment, to produce music. a singer’s performance may or may not include actual words."@en .

<http://rdaregistry.info/Elements/u/P60157>
    reg:lexicalAlias <http://rdaregistry.info/Elements/u/medium.en> ;
    reg:name "medium"@en ;
    reg:status <http://metadataregistry.org/uri/RegStatus/1001> ;
    a rdf:Property ;
    rdfs:isDefinedBy <http://rdaregistry.info/Elements/u/> ;
    rdfs:label "has medium"@en ;
    rdfs:subPropertyOf <http://rdaregistry.info/Elements/u/P60374> ;
    owl:inverseOf <http://rdaregistry.info/Elements/u/P60032> ;
    skos:definition "Relates a resource to a person held to be a channel of communication between the earthly world and a world of spirits."@en .

<http://rdaregistry.info/Elements/u/P60158>
    reg:status <http://metadataregistry.org/uri/RegStatus/1008> ;
    rdfs:isDefinedBy <http://rdaregistry.info/Elements/u/> .

<http://rdaregistry.info/Elements/u/P60159>
    reg:hasSubproperty <http://rdaregistry.info/Elements/m/P30084>, <http://rdaregistry.info/Elements/u/P60344> ;
    reg:lexicalAlias <http://rdaregistry.info/Elements/u/appliedMaterial.en> ;
    reg:name "appliedMaterial"@en ;
    reg:status <http://metadataregistry.org/uri/RegStatus/1001> ;
    a rdf:Property ;
    rdfs:isDefinedBy <http://rdaregistry.info/Elements/u/> ;
    rdfs:label "has applied material"@en ;
    skos:definition "Relates a resource to a physical or chemical substance applied to a base material of a resource."@en .

<http://rdaregistry.info/Elements/u/P60160>
    reg:hasSubproperty <http://rdaregistry.info/Elements/m/P30085> ;
    reg:lexicalAlias <http://rdaregistry.info/Elements/u/placeOfDistribution.en> ;
    reg:name "placeOfDistribution"@en ;
    reg:status <http://metadataregistry.org/uri/RegStatus/1001> ;
    a rdf:Property ;
    rdfs:isDefinedBy <http://rdaregistry.info/Elements/u/> ;
    rdfs:label "has place of distribution"@en ;
    skos:definition "Relates a resource to a place associated with the distribution of a resource in a published form."@en .

<http://rdaregistry.info/Elements/u/P60161>
    reg:hasSubproperty <http://rdaregistry.info/Elements/m/P30086> ;
    reg:lexicalAlias <http://rdaregistry.info/Elements/u/placeOfProduction.en> ;
    reg:name "placeOfProduction"@en ;
    reg:status <http://metadataregistry.org/uri/RegStatus/1001> ;
    a rdf:Property ;
    rdfs:isDefinedBy <http://rdaregistry.info/Elements/u/> ;
    rdfs:label "has place of production"@en ;
    skos:definition "Relates a resource to a place associated with the inscription, fabrication, construction, etc., of a resource in an unpublished form."@en .

<http://rdaregistry.info/Elements/u/P60162>
    reg:hasSubproperty <http://rdaregistry.info/Elements/m/P30087> ;
    reg:lexicalAlias <http://rdaregistry.info/Elements/u/placeOfManufacture.en> ;
    reg:name "placeOfManufacture"@en ;
    reg:status <http://metadataregistry.org/uri/RegStatus/1001> ;
    a rdf:Property ;
    rdfs:isDefinedBy <http://rdaregistry.info/Elements/u/> ;
    rdfs:label "has place of manufacture"@en ;
    skos:definition "Relates a resource to a place associated with the printing, duplicating, casting, etc., of a resource in a published form."@en .

<http://rdaregistry.info/Elements/u/P60163>
    reg:hasSubproperty <http://rdaregistry.info/Elements/m/P30088> ;
    reg:lexicalAlias <http://rdaregistry.info/Elements/u/placeOfPublication.en> ;
    reg:name "placeOfPublication"@en ;
    reg:status <http://metadataregistry.org/uri/RegStatus/1001> ;
    a rdf:Property ;
    rdfs:isDefinedBy <http://rdaregistry.info/Elements/u/> ;
    rdfs:label "has place of publication"@en ;
    skos:definition "Relates a resource to a place associated with the publication, release, or issuing of a resource."@en .

<http://rdaregistry.info/Elements/u/P60164>
    reg:hasSubproperty <http://rdaregistry.info/Elements/m/P30089> ;
    reg:lexicalAlias <http://rdaregistry.info/Elements/u/parallelPlaceOfDistribution.en> ;
    reg:name "parallelPlaceOfDistribution"@en ;
    reg:status <http://metadataregistry.org/uri/RegStatus/1001> ;
    a rdf:Property ;
    rdfs:isDefinedBy <http://rdaregistry.info/Elements/u/> ;
    rdfs:label "has parallel place of distribution"@en ;
    skos:definition "Relates a resource to a place of distribution in a language and/or script that differs from that recorded in the place of distribution element."@en .

<http://rdaregistry.info/Elements/u/P60165>
    reg:hasSubproperty <http://rdaregistry.info/Elements/m/P30090> ;
    reg:lexicalAlias <http://rdaregistry.info/Elements/u/parallelPlaceOfManufacture.en> ;
    reg:name "parallelPlaceOfManufacture"@en ;
    reg:status <http://metadataregistry.org/uri/RegStatus/1001> ;
    a rdf:Property ;
    rdfs:isDefinedBy <http://rdaregistry.info/Elements/u/> ;
    rdfs:label "has parallel place of manufacture"@en ;
    skos:definition "Relates a resource to a place of manufacture in a language and/or script that differs from that recorded in the place of manufacture element."@en .

<http://rdaregistry.info/Elements/u/P60166>
    reg:hasSubproperty <http://rdaregistry.info/Elements/m/P30091> ;
    reg:lexicalAlias <http://rdaregistry.info/Elements/u/parallelPlaceOfProduction.en> ;
    reg:name "parallelPlaceOfProduction"@en ;
    reg:status <http://metadataregistry.org/uri/RegStatus/1001> ;
    a rdf:Property ;
    rdfs:isDefinedBy <http://rdaregistry.info/Elements/u/> ;
    rdfs:label "has parallel place of production"@en ;
    skos:definition "Relates a resource to a place of production in a language and/or script that differs from that recorded in the place of production element."@en .

<http://rdaregistry.info/Elements/u/P60167>
    reg:hasSubproperty <http://rdaregistry.info/Elements/m/P30092> ;
    reg:lexicalAlias <http://rdaregistry.info/Elements/u/parallelPlaceOfPublication.en> ;
    reg:name "parallelPlaceOfPublication"@en ;
    reg:status <http://metadataregistry.org/uri/RegStatus/1001> ;
    a rdf:Property ;
    rdfs:isDefinedBy <http://rdaregistry.info/Elements/u/> ;
    rdfs:label "has parallel place of publication"@en ;
    skos:definition "Relates a resource to a place of publication in a language and/or script that differs from that recorded in the place of publication element."@en .

<http://rdaregistry.info/Elements/u/P60168>
    reg:hasSubproperty <http://rdaregistry.info/Elements/i/P40038>, <http://rdaregistry.info/Elements/m/P30093> ;
    reg:lexicalAlias <http://rdaregistry.info/Elements/u/reprintOf.en> ;
    reg:name "reprintOf"@en ;
    reg:status <http://metadataregistry.org/uri/RegStatus/1001> ;
    a rdf:Property ;
    rdfs:isDefinedBy <http://rdaregistry.info/Elements/u/> ;
    rdfs:label "is reprint of"@en ;
    rdfs:subPropertyOf <http://rdaregistry.info/Elements/u/P60297> ;
    owl:inverseOf <http://rdaregistry.info/Elements/u/P60271> ;
    skos:definition "Relates a resource to a printed resource that is used as the basis for a reissue with the same content as the resource being described."@en .

<http://rdaregistry.info/Elements/u/P60169>
    reg:lexicalAlias <http://rdaregistry.info/Elements/u/filmProducer.en> ;
    reg:name "filmProducer"@en ;
    reg:status <http://metadataregistry.org/uri/RegStatus/1001> ;
    a rdf:Property ;
    rdfs:isDefinedBy <http://rdaregistry.info/Elements/u/> ;
    rdfs:label "has film producer"@en ;
    rdfs:subPropertyOf <http://rdaregistry.info/Elements/u/P60441> ;
    owl:inverseOf <http://rdaregistry.info/Elements/u/P60033> ;
    skos:definition "Relates a resource to a producer responsible for most of the business aspects of a film."@en .

<http://rdaregistry.info/Elements/u/P60170>
    reg:lexicalAlias <http://rdaregistry.info/Elements/u/radioProducer.en> ;
    reg:name "radioProducer"@en ;
    reg:status <http://metadataregistry.org/uri/RegStatus/1001> ;
    a rdf:Property ;
    rdfs:isDefinedBy <http://rdaregistry.info/Elements/u/> ;
    rdfs:label "has radio producer"@en ;
    rdfs:subPropertyOf <http://rdaregistry.info/Elements/u/P60441> ;
    owl:inverseOf <http://rdaregistry.info/Elements/u/P60034> ;
    skos:definition "Relates a resource to a producer responsible for most of the business aspects of a radio program."@en .

<http://rdaregistry.info/Elements/u/P60171>
    reg:lexicalAlias <http://rdaregistry.info/Elements/u/televisionProducer.en> ;
    reg:name "televisionProducer"@en ;
    reg:status <http://metadataregistry.org/uri/RegStatus/1001> ;
    a rdf:Property ;
    rdfs:isDefinedBy <http://rdaregistry.info/Elements/u/> ;
    rdfs:label "has television producer"@en ;
    rdfs:subPropertyOf <http://rdaregistry.info/Elements/u/P60441> ;
    owl:inverseOf <http://rdaregistry.info/Elements/u/P60035> ;
    skos:definition "Relates a resource to a producer responsible for most of the business aspects of a television program."@en .

<http://rdaregistry.info/Elements/u/P60172>
    reg:hasSubproperty <http://rdaregistry.info/Elements/m/P30094> ;
    reg:lexicalAlias <http://rdaregistry.info/Elements/u/parallelProducersName.en> ;
    reg:name "parallelProducersName"@en ;
    reg:status <http://metadataregistry.org/uri/RegStatus/1001> ;
    a rdf:Property ;
    rdfs:isDefinedBy <http://rdaregistry.info/Elements/u/> ;
    rdfs:label "has parallel producer’s name"@en ;
    skos:definition "Relates a resource to a producer's name in a language and/or script that differs from that recorded in the producer's name element."@en .

<http://rdaregistry.info/Elements/u/P60173>
    reg:hasSubproperty <http://rdaregistry.info/Elements/m/P30095> ;
    reg:lexicalAlias <http://rdaregistry.info/Elements/u/parallelPublishersName.en> ;
    reg:name "parallelPublishersName"@en ;
    reg:status <http://metadataregistry.org/uri/RegStatus/1001> ;
    a rdf:Property ;
    rdfs:isDefinedBy <http://rdaregistry.info/Elements/u/> ;
    rdfs:label "has parallel publisher’s name"@en ;
    skos:definition "Relates a resource to a publisher's name in a language and/or script that differs from that recorded in the publisher's name element."@en .

<http://rdaregistry.info/Elements/u/P60174>
    reg:hasSubproperty <http://rdaregistry.info/Elements/e/P20060> ;
    reg:lexicalAlias <http://rdaregistry.info/Elements/u/adaptedAsARadioProgram.en> ;
    reg:name "adaptedAsARadioProgram"@en ;
    reg:status <http://metadataregistry.org/uri/RegStatus/1001> ;
    a rdf:Property ;
    rdfs:isDefinedBy <http://rdaregistry.info/Elements/u/> ;
    rdfs:label "is adapted as radio program"@en ;
    rdfs:subPropertyOf <http://rdaregistry.info/Elements/u/P60260> ;
    owl:inverseOf <http://rdaregistry.info/Elements/u/P60229> ;
    skos:definition "Relates a resource to a radio program based on the source resource."@en .

<http://rdaregistry.info/Elements/u/P60175>
    reg:lexicalAlias <http://rdaregistry.info/Elements/u/academicDegree.en> ;
    reg:name "academicDegree"@en ;
    reg:status <http://metadataregistry.org/uri/RegStatus/1001> ;
    a rdf:Property ;
    rdfs:isDefinedBy <http://rdaregistry.info/Elements/u/> ;
    rdfs:label "has academic degree"@en ;
    skos:definition "Relates a resource to a rank conferred as a guarantee of academic proficiency."@en .

<http://rdaregistry.info/Elements/u/P60176>
    reg:hasSubproperty <http://rdaregistry.info/Elements/i/P40026> ;
    reg:lexicalAlias <http://rdaregistry.info/Elements/u/custodialHistoryOfResource.en> ;
    reg:name "custodialHistoryOfResource"@en ;
    reg:status <http://metadataregistry.org/uri/RegStatus/1001> ;
    a rdf:Property ;
    rdfs:isDefinedBy <http://rdaregistry.info/Elements/u/> ;
    rdfs:label "has custodial history of resource"@en ;
    skos:definition "Relates a resource to a record of previous ownership or custodianship of a resource."@en .

<http://rdaregistry.info/Elements/u/P60177>
    reg:hasSubproperty <http://rdaregistry.info/Elements/e/P20090> ;
    reg:lexicalAlias <http://rdaregistry.info/Elements/u/abstractedIn.en> ;
    reg:name "abstractedIn"@en ;
    reg:status <http://metadataregistry.org/uri/RegStatus/1001> ;
    a rdf:Property ;
    rdfs:isDefinedBy <http://rdaregistry.info/Elements/u/> ;
    rdfs:label "is abstracted in"@en ;
    rdfs:subPropertyOf <http://rdaregistry.info/Elements/u/P60250> ;
    owl:inverseOf <http://rdaregistry.info/Elements/u/P60308> ;
    skos:definition "Relates a resource to a resource (an abstracting and indexing service) that abstracts the contents of a source entity."@en .

<http://rdaregistry.info/Elements/u/P60178>
    reg:hasSubproperty <http://rdaregistry.info/Elements/e/P20091> ;
    reg:lexicalAlias <http://rdaregistry.info/Elements/u/indexedIn.en> ;
    reg:name "indexedIn"@en ;
    reg:status <http://metadataregistry.org/uri/RegStatus/1001> ;
    a rdf:Property ;
    rdfs:isDefinedBy <http://rdaregistry.info/Elements/u/> ;
    rdfs:label "is indexed in"@en ;
    rdfs:subPropertyOf <http://rdaregistry.info/Elements/u/P60250> ;
    owl:inverseOf <http://rdaregistry.info/Elements/u/P60309> ;
    skos:definition "Relates a resource to a resource (an abstracting and indexing service) that indexes the contents of the source resource."@en .

<http://rdaregistry.info/Elements/u/P60179>
    reg:hasSubproperty <http://rdaregistry.info/Elements/i/P40059>, <http://rdaregistry.info/Elements/m/P30021> ;
    reg:lexicalAlias <http://rdaregistry.info/Elements/u/preservationFacsimile.en> ;
    reg:name "preservationFacsimile"@en ;
    reg:status <http://metadataregistry.org/uri/RegStatus/1001> ;
    a rdf:Property ;
    rdfs:isDefinedBy <http://rdaregistry.info/Elements/u/> ;
    rdfs:label "has preservation facsimile"@en ;
    rdfs:subPropertyOf <http://rdaregistry.info/Elements/u/P60217> ;
    owl:inverseOf <http://rdaregistry.info/Elements/u/P60299> ;
    skos:definition "Relates a resource to a resource that consists of an exact reproduction on preservation-quality media, such as acid-free permanent or archival paper."@en .

<http://rdaregistry.info/Elements/u/P60180>
    reg:hasSubproperty <http://rdaregistry.info/Elements/e/P20092> ;
    reg:lexicalAlias <http://rdaregistry.info/Elements/u/adaptedAsChoreography.en> ;
    reg:name "adaptedAsChoreography"@en ;
    reg:status <http://metadataregistry.org/uri/RegStatus/1001> ;
    a rdf:Property ;
    rdfs:isDefinedBy <http://rdaregistry.info/Elements/u/> ;
    rdfs:label "is adapted as choreography"@en ;
    rdfs:subPropertyOf <http://rdaregistry.info/Elements/u/P60250> ;
    owl:inverseOf <http://rdaregistry.info/Elements/u/P60293> ;
    skos:definition "Relates a resource to a resource consisting of movement (e.g., dance) based on the source resource."@en .

<http://rdaregistry.info/Elements/u/P60181>
    reg:hasSubproperty <http://rdaregistry.info/Elements/e/P20093> ;
    reg:lexicalAlias <http://rdaregistry.info/Elements/u/errata.en> ;
    reg:name "errata"@en ;
    reg:status <http://metadataregistry.org/uri/RegStatus/1001> ;
    a rdf:Property ;
    rdfs:isDefinedBy <http://rdaregistry.info/Elements/u/> ;
    rdfs:label "is errata"@en ;
    rdfs:subPropertyOf <http://rdaregistry.info/Elements/u/P60204> ;
    owl:inverseOf <http://rdaregistry.info/Elements/u/P60251> ;
    skos:definition "Relates a resource to a resource consisting of errors discovered after the publication of the predominant resource, with their corrections."@en .

<http://rdaregistry.info/Elements/u/P60182>
    reg:hasSubproperty <http://rdaregistry.info/Elements/e/P20094> ;
    reg:lexicalAlias <http://rdaregistry.info/Elements/u/illustrations.en> ;
    reg:name "illustrations"@en ;
    reg:status <http://metadataregistry.org/uri/RegStatus/1001> ;
    a rdf:Property ;
    rdfs:isDefinedBy <http://rdaregistry.info/Elements/u/> ;
    rdfs:label "is illustrations"@en ;
    rdfs:subPropertyOf <http://rdaregistry.info/Elements/u/P60204> ;
    owl:inverseOf <http://rdaregistry.info/Elements/u/P60254> ;
    skos:definition "Relates a resource to a resource consisting of pictorial content designed to explain or decorate the augmented resource."@en .

<http://rdaregistry.info/Elements/u/P60183>
    reg:hasSubproperty <http://rdaregistry.info/Elements/m/P30022> ;
    reg:lexicalAlias <http://rdaregistry.info/Elements/u/insert.en> ;
    reg:name "insert"@en ;
    reg:status <http://metadataregistry.org/uri/RegStatus/1001> ;
    a rdf:Property ;
    rdfs:isDefinedBy <http://rdaregistry.info/Elements/u/> ;
    rdfs:label "is insert"@en ;
    rdfs:subPropertyOf <http://rdaregistry.info/Elements/u/P60249> ;
    owl:inverseOf <http://rdaregistry.info/Elements/u/P60194> ;
    skos:definition "Relates a resource to a resource consisting of separately issued material that is not an integral part of the larger resource into which it has been inserted."@en .

<http://rdaregistry.info/Elements/u/P60184>
    reg:hasSubproperty <http://rdaregistry.info/Elements/e/P20095> ;
    reg:lexicalAlias <http://rdaregistry.info/Elements/u/adaptedAsAMotionPictureScreenplay.en> ;
    reg:name "adaptedAsAMotionPictureScreenplay"@en ;
    reg:status <http://metadataregistry.org/uri/RegStatus/1001> ;
    a rdf:Property ;
    rdfs:isDefinedBy <http://rdaregistry.info/Elements/u/> ;
    rdfs:label "is adapted as motion picture screenplay"@en ;
    rdfs:subPropertyOf <http://rdaregistry.info/Elements/u/P60185> ;
    owl:inverseOf <http://rdaregistry.info/Elements/u/P60232> ;
    skos:definition "Relates a resource to a resource consisting of the screenplay for a motion picture, based on the source resource."@en .

<http://rdaregistry.info/Elements/u/P60185>
    reg:hasSubproperty <http://rdaregistry.info/Elements/e/P20096>, <http://rdaregistry.info/Elements/u/P60184>, <http://rdaregistry.info/Elements/u/P60186>, <http://rdaregistry.info/Elements/u/P60187> ;
    reg:lexicalAlias <http://rdaregistry.info/Elements/u/adaptedAsAScreenplay.en> ;
    reg:name "adaptedAsAScreenplay"@en ;
    reg:status <http://metadataregistry.org/uri/RegStatus/1001> ;
    a rdf:Property ;
    rdfs:isDefinedBy <http://rdaregistry.info/Elements/u/> ;
    rdfs:label "is adapted as a screenplay"@en ;
    rdfs:subPropertyOf <http://rdaregistry.info/Elements/u/P60260> ;
    owl:inverseOf <http://rdaregistry.info/Elements/u/P60231> ;
    skos:definition "Relates a resource to a resource consisting of the screenplay for a motion picture, television program, or video, based on the source resource."@en .

<http://rdaregistry.info/Elements/u/P60186>
    reg:hasSubproperty <http://rdaregistry.info/Elements/e/P20097> ;
    reg:lexicalAlias <http://rdaregistry.info/Elements/u/adaptedAsATelevisionScreenplay.en> ;
    reg:name "adaptedAsATelevisionScreenplay"@en ;
    reg:status <http://metadataregistry.org/uri/RegStatus/1001> ;
    a rdf:Property ;
    rdfs:isDefinedBy <http://rdaregistry.info/Elements/u/> ;
    rdfs:label "is adapted as television screenplay"@en ;
    rdfs:subPropertyOf <http://rdaregistry.info/Elements/u/P60185> ;
    owl:inverseOf <http://rdaregistry.info/Elements/u/P60233> ;
    skos:definition "Relates a resource to a resource consisting of the screenplay for a television program, based on the source resource."@en .

<http://rdaregistry.info/Elements/u/P60187>
    reg:hasSubproperty <http://rdaregistry.info/Elements/e/P20098> ;
    reg:lexicalAlias <http://rdaregistry.info/Elements/u/adaptedAsAVideoScreenplay.en> ;
    reg:name "adaptedAsAVideoScreenplay"@en ;
    reg:status <http://metadataregistry.org/uri/RegStatus/1001> ;
    a rdf:Property ;
    rdfs:isDefinedBy <http://rdaregistry.info/Elements/u/> ;
    rdfs:label "is adapted as video screenplay"@en ;
    rdfs:subPropertyOf <http://rdaregistry.info/Elements/u/P60185> ;
    owl:inverseOf <http://rdaregistry.info/Elements/u/P60234> ;
    skos:definition "Relates a resource to a resource consisting of the screenplay for a video, based on the source resource."@en .

<http://rdaregistry.info/Elements/u/P60188>
    reg:hasSubproperty <http://rdaregistry.info/Elements/e/P20099> ;
    reg:lexicalAlias <http://rdaregistry.info/Elements/u/adaptedAsARadioScript.en> ;
    reg:name "adaptedAsARadioScript"@en ;
    reg:status <http://metadataregistry.org/uri/RegStatus/1001> ;
    a rdf:Property ;
    rdfs:isDefinedBy <http://rdaregistry.info/Elements/u/> ;
    rdfs:label "is adapted as radio script"@en ;
    rdfs:subPropertyOf <http://rdaregistry.info/Elements/u/P60260> ;
    owl:inverseOf <http://rdaregistry.info/Elements/u/P60235> ;
    skos:definition "Relates a resource to a resource consisting of the script for a radio program, based on the source resource."@en .

<http://rdaregistry.info/Elements/u/P60189>
    reg:hasSubproperty <http://rdaregistry.info/Elements/e/P20119> ;
    reg:lexicalAlias <http://rdaregistry.info/Elements/u/freelyTranslatedAs.en> ;
    reg:name "freelyTranslatedAs"@en ;
    reg:status <http://metadataregistry.org/uri/RegStatus/1001> ;
    a rdf:Property ;
    rdfs:isDefinedBy <http://rdaregistry.info/Elements/u/> ;
    rdfs:label "is freely translated as"@en ;
    rdfs:subPropertyOf <http://rdaregistry.info/Elements/u/P60250> ;
    owl:inverseOf <http://rdaregistry.info/Elements/u/P60243> ;
    skos:definition "Relates a resource to a resource created by freely translating the source resource into another language, preserving the spirit of the original, but not its linguistic details."@en .

<http://rdaregistry.info/Elements/u/P60190>
    reg:hasSubproperty <http://rdaregistry.info/Elements/u/P60239>, <http://rdaregistry.info/Elements/u/P60255>, <http://rdaregistry.info/Elements/u/P60288>, <http://rdaregistry.info/Elements/u/P60292>, <http://rdaregistry.info/Elements/u/P60298>, <http://rdaregistry.info/Elements/w/P10265>, <http://rdaregistry.info/Elements/w/P10271>, <http://rdaregistry.info/Elements/w/P10277> ;
    reg:lexicalAlias <http://rdaregistry.info/Elements/u/descriptionOf.en> ;
    reg:name "descriptionOf"@en ;
    reg:status <http://metadataregistry.org/uri/RegStatus/1001> ;
    a rdf:Property ;
    rdfs:isDefinedBy <http://rdaregistry.info/Elements/u/> ;
    rdfs:label "is description of"@en ;
    rdfs:subPropertyOf <http://rdaregistry.info/Elements/u/P60805> ;
    owl:inverseOf <http://rdaregistry.info/Elements/u/P60215> ;
    skos:definition "Relates a resource to a resource described by a describing entity."@en .

<http://rdaregistry.info/Elements/u/P60191>
    reg:hasSubproperty <http://rdaregistry.info/Elements/i/P40031>, <http://rdaregistry.info/Elements/m/P30024>, <http://rdaregistry.info/Elements/u/P60195>, <http://rdaregistry.info/Elements/u/P60197>, <http://rdaregistry.info/Elements/u/P60272>, <http://rdaregistry.info/Elements/u/P60297> ;
    reg:lexicalAlias <http://rdaregistry.info/Elements/u/equivalent.en> ;
    reg:name "equivalent"@en ;
    reg:status <http://metadataregistry.org/uri/RegStatus/1001> ;
    a rdf:Property ;
    rdfs:isDefinedBy <http://rdaregistry.info/Elements/u/> ;
    rdfs:label "has equivalent"@en ;
    rdfs:subPropertyOf <http://rdaregistry.info/Elements/u/P60712> ;
    owl:inverseOf <http://rdaregistry.info/Elements/u/P60191> ;
    skos:definition "Relates a resource to a resource that carries the same content as the resource."@en .

<http://rdaregistry.info/Elements/u/P60192>
    reg:lexicalAlias <http://rdaregistry.info/Elements/u/subseriesOf.en> ;
    reg:name "subseriesOf"@en ;
    reg:status <http://metadataregistry.org/uri/RegStatus/1001> ;
    a rdf:Property ;
    rdfs:isDefinedBy <http://rdaregistry.info/Elements/u/> ;
    rdfs:label "is subseries of"@en ;
    rdfs:subPropertyOf <http://rdaregistry.info/Elements/u/P60101> ;
    owl:inverseOf <http://rdaregistry.info/Elements/u/P60316> ;
    skos:definition "Relates a resource to a resource in which the part consistently appears; the title of the larger resource appears on all issues or parts of the subseries."@en .

<http://rdaregistry.info/Elements/u/P60193>
    reg:lexicalAlias <http://rdaregistry.info/Elements/u/inSeries.en> ;
    reg:name "inSeries"@en ;
    reg:status <http://metadataregistry.org/uri/RegStatus/1001> ;
    a rdf:Property ;
    rdfs:isDefinedBy <http://rdaregistry.info/Elements/u/> ;
    rdfs:label "is in series"@en ;
    rdfs:subPropertyOf <http://rdaregistry.info/Elements/u/P60101> ;
    owl:inverseOf <http://rdaregistry.info/Elements/u/P60240> ;
    skos:definition "Relates a resource to a resource in which the part has been issued; the title of the larger resource appears on the part."@en .

<http://rdaregistry.info/Elements/u/P60194>
    reg:hasSubproperty <http://rdaregistry.info/Elements/m/P30025> ;
    reg:lexicalAlias <http://rdaregistry.info/Elements/u/insertedIn.en> ;
    reg:name "insertedIn"@en ;
    reg:status <http://metadataregistry.org/uri/RegStatus/1001> ;
    a rdf:Property ;
    rdfs:isDefinedBy <http://rdaregistry.info/Elements/u/> ;
    rdfs:label "is inserted in"@en ;
    rdfs:subPropertyOf <http://rdaregistry.info/Elements/u/P60101> ;
    owl:inverseOf <http://rdaregistry.info/Elements/u/P60183> ;
    skos:definition "Relates a resource to a resource into which material has been inserted that is not an integral part of the publication."@en .

<http://rdaregistry.info/Elements/u/P60195>
    reg:hasSubproperty <http://rdaregistry.info/Elements/m/P30026> ;
    reg:lexicalAlias <http://rdaregistry.info/Elements/u/alsoIssuedAs.en> ;
    reg:name "alsoIssuedAs"@en ;
    reg:status <http://metadataregistry.org/uri/RegStatus/1001> ;
    a rdf:Property ;
    rdfs:isDefinedBy <http://rdaregistry.info/Elements/u/> ;
    rdfs:label "is also issued as"@en ;
    rdfs:subPropertyOf <http://rdaregistry.info/Elements/u/P60191> ;
    owl:inverseOf <http://rdaregistry.info/Elements/u/P60195> ;
    skos:definition "Relates a resource to a resource that carries the same content of a resource in a different format."@en .

<http://rdaregistry.info/Elements/u/P60196>
    reg:hasSubproperty <http://rdaregistry.info/Elements/i/P40029>, <http://rdaregistry.info/Elements/m/P30027>, <http://rdaregistry.info/Elements/u/P60237>, <http://rdaregistry.info/Elements/u/P60256> ;
    reg:lexicalAlias <http://rdaregistry.info/Elements/u/accompaniedBy.en> ;
    reg:name "accompaniedBy"@en ;
    reg:status <http://metadataregistry.org/uri/RegStatus/1001> ;
    a rdf:Property ;
    rdfs:isDefinedBy <http://rdaregistry.info/Elements/u/> ;
    rdfs:label "is accompanied by"@en ;
    rdfs:subPropertyOf <http://rdaregistry.info/Elements/u/P60709> ;
    owl:inverseOf <http://rdaregistry.info/Elements/u/P60196> ;
    skos:definition "Relates a resource to a resource issued with another resource, without any relationship to its content."@en .

<http://rdaregistry.info/Elements/u/P60197>
    reg:hasSubproperty <http://rdaregistry.info/Elements/m/P30028> ;
    reg:lexicalAlias <http://rdaregistry.info/Elements/u/mirrorSite.en> ;
    reg:name "mirrorSite"@en ;
    reg:status <http://metadataregistry.org/uri/RegStatus/1001> ;
    a rdf:Property ;
    rdfs:isDefinedBy <http://rdaregistry.info/Elements/u/> ;
    rdfs:label "is mirror site"@en ;
    rdfs:subPropertyOf <http://rdaregistry.info/Elements/u/P60191> ;
    owl:inverseOf <http://rdaregistry.info/Elements/u/P60197> ;
    skos:definition "Relates a resource to a resource that is an exact copy of a website , used to reduce network traffic or improve the availability of the content of the original site."@en .

<http://rdaregistry.info/Elements/u/P60198>
    reg:hasSubproperty <http://rdaregistry.info/Elements/e/P20100>, <http://rdaregistry.info/Elements/u/P60117>, <http://rdaregistry.info/Elements/u/P60201>, <http://rdaregistry.info/Elements/u/P60264>, <http://rdaregistry.info/Elements/u/P60267>, <http://rdaregistry.info/Elements/u/P60270>, <http://rdaregistry.info/Elements/u/P60285>, <http://rdaregistry.info/Elements/u/P60740>, <http://rdaregistry.info/Elements/u/P60741> ;
    reg:lexicalAlias <http://rdaregistry.info/Elements/u/complementedBy.en> ;
    reg:name "complementedBy"@en ;
    reg:status <http://metadataregistry.org/uri/RegStatus/1001> ;
    a rdf:Property ;
    rdfs:isDefinedBy <http://rdaregistry.info/Elements/u/> ;
    rdfs:label "is complemented by"@en ;
    rdfs:subPropertyOf <http://rdaregistry.info/Elements/u/P60709> ;
    owl:inverseOf <http://rdaregistry.info/Elements/u/P60198> ;
    skos:definition "Relates a resource to a resource paired with another resource without either resource being considered to predominate."@en .

<http://rdaregistry.info/Elements/u/P60199>
    reg:hasSubproperty <http://rdaregistry.info/Elements/e/P20101> ;
    reg:lexicalAlias <http://rdaregistry.info/Elements/u/continuedInPartBy.en> ;
    reg:name "continuedInPartBy"@en ;
    reg:status <http://metadataregistry.org/uri/RegStatus/1001> ;
    a rdf:Property ;
    rdfs:isDefinedBy <http://rdaregistry.info/Elements/u/> ;
    rdfs:label "is continued in part by"@en ;
    rdfs:subPropertyOf <http://rdaregistry.info/Elements/u/P60278> ;
    owl:inverseOf <http://rdaregistry.info/Elements/u/P60277> ;
    skos:definition "Relates a resource to a resource part of whose content separated from an earlier resource to form a new resource."@en .

<http://rdaregistry.info/Elements/u/P60200>
    reg:hasSubproperty <http://rdaregistry.info/Elements/i/P40056>, <http://rdaregistry.info/Elements/m/P30029> ;
    reg:lexicalAlias <http://rdaregistry.info/Elements/u/digitalTransfer.en> ;
    reg:name "digitalTransfer"@en ;
    reg:status <http://metadataregistry.org/uri/RegStatus/1001> ;
    a rdf:Property ;
    rdfs:isDefinedBy <http://rdaregistry.info/Elements/u/> ;
    rdfs:label "has digital transfer"@en ;
    rdfs:subPropertyOf <http://rdaregistry.info/Elements/u/P60272> ;
    owl:inverseOf <http://rdaregistry.info/Elements/u/P60287> ;
    skos:definition "Relates a resource to a resource in a digital format that results from the transfer of a resource in another digital format."@en .

<http://rdaregistry.info/Elements/u/P60201>
    reg:hasSubproperty <http://rdaregistry.info/Elements/e/P20102>, <http://rdaregistry.info/Elements/u/P60282>, <http://rdaregistry.info/Elements/u/P60283>, <http://rdaregistry.info/Elements/u/P60284> ;
    reg:lexicalAlias <http://rdaregistry.info/Elements/u/screenplayFor.en> ;
    reg:name "screenplayFor"@en ;
    reg:status <http://metadataregistry.org/uri/RegStatus/1001> ;
    a rdf:Property ;
    rdfs:isDefinedBy <http://rdaregistry.info/Elements/u/> ;
    rdfs:label "is screenplay for"@en ;
    rdfs:subPropertyOf <http://rdaregistry.info/Elements/u/P60198> ;
    owl:inverseOf <http://rdaregistry.info/Elements/u/P60264> ;
    skos:definition "Relates a resource to a resource such as a motion picture, television program, or video, that uses the text of the resource as a screenplay."@en .

<http://rdaregistry.info/Elements/u/P60202>
    reg:hasSubproperty <http://rdaregistry.info/Elements/e/P20103> ;
    reg:lexicalAlias <http://rdaregistry.info/Elements/u/incidentalMusicFor.en> ;
    reg:name "incidentalMusicFor"@en ;
    reg:status <http://metadataregistry.org/uri/RegStatus/1001> ;
    a rdf:Property ;
    rdfs:isDefinedBy <http://rdaregistry.info/Elements/u/> ;
    rdfs:label "is incidental music for"@en ;
    rdfs:subPropertyOf <http://rdaregistry.info/Elements/u/P60724> ;
    owl:inverseOf <http://rdaregistry.info/Elements/u/P60118> ;
    skos:definition "Relates a resource to a resource such as a play or other spoken work for the stage that uses the musical resource as incidental music."@en .

<http://rdaregistry.info/Elements/u/P60203>
    reg:hasSubproperty <http://rdaregistry.info/Elements/e/P20104> ;
    reg:lexicalAlias <http://rdaregistry.info/Elements/u/abstractedAs.en> ;
    reg:name "abstractedAs"@en ;
    reg:status <http://metadataregistry.org/uri/RegStatus/1001> ;
    a rdf:Property ;
    rdfs:isDefinedBy <http://rdaregistry.info/Elements/u/> ;
    rdfs:label "is abstracted as"@en ;
    rdfs:subPropertyOf <http://rdaregistry.info/Elements/u/P60250> ;
    owl:inverseOf <http://rdaregistry.info/Elements/u/P60224> ;
    skos:definition "Relates a resource to a resource that abbreviates the source resource in a brief, objective manner."@en .

<http://rdaregistry.info/Elements/u/P60204>
    reg:hasSubproperty <http://rdaregistry.info/Elements/e/P20105>, <http://rdaregistry.info/Elements/u/P60113>, <http://rdaregistry.info/Elements/u/P60181>, <http://rdaregistry.info/Elements/u/P60182>, <http://rdaregistry.info/Elements/u/P60206>, <http://rdaregistry.info/Elements/u/P60208>, <http://rdaregistry.info/Elements/u/P60209>, <http://rdaregistry.info/Elements/u/P60221>, <http://rdaregistry.info/Elements/u/P60222>, <http://rdaregistry.info/Elements/u/P60262>, <http://rdaregistry.info/Elements/u/P60263>, <http://rdaregistry.info/Elements/u/P60281> ;
    reg:lexicalAlias <http://rdaregistry.info/Elements/u/augmentedBy.en> ;
    reg:name "augmentedBy"@en ;
    reg:status <http://metadataregistry.org/uri/RegStatus/1001> ;
    a rdf:Property ;
    rdfs:isDefinedBy <http://rdaregistry.info/Elements/u/> ;
    rdfs:label "is augmented by"@en ;
    rdfs:subPropertyOf <http://rdaregistry.info/Elements/u/P60709> ;
    owl:inverseOf <http://rdaregistry.info/Elements/u/P60307> ;
    skos:definition "Relates a resource to a resource that adds to the content of a predominant resource."@en .

<http://rdaregistry.info/Elements/u/P60205>
    reg:hasSubproperty <http://rdaregistry.info/Elements/e/P20106> ;
    reg:lexicalAlias <http://rdaregistry.info/Elements/u/summarizedAs.en> ;
    reg:name "summarizedAs"@en ;
    reg:status <http://metadataregistry.org/uri/RegStatus/1001> ;
    a rdf:Property ;
    rdfs:isDefinedBy <http://rdaregistry.info/Elements/u/> ;
    rdfs:label "is summarized as"@en ;
    rdfs:subPropertyOf <http://rdaregistry.info/Elements/u/P60250> ;
    owl:inverseOf <http://rdaregistry.info/Elements/u/P60289> ;
    skos:definition "Relates a resource to a resource that consists of a brief recapitulation of the content of the source resource."@en .

<http://rdaregistry.info/Elements/u/P60206>
    reg:hasSubproperty <http://rdaregistry.info/Elements/e/P20107> ;
    reg:lexicalAlias <http://rdaregistry.info/Elements/u/catalogue.en> ;
    reg:name "catalogue"@en ;
    reg:status <http://metadataregistry.org/uri/RegStatus/1001> ;
    a rdf:Property ;
    rdfs:isDefinedBy <http://rdaregistry.info/Elements/u/> ;
    rdfs:label "is catalogue"@en ;
    rdfs:subPropertyOf <http://rdaregistry.info/Elements/u/P60204> ;
    owl:inverseOf <http://rdaregistry.info/Elements/u/P60290> ;
    skos:definition "Relates a resource to a resource that consists of a complete enumeration of resources arranged systematically."@en .

<http://rdaregistry.info/Elements/u/P60207>
    reg:hasSubproperty <http://rdaregistry.info/Elements/m/P30030> ;
    reg:lexicalAlias <http://rdaregistry.info/Elements/u/specialIssue.en> ;
    reg:name "specialIssue"@en ;
    reg:status <http://metadataregistry.org/uri/RegStatus/1001> ;
    a rdf:Property ;
    rdfs:isDefinedBy <http://rdaregistry.info/Elements/u/> ;
    rdfs:label "is special issue"@en ;
    rdfs:subPropertyOf <http://rdaregistry.info/Elements/u/P60249> ;
    owl:inverseOf <http://rdaregistry.info/Elements/u/P60317> ;
    skos:definition "Relates a resource to a resource that consists of a single issue or a supplementary section of a serial or newspaper devoted to a special subject."@en .

<http://rdaregistry.info/Elements/u/P60208>
    reg:hasSubproperty <http://rdaregistry.info/Elements/e/P20108> ;
    reg:lexicalAlias <http://rdaregistry.info/Elements/u/concordance.en> ;
    reg:name "concordance"@en ;
    reg:status <http://metadataregistry.org/uri/RegStatus/1001> ;
    a rdf:Property ;
    rdfs:isDefinedBy <http://rdaregistry.info/Elements/u/> ;
    rdfs:label "is concordance"@en ;
    rdfs:subPropertyOf <http://rdaregistry.info/Elements/u/P60204> ;
    owl:inverseOf <http://rdaregistry.info/Elements/u/P60291> ;
    skos:definition "Relates a resource to a resource that consists of an index of all the words in the predominant resource."@en .

<http://rdaregistry.info/Elements/u/P60209>
    reg:hasSubproperty <http://rdaregistry.info/Elements/e/P20109> ;
    reg:lexicalAlias <http://rdaregistry.info/Elements/u/addenda.en> ;
    reg:name "addenda"@en ;
    reg:status <http://metadataregistry.org/uri/RegStatus/1001> ;
    a rdf:Property ;
    rdfs:isDefinedBy <http://rdaregistry.info/Elements/u/> ;
    rdfs:label "is addenda"@en ;
    rdfs:subPropertyOf <http://rdaregistry.info/Elements/u/P60204> ;
    owl:inverseOf <http://rdaregistry.info/Elements/u/P60286> ;
    skos:definition "Relates a resource to a resource that is conceived as brief material, less extensive than a supplement but essential to the completeness of the predominant resource, usually added at the end of the predominant resource but sometimes issued separately."@en .

<http://rdaregistry.info/Elements/u/P60210>
    reg:hasSubproperty <http://rdaregistry.info/Elements/e/P20110> ;
    reg:lexicalAlias <http://rdaregistry.info/Elements/u/adaptedAsLibretto.en> ;
    reg:name "adaptedAsLibretto"@en ;
    reg:status <http://metadataregistry.org/uri/RegStatus/1001> ;
    a rdf:Property ;
    rdfs:isDefinedBy <http://rdaregistry.info/Elements/u/> ;
    rdfs:label "is adapted as libretto"@en ;
    rdfs:subPropertyOf <http://rdaregistry.info/Elements/u/P60250> ;
    owl:inverseOf <http://rdaregistry.info/Elements/u/P60304> ;
    skos:definition "Relates a resource to a resource consisting of the text of an opera or other resource for the musical stage, or an oratorio, based on the source resource."@en .

<http://rdaregistry.info/Elements/u/P60211>
    reg:hasSubproperty <http://rdaregistry.info/Elements/e/P20274>, <http://rdaregistry.info/Elements/i/P40067>, <http://rdaregistry.info/Elements/m/P30259> ;
    reg:lexicalAlias <http://rdaregistry.info/Elements/u/reviewedIn.en> ;
    reg:name "reviewedIn"@en ;
    reg:status <http://metadataregistry.org/uri/RegStatus/1001> ;
    a rdf:Property ;
    rdfs:isDefinedBy <http://rdaregistry.info/Elements/u/> ;
    rdfs:label "is reviewed in"@en ;
    rdfs:subPropertyOf <http://rdaregistry.info/Elements/u/P60215> ;
    owl:inverseOf <http://rdaregistry.info/Elements/u/P60288> ;
    skos:definition "Relates a resource to a resource that contains a brief evaluation of the described resource."@en .

<http://rdaregistry.info/Elements/u/P60212>
    reg:hasSubproperty <http://rdaregistry.info/Elements/e/P20272>, <http://rdaregistry.info/Elements/i/P40065>, <http://rdaregistry.info/Elements/m/P30257> ;
    reg:lexicalAlias <http://rdaregistry.info/Elements/u/critiquedIn.en> ;
    reg:name "critiquedIn"@en ;
    reg:status <http://metadataregistry.org/uri/RegStatus/1001> ;
    a rdf:Property ;
    rdfs:isDefinedBy <http://rdaregistry.info/Elements/u/> ;
    rdfs:label "is critiqued in"@en ;
    rdfs:subPropertyOf <http://rdaregistry.info/Elements/u/P60215> ;
    owl:inverseOf <http://rdaregistry.info/Elements/u/P60292> ;
    skos:definition "Relates a resource to a resource that contains a critical evaluation of the described resource."@en .

<http://rdaregistry.info/Elements/u/P60213>
    reg:hasSubproperty <http://rdaregistry.info/Elements/e/P20271>, <http://rdaregistry.info/Elements/i/P40064>, <http://rdaregistry.info/Elements/m/P30256> ;
    reg:lexicalAlias <http://rdaregistry.info/Elements/u/commentaryIn.en> ;
    reg:name "commentaryIn"@en ;
    reg:status <http://metadataregistry.org/uri/RegStatus/1001> ;
    a rdf:Property ;
    rdfs:isDefinedBy <http://rdaregistry.info/Elements/u/> ;
    rdfs:label "is commentary in"@en ;
    rdfs:subPropertyOf <http://rdaregistry.info/Elements/u/P60215> ;
    owl:inverseOf <http://rdaregistry.info/Elements/u/P60298> ;
    skos:definition "Relates a resource to a resource that contains a set of explanatory or critical notes on the described resource"@en .

<http://rdaregistry.info/Elements/u/P60214>
    reg:hasSubproperty <http://rdaregistry.info/Elements/e/P20114>, <http://rdaregistry.info/Elements/u/P60246> ;
    reg:lexicalAlias <http://rdaregistry.info/Elements/u/imitatedAs.en> ;
    reg:name "imitatedAs"@en ;
    reg:status <http://metadataregistry.org/uri/RegStatus/1001> ;
    a rdf:Property ;
    rdfs:isDefinedBy <http://rdaregistry.info/Elements/u/> ;
    rdfs:label "is imitated as"@en ;
    rdfs:subPropertyOf <http://rdaregistry.info/Elements/u/P60250> ;
    owl:inverseOf <http://rdaregistry.info/Elements/u/P60311> ;
    skos:definition "Relates a resource to a resource that copies the style or content of the source resource."@en .

<http://rdaregistry.info/Elements/u/P60215>
    reg:hasSubproperty <http://rdaregistry.info/Elements/e/P20269>, <http://rdaregistry.info/Elements/i/P40062>, <http://rdaregistry.info/Elements/m/P30254>, <http://rdaregistry.info/Elements/u/P60211>, <http://rdaregistry.info/Elements/u/P60212>, <http://rdaregistry.info/Elements/u/P60213>, <http://rdaregistry.info/Elements/u/P60218>, <http://rdaregistry.info/Elements/u/P60219> ;
    reg:lexicalAlias <http://rdaregistry.info/Elements/u/describedIn.en> ;
    reg:name "describedIn"@en ;
    reg:status <http://metadataregistry.org/uri/RegStatus/1001> ;
    a rdf:Property ;
    rdfs:isDefinedBy <http://rdaregistry.info/Elements/u/> ;
    rdfs:label "is described in"@en ;
    rdfs:subPropertyOf <http://rdaregistry.info/Elements/u/P60806> ;
    owl:inverseOf <http://rdaregistry.info/Elements/u/P60190> ;
    skos:definition "Relates a resource to a resource that describes a described entity."@en .

<http://rdaregistry.info/Elements/u/P60216>
    reg:hasSubproperty <http://rdaregistry.info/Elements/e/P20115> ;
    reg:lexicalAlias <http://rdaregistry.info/Elements/u/expandedAs.en> ;
    reg:name "expandedAs"@en ;
    reg:status <http://metadataregistry.org/uri/RegStatus/1001> ;
    a rdf:Property ;
    rdfs:isDefinedBy <http://rdaregistry.info/Elements/u/> ;
    rdfs:label "is expanded as"@en ;
    rdfs:subPropertyOf <http://rdaregistry.info/Elements/u/P60250> ;
    owl:inverseOf <http://rdaregistry.info/Elements/u/P60294> ;
    skos:definition "Relates a resource to a resource that enlarges upon the content of the source resource."@en .

<http://rdaregistry.info/Elements/u/P60217>
    reg:hasSubproperty <http://rdaregistry.info/Elements/i/P40058>, <http://rdaregistry.info/Elements/m/P30031>, <http://rdaregistry.info/Elements/u/P60179> ;
    reg:lexicalAlias <http://rdaregistry.info/Elements/u/facsimile.en> ;
    reg:name "facsimile"@en ;
    reg:status <http://metadataregistry.org/uri/RegStatus/1001> ;
    a rdf:Property ;
    rdfs:isDefinedBy <http://rdaregistry.info/Elements/u/> ;
    rdfs:label "has facsimile"@en ;
    rdfs:subPropertyOf <http://rdaregistry.info/Elements/u/P60272> ;
    owl:inverseOf <http://rdaregistry.info/Elements/u/P60301> ;
    skos:definition "Relates a resource to a resource that exactly reproduces another resource embodying the resource."@en .

<http://rdaregistry.info/Elements/u/P60218>
    reg:hasSubproperty <http://rdaregistry.info/Elements/e/P20273>, <http://rdaregistry.info/Elements/i/P40066>, <http://rdaregistry.info/Elements/m/P30258> ;
    reg:lexicalAlias <http://rdaregistry.info/Elements/u/evaluatedIn.en> ;
    reg:name "evaluatedIn"@en ;
    reg:status <http://metadataregistry.org/uri/RegStatus/1001> ;
    a rdf:Property ;
    rdfs:isDefinedBy <http://rdaregistry.info/Elements/u/> ;
    rdfs:label "is evaluated in"@en ;
    rdfs:subPropertyOf <http://rdaregistry.info/Elements/u/P60215> ;
    owl:inverseOf <http://rdaregistry.info/Elements/u/P60255> ;
    skos:definition "Relates a resource to a resource that examines or judges the described resource."@en .

<http://rdaregistry.info/Elements/u/P60219>
    reg:hasSubproperty <http://rdaregistry.info/Elements/e/P20270>, <http://rdaregistry.info/Elements/i/P40063>, <http://rdaregistry.info/Elements/m/P30255> ;
    reg:lexicalAlias <http://rdaregistry.info/Elements/u/analysedIn.en> ;
    reg:name "analysedIn"@en ;
    reg:status <http://metadataregistry.org/uri/RegStatus/1001> ;
    a rdf:Property ;
    rdfs:isDefinedBy <http://rdaregistry.info/Elements/u/> ;
    rdfs:label "is analysed in"@en ;
    rdfs:subPropertyOf <http://rdaregistry.info/Elements/u/P60215> ;
    owl:inverseOf <http://rdaregistry.info/Elements/u/P60239> ;
    skos:definition "Relates a resource to a resource that examines the source resource to identify its components and their relations."@en .

<http://rdaregistry.info/Elements/u/P60220>
    reg:lexicalAlias <http://rdaregistry.info/Elements/u/prequel.en> ;
    reg:name "prequel"@en ;
    reg:status <http://metadataregistry.org/uri/RegStatus/1001> ;
    a rdf:Property ;
    rdfs:isDefinedBy <http://rdaregistry.info/Elements/u/> ;
    rdfs:label "is prequel"@en ;
    rdfs:subPropertyOf <http://rdaregistry.info/Elements/u/P60261> ;
    owl:inverseOf <http://rdaregistry.info/Elements/u/P60310> ;
    skos:definition "Relates a resource to a resource that extends the narrative of an earlier resource backwards in time."@en .

<http://rdaregistry.info/Elements/u/P60221>
    reg:hasSubproperty <http://rdaregistry.info/Elements/e/P20118> ;
    reg:lexicalAlias <http://rdaregistry.info/Elements/u/appendix.en> ;
    reg:name "appendix"@en ;
    reg:status <http://metadataregistry.org/uri/RegStatus/1001> ;
    a rdf:Property ;
    rdfs:isDefinedBy <http://rdaregistry.info/Elements/u/> ;
    rdfs:label "is appendix"@en ;
    rdfs:subPropertyOf <http://rdaregistry.info/Elements/u/P60204> ;
    owl:inverseOf <http://rdaregistry.info/Elements/u/P60253> ;
    skos:definition "Relates a resource to a resource that forms an augmenting part of another resource which is not essential to the completeness of the content, such as a list of references, statistical tables, and explanatory matter; it can either be material which comes at the end of the content of the predominant resource, or be issued separately."@en .

<http://rdaregistry.info/Elements/u/P60222>
    reg:hasSubproperty <http://rdaregistry.info/Elements/e/P20120> ;
    reg:lexicalAlias <http://rdaregistry.info/Elements/u/guide.en> ;
    reg:name "guide"@en ;
    reg:status <http://metadataregistry.org/uri/RegStatus/1001> ;
    a rdf:Property ;
    rdfs:isDefinedBy <http://rdaregistry.info/Elements/u/> ;
    rdfs:label "is guide"@en ;
    rdfs:subPropertyOf <http://rdaregistry.info/Elements/u/P60204> ;
    owl:inverseOf <http://rdaregistry.info/Elements/u/P60252> ;
    skos:definition "Relates a resource to a resource that guides a user through the use of the predominant resource, using notes, learning and study aids, exercises, problems, questions and answers, instructor or student materials, etc."@en .

<http://rdaregistry.info/Elements/u/P60223>
    reg:hasSubproperty <http://rdaregistry.info/Elements/e/P20121> ;
    reg:lexicalAlias <http://rdaregistry.info/Elements/u/abridgementOf.en> ;
    reg:name "abridgementOf"@en ;
    reg:status <http://metadataregistry.org/uri/RegStatus/1001> ;
    a rdf:Property ;
    rdfs:isDefinedBy <http://rdaregistry.info/Elements/u/> ;
    rdfs:label "is abridgement of"@en ;
    rdfs:subPropertyOf <http://rdaregistry.info/Elements/u/P60305> ;
    owl:inverseOf <http://rdaregistry.info/Elements/u/P60275> ;
    skos:definition "Relates a resource to a resource that has been abridged, i.e., shortened without changing the general meaning or manner of presentation of the source resource."@en .

<http://rdaregistry.info/Elements/u/P60224>
    reg:hasSubproperty <http://rdaregistry.info/Elements/e/P20122> ;
    reg:lexicalAlias <http://rdaregistry.info/Elements/u/abstractOf.en> ;
    reg:name "abstractOf"@en ;
    reg:status <http://metadataregistry.org/uri/RegStatus/1001> ;
    a rdf:Property ;
    rdfs:isDefinedBy <http://rdaregistry.info/Elements/u/> ;
    rdfs:label "is abstract of"@en ;
    rdfs:subPropertyOf <http://rdaregistry.info/Elements/u/P60305> ;
    owl:inverseOf <http://rdaregistry.info/Elements/u/P60203> ;
    skos:definition "Relates a resource to a resource that has been abstracted, i.e., abbreviated in a brief, objective manner."@en .

<http://rdaregistry.info/Elements/u/P60225>
    reg:hasSubproperty <http://rdaregistry.info/Elements/e/P20123> ;
    reg:lexicalAlias <http://rdaregistry.info/Elements/u/dramatizationOf.en> ;
    reg:name "dramatizationOf"@en ;
    reg:status <http://metadataregistry.org/uri/RegStatus/1001> ;
    a rdf:Property ;
    rdfs:isDefinedBy <http://rdaregistry.info/Elements/u/> ;
    rdfs:label "is dramatization of"@en ;
    rdfs:subPropertyOf <http://rdaregistry.info/Elements/u/P60241> ;
    owl:inverseOf <http://rdaregistry.info/Elements/u/P60088> ;
    skos:definition "Relates a resource to a resource that has been adapted as a drama."@en .

<http://rdaregistry.info/Elements/u/P60226>
    reg:hasSubproperty <http://rdaregistry.info/Elements/e/P20124> ;
    reg:lexicalAlias <http://rdaregistry.info/Elements/u/verseAdaptationOf.en> ;
    reg:name "verseAdaptationOf"@en ;
    reg:status <http://metadataregistry.org/uri/RegStatus/1001> ;
    a rdf:Property ;
    rdfs:isDefinedBy <http://rdaregistry.info/Elements/u/> ;
    rdfs:label "is verse adaptation of"@en ;
    rdfs:subPropertyOf <http://rdaregistry.info/Elements/u/P60241> ;
    owl:inverseOf <http://rdaregistry.info/Elements/u/P60106> ;
    skos:definition "Relates a resource to a resource that has been adapted as a literary composition in verse form."@en .

<http://rdaregistry.info/Elements/u/P60227>
    reg:hasSubproperty <http://rdaregistry.info/Elements/e/P20125> ;
    reg:lexicalAlias <http://rdaregistry.info/Elements/u/motionPictureAdaptationOf.en> ;
    reg:name "motionPictureAdaptationOf"@en ;
    reg:status <http://metadataregistry.org/uri/RegStatus/1001> ;
    a rdf:Property ;
    rdfs:isDefinedBy <http://rdaregistry.info/Elements/u/> ;
    rdfs:label "is motion picture adaptation of"@en ;
    rdfs:subPropertyOf <http://rdaregistry.info/Elements/u/P60241> ;
    owl:inverseOf <http://rdaregistry.info/Elements/u/P60110> ;
    skos:definition "Relates a resource to a resource that has been adapted as a motion picture."@en .

<http://rdaregistry.info/Elements/u/P60228>
    reg:hasSubproperty <http://rdaregistry.info/Elements/e/P20126> ;
    reg:lexicalAlias <http://rdaregistry.info/Elements/u/novelizationOf.en> ;
    reg:name "novelizationOf"@en ;
    reg:status <http://metadataregistry.org/uri/RegStatus/1001> ;
    a rdf:Property ;
    rdfs:isDefinedBy <http://rdaregistry.info/Elements/u/> ;
    rdfs:label "is novelization of"@en ;
    rdfs:subPropertyOf <http://rdaregistry.info/Elements/u/P60241> ;
    owl:inverseOf <http://rdaregistry.info/Elements/u/P60138> ;
    skos:definition "Relates a resource to a resource that has been adapted as a novel."@en .

<http://rdaregistry.info/Elements/u/P60229>
    reg:hasSubproperty <http://rdaregistry.info/Elements/e/P20127> ;
    reg:lexicalAlias <http://rdaregistry.info/Elements/u/radioAdaptationOf.en> ;
    reg:name "radioAdaptationOf"@en ;
    reg:status <http://metadataregistry.org/uri/RegStatus/1001> ;
    a rdf:Property ;
    rdfs:isDefinedBy <http://rdaregistry.info/Elements/u/> ;
    rdfs:label "is radio adaptation of"@en ;
    rdfs:subPropertyOf <http://rdaregistry.info/Elements/u/P60241> ;
    owl:inverseOf <http://rdaregistry.info/Elements/u/P60174> ;
    skos:definition "Relates a resource to a resource that has been adapted as a radio program."@en .

<http://rdaregistry.info/Elements/u/P60230>
    reg:hasSubproperty <http://rdaregistry.info/Elements/e/P20128> ;
    reg:lexicalAlias <http://rdaregistry.info/Elements/u/televisionAdaptationOf.en> ;
    reg:name "televisionAdaptationOf"@en ;
    reg:status <http://metadataregistry.org/uri/RegStatus/1001> ;
    a rdf:Property ;
    rdfs:isDefinedBy <http://rdaregistry.info/Elements/u/> ;
    rdfs:label "is television adaptation of"@en ;
    rdfs:subPropertyOf <http://rdaregistry.info/Elements/u/P60241> ;
    owl:inverseOf <http://rdaregistry.info/Elements/u/P60354> ;
    skos:definition "Relates a resource to a resource that has been adapted as a television program."@en .

<http://rdaregistry.info/Elements/u/P60231>
    reg:hasSubproperty <http://rdaregistry.info/Elements/e/P20129>, <http://rdaregistry.info/Elements/u/P60232>, <http://rdaregistry.info/Elements/u/P60233>, <http://rdaregistry.info/Elements/u/P60234> ;
    reg:lexicalAlias <http://rdaregistry.info/Elements/u/screenplayBasedOn.en> ;
    reg:name "screenplayBasedOn"@en ;
    reg:status <http://metadataregistry.org/uri/RegStatus/1001> ;
    a rdf:Property ;
    rdfs:isDefinedBy <http://rdaregistry.info/Elements/u/> ;
    rdfs:label "is screenplay based on"@en ;
    rdfs:subPropertyOf <http://rdaregistry.info/Elements/u/P60241> ;
    owl:inverseOf <http://rdaregistry.info/Elements/u/P60185> ;
    skos:definition "Relates a resource to a resource that has been adapted as the screenplay for a motion picture, television program, or video."@en .

<http://rdaregistry.info/Elements/u/P60232>
    reg:hasSubproperty <http://rdaregistry.info/Elements/e/P20130> ;
    reg:lexicalAlias <http://rdaregistry.info/Elements/u/motionPictureScreenplayBasedOn.en> ;
    reg:name "motionPictureScreenplayBasedOn"@en ;
    reg:status <http://metadataregistry.org/uri/RegStatus/1001> ;
    a rdf:Property ;
    rdfs:isDefinedBy <http://rdaregistry.info/Elements/u/> ;
    rdfs:label "is motion picture screenplay based on"@en ;
    rdfs:subPropertyOf <http://rdaregistry.info/Elements/u/P60231> ;
    owl:inverseOf <http://rdaregistry.info/Elements/u/P60184> ;
    skos:definition "Relates a resource to a resource that has been adapted as the screenplay for a motion picture."@en .

<http://rdaregistry.info/Elements/u/P60233>
    reg:hasSubproperty <http://rdaregistry.info/Elements/e/P20131> ;
    reg:lexicalAlias <http://rdaregistry.info/Elements/u/televisionScreenplayBasedOn.en> ;
    reg:name "televisionScreenplayBasedOn"@en ;
    reg:status <http://metadataregistry.org/uri/RegStatus/1001> ;
    a rdf:Property ;
    rdfs:isDefinedBy <http://rdaregistry.info/Elements/u/> ;
    rdfs:label "is television screenplay based on"@en ;
    rdfs:subPropertyOf <http://rdaregistry.info/Elements/u/P60231> ;
    owl:inverseOf <http://rdaregistry.info/Elements/u/P60186> ;
    skos:definition "Relates a resource to a resource that has been adapted as the screenplay for a television program."@en .

<http://rdaregistry.info/Elements/u/P60234>
    reg:hasSubproperty <http://rdaregistry.info/Elements/e/P20132> ;
    reg:lexicalAlias <http://rdaregistry.info/Elements/u/videoScreenplayBasedOn.en> ;
    reg:name "videoScreenplayBasedOn"@en ;
    reg:status <http://metadataregistry.org/uri/RegStatus/1001> ;
    a rdf:Property ;
    rdfs:isDefinedBy <http://rdaregistry.info/Elements/u/> ;
    rdfs:label "is video screenplay based on"@en ;
    rdfs:subPropertyOf <http://rdaregistry.info/Elements/u/P60231> ;
    owl:inverseOf <http://rdaregistry.info/Elements/u/P60187> ;
    skos:definition "Relates a resource to a resource that has been adapted as the screenplay for a video."@en .

<http://rdaregistry.info/Elements/u/P60235>
    reg:hasSubproperty <http://rdaregistry.info/Elements/e/P20133> ;
    reg:lexicalAlias <http://rdaregistry.info/Elements/u/radioScriptBasedOn.en> ;
    reg:name "radioScriptBasedOn"@en ;
    reg:status <http://metadataregistry.org/uri/RegStatus/1001> ;
    a rdf:Property ;
    rdfs:isDefinedBy <http://rdaregistry.info/Elements/u/> ;
    rdfs:label "is radio script based on"@en ;
    rdfs:subPropertyOf <http://rdaregistry.info/Elements/u/P60241> ;
    owl:inverseOf <http://rdaregistry.info/Elements/u/P60188> ;
    skos:definition "Relates a resource to a resource that has been adapted as the script for a radio program."@en .

<http://rdaregistry.info/Elements/u/P60236>
    reg:hasSubproperty <http://rdaregistry.info/Elements/e/P20134> ;
    reg:lexicalAlias <http://rdaregistry.info/Elements/u/videoAdaptationOf.en> ;
    reg:name "videoAdaptationOf"@en ;
    reg:status <http://metadataregistry.org/uri/RegStatus/1001> ;
    a rdf:Property ;
    rdfs:isDefinedBy <http://rdaregistry.info/Elements/u/> ;
    rdfs:label "is video adaptation of"@en ;
    rdfs:subPropertyOf <http://rdaregistry.info/Elements/u/P60241> ;
    owl:inverseOf <http://rdaregistry.info/Elements/u/P60361> ;
    skos:definition "Relates a resource to a resource that has been adapted for video."@en .

<http://rdaregistry.info/Elements/u/P60237>
    reg:hasSubproperty <http://rdaregistry.info/Elements/i/P40032> ;
    reg:lexicalAlias <http://rdaregistry.info/Elements/u/boundWith.en> ;
    reg:name "boundWith"@en ;
    reg:status <http://metadataregistry.org/uri/RegStatus/1001> ;
    a rdf:Property ;
    rdfs:isDefinedBy <http://rdaregistry.info/Elements/u/> ;
    rdfs:label "is bound with"@en ;
    rdfs:subPropertyOf <http://rdaregistry.info/Elements/u/P60196> ;
    owl:inverseOf <http://rdaregistry.info/Elements/u/P60237> ;
    skos:definition "Relates a resource to a resource that has been bound within the same binding as the resource being described."@en .

<http://rdaregistry.info/Elements/u/P60238>
    reg:hasSubproperty <http://rdaregistry.info/Elements/e/P20135> ;
    reg:lexicalAlias <http://rdaregistry.info/Elements/u/digestOf.en> ;
    reg:name "digestOf"@en ;
    reg:status <http://metadataregistry.org/uri/RegStatus/1001> ;
    a rdf:Property ;
    rdfs:isDefinedBy <http://rdaregistry.info/Elements/u/> ;
    rdfs:label "is digest of"@en ;
    rdfs:subPropertyOf <http://rdaregistry.info/Elements/u/P60305> ;
    owl:inverseOf <http://rdaregistry.info/Elements/u/P60279> ;
    skos:definition "Relates a resource to a resource that has been digested, i.e., systematically and comprehensively condensed."@en .

<http://rdaregistry.info/Elements/u/P60239>
    reg:hasSubproperty <http://rdaregistry.info/Elements/w/P10266>, <http://rdaregistry.info/Elements/w/P10272>, <http://rdaregistry.info/Elements/w/P10278> ;
    reg:lexicalAlias <http://rdaregistry.info/Elements/u/analysisOf.en> ;
    reg:name "analysisOf"@en ;
    reg:status <http://metadataregistry.org/uri/RegStatus/1001> ;
    a rdf:Property ;
    rdfs:isDefinedBy <http://rdaregistry.info/Elements/u/> ;
    rdfs:label "is analysis of"@en ;
    rdfs:subPropertyOf <http://rdaregistry.info/Elements/u/P60190> ;
    owl:inverseOf <http://rdaregistry.info/Elements/u/P60219> ;
    skos:definition "Relates a resource to a resource that has been examined to identify its components and their relations."@en .

<http://rdaregistry.info/Elements/u/P60240>
    reg:lexicalAlias <http://rdaregistry.info/Elements/u/seriesContainerOf.en> ;
    reg:name "seriesContainerOf"@en ;
    reg:status <http://metadataregistry.org/uri/RegStatus/1001> ;
    a rdf:Property ;
    rdfs:isDefinedBy <http://rdaregistry.info/Elements/u/> ;
    rdfs:label "is series container of"@en ;
    rdfs:subPropertyOf <http://rdaregistry.info/Elements/u/P60249> ;
    owl:inverseOf <http://rdaregistry.info/Elements/u/P60193> ;
    skos:definition "Relates a resource to a resource that has been issued as part of a series."@en .

<http://rdaregistry.info/Elements/u/P60241>
    reg:hasSubproperty <http://rdaregistry.info/Elements/e/P20152>, <http://rdaregistry.info/Elements/u/P60225>, <http://rdaregistry.info/Elements/u/P60226>, <http://rdaregistry.info/Elements/u/P60227>, <http://rdaregistry.info/Elements/u/P60228>, <http://rdaregistry.info/Elements/u/P60229>, <http://rdaregistry.info/Elements/u/P60230>, <http://rdaregistry.info/Elements/u/P60231>, <http://rdaregistry.info/Elements/u/P60235>, <http://rdaregistry.info/Elements/u/P60236>, <http://rdaregistry.info/Elements/u/P60743>, <http://rdaregistry.info/Elements/u/P60745> ;
    reg:lexicalAlias <http://rdaregistry.info/Elements/u/adaptationOf.en> ;
    reg:name "adaptationOf"@en ;
    reg:status <http://metadataregistry.org/uri/RegStatus/1001> ;
    a rdf:Property ;
    rdfs:isDefinedBy <http://rdaregistry.info/Elements/u/> ;
    rdfs:label "is adaptation of"@en ;
    rdfs:subPropertyOf <http://rdaregistry.info/Elements/u/P60305> ;
    owl:inverseOf <http://rdaregistry.info/Elements/u/P60260> ;
    skos:definition "Relates a resource to a resource that has been modified for a purpose, use, or medium other than that for which it was originally intended."@en .

<http://rdaregistry.info/Elements/u/P60242>
    reg:hasSubproperty <http://rdaregistry.info/Elements/e/P20139> ;
    reg:lexicalAlias <http://rdaregistry.info/Elements/u/arrangementOf.en> ;
    reg:name "arrangementOf"@en ;
    reg:status <http://metadataregistry.org/uri/RegStatus/1001> ;
    a rdf:Property ;
    rdfs:isDefinedBy <http://rdaregistry.info/Elements/u/> ;
    rdfs:label "is arrangement of"@en ;
    rdfs:subPropertyOf <http://rdaregistry.info/Elements/u/P60305> ;
    owl:inverseOf <http://rdaregistry.info/Elements/u/P60274> ;
    skos:definition "Relates a resource to a musical resource that has been rewritten for a medium of performance different from that for which the resource was originally intended."@en .

<http://rdaregistry.info/Elements/u/P60243>
    reg:hasSubproperty <http://rdaregistry.info/Elements/e/P20140> ;
    reg:lexicalAlias <http://rdaregistry.info/Elements/u/freeTranslationOf.en> ;
    reg:name "freeTranslationOf"@en ;
    reg:status <http://metadataregistry.org/uri/RegStatus/1001> ;
    a rdf:Property ;
    rdfs:isDefinedBy <http://rdaregistry.info/Elements/u/> ;
    rdfs:label "is free translation of"@en ;
    rdfs:subPropertyOf <http://rdaregistry.info/Elements/u/P60305> ;
    owl:inverseOf <http://rdaregistry.info/Elements/u/P60189> ;
    skos:definition "Relates a resource to a resource that has been translated freely, preserving the spirit of the original, but not its linguistic details."@en .

<http://rdaregistry.info/Elements/u/P60244>
    reg:hasSubproperty <http://rdaregistry.info/Elements/e/P20141>, <http://rdaregistry.info/Elements/u/P60111> ;
    reg:lexicalAlias <http://rdaregistry.info/Elements/u/translationOf.en> ;
    reg:name "translationOf"@en ;
    reg:status <http://metadataregistry.org/uri/RegStatus/1001> ;
    a rdf:Property ;
    rdfs:isDefinedBy <http://rdaregistry.info/Elements/u/> ;
    rdfs:label "is translation of"@en ;
    rdfs:subPropertyOf <http://rdaregistry.info/Elements/u/P60305> ;
    owl:inverseOf <http://rdaregistry.info/Elements/u/P60280> ;
    skos:definition "Relates a resource to a resource that has been translated, i.e., the text expressed in a language different from that of the original resource."@en .

<http://rdaregistry.info/Elements/u/P60245>
    reg:hasSubproperty <http://rdaregistry.info/Elements/e/P20211> ;
    reg:lexicalAlias <http://rdaregistry.info/Elements/u/revisedAs.en> ;
    reg:name "revisedAs"@en ;
    reg:status <http://metadataregistry.org/uri/RegStatus/1001> ;
    a rdf:Property ;
    rdfs:isDefinedBy <http://rdaregistry.info/Elements/u/> ;
    rdfs:label "is revised as"@en ;
    rdfs:subPropertyOf <http://rdaregistry.info/Elements/u/P60250> ;
    owl:inverseOf <http://rdaregistry.info/Elements/u/P60303> ;
    skos:definition "Relates a resource to a resource that has been updated, corrected, or expanded."@en .

<http://rdaregistry.info/Elements/u/P60246>
    reg:hasSubproperty <http://rdaregistry.info/Elements/e/P20142> ;
    reg:lexicalAlias <http://rdaregistry.info/Elements/u/parodiedAs.en> ;
    reg:name "parodiedAs"@en ;
    reg:status <http://metadataregistry.org/uri/RegStatus/1001> ;
    a rdf:Property ;
    rdfs:isDefinedBy <http://rdaregistry.info/Elements/u/> ;
    rdfs:label "is parodied as"@en ;
    rdfs:subPropertyOf <http://rdaregistry.info/Elements/u/P60214> ;
    owl:inverseOf <http://rdaregistry.info/Elements/u/P60312> ;
    skos:definition "Relates a resource to a resource that imitates the style or content of the source resource for comic effect."@en .

<http://rdaregistry.info/Elements/u/P60247>
    reg:hasSubproperty <http://rdaregistry.info/Elements/e/P20143> ;
    reg:lexicalAlias <http://rdaregistry.info/Elements/u/absorbedBy.en> ;
    reg:name "absorbedBy"@en ;
    reg:status <http://metadataregistry.org/uri/RegStatus/1001> ;
    a rdf:Property ;
    rdfs:isDefinedBy <http://rdaregistry.info/Elements/u/> ;
    rdfs:label "is absorbed by"@en ;
    rdfs:subPropertyOf <http://rdaregistry.info/Elements/u/P60278> ;
    owl:inverseOf <http://rdaregistry.info/Elements/u/P60574> ;
    skos:definition "Relates a resource to a resource that incorporates another resource."@en .

<http://rdaregistry.info/Elements/u/P60248>
    reg:hasSubproperty <http://rdaregistry.info/Elements/e/P20144> ;
    reg:lexicalAlias <http://rdaregistry.info/Elements/u/absorbedInPartBy.en> ;
    reg:name "absorbedInPartBy"@en ;
    reg:status <http://metadataregistry.org/uri/RegStatus/1001> ;
    a rdf:Property ;
    rdfs:isDefinedBy <http://rdaregistry.info/Elements/u/> ;
    rdfs:label "is absorbed in part by"@en ;
    rdfs:subPropertyOf <http://rdaregistry.info/Elements/u/P60278> ;
    owl:inverseOf <http://rdaregistry.info/Elements/u/P60575> ;
    skos:definition "Relates a resource to a resource that incorporates part of the content of another resource."@en .

<http://rdaregistry.info/Elements/u/P60249>
    reg:hasSubproperty <http://rdaregistry.info/Elements/e/P20145>, <http://rdaregistry.info/Elements/i/P40034>, <http://rdaregistry.info/Elements/m/P30033>, <http://rdaregistry.info/Elements/u/P60183>, <http://rdaregistry.info/Elements/u/P60207>, <http://rdaregistry.info/Elements/u/P60240>, <http://rdaregistry.info/Elements/u/P60300>, <http://rdaregistry.info/Elements/u/P60316> ;
    reg:lexicalAlias <http://rdaregistry.info/Elements/u/containerOf.en> ;
    reg:name "containerOf"@en ;
    reg:status <http://metadataregistry.org/uri/RegStatus/1001> ;
    a rdf:Property ;
    rdfs:isDefinedBy <http://rdaregistry.info/Elements/u/> ;
    rdfs:label "is container of"@en ;
    rdfs:subPropertyOf <http://rdaregistry.info/Elements/u/P60714> ;
    owl:inverseOf <http://rdaregistry.info/Elements/u/P60101> ;
    skos:definition "Relates a resource to a resource that is a discrete component of a larger resource."@en .

<http://rdaregistry.info/Elements/u/P60250>
    reg:hasSubproperty <http://rdaregistry.info/Elements/e/P20203>, <http://rdaregistry.info/Elements/u/P60115>, <http://rdaregistry.info/Elements/u/P60120>, <http://rdaregistry.info/Elements/u/P60121>, <http://rdaregistry.info/Elements/u/P60177>, <http://rdaregistry.info/Elements/u/P60178>, <http://rdaregistry.info/Elements/u/P60180>, <http://rdaregistry.info/Elements/u/P60189>, <http://rdaregistry.info/Elements/u/P60203>, <http://rdaregistry.info/Elements/u/P60205>, <http://rdaregistry.info/Elements/u/P60210>, <http://rdaregistry.info/Elements/u/P60214>, <http://rdaregistry.info/Elements/u/P60216>, <http://rdaregistry.info/Elements/u/P60245>, <http://rdaregistry.info/Elements/u/P60260>, <http://rdaregistry.info/Elements/u/P60273>, <http://rdaregistry.info/Elements/u/P60274>, <http://rdaregistry.info/Elements/u/P60275>, <http://rdaregistry.info/Elements/u/P60279>, <http://rdaregistry.info/Elements/u/P60280>, <http://rdaregistry.info/Elements/u/P60831>, <http://rdaregistry.info/Elements/u/P60833> ;
    reg:lexicalAlias <http://rdaregistry.info/Elements/u/derivative.en> ;
    reg:name "derivative"@en ;
    reg:status <http://metadataregistry.org/uri/RegStatus/1001> ;
    a rdf:Property ;
    rdfs:isDefinedBy <http://rdaregistry.info/Elements/u/> ;
    rdfs:label "is derivative"@en ;
    rdfs:subPropertyOf <http://rdaregistry.info/Elements/u/P60710> ;
    owl:inverseOf <http://rdaregistry.info/Elements/u/P60305> ;
    skos:definition "Relates a resource to a resource that is a modification of a source resource."@en .

<http://rdaregistry.info/Elements/u/P60251>
    reg:hasSubproperty <http://rdaregistry.info/Elements/e/P20146> ;
    reg:lexicalAlias <http://rdaregistry.info/Elements/u/errataTo.en> ;
    reg:name "errataTo"@en ;
    reg:status <http://metadataregistry.org/uri/RegStatus/1001> ;
    a rdf:Property ;
    rdfs:isDefinedBy <http://rdaregistry.info/Elements/u/> ;
    rdfs:label "is errata to"@en ;
    rdfs:subPropertyOf <http://rdaregistry.info/Elements/u/P60307> ;
    owl:inverseOf <http://rdaregistry.info/Elements/u/P60181> ;
    skos:definition "Relates a resource to a resource that is augmented by a list of errors in the predominant resource, discovered after publication, with their corrections."@en .

<http://rdaregistry.info/Elements/u/P60252>
    reg:hasSubproperty <http://rdaregistry.info/Elements/e/P20147> ;
    reg:lexicalAlias <http://rdaregistry.info/Elements/u/guideTo.en> ;
    reg:name "guideTo"@en ;
    reg:status <http://metadataregistry.org/uri/RegStatus/1001> ;
    a rdf:Property ;
    rdfs:isDefinedBy <http://rdaregistry.info/Elements/u/> ;
    rdfs:label "is guide to"@en ;
    rdfs:subPropertyOf <http://rdaregistry.info/Elements/u/P60307> ;
    owl:inverseOf <http://rdaregistry.info/Elements/u/P60222> ;
    skos:definition "Relates a resource to a resource that is augmented by another resource consisting of material to help the user of the predominant resource, such as notes, learning and study aids, exercises, problems, questions and answers, instructor or student materials, etc."@en .

<http://rdaregistry.info/Elements/u/P60253>
    reg:hasSubproperty <http://rdaregistry.info/Elements/e/P20089> ;
    reg:lexicalAlias <http://rdaregistry.info/Elements/u/appendixTo.en> ;
    reg:name "appendixTo"@en ;
    reg:status <http://metadataregistry.org/uri/RegStatus/1001> ;
    a rdf:Property ;
    rdfs:isDefinedBy <http://rdaregistry.info/Elements/u/> ;
    rdfs:label "is appendix to"@en ;
    rdfs:subPropertyOf <http://rdaregistry.info/Elements/u/P60307> ;
    owl:inverseOf <http://rdaregistry.info/Elements/u/P60221> ;
    skos:definition "Relates a resource to a resource that is augmented by another resource that consists of material that is not essential to the completeness of the content, such as a list of references, statistical tables, and explanatory matter; the augmenting resource can either come at the end of the content, or be issued separately."@en .

<http://rdaregistry.info/Elements/u/P60254>
    reg:hasSubproperty <http://rdaregistry.info/Elements/e/P20148> ;
    reg:lexicalAlias <http://rdaregistry.info/Elements/u/illustrationsFor.en> ;
    reg:name "illustrationsFor"@en ;
    reg:status <http://metadataregistry.org/uri/RegStatus/1001> ;
    a rdf:Property ;
    rdfs:isDefinedBy <http://rdaregistry.info/Elements/u/> ;
    rdfs:label "is illustrations for"@en ;
    rdfs:subPropertyOf <http://rdaregistry.info/Elements/u/P60307> ;
    owl:inverseOf <http://rdaregistry.info/Elements/u/P60182> ;
    skos:definition "Relates a resource to a resource that is augmented by pictorial content designed to explain or decorate it."@en .

<http://rdaregistry.info/Elements/u/P60255>
    reg:hasSubproperty <http://rdaregistry.info/Elements/w/P10267>, <http://rdaregistry.info/Elements/w/P10273>, <http://rdaregistry.info/Elements/w/P10279> ;
    reg:lexicalAlias <http://rdaregistry.info/Elements/u/evaluationOf.en> ;
    reg:name "evaluationOf"@en ;
    reg:status <http://metadataregistry.org/uri/RegStatus/1001> ;
    a rdf:Property ;
    rdfs:isDefinedBy <http://rdaregistry.info/Elements/u/> ;
    rdfs:label "is evaluation of"@en ;
    rdfs:subPropertyOf <http://rdaregistry.info/Elements/u/P60190> ;
    owl:inverseOf <http://rdaregistry.info/Elements/u/P60218> ;
    skos:definition "Relates a resource to a resource that is examined or judged."@en .

<http://rdaregistry.info/Elements/u/P60256>
    reg:hasSubproperty <http://rdaregistry.info/Elements/m/P30035>, <http://rdaregistry.info/Elements/u/P60257>, <http://rdaregistry.info/Elements/u/P60258> ;
    reg:lexicalAlias <http://rdaregistry.info/Elements/u/issuedWith.en> ;
    reg:name "issuedWith"@en ;
    reg:status <http://metadataregistry.org/uri/RegStatus/1001> ;
    a rdf:Property ;
    rdfs:isDefinedBy <http://rdaregistry.info/Elements/u/> ;
    rdfs:label "is issued with"@en ;
    rdfs:subPropertyOf <http://rdaregistry.info/Elements/u/P60196> ;
    owl:inverseOf <http://rdaregistry.info/Elements/u/P60256> ;
    skos:definition "Relates a resource to a resource that is issued on the same carrier as the resource being described."@en .

<http://rdaregistry.info/Elements/u/P60257>
    reg:hasSubproperty <http://rdaregistry.info/Elements/i/P40035>, <http://rdaregistry.info/Elements/m/P30036> ;
    reg:lexicalAlias <http://rdaregistry.info/Elements/u/onDiscWith.en> ;
    reg:name "onDiscWith"@en ;
    reg:status <http://metadataregistry.org/uri/RegStatus/1001> ;
    a rdf:Property ;
    rdfs:isDefinedBy <http://rdaregistry.info/Elements/u/> ;
    rdfs:label "is on disc with"@en ;
    rdfs:subPropertyOf <http://rdaregistry.info/Elements/u/P60256> ;
    owl:inverseOf <http://rdaregistry.info/Elements/u/P60257> ;
    skos:definition "Relates a resource to a resource that is issued on the same disc with the resource being described."@en .

<http://rdaregistry.info/Elements/u/P60258>
    reg:hasSubproperty <http://rdaregistry.info/Elements/i/P40036>, <http://rdaregistry.info/Elements/m/P30037> ;
    reg:lexicalAlias <http://rdaregistry.info/Elements/u/filmedWith.en> ;
    reg:name "filmedWith"@en ;
    reg:status <http://metadataregistry.org/uri/RegStatus/1001> ;
    a rdf:Property ;
    rdfs:isDefinedBy <http://rdaregistry.info/Elements/u/> ;
    rdfs:label "is filmed with"@en ;
    rdfs:subPropertyOf <http://rdaregistry.info/Elements/u/P60256> ;
    owl:inverseOf <http://rdaregistry.info/Elements/u/P60258> ;
    skos:definition "Relates a resource to a resource that is issued on the same microform with the resource being described."@en .

<http://rdaregistry.info/Elements/u/P60259>
    reg:hasSubproperty <http://rdaregistry.info/Elements/e/P20151> ;
    reg:lexicalAlias <http://rdaregistry.info/Elements/u/supplementTo.en> ;
    reg:name "supplementTo"@en ;
    reg:status <http://metadataregistry.org/uri/RegStatus/1001> ;
    a rdf:Property ;
    rdfs:isDefinedBy <http://rdaregistry.info/Elements/u/> ;
    rdfs:label "is supplement to"@en ;
    rdfs:subPropertyOf <http://rdaregistry.info/Elements/u/P60307> ;
    owl:inverseOf <http://rdaregistry.info/Elements/u/P60281> ;
    skos:definition "Relates a resource to a resource that is updated or otherwise complemented by the augmenting resource."@en .

<http://rdaregistry.info/Elements/u/P60260>
    reg:hasSubproperty <http://rdaregistry.info/Elements/e/P20153>, <http://rdaregistry.info/Elements/u/P60088>, <http://rdaregistry.info/Elements/u/P60106>, <http://rdaregistry.info/Elements/u/P60110>, <http://rdaregistry.info/Elements/u/P60138>, <http://rdaregistry.info/Elements/u/P60174>, <http://rdaregistry.info/Elements/u/P60185>, <http://rdaregistry.info/Elements/u/P60188>, <http://rdaregistry.info/Elements/u/P60354>, <http://rdaregistry.info/Elements/u/P60361>, <http://rdaregistry.info/Elements/u/P60742>, <http://rdaregistry.info/Elements/u/P60744> ;
    reg:lexicalAlias <http://rdaregistry.info/Elements/u/adaptedAs.en> ;
    reg:name "adaptedAs"@en ;
    reg:status <http://metadataregistry.org/uri/RegStatus/1001> ;
    a rdf:Property ;
    rdfs:isDefinedBy <http://rdaregistry.info/Elements/u/> ;
    rdfs:label "is adapted as"@en ;
    rdfs:subPropertyOf <http://rdaregistry.info/Elements/u/P60250> ;
    owl:inverseOf <http://rdaregistry.info/Elements/u/P60241> ;
    skos:definition "Relates a resource to a resource that modifies the source resource for a purpose, use, or medium other than that for which it was originally intended."@en .

<http://rdaregistry.info/Elements/u/P60261>
    reg:hasSubproperty <http://rdaregistry.info/Elements/e/P20154>, <http://rdaregistry.info/Elements/u/P60220>, <http://rdaregistry.info/Elements/u/P60276>, <http://rdaregistry.info/Elements/u/P60277>, <http://rdaregistry.info/Elements/u/P60479>, <http://rdaregistry.info/Elements/u/P60480>, <http://rdaregistry.info/Elements/u/P60505>, <http://rdaregistry.info/Elements/u/P60574>, <http://rdaregistry.info/Elements/u/P60575>, <http://rdaregistry.info/Elements/u/P60576>, <http://rdaregistry.info/Elements/u/P60577> ;
    reg:lexicalAlias <http://rdaregistry.info/Elements/u/precededBy.en> ;
    reg:name "precededBy"@en ;
    reg:status <http://metadataregistry.org/uri/RegStatus/1001> ;
    a rdf:Property ;
    rdfs:isDefinedBy <http://rdaregistry.info/Elements/u/> ;
    rdfs:label "is preceded by"@en ;
    rdfs:subPropertyOf <http://rdaregistry.info/Elements/u/P60713> ;
    owl:inverseOf <http://rdaregistry.info/Elements/u/P60278> ;
    skos:definition "Relates a resource to a resource that precedes (e.g., is earlier in time or before in a narrative) the succeeding resource."@en .

<http://rdaregistry.info/Elements/u/P60262>
    reg:hasSubproperty <http://rdaregistry.info/Elements/e/P20155> ;
    reg:lexicalAlias <http://rdaregistry.info/Elements/u/findingAid.en> ;
    reg:name "findingAid"@en ;
    reg:status <http://metadataregistry.org/uri/RegStatus/1001> ;
    a rdf:Property ;
    rdfs:isDefinedBy <http://rdaregistry.info/Elements/u/> ;
    rdfs:label "is finding aid"@en ;
    rdfs:subPropertyOf <http://rdaregistry.info/Elements/u/P60204> ;
    owl:inverseOf <http://rdaregistry.info/Elements/u/P60474> ;
    skos:definition "Relates a resource to a resource that provides a guide to the organization, arrangement, and contents of an archival collection."@en .

<http://rdaregistry.info/Elements/u/P60263>
    reg:hasSubproperty <http://rdaregistry.info/Elements/e/P20156> ;
    reg:lexicalAlias <http://rdaregistry.info/Elements/u/index.en> ;
    reg:name "index"@en ;
    reg:status <http://metadataregistry.org/uri/RegStatus/1001> ;
    a rdf:Property ;
    rdfs:isDefinedBy <http://rdaregistry.info/Elements/u/> ;
    rdfs:label "is index"@en ;
    rdfs:subPropertyOf <http://rdaregistry.info/Elements/u/P60204> ;
    owl:inverseOf <http://rdaregistry.info/Elements/u/P60302> ;
    skos:definition "Relates a resource to a resource that provides a systematic, alphabetical guide to the contents of the predominant resource, usually keyed to page numbers or other reference codes."@en .

<http://rdaregistry.info/Elements/u/P60264>
    reg:hasSubproperty <http://rdaregistry.info/Elements/e/P20157>, <http://rdaregistry.info/Elements/u/P60265>, <http://rdaregistry.info/Elements/u/P60268>, <http://rdaregistry.info/Elements/u/P60269> ;
    reg:lexicalAlias <http://rdaregistry.info/Elements/u/screenplay.en> ;
    reg:name "screenplay"@en ;
    reg:status <http://metadataregistry.org/uri/RegStatus/1001> ;
    a rdf:Property ;
    rdfs:isDefinedBy <http://rdaregistry.info/Elements/u/> ;
    rdfs:label "is screenplay"@en ;
    rdfs:subPropertyOf <http://rdaregistry.info/Elements/u/P60198> ;
    owl:inverseOf <http://rdaregistry.info/Elements/u/P60201> ;
    skos:definition "Relates a resource to a resource that provides the text for a motion picture, television program or video."@en .

<http://rdaregistry.info/Elements/u/P60265>
    reg:hasSubproperty <http://rdaregistry.info/Elements/e/P20158> ;
    reg:lexicalAlias <http://rdaregistry.info/Elements/u/motionPictureScreenplay.en> ;
    reg:name "motionPictureScreenplay"@en ;
    reg:status <http://metadataregistry.org/uri/RegStatus/1001> ;
    a rdf:Property ;
    rdfs:isDefinedBy <http://rdaregistry.info/Elements/u/> ;
    rdfs:label "is motion picture screenplay"@en ;
    rdfs:subPropertyOf <http://rdaregistry.info/Elements/u/P60264> ;
    owl:inverseOf <http://rdaregistry.info/Elements/u/P60282> ;
    skos:definition "Relates a resource to a resource that provides the text for a motion picture."@en .

<http://rdaregistry.info/Elements/u/P60266>
    reg:hasSubproperty <http://rdaregistry.info/Elements/e/P20159> ;
    reg:lexicalAlias <http://rdaregistry.info/Elements/u/musicalSettingOf.en> ;
    reg:name "musicalSettingOf"@en ;
    reg:status <http://metadataregistry.org/uri/RegStatus/1001> ;
    a rdf:Property ;
    rdfs:isDefinedBy <http://rdaregistry.info/Elements/u/> ;
    rdfs:label "is musical setting of"@en ;
    rdfs:subPropertyOf <http://rdaregistry.info/Elements/u/P60305> ;
    owl:inverseOf <http://rdaregistry.info/Elements/u/P60121> ;
    skos:definition "Relates a resource to a resource that provides the text for a non-dramatic musical resource, other than an oratorio."@en .

<http://rdaregistry.info/Elements/u/P60267>
    reg:hasSubproperty <http://rdaregistry.info/Elements/e/P20160> ;
    reg:lexicalAlias <http://rdaregistry.info/Elements/u/radioScript.en> ;
    reg:name "radioScript"@en ;
    reg:status <http://metadataregistry.org/uri/RegStatus/1001> ;
    a rdf:Property ;
    rdfs:isDefinedBy <http://rdaregistry.info/Elements/u/> ;
    rdfs:label "is radio script"@en ;
    rdfs:subPropertyOf <http://rdaregistry.info/Elements/u/P60198> ;
    owl:inverseOf <http://rdaregistry.info/Elements/u/P60285> ;
    skos:definition "Relates a resource to a resource that provides the text for a radio program."@en .

<http://rdaregistry.info/Elements/u/P60268>
    reg:hasSubproperty <http://rdaregistry.info/Elements/e/P20161> ;
    reg:lexicalAlias <http://rdaregistry.info/Elements/u/televisionScreenplay.en> ;
    reg:name "televisionScreenplay"@en ;
    reg:status <http://metadataregistry.org/uri/RegStatus/1001> ;
    a rdf:Property ;
    rdfs:isDefinedBy <http://rdaregistry.info/Elements/u/> ;
    rdfs:label "is television screenplay"@en ;
    rdfs:subPropertyOf <http://rdaregistry.info/Elements/u/P60264> ;
    owl:inverseOf <http://rdaregistry.info/Elements/u/P60283> ;
    skos:definition "Relates a resource to a resource that provides the text for a television program."@en .

<http://rdaregistry.info/Elements/u/P60269>
    reg:hasSubproperty <http://rdaregistry.info/Elements/e/P20162> ;
    reg:lexicalAlias <http://rdaregistry.info/Elements/u/videoScreenplay.en> ;
    reg:name "videoScreenplay"@en ;
    reg:status <http://metadataregistry.org/uri/RegStatus/1001> ;
    a rdf:Property ;
    rdfs:isDefinedBy <http://rdaregistry.info/Elements/u/> ;
    rdfs:label "is video screenplay"@en ;
    rdfs:subPropertyOf <http://rdaregistry.info/Elements/u/P60264> ;
    owl:inverseOf <http://rdaregistry.info/Elements/u/P60284> ;
    skos:definition "Relates a resource to a resource that provides the text for a video."@en .

<http://rdaregistry.info/Elements/u/P60270>
    reg:hasSubproperty <http://rdaregistry.info/Elements/e/P20163> ;
    reg:lexicalAlias <http://rdaregistry.info/Elements/u/libretto.en> ;
    reg:name "libretto"@en ;
    reg:status <http://metadataregistry.org/uri/RegStatus/1001> ;
    a rdf:Property ;
    rdfs:isDefinedBy <http://rdaregistry.info/Elements/u/> ;
    rdfs:label "is libretto"@en ;
    rdfs:subPropertyOf <http://rdaregistry.info/Elements/u/P60198> ;
    owl:inverseOf <http://rdaregistry.info/Elements/u/P60117> ;
    skos:definition "Relates a resource to a resource that provides the text of an opera or other resource for the musical stage, or an oratorio."@en .

<http://rdaregistry.info/Elements/u/P60271>
    reg:hasSubproperty <http://rdaregistry.info/Elements/i/P40060>, <http://rdaregistry.info/Elements/m/P30038> ;
    reg:lexicalAlias <http://rdaregistry.info/Elements/u/reprintedAs.en> ;
    reg:name "reprintedAs"@en ;
    reg:status <http://metadataregistry.org/uri/RegStatus/1001> ;
    a rdf:Property ;
    rdfs:isDefinedBy <http://rdaregistry.info/Elements/u/> ;
    rdfs:label "is reprinted as"@en ;
    rdfs:subPropertyOf <http://rdaregistry.info/Elements/u/P60272> ;
    owl:inverseOf <http://rdaregistry.info/Elements/u/P60168> ;
    skos:definition "Relates a resource to a resource that reissues the same expression of the resource as the printed resource being described."@en .

<http://rdaregistry.info/Elements/u/P60272>
    reg:hasSubproperty <http://rdaregistry.info/Elements/i/P40055>, <http://rdaregistry.info/Elements/m/P30039>, <http://rdaregistry.info/Elements/u/P60083>, <http://rdaregistry.info/Elements/u/P60200>, <http://rdaregistry.info/Elements/u/P60217>, <http://rdaregistry.info/Elements/u/P60271> ;
    reg:lexicalAlias <http://rdaregistry.info/Elements/u/reproducedAs.en> ;
    reg:name "reproducedAs"@en ;
    reg:status <http://metadataregistry.org/uri/RegStatus/1001> ;
    a rdf:Property ;
    rdfs:isDefinedBy <http://rdaregistry.info/Elements/u/> ;
    rdfs:label "is reproduced as"@en ;
    rdfs:subPropertyOf <http://rdaregistry.info/Elements/u/P60191> ;
    owl:inverseOf <http://rdaregistry.info/Elements/u/P60297> ;
    skos:definition "Relates a resource to a resource that reproduces another resource."@en .

<http://rdaregistry.info/Elements/u/P60273>
    reg:hasSubproperty <http://rdaregistry.info/Elements/e/P20164> ;
    reg:lexicalAlias <http://rdaregistry.info/Elements/u/paraphrasedAs.en> ;
    reg:name "paraphrasedAs"@en ;
    reg:status <http://metadataregistry.org/uri/RegStatus/1001> ;
    a rdf:Property ;
    rdfs:isDefinedBy <http://rdaregistry.info/Elements/u/> ;
    rdfs:label "is paraphrased as"@en ;
    rdfs:subPropertyOf <http://rdaregistry.info/Elements/u/P60250> ;
    owl:inverseOf <http://rdaregistry.info/Elements/u/P60296> ;
    skos:definition "Relates a resource to a resource that restates the content of the source resource in a different form."@en .

<http://rdaregistry.info/Elements/u/P60274>
    reg:hasSubproperty <http://rdaregistry.info/Elements/e/P20165> ;
    reg:lexicalAlias <http://rdaregistry.info/Elements/u/arrangedAs.en> ;
    reg:name "arrangedAs"@en ;
    reg:status <http://metadataregistry.org/uri/RegStatus/1001> ;
    a rdf:Property ;
    rdfs:isDefinedBy <http://rdaregistry.info/Elements/u/> ;
    rdfs:label "is arranged as"@en ;
    rdfs:subPropertyOf <http://rdaregistry.info/Elements/u/P60250> ;
    owl:inverseOf <http://rdaregistry.info/Elements/u/P60242> ;
    skos:definition "Relates a resource to a musical resource that rewrites the source resource for a medium of performance different from that for which the resource was originally intended."@en .

<http://rdaregistry.info/Elements/u/P60275>
    reg:hasSubproperty <http://rdaregistry.info/Elements/e/P20166> ;
    reg:lexicalAlias <http://rdaregistry.info/Elements/u/abridgedAs.en> ;
    reg:name "abridgedAs"@en ;
    reg:status <http://metadataregistry.org/uri/RegStatus/1001> ;
    a rdf:Property ;
    rdfs:isDefinedBy <http://rdaregistry.info/Elements/u/> ;
    rdfs:label "is abridged as"@en ;
    rdfs:subPropertyOf <http://rdaregistry.info/Elements/u/P60250> ;
    owl:inverseOf <http://rdaregistry.info/Elements/u/P60223> ;
    skos:definition "Relates a resource to a resource that shortens the source resource without changing the general meaning or manner of presentation."@en .

<http://rdaregistry.info/Elements/u/P60276>
    reg:hasSubproperty <http://rdaregistry.info/Elements/e/P20167> ;
    reg:lexicalAlias <http://rdaregistry.info/Elements/u/continuationInPartOf.en> ;
    reg:name "continuationInPartOf"@en ;
    reg:status <http://metadataregistry.org/uri/RegStatus/1001> ;
    a rdf:Property ;
    rdfs:isDefinedBy <http://rdaregistry.info/Elements/u/> ;
    rdfs:label "is continuation in part of"@en ;
    rdfs:subPropertyOf <http://rdaregistry.info/Elements/u/P60261> ;
    owl:inverseOf <http://rdaregistry.info/Elements/u/P60503> ;
    skos:definition "Relates a resource to a resource that split into two or more separate resources with new titles."@en .

<http://rdaregistry.info/Elements/u/P60277>
    reg:hasSubproperty <http://rdaregistry.info/Elements/e/P20168> ;
    reg:lexicalAlias <http://rdaregistry.info/Elements/u/separatedFrom.en> ;
    reg:name "separatedFrom"@en ;
    reg:status <http://metadataregistry.org/uri/RegStatus/1001> ;
    a rdf:Property ;
    rdfs:isDefinedBy <http://rdaregistry.info/Elements/u/> ;
    rdfs:label "is separated from"@en ;
    rdfs:subPropertyOf <http://rdaregistry.info/Elements/u/P60261> ;
    owl:inverseOf <http://rdaregistry.info/Elements/u/P60199> ;
    skos:definition "Relates a resource to a resource that spun off a part of its content to form a new resource."@en .

<http://rdaregistry.info/Elements/u/P60278>
    reg:hasSubproperty <http://rdaregistry.info/Elements/e/P20169>, <http://rdaregistry.info/Elements/u/P60102>, <http://rdaregistry.info/Elements/u/P60103>, <http://rdaregistry.info/Elements/u/P60104>, <http://rdaregistry.info/Elements/u/P60199>, <http://rdaregistry.info/Elements/u/P60247>, <http://rdaregistry.info/Elements/u/P60248>, <http://rdaregistry.info/Elements/u/P60306>, <http://rdaregistry.info/Elements/u/P60310>, <http://rdaregistry.info/Elements/u/P60503>, <http://rdaregistry.info/Elements/u/P60504> ;
    reg:lexicalAlias <http://rdaregistry.info/Elements/u/succeededBy.en> ;
    reg:name "succeededBy"@en ;
    reg:status <http://metadataregistry.org/uri/RegStatus/1001> ;
    a rdf:Property ;
    rdfs:isDefinedBy <http://rdaregistry.info/Elements/u/> ;
    rdfs:label "is succeeded by"@en ;
    rdfs:subPropertyOf <http://rdaregistry.info/Elements/u/P60713> ;
    owl:inverseOf <http://rdaregistry.info/Elements/u/P60261> ;
    skos:definition "Relates a resource to a resource that succeeds (e.g., later in time or after in a narrative) the preceding resource."@en .

<http://rdaregistry.info/Elements/u/P60279>
    reg:hasSubproperty <http://rdaregistry.info/Elements/e/P20170> ;
    reg:lexicalAlias <http://rdaregistry.info/Elements/u/digestedAs.en> ;
    reg:name "digestedAs"@en ;
    reg:status <http://metadataregistry.org/uri/RegStatus/1001> ;
    a rdf:Property ;
    rdfs:isDefinedBy <http://rdaregistry.info/Elements/u/> ;
    rdfs:label "is digested as"@en ;
    rdfs:subPropertyOf <http://rdaregistry.info/Elements/u/P60250> ;
    owl:inverseOf <http://rdaregistry.info/Elements/u/P60238> ;
    skos:definition "Relates a resource to a resource that systematically and comprehensively condenses the source resource."@en .

<http://rdaregistry.info/Elements/u/P60280>
    reg:hasSubproperty <http://rdaregistry.info/Elements/e/P20171>, <http://rdaregistry.info/Elements/u/P60112> ;
    reg:lexicalAlias <http://rdaregistry.info/Elements/u/translatedAs.en> ;
    reg:name "translatedAs"@en ;
    reg:status <http://metadataregistry.org/uri/RegStatus/1001> ;
    a rdf:Property ;
    rdfs:isDefinedBy <http://rdaregistry.info/Elements/u/> ;
    rdfs:label "is translated as"@en ;
    rdfs:subPropertyOf <http://rdaregistry.info/Elements/u/P60250> ;
    owl:inverseOf <http://rdaregistry.info/Elements/u/P60244> ;
    skos:definition "Relates a resource to a resource that translates the text of the source entity into a language different from that of the original resource."@en .

<http://rdaregistry.info/Elements/u/P60281>
    reg:hasSubproperty <http://rdaregistry.info/Elements/e/P20172> ;
    reg:lexicalAlias <http://rdaregistry.info/Elements/u/supplement.en> ;
    reg:name "supplement"@en ;
    reg:status <http://metadataregistry.org/uri/RegStatus/1001> ;
    a rdf:Property ;
    rdfs:isDefinedBy <http://rdaregistry.info/Elements/u/> ;
    rdfs:label "is supplement"@en ;
    rdfs:subPropertyOf <http://rdaregistry.info/Elements/u/P60204> ;
    owl:inverseOf <http://rdaregistry.info/Elements/u/P60259> ;
    skos:definition "Relates a resource to a resource that updates or otherwise complements the predominant resource."@en .

<http://rdaregistry.info/Elements/u/P60282>
    reg:hasSubproperty <http://rdaregistry.info/Elements/e/P20173> ;
    reg:lexicalAlias <http://rdaregistry.info/Elements/u/screenplayForTheMotionPicture.en> ;
    reg:name "screenplayForTheMotionPicture"@en ;
    reg:status <http://metadataregistry.org/uri/RegStatus/1001> ;
    a rdf:Property ;
    rdfs:isDefinedBy <http://rdaregistry.info/Elements/u/> ;
    rdfs:label "is screenplay for motion picture"@en ;
    rdfs:subPropertyOf <http://rdaregistry.info/Elements/u/P60201> ;
    owl:inverseOf <http://rdaregistry.info/Elements/u/P60265> ;
    skos:definition "Relates a resource to a resource that uses the text as a screenplay for a motion picture."@en .

<http://rdaregistry.info/Elements/u/P60283>
    reg:hasSubproperty <http://rdaregistry.info/Elements/e/P20174> ;
    reg:lexicalAlias <http://rdaregistry.info/Elements/u/screenplayForTheTelevisionProgram.en> ;
    reg:name "screenplayForTheTelevisionProgram"@en ;
    reg:status <http://metadataregistry.org/uri/RegStatus/1001> ;
    a rdf:Property ;
    rdfs:isDefinedBy <http://rdaregistry.info/Elements/u/> ;
    rdfs:label "is screenplay for television program"@en ;
    rdfs:subPropertyOf <http://rdaregistry.info/Elements/u/P60201> ;
    owl:inverseOf <http://rdaregistry.info/Elements/u/P60268> ;
    skos:definition "Relates a resource to a resource that uses the text as a screenplay for a television program."@en .

<http://rdaregistry.info/Elements/u/P60284>
    reg:hasSubproperty <http://rdaregistry.info/Elements/e/P20175> ;
    reg:lexicalAlias <http://rdaregistry.info/Elements/u/screenplayForTheVideo.en> ;
    reg:name "screenplayForTheVideo"@en ;
    reg:status <http://metadataregistry.org/uri/RegStatus/1001> ;
    a rdf:Property ;
    rdfs:isDefinedBy <http://rdaregistry.info/Elements/u/> ;
    rdfs:label "is screenplay for video"@en ;
    rdfs:subPropertyOf <http://rdaregistry.info/Elements/u/P60201> ;
    owl:inverseOf <http://rdaregistry.info/Elements/u/P60269> ;
    skos:definition "Relates a resource to a resource that uses the text as a screenplay for a video."@en .

<http://rdaregistry.info/Elements/u/P60285>
    reg:hasSubproperty <http://rdaregistry.info/Elements/e/P20176> ;
    reg:lexicalAlias <http://rdaregistry.info/Elements/u/scriptForTheRadioProgram.en> ;
    reg:name "scriptForTheRadioProgram"@en ;
    reg:status <http://metadataregistry.org/uri/RegStatus/1001> ;
    a rdf:Property ;
    rdfs:isDefinedBy <http://rdaregistry.info/Elements/u/> ;
    rdfs:label "is script for radio program"@en ;
    rdfs:subPropertyOf <http://rdaregistry.info/Elements/u/P60198> ;
    owl:inverseOf <http://rdaregistry.info/Elements/u/P60267> ;
    skos:definition "Relates a resource to a resource that uses the text of the source resource as the script for a radio program."@en .

<http://rdaregistry.info/Elements/u/P60286>
    reg:hasSubproperty <http://rdaregistry.info/Elements/e/P20177> ;
    reg:lexicalAlias <http://rdaregistry.info/Elements/u/addendaTo.en> ;
    reg:name "addendaTo"@en ;
    reg:status <http://metadataregistry.org/uri/RegStatus/1001> ;
    a rdf:Property ;
    rdfs:isDefinedBy <http://rdaregistry.info/Elements/u/> ;
    rdfs:label "is addenda to"@en ;
    rdfs:subPropertyOf <http://rdaregistry.info/Elements/u/P60307> ;
    owl:inverseOf <http://rdaregistry.info/Elements/u/P60209> ;
    skos:definition "Relates a resource to a resource that is a predominant resource augmented with brief material, less extensive than a supplement but essential to the completeness of the predominant resource, usually added at the end of the predominant resource but sometimes issued separately."@en .

<http://rdaregistry.info/Elements/u/P60287>
    reg:hasSubproperty <http://rdaregistry.info/Elements/i/P40039>, <http://rdaregistry.info/Elements/m/P30040> ;
    reg:lexicalAlias <http://rdaregistry.info/Elements/u/digitalTransferOf.en> ;
    reg:name "digitalTransferOf"@en ;
    reg:status <http://metadataregistry.org/uri/RegStatus/1001> ;
    a rdf:Property ;
    rdfs:isDefinedBy <http://rdaregistry.info/Elements/u/> ;
    rdfs:label "is digital transfer of"@en ;
    rdfs:subPropertyOf <http://rdaregistry.info/Elements/u/P60297> ;
    owl:inverseOf <http://rdaregistry.info/Elements/u/P60200> ;
    skos:definition "Relates a resource to a resource in a digital format that is transferred to another digital format."@en .

<http://rdaregistry.info/Elements/u/P60288>
    reg:hasSubproperty <http://rdaregistry.info/Elements/w/P10268>, <http://rdaregistry.info/Elements/w/P10274>, <http://rdaregistry.info/Elements/w/P10280> ;
    reg:lexicalAlias <http://rdaregistry.info/Elements/u/reviewOf.en> ;
    reg:name "reviewOf"@en ;
    reg:status <http://metadataregistry.org/uri/RegStatus/1001> ;
    a rdf:Property ;
    rdfs:isDefinedBy <http://rdaregistry.info/Elements/u/> ;
    rdfs:label "is review of"@en ;
    rdfs:subPropertyOf <http://rdaregistry.info/Elements/u/P60190> ;
    owl:inverseOf <http://rdaregistry.info/Elements/u/P60211> ;
    skos:definition "Relates a resource to a resource used as the basis for a brief evaluation."@en .

<http://rdaregistry.info/Elements/u/P60289>
    reg:hasSubproperty <http://rdaregistry.info/Elements/e/P20179> ;
    reg:lexicalAlias <http://rdaregistry.info/Elements/u/summaryOf.en> ;
    reg:name "summaryOf"@en ;
    reg:status <http://metadataregistry.org/uri/RegStatus/1001> ;
    a rdf:Property ;
    rdfs:isDefinedBy <http://rdaregistry.info/Elements/u/> ;
    rdfs:label "is summary of"@en ;
    rdfs:subPropertyOf <http://rdaregistry.info/Elements/u/P60305> ;
    owl:inverseOf <http://rdaregistry.info/Elements/u/P60205> ;
    skos:definition "Relates a resource to a resource used as the basis for a brief recapitulation of its content."@en .

<http://rdaregistry.info/Elements/u/P60290>
    reg:hasSubproperty <http://rdaregistry.info/Elements/e/P20180> ;
    reg:lexicalAlias <http://rdaregistry.info/Elements/u/catalogueOf.en> ;
    reg:name "catalogueOf"@en ;
    reg:status <http://metadataregistry.org/uri/RegStatus/1001> ;
    a rdf:Property ;
    rdfs:isDefinedBy <http://rdaregistry.info/Elements/u/> ;
    rdfs:label "is catalogue of"@en ;
    rdfs:subPropertyOf <http://rdaregistry.info/Elements/u/P60307> ;
    owl:inverseOf <http://rdaregistry.info/Elements/u/P60206> ;
    skos:definition "Relates a resource to a resource used as the basis for a catalogue, i.e., a complete enumeration of resources arranged systematically."@en .

<http://rdaregistry.info/Elements/u/P60291>
    reg:hasSubproperty <http://rdaregistry.info/Elements/e/P20181> ;
    reg:lexicalAlias <http://rdaregistry.info/Elements/u/concordanceTo.en> ;
    reg:name "concordanceTo"@en ;
    reg:status <http://metadataregistry.org/uri/RegStatus/1001> ;
    a rdf:Property ;
    rdfs:isDefinedBy <http://rdaregistry.info/Elements/u/> ;
    rdfs:label "is concordance to"@en ;
    rdfs:subPropertyOf <http://rdaregistry.info/Elements/u/P60307> ;
    owl:inverseOf <http://rdaregistry.info/Elements/u/P60208> ;
    skos:definition "Relates a resource to a resource used as the basis for a concordance, i.e. an index of all the words in the predominant resource."@en .

<http://rdaregistry.info/Elements/u/P60292>
    reg:hasSubproperty <http://rdaregistry.info/Elements/w/P10269>, <http://rdaregistry.info/Elements/w/P10275>, <http://rdaregistry.info/Elements/w/P10281> ;
    reg:lexicalAlias <http://rdaregistry.info/Elements/u/critiqueOf.en> ;
    reg:name "critiqueOf"@en ;
    reg:status <http://metadataregistry.org/uri/RegStatus/1001> ;
    a rdf:Property ;
    rdfs:isDefinedBy <http://rdaregistry.info/Elements/u/> ;
    rdfs:label "is critique of"@en ;
    rdfs:subPropertyOf <http://rdaregistry.info/Elements/u/P60190> ;
    owl:inverseOf <http://rdaregistry.info/Elements/u/P60212> ;
    skos:definition "Relates a resource to a resource used as the basis for a critical evaluation."@en .

<http://rdaregistry.info/Elements/u/P60293>
    reg:hasSubproperty <http://rdaregistry.info/Elements/e/P20183> ;
    reg:lexicalAlias <http://rdaregistry.info/Elements/u/choreographicAdaptationOf.en> ;
    reg:name "choreographicAdaptationOf"@en ;
    reg:status <http://metadataregistry.org/uri/RegStatus/1001> ;
    a rdf:Property ;
    rdfs:isDefinedBy <http://rdaregistry.info/Elements/u/> ;
    rdfs:label "is choreographic adaptation of"@en ;
    rdfs:subPropertyOf <http://rdaregistry.info/Elements/u/P60305> ;
    owl:inverseOf <http://rdaregistry.info/Elements/u/P60180> ;
    skos:definition "Relates a resource to a resource that has been adapted as a resource consisting of movement (e.g., dance)."@en .

<http://rdaregistry.info/Elements/u/P60294>
    reg:hasSubproperty <http://rdaregistry.info/Elements/e/P20184> ;
    reg:lexicalAlias <http://rdaregistry.info/Elements/u/expandedVersionOf.en> ;
    reg:name "expandedVersionOf"@en ;
    reg:status <http://metadataregistry.org/uri/RegStatus/1001> ;
    a rdf:Property ;
    rdfs:isDefinedBy <http://rdaregistry.info/Elements/u/> ;
    rdfs:label "is expanded version of"@en ;
    rdfs:subPropertyOf <http://rdaregistry.info/Elements/u/P60305> ;
    owl:inverseOf <http://rdaregistry.info/Elements/u/P60216> ;
    skos:definition "Relates a resource to a resource used as the basis for a derivative resource that enlarges upon the content of the source resource."@en .

<http://rdaregistry.info/Elements/u/P60295>
    reg:hasSubproperty <http://rdaregistry.info/Elements/e/P20185> ;
    reg:lexicalAlias <http://rdaregistry.info/Elements/u/remakeOf.en> ;
    reg:name "remakeOf"@en ;
    reg:status <http://metadataregistry.org/uri/RegStatus/1001> ;
    a rdf:Property ;
    rdfs:isDefinedBy <http://rdaregistry.info/Elements/u/> ;
    rdfs:label "is remake of"@en ;
    rdfs:subPropertyOf <http://rdaregistry.info/Elements/u/P60305> ;
    owl:inverseOf <http://rdaregistry.info/Elements/u/P60120> ;
    skos:definition "Relates a resource to a resource used as the basis for a new motion picture, radio program, television program, or video."@en .

<http://rdaregistry.info/Elements/u/P60296>
    reg:hasSubproperty <http://rdaregistry.info/Elements/e/P20186> ;
    reg:lexicalAlias <http://rdaregistry.info/Elements/u/paraphraseOf.en> ;
    reg:name "paraphraseOf"@en ;
    reg:status <http://metadataregistry.org/uri/RegStatus/1001> ;
    a rdf:Property ;
    rdfs:isDefinedBy <http://rdaregistry.info/Elements/u/> ;
    rdfs:label "is paraphrase of"@en ;
    rdfs:subPropertyOf <http://rdaregistry.info/Elements/u/P60305> ;
    owl:inverseOf <http://rdaregistry.info/Elements/u/P60273> ;
    skos:definition "Relates a resource to a resource used as the basis for a paraphrase, i.e., a restating of the content of the source resource in a different form."@en .

<http://rdaregistry.info/Elements/u/P60297>
    reg:hasSubproperty <http://rdaregistry.info/Elements/i/P40042>, <http://rdaregistry.info/Elements/m/P30043>, <http://rdaregistry.info/Elements/u/P60168>, <http://rdaregistry.info/Elements/u/P60287>, <http://rdaregistry.info/Elements/u/P60301>, <http://rdaregistry.info/Elements/u/P60469> ;
    reg:lexicalAlias <http://rdaregistry.info/Elements/u/reproductionOf.en> ;
    reg:name "reproductionOf"@en ;
    reg:status <http://metadataregistry.org/uri/RegStatus/1001> ;
    a rdf:Property ;
    rdfs:isDefinedBy <http://rdaregistry.info/Elements/u/> ;
    rdfs:label "is reproduction of"@en ;
    rdfs:subPropertyOf <http://rdaregistry.info/Elements/u/P60191> ;
    owl:inverseOf <http://rdaregistry.info/Elements/u/P60272> ;
    skos:definition "Relates a resource to a resource that is used as the basis for a reproduction."@en .

<http://rdaregistry.info/Elements/u/P60298>
    reg:hasSubproperty <http://rdaregistry.info/Elements/w/P10270>, <http://rdaregistry.info/Elements/w/P10276>, <http://rdaregistry.info/Elements/w/P10282> ;
    reg:lexicalAlias <http://rdaregistry.info/Elements/u/commentaryOn.en> ;
    reg:name "commentaryOn"@en ;
    reg:status <http://metadataregistry.org/uri/RegStatus/1001> ;
    a rdf:Property ;
    rdfs:isDefinedBy <http://rdaregistry.info/Elements/u/> ;
    rdfs:label "is commentary on"@en ;
    rdfs:subPropertyOf <http://rdaregistry.info/Elements/u/P60190> ;
    owl:inverseOf <http://rdaregistry.info/Elements/u/P60213> ;
    skos:definition "Relates a resource to a resource used as the basis for a set of explanatory or critical notes."@en .

<http://rdaregistry.info/Elements/u/P60299>
    reg:hasSubproperty <http://rdaregistry.info/Elements/i/P40044>, <http://rdaregistry.info/Elements/m/P30045> ;
    reg:lexicalAlias <http://rdaregistry.info/Elements/u/preservationFacsimileOf.en> ;
    reg:name "preservationFacsimileOf"@en ;
    reg:status <http://metadataregistry.org/uri/RegStatus/1001> ;
    a rdf:Property ;
    rdfs:isDefinedBy <http://rdaregistry.info/Elements/u/> ;
    rdfs:label "is preservation facsimile of"@en ;
    rdfs:subPropertyOf <http://rdaregistry.info/Elements/u/P60301> ;
    owl:inverseOf <http://rdaregistry.info/Elements/u/P60179> ;
    skos:definition "Relates a resource to a resource that is used as the basis for an exact reproduction on preservation-quality media, such as acid-free permanent or archival paper."@en .

<http://rdaregistry.info/Elements/u/P60300>
    reg:hasSubproperty <http://rdaregistry.info/Elements/m/P30046> ;
    reg:lexicalAlias <http://rdaregistry.info/Elements/u/facsimileContainerOf.en> ;
    reg:name "facsimileContainerOf"@en ;
    reg:status <http://metadataregistry.org/uri/RegStatus/1001> ;
    a rdf:Property ;
    rdfs:isDefinedBy <http://rdaregistry.info/Elements/u/> ;
    rdfs:label "is facsimile container of"@en ;
    rdfs:subPropertyOf <http://rdaregistry.info/Elements/u/P60249> ;
    owl:inverseOf <http://rdaregistry.info/Elements/u/P60100> ;
    skos:definition "Relates a resource to a resource used as the basis for an exact reproduction that is a discrete component of a larger entity."@en .

<http://rdaregistry.info/Elements/u/P60301>
    reg:hasSubproperty <http://rdaregistry.info/Elements/i/P40045>, <http://rdaregistry.info/Elements/m/P30047>, <http://rdaregistry.info/Elements/u/P60299> ;
    reg:lexicalAlias <http://rdaregistry.info/Elements/u/facsimileOf.en> ;
    reg:name "facsimileOf"@en ;
    reg:status <http://metadataregistry.org/uri/RegStatus/1001> ;
    a rdf:Property ;
    rdfs:isDefinedBy <http://rdaregistry.info/Elements/u/> ;
    rdfs:label "is facsimile of"@en ;
    rdfs:subPropertyOf <http://rdaregistry.info/Elements/u/P60297> ;
    owl:inverseOf <http://rdaregistry.info/Elements/u/P60217> ;
    skos:definition "Relates a resource to a resource that is used as the basis for an exact reproduction."@en .

<http://rdaregistry.info/Elements/u/P60302>
    reg:hasSubproperty <http://rdaregistry.info/Elements/e/P20188> ;
    reg:lexicalAlias <http://rdaregistry.info/Elements/u/indexTo.en> ;
    reg:name "indexTo"@en ;
    reg:status <http://metadataregistry.org/uri/RegStatus/1001> ;
    a rdf:Property ;
    rdfs:isDefinedBy <http://rdaregistry.info/Elements/u/> ;
    rdfs:label "is index to"@en ;
    rdfs:subPropertyOf <http://rdaregistry.info/Elements/u/P60307> ;
    owl:inverseOf <http://rdaregistry.info/Elements/u/P60263> ;
    skos:definition "Relates a resource to a resource used as the basis for an index, i.e., a systematic, alphabetical guide to the contents of the predominant resource, usually keyed to page numbers or other reference codes."@en .

<http://rdaregistry.info/Elements/u/P60303>
    reg:hasSubproperty <http://rdaregistry.info/Elements/e/P20189> ;
    reg:lexicalAlias <http://rdaregistry.info/Elements/u/revisionOf.en> ;
    reg:name "revisionOf"@en ;
    reg:status <http://metadataregistry.org/uri/RegStatus/1001> ;
    a rdf:Property ;
    rdfs:isDefinedBy <http://rdaregistry.info/Elements/u/> ;
    rdfs:label "is revision of"@en ;
    rdfs:subPropertyOf <http://rdaregistry.info/Elements/u/P60305> ;
    owl:inverseOf <http://rdaregistry.info/Elements/u/P60245> ;
    skos:definition "Relates a resource to a resource used as the basis for an updated, corrected, or expanded version."@en .

<http://rdaregistry.info/Elements/u/P60304>
    reg:hasSubproperty <http://rdaregistry.info/Elements/e/P20190> ;
    reg:lexicalAlias <http://rdaregistry.info/Elements/u/librettoBasedOn.en> ;
    reg:name "librettoBasedOn"@en ;
    reg:status <http://metadataregistry.org/uri/RegStatus/1001> ;
    a rdf:Property ;
    rdfs:isDefinedBy <http://rdaregistry.info/Elements/u/> ;
    rdfs:label "is libretto based on"@en ;
    rdfs:subPropertyOf <http://rdaregistry.info/Elements/u/P60305> ;
    owl:inverseOf <http://rdaregistry.info/Elements/u/P60210> ;
    skos:definition "Relates a resource to a resource that has been adapted as the text of an opera or other resource for the musical stage, or an oratorio."@en .

<http://rdaregistry.info/Elements/u/P60305>
    reg:hasSubproperty <http://rdaregistry.info/Elements/e/P20204>, <http://rdaregistry.info/Elements/u/P60114>, <http://rdaregistry.info/Elements/u/P60223>, <http://rdaregistry.info/Elements/u/P60224>, <http://rdaregistry.info/Elements/u/P60238>, <http://rdaregistry.info/Elements/u/P60241>, <http://rdaregistry.info/Elements/u/P60242>, <http://rdaregistry.info/Elements/u/P60243>, <http://rdaregistry.info/Elements/u/P60244>, <http://rdaregistry.info/Elements/u/P60266>, <http://rdaregistry.info/Elements/u/P60289>, <http://rdaregistry.info/Elements/u/P60293>, <http://rdaregistry.info/Elements/u/P60294>, <http://rdaregistry.info/Elements/u/P60295>, <http://rdaregistry.info/Elements/u/P60296>, <http://rdaregistry.info/Elements/u/P60303>, <http://rdaregistry.info/Elements/u/P60304>, <http://rdaregistry.info/Elements/u/P60308>, <http://rdaregistry.info/Elements/u/P60309>, <http://rdaregistry.info/Elements/u/P60311>, <http://rdaregistry.info/Elements/u/P60830>, <http://rdaregistry.info/Elements/u/P60832> ;
    reg:lexicalAlias <http://rdaregistry.info/Elements/u/basedOn.en> ;
    reg:name "basedOn"@en ;
    reg:status <http://metadataregistry.org/uri/RegStatus/1001> ;
    a rdf:Property ;
    rdfs:isDefinedBy <http://rdaregistry.info/Elements/u/> ;
    rdfs:label "is based on"@en ;
    rdfs:subPropertyOf <http://rdaregistry.info/Elements/u/P60710> ;
    owl:inverseOf <http://rdaregistry.info/Elements/u/P60250> ;
    skos:definition "Relates a resource to a resource used as the source for a derivative resource."@en .

<http://rdaregistry.info/Elements/u/P60306>
    reg:hasSubproperty <http://rdaregistry.info/Elements/e/P20191> ;
    reg:lexicalAlias <http://rdaregistry.info/Elements/u/continuedBy.en> ;
    reg:name "continuedBy"@en ;
    reg:status <http://metadataregistry.org/uri/RegStatus/1001> ;
    a rdf:Property ;
    rdfs:isDefinedBy <http://rdaregistry.info/Elements/u/> ;
    rdfs:label "is continued by"@en ;
    rdfs:subPropertyOf <http://rdaregistry.info/Elements/u/P60278> ;
    owl:inverseOf <http://rdaregistry.info/Elements/u/P60576> ;
    skos:definition "Relates a resource to a resource whose content continues an earlier resource under a new title."@en .

<http://rdaregistry.info/Elements/u/P60307>
    reg:hasSubproperty <http://rdaregistry.info/Elements/e/P20192>, <http://rdaregistry.info/Elements/u/P60116>, <http://rdaregistry.info/Elements/u/P60251>, <http://rdaregistry.info/Elements/u/P60252>, <http://rdaregistry.info/Elements/u/P60253>, <http://rdaregistry.info/Elements/u/P60254>, <http://rdaregistry.info/Elements/u/P60259>, <http://rdaregistry.info/Elements/u/P60286>, <http://rdaregistry.info/Elements/u/P60290>, <http://rdaregistry.info/Elements/u/P60291>, <http://rdaregistry.info/Elements/u/P60302>, <http://rdaregistry.info/Elements/u/P60474> ;
    reg:lexicalAlias <http://rdaregistry.info/Elements/u/augmentationOf.en> ;
    reg:name "augmentationOf"@en ;
    reg:status <http://metadataregistry.org/uri/RegStatus/1001> ;
    a rdf:Property ;
    rdfs:isDefinedBy <http://rdaregistry.info/Elements/u/> ;
    rdfs:label "is augmentation of"@en ;
    rdfs:subPropertyOf <http://rdaregistry.info/Elements/u/P60709> ;
    owl:inverseOf <http://rdaregistry.info/Elements/u/P60204> ;
    skos:definition "Relates a resource to a resource whose content is added to by another resource."@en .

<http://rdaregistry.info/Elements/u/P60308>
    reg:hasSubproperty <http://rdaregistry.info/Elements/e/P20193> ;
    reg:lexicalAlias <http://rdaregistry.info/Elements/u/abstractsFor.en> ;
    reg:name "abstractsFor"@en ;
    reg:status <http://metadataregistry.org/uri/RegStatus/1001> ;
    a rdf:Property ;
    rdfs:isDefinedBy <http://rdaregistry.info/Elements/u/> ;
    rdfs:label "is abstracts for"@en ;
    rdfs:subPropertyOf <http://rdaregistry.info/Elements/u/P60305> ;
    owl:inverseOf <http://rdaregistry.info/Elements/u/P60177> ;
    skos:definition "Relates a resource to a resource whose contents have been abstracted by an abstracting and indexing service."@en .

<http://rdaregistry.info/Elements/u/P60309>
    reg:hasSubproperty <http://rdaregistry.info/Elements/e/P20194> ;
    reg:lexicalAlias <http://rdaregistry.info/Elements/u/indexingFor.en> ;
    reg:name "indexingFor"@en ;
    reg:status <http://metadataregistry.org/uri/RegStatus/1001> ;
    a rdf:Property ;
    rdfs:isDefinedBy <http://rdaregistry.info/Elements/u/> ;
    rdfs:label "is indexing for"@en ;
    rdfs:subPropertyOf <http://rdaregistry.info/Elements/u/P60305> ;
    owl:inverseOf <http://rdaregistry.info/Elements/u/P60178> ;
    skos:definition "Relates a resource to a resource whose contents have been indexed by an abstracting and indexing service."@en .

<http://rdaregistry.info/Elements/u/P60310>
    reg:lexicalAlias <http://rdaregistry.info/Elements/u/prequelTo.en> ;
    reg:name "prequelTo"@en ;
    reg:status <http://metadataregistry.org/uri/RegStatus/1001> ;
    a rdf:Property ;
    rdfs:isDefinedBy <http://rdaregistry.info/Elements/u/> ;
    rdfs:label "is prequel to"@en ;
    rdfs:subPropertyOf <http://rdaregistry.info/Elements/u/P60278> ;
    owl:inverseOf <http://rdaregistry.info/Elements/u/P60220> ;
    skos:definition "Relates a resource to a resource whose narrative is extended backwards in time by the later resource."@en .

<http://rdaregistry.info/Elements/u/P60311>
    reg:hasSubproperty <http://rdaregistry.info/Elements/e/P20195>, <http://rdaregistry.info/Elements/u/P60312> ;
    reg:lexicalAlias <http://rdaregistry.info/Elements/u/imitationOf.en> ;
    reg:name "imitationOf"@en ;
    reg:status <http://metadataregistry.org/uri/RegStatus/1001> ;
    a rdf:Property ;
    rdfs:isDefinedBy <http://rdaregistry.info/Elements/u/> ;
    rdfs:label "is imitation of"@en ;
    rdfs:subPropertyOf <http://rdaregistry.info/Elements/u/P60305> ;
    owl:inverseOf <http://rdaregistry.info/Elements/u/P60214> ;
    skos:definition "Relates a resource to a resource whose style or content is copied in a derivative resource."@en .

<http://rdaregistry.info/Elements/u/P60312>
    reg:hasSubproperty <http://rdaregistry.info/Elements/e/P20196> ;
    reg:lexicalAlias <http://rdaregistry.info/Elements/u/parodyOf.en> ;
    reg:name "parodyOf"@en ;
    reg:status <http://metadataregistry.org/uri/RegStatus/1001> ;
    a rdf:Property ;
    rdfs:isDefinedBy <http://rdaregistry.info/Elements/u/> ;
    rdfs:label "is parody of"@en ;
    rdfs:subPropertyOf <http://rdaregistry.info/Elements/u/P60311> ;
    owl:inverseOf <http://rdaregistry.info/Elements/u/P60246> ;
    skos:definition "Relates a resource to a resource whose style or content is imitated for comic effect."@en .

<http://rdaregistry.info/Elements/u/P60313>
    reg:hasSubproperty <http://rdaregistry.info/Elements/e/P20205>, <http://rdaregistry.info/Elements/m/P30048>, <http://rdaregistry.info/Elements/m/P30140> ;
    reg:lexicalAlias <http://rdaregistry.info/Elements/u/relatedResource.en> ;
    reg:name "relatedResource"@en ;
    reg:status <http://metadataregistry.org/uri/RegStatus/1001> ;
    a rdf:Property ;
    rdfs:isDefinedBy <http://rdaregistry.info/Elements/u/> ;
    rdfs:label "has related resource"@en ;
    skos:definition "Relates a resource to a resource, represented by an identifier, an authorized access point, or a description, that is related to the resource being described."@en .

<http://rdaregistry.info/Elements/u/P60314>
    reg:hasSubproperty <http://rdaregistry.info/Elements/m/P30096> ;
    reg:lexicalAlias <http://rdaregistry.info/Elements/u/encodingFormat.en> ;
    reg:name "encodingFormat"@en ;
    reg:status <http://metadataregistry.org/uri/RegStatus/1001> ;
    a rdf:Property ;
    rdfs:isDefinedBy <http://rdaregistry.info/Elements/u/> ;
    rdfs:label "has encoding format"@en ;
    rdfs:subPropertyOf <http://rdaregistry.info/Elements/u/P60350> ;
    skos:definition "Relates a resource to a schema, standard, etc., used to encode the digital content of a resource."@en .

<http://rdaregistry.info/Elements/u/P60315>
    reg:lexicalAlias <http://rdaregistry.info/Elements/u/numericDesignationOfAMusicalResource.en> ;
    reg:name "numericDesignationOfAMusicalResource"@en ;
    reg:status <http://metadataregistry.org/uri/RegStatus/1001> ;
    a rdf:Property ;
    rdfs:isDefinedBy <http://rdaregistry.info/Elements/u/> ;
    rdfs:label "has numeric designation of a musical resource"@en ;
    skos:definition "Relates a resource to a serial number, opus number, or thematic index number assigned to a musical resource by a composer, publisher, or a musicologist."@en .

<http://rdaregistry.info/Elements/u/P60316>
    reg:lexicalAlias <http://rdaregistry.info/Elements/u/subseries.en> ;
    reg:name "subseries"@en ;
    reg:status <http://metadataregistry.org/uri/RegStatus/1001> ;
    a rdf:Property ;
    rdfs:isDefinedBy <http://rdaregistry.info/Elements/u/> ;
    rdfs:label "is subseries"@en ;
    rdfs:subPropertyOf <http://rdaregistry.info/Elements/u/P60249> ;
    owl:inverseOf <http://rdaregistry.info/Elements/u/P60192> ;
    skos:definition "Relates a resource to a serial or multipart resource that consistently appears in a larger resource; the title of the larger resource appears on all issues or parts of the subseries"@en .

<http://rdaregistry.info/Elements/u/P60317>
    reg:hasSubproperty <http://rdaregistry.info/Elements/m/P30101> ;
    reg:lexicalAlias <http://rdaregistry.info/Elements/u/specialIssueOf.en> ;
    reg:name "specialIssueOf"@en ;
    reg:status <http://metadataregistry.org/uri/RegStatus/1001> ;
    a rdf:Property ;
    rdfs:isDefinedBy <http://rdaregistry.info/Elements/u/> ;
    rdfs:label "is special issue of"@en ;
    rdfs:subPropertyOf <http://rdaregistry.info/Elements/u/P60101> ;
    owl:inverseOf <http://rdaregistry.info/Elements/u/P60207> ;
    skos:definition "Relates a resource to a serial or newspaper containing a single issue or a supplementary section devoted to a special subject, with or without serial numbering, such as an anniversary number of a periodical or newspaper."@en .

<http://rdaregistry.info/Elements/u/P60318>
    reg:hasSubproperty <http://rdaregistry.info/Elements/e/P20061> ;
    reg:lexicalAlias <http://rdaregistry.info/Elements/u/formOfTactileNotation.en> ;
    reg:name "formOfTactileNotation"@en ;
    reg:status <http://metadataregistry.org/uri/RegStatus/1001> ;
    a rdf:Property ;
    rdfs:isDefinedBy <http://rdaregistry.info/Elements/u/> ;
    rdfs:label "has form of tactile notation"@en ;
    rdfs:subPropertyOf <http://rdaregistry.info/Elements/u/P60319> ;
    skos:definition "Relates a resource to a set of characters and/or symbols used to express the content of a resource in a form that can be perceived through touch."@en .

<http://rdaregistry.info/Elements/u/P60319>
    reg:hasSubproperty <http://rdaregistry.info/Elements/e/P20062>, <http://rdaregistry.info/Elements/u/P60318>, <http://rdaregistry.info/Elements/u/P60320>, <http://rdaregistry.info/Elements/u/P60321>, <http://rdaregistry.info/Elements/u/P60322> ;
    reg:lexicalAlias <http://rdaregistry.info/Elements/u/formOfNotation.en> ;
    reg:name "formOfNotation"@en ;
    reg:status <http://metadataregistry.org/uri/RegStatus/1001> ;
    a rdf:Property ;
    rdfs:isDefinedBy <http://rdaregistry.info/Elements/u/> ;
    rdfs:label "has form of notation"@en ;
    skos:definition "Relates a resource to a set of characters and/or symbols used to express the content of a resource."@en .

<http://rdaregistry.info/Elements/u/P60320>
    reg:hasSubproperty <http://rdaregistry.info/Elements/e/P20063> ;
    reg:lexicalAlias <http://rdaregistry.info/Elements/u/formOfNotatedMovement.en> ;
    reg:name "formOfNotatedMovement"@en ;
    reg:status <http://metadataregistry.org/uri/RegStatus/1001> ;
    a rdf:Property ;
    rdfs:isDefinedBy <http://rdaregistry.info/Elements/u/> ;
    rdfs:label "has form of notated movement"@en ;
    rdfs:subPropertyOf <http://rdaregistry.info/Elements/u/P60319> ;
    skos:definition "Relates a resource to a set of characters and/or symbols used to express the movement content of a resource."@en .

<http://rdaregistry.info/Elements/u/P60321>
    reg:hasSubproperty <http://rdaregistry.info/Elements/e/P20064> ;
    reg:lexicalAlias <http://rdaregistry.info/Elements/u/formOfMusicalNotation.en> ;
    reg:name "formOfMusicalNotation"@en ;
    reg:status <http://metadataregistry.org/uri/RegStatus/1001> ;
    a rdf:Property ;
    rdfs:isDefinedBy <http://rdaregistry.info/Elements/u/> ;
    rdfs:label "has form of musical notation"@en ;
    rdfs:subPropertyOf <http://rdaregistry.info/Elements/u/P60319> ;
    skos:definition "Relates a resource to a set of characters and/or symbols used to express the musical content of a resource."@en .

<http://rdaregistry.info/Elements/u/P60322>
    reg:hasSubproperty <http://rdaregistry.info/Elements/e/P20065> ;
    reg:lexicalAlias <http://rdaregistry.info/Elements/u/script.en> ;
    reg:name "script"@en ;
    reg:status <http://metadataregistry.org/uri/RegStatus/1001> ;
    a rdf:Property ;
    rdfs:isDefinedBy <http://rdaregistry.info/Elements/u/> ;
    rdfs:label "has script"@en ;
    rdfs:subPropertyOf <http://rdaregistry.info/Elements/u/P60319> ;
    skos:definition "Relates a resource to a set of characters and/or symbols used to express the written language content of a resource."@en .

<http://rdaregistry.info/Elements/u/P60323>
    reg:hasSubproperty <http://rdaregistry.info/Elements/m/P30102> ;
    reg:lexicalAlias <http://rdaregistry.info/Elements/u/digitalRepresentationOfCartographicContent.en> ;
    reg:name "digitalRepresentationOfCartographicContent"@en ;
    reg:status <http://metadataregistry.org/uri/RegStatus/1001> ;
    a rdf:Property ;
    rdfs:isDefinedBy <http://rdaregistry.info/Elements/u/> ;
    rdfs:label "has digital representation of cartographic content"@en ;
    rdfs:subPropertyOf <http://rdaregistry.info/Elements/u/P60350> ;
    skos:definition "Relates a resource to a set of technical details relating to the encoding of geospatial information in a cartographic resource."@en .

<http://rdaregistry.info/Elements/u/P60324>
    reg:hasSubproperty <http://rdaregistry.info/Elements/a/P50040>, <http://rdaregistry.info/Elements/a/P50058>, <http://rdaregistry.info/Elements/a/P50107>, <http://rdaregistry.info/Elements/u/P60076>, <http://rdaregistry.info/Elements/u/P60524>, <http://rdaregistry.info/Elements/u/P60525>, <http://rdaregistry.info/Elements/u/P60526>, <http://rdaregistry.info/Elements/u/P60598>, <http://rdaregistry.info/Elements/u/P60599> ;
    reg:lexicalAlias <http://rdaregistry.info/Elements/u/dateAssociatedWithTheAgent.en> ;
    reg:name "dateAssociatedWithTheAgent"@en ;
    reg:status <http://metadataregistry.org/uri/RegStatus/1001> ;
    a rdf:Property ;
    rdfs:isDefinedBy <http://rdaregistry.info/Elements/u/> ;
    rdfs:label "has date associated with the agent"@en ;
    skos:definition "Relates a resource to a significant date associated with an agent (e.g., date of birth, date of death), or the date or range of dates on which a conference, etc., was held, or a date with which an agent is otherwise associated (e.g., date of founding)."@en .

<http://rdaregistry.info/Elements/u/P60325>
    reg:hasSubproperty <http://rdaregistry.info/Elements/a/P50031>, <http://rdaregistry.info/Elements/a/P50057>, <http://rdaregistry.info/Elements/a/P50260>, <http://rdaregistry.info/Elements/u/P60064>, <http://rdaregistry.info/Elements/u/P60107> ;
    reg:lexicalAlias <http://rdaregistry.info/Elements/u/placeAssociatedWithTheAgent.en> ;
    reg:name "placeAssociatedWithTheAgent"@en ;
    reg:status <http://metadataregistry.org/uri/RegStatus/1001> ;
    a rdf:Property ;
    rdfs:isDefinedBy <http://rdaregistry.info/Elements/u/> ;
    rdfs:label "has place associated with the agent"@en ;
    skos:definition "Relates a resource to a significant location associated with an agent, or a place where an agent resides or has resided or has some connection."@en .

<http://rdaregistry.info/Elements/u/P60326>
    reg:hasSubproperty <http://rdaregistry.info/Elements/m/P30104> ;
    reg:lexicalAlias <http://rdaregistry.info/Elements/u/videoFormat.en> ;
    reg:name "videoFormat"@en ;
    reg:status <http://metadataregistry.org/uri/RegStatus/1001> ;
    a rdf:Property ;
    rdfs:isDefinedBy <http://rdaregistry.info/Elements/u/> ;
    rdfs:label "has video format"@en ;
    rdfs:subPropertyOf <http://rdaregistry.info/Elements/u/P60352> ;
    skos:definition "Relates a resource to a standard, etc., used to encode the analog video content of a resource."@en .

<http://rdaregistry.info/Elements/u/P60327>
    reg:hasSubproperty <http://rdaregistry.info/Elements/m/P30105> ;
    reg:lexicalAlias <http://rdaregistry.info/Elements/u/statementOfResponsibilityRelatingToTitleProper.en> ;
    reg:name "statementOfResponsibilityRelatingToTitleProper"@en ;
    reg:status <http://metadataregistry.org/uri/RegStatus/1001> ;
    a rdf:Property ;
    rdfs:isDefinedBy <http://rdaregistry.info/Elements/u/> ;
    rdfs:label "has statement of responsibility relating to title proper"@en ;
    rdfs:subPropertyOf <http://rdaregistry.info/Elements/u/P60339> ;
    skos:definition "Relates a resource to a statement associated with the title proper of a resource that relates to the identification and/or function of any agents responsible for the creation of, or contributing to the realization of, the intellectual or artistic content of the resource."@en .

<http://rdaregistry.info/Elements/u/P60328>
    reg:hasSubproperty <http://rdaregistry.info/Elements/m/P30106> ;
    reg:lexicalAlias <http://rdaregistry.info/Elements/u/seriesStatement.en> ;
    reg:name "seriesStatement"@en ;
    reg:status <http://metadataregistry.org/uri/RegStatus/1001> ;
    a rdf:Property ;
    rdfs:isDefinedBy <http://rdaregistry.info/Elements/u/> ;
    rdfs:label "has series statement"@en ;
    skos:definition "Relates a resource to a statement identifying a series to which a resource belongs and the numbering of the resource within the series."@en .

<http://rdaregistry.info/Elements/u/P60329>
    reg:hasSubproperty <http://rdaregistry.info/Elements/m/P30107> ;
    reg:lexicalAlias <http://rdaregistry.info/Elements/u/editionStatement.en> ;
    reg:name "editionStatement"@en ;
    reg:status <http://metadataregistry.org/uri/RegStatus/1001> ;
    a rdf:Property ;
    rdfs:isDefinedBy <http://rdaregistry.info/Elements/u/> ;
    rdfs:label "has edition statement"@en ;
    skos:definition "Relates a resource to a statement identifying the edition to which a resource belongs."@en .

<http://rdaregistry.info/Elements/u/P60330>
    reg:hasSubproperty <http://rdaregistry.info/Elements/m/P30108> ;
    reg:lexicalAlias <http://rdaregistry.info/Elements/u/distributionStatement.en> ;
    reg:name "distributionStatement"@en ;
    reg:status <http://metadataregistry.org/uri/RegStatus/1001> ;
    a rdf:Property ;
    rdfs:isDefinedBy <http://rdaregistry.info/Elements/u/> ;
    rdfs:label "has distribution statement"@en ;
    skos:definition "Relates a resource to a statement identifying the place or places of distribution, distributor or distributors, and date or dates of distribution of a resource in a published form."@en .

<http://rdaregistry.info/Elements/u/P60331>
    reg:hasSubproperty <http://rdaregistry.info/Elements/m/P30109> ;
    reg:lexicalAlias <http://rdaregistry.info/Elements/u/manufactureStatement.en> ;
    reg:name "manufactureStatement"@en ;
    reg:status <http://metadataregistry.org/uri/RegStatus/1001> ;
    a rdf:Property ;
    rdfs:isDefinedBy <http://rdaregistry.info/Elements/u/> ;
    rdfs:label "has manufacture statement"@en ;
    skos:definition "Relates a resource to a statement identifying the place or places of manufacture, manufacturer or manufacturers, and date or dates of manufacture of a resource in a published form."@en .

<http://rdaregistry.info/Elements/u/P60332>
    reg:hasSubproperty <http://rdaregistry.info/Elements/m/P30110> ;
    reg:lexicalAlias <http://rdaregistry.info/Elements/u/productionStatement.en> ;
    reg:name "productionStatement"@en ;
    reg:status <http://metadataregistry.org/uri/RegStatus/1001> ;
    a rdf:Property ;
    rdfs:isDefinedBy <http://rdaregistry.info/Elements/u/> ;
    rdfs:label "has production statement"@en ;
    skos:definition "Relates a resource to a statement identifying the place or places of production, producer or producers, and date or dates of production of a resource in an unpublished form."@en .

<http://rdaregistry.info/Elements/u/P60333>
    reg:hasSubproperty <http://rdaregistry.info/Elements/m/P30111> ;
    reg:lexicalAlias <http://rdaregistry.info/Elements/u/publicationStatement.en> ;
    reg:name "publicationStatement"@en ;
    reg:status <http://metadataregistry.org/uri/RegStatus/1001> ;
    a rdf:Property ;
    rdfs:isDefinedBy <http://rdaregistry.info/Elements/u/> ;
    rdfs:label "has publication statement"@en ;
    skos:definition "Relates a resource to a statement identifying the place or places of publication, publisher or publishers, and date or dates of publication of a resource."@en .

<http://rdaregistry.info/Elements/u/P60334>
    reg:hasSubproperty <http://rdaregistry.info/Elements/m/P30112> ;
    reg:lexicalAlias <http://rdaregistry.info/Elements/u/parallelStatementOfResponsibilityRelatingToANamedRevisionOfAnEdition.en> ;
    reg:name "parallelStatementOfResponsibilityRelatingToANamedRevisionOfAnEdition"@en ;
    reg:status <http://metadataregistry.org/uri/RegStatus/1001> ;
    a rdf:Property ;
    rdfs:isDefinedBy <http://rdaregistry.info/Elements/u/> ;
    rdfs:label "has parallel statement of responsibility relating to a named revision of an edition"@en ;
    skos:definition "Relates a resource to a statement of responsibility relating to a named revision of an edition in a language and/or script that differs from that recorded in the statement of responsibility relating to a named revision of an edition element."@en .

<http://rdaregistry.info/Elements/u/P60335>
    reg:hasSubproperty <http://rdaregistry.info/Elements/m/P30113> ;
    reg:lexicalAlias <http://rdaregistry.info/Elements/u/parallelStatementOfResponsibilityRelatingToSeries.en> ;
    reg:name "parallelStatementOfResponsibilityRelatingToSeries"@en ;
    reg:status <http://metadataregistry.org/uri/RegStatus/1001> ;
    a rdf:Property ;
    rdfs:isDefinedBy <http://rdaregistry.info/Elements/u/> ;
    rdfs:label "has parallel statement of responsibility relating to series"@en ;
    skos:definition "Relates a resource to a statement of responsibility relating to series in a language and/or script that differs from that recorded in the statement of responsibility relating to series element."@en .

<http://rdaregistry.info/Elements/u/P60336>
    reg:hasSubproperty <http://rdaregistry.info/Elements/m/P30114> ;
    reg:lexicalAlias <http://rdaregistry.info/Elements/u/parallelStatementOfResponsibilityRelatingToSubseries.en> ;
    reg:name "parallelStatementOfResponsibilityRelatingToSubseries"@en ;
    reg:status <http://metadataregistry.org/uri/RegStatus/1001> ;
    a rdf:Property ;
    rdfs:isDefinedBy <http://rdaregistry.info/Elements/u/> ;
    rdfs:label "has parallel statement of responsibility relating to subseries"@en ;
    skos:definition "Relates a resource to a statement of responsibility relating to subseries in a language and/or script that differs from that recorded in the statement of responsibility relating to subseries element."@en .

<http://rdaregistry.info/Elements/u/P60337>
    reg:hasSubproperty <http://rdaregistry.info/Elements/m/P30115> ;
    reg:lexicalAlias <http://rdaregistry.info/Elements/u/parallelStatementOfResponsibilityRelatingToTheEdition.en> ;
    reg:name "parallelStatementOfResponsibilityRelatingToTheEdition"@en ;
    reg:status <http://metadataregistry.org/uri/RegStatus/1001> ;
    a rdf:Property ;
    rdfs:isDefinedBy <http://rdaregistry.info/Elements/u/> ;
    rdfs:label "has parallel statement of responsibility relating to the edition"@en ;
    skos:definition "Relates a resource to a statement of responsibility relating to the edition in a language and/or script that differs from that recorded in the statement of responsibility relating to the edition element."@en .

<http://rdaregistry.info/Elements/u/P60338>
    reg:hasSubproperty <http://rdaregistry.info/Elements/m/P30116> ;
    reg:lexicalAlias <http://rdaregistry.info/Elements/u/parallelStatementOfResponsibilityRelatingToTitleProper.en> ;
    reg:name "parallelStatementOfResponsibilityRelatingToTitleProper"@en ;
    reg:status <http://metadataregistry.org/uri/RegStatus/1001> ;
    a rdf:Property ;
    rdfs:isDefinedBy <http://rdaregistry.info/Elements/u/> ;
    rdfs:label "has parallel statement of responsibility relating to title proper"@en ;
    rdfs:subPropertyOf <http://rdaregistry.info/Elements/u/P60339> ;
    skos:definition "Relates a resource to a statement of responsibility relating to title proper in a language and/or script that differs from that recorded in the statement of responsibility relating to title proper element."@en .

<http://rdaregistry.info/Elements/u/P60339>
    reg:hasSubproperty <http://rdaregistry.info/Elements/m/P30117>, <http://rdaregistry.info/Elements/u/P60327>, <http://rdaregistry.info/Elements/u/P60338> ;
    reg:lexicalAlias <http://rdaregistry.info/Elements/u/statementOfResponsibility.en> ;
    reg:name "statementOfResponsibility"@en ;
    reg:status <http://metadataregistry.org/uri/RegStatus/1001> ;
    a rdf:Property ;
    rdfs:isDefinedBy <http://rdaregistry.info/Elements/u/> ;
    rdfs:label "has statement of responsibility"@en ;
    skos:definition "Relates a resource to a statement relating to the identification and/or function of any agents responsible for the creation of, or contributing to the realization of, the intellectual or artistic content of a resource."@en .

<http://rdaregistry.info/Elements/u/P60340>
    reg:hasSubproperty <http://rdaregistry.info/Elements/m/P30118> ;
    reg:lexicalAlias <http://rdaregistry.info/Elements/u/statementOfResponsibilityRelatingToANamedRevisionOfAnEdition.en> ;
    reg:name "statementOfResponsibilityRelatingToANamedRevisionOfAnEdition"@en ;
    reg:status <http://metadataregistry.org/uri/RegStatus/1001> ;
    a rdf:Property ;
    rdfs:isDefinedBy <http://rdaregistry.info/Elements/u/> ;
    rdfs:label "has statement of responsibility relating to a named revision of an edition"@en ;
    skos:definition "Relates a resource to a statement relating to the identification of any agents responsible for a named revision of an edition."@en .

<http://rdaregistry.info/Elements/u/P60341>
    reg:hasSubproperty <http://rdaregistry.info/Elements/m/P30119> ;
    reg:lexicalAlias <http://rdaregistry.info/Elements/u/statementOfResponsibilityRelatingToSeries.en> ;
    reg:name "statementOfResponsibilityRelatingToSeries"@en ;
    reg:status <http://metadataregistry.org/uri/RegStatus/1001> ;
    a rdf:Property ;
    rdfs:isDefinedBy <http://rdaregistry.info/Elements/u/> ;
    rdfs:label "has statement of responsibility relating to series"@en ;
    skos:definition "Relates a resource to a statement relating to the identification of any agents responsible for a series."@en .

<http://rdaregistry.info/Elements/u/P60342>
    reg:hasSubproperty <http://rdaregistry.info/Elements/m/P30120> ;
    reg:lexicalAlias <http://rdaregistry.info/Elements/u/statementOfResponsibilityRelatingToSubseries.en> ;
    reg:name "statementOfResponsibilityRelatingToSubseries"@en ;
    reg:status <http://metadataregistry.org/uri/RegStatus/1001> ;
    a rdf:Property ;
    rdfs:isDefinedBy <http://rdaregistry.info/Elements/u/> ;
    rdfs:label "has statement of responsibility relating to subseries"@en ;
    skos:definition "Relates a resource to a statement relating to the identification of any agents responsible for a subseries."@en .

<http://rdaregistry.info/Elements/u/P60343>
    reg:hasSubproperty <http://rdaregistry.info/Elements/m/P30121> ;
    reg:lexicalAlias <http://rdaregistry.info/Elements/u/statementOfResponsibilityRelatingToTheEdition.en> ;
    reg:name "statementOfResponsibilityRelatingToTheEdition"@en ;
    reg:status <http://metadataregistry.org/uri/RegStatus/1001> ;
    a rdf:Property ;
    rdfs:isDefinedBy <http://rdaregistry.info/Elements/u/> ;
    rdfs:label "has statement of responsibility relating to the edition"@en ;
    skos:definition "Relates a resource to a statement relating to the identification of any agents responsible for the edition being described but not to all editions."@en .

<http://rdaregistry.info/Elements/u/P60344>
    reg:hasSubproperty <http://rdaregistry.info/Elements/m/P30122> ;
    reg:lexicalAlias <http://rdaregistry.info/Elements/u/emulsionOnMicrofilmAndMicrofiche.en> ;
    reg:name "emulsionOnMicrofilmAndMicrofiche"@en ;
    reg:status <http://metadataregistry.org/uri/RegStatus/1001> ;
    a rdf:Property ;
    rdfs:isDefinedBy <http://rdaregistry.info/Elements/u/> ;
    rdfs:label "has emulsion on microfilm and microfiche"@en ;
    rdfs:subPropertyOf <http://rdaregistry.info/Elements/u/P60159> ;
    skos:definition "Relates a resource to a suspension of light-sensitive chemicals used as a coating on a microfilm or microfiche (e.g., silver halide)."@en .

<http://rdaregistry.info/Elements/u/P60345>
    reg:lexicalAlias <http://rdaregistry.info/Elements/u/longitudeAndLatitude.en> ;
    reg:name "longitudeAndLatitude"@en ;
    reg:status <http://metadataregistry.org/uri/RegStatus/1001> ;
    a rdf:Property ;
    rdfs:isDefinedBy <http://rdaregistry.info/Elements/u/> ;
    rdfs:label "has longitude and latitude"@en ;
    rdfs:subPropertyOf <http://rdaregistry.info/Elements/u/P60109> ;
    skos:definition "Relates a resource to a system for identifying the area covered by the cartographic content of a resource using longitude of the westernmost and easternmost boundaries and latitude of the northernmost and southernmost boundaries."@en .

<http://rdaregistry.info/Elements/u/P60346>
    reg:lexicalAlias <http://rdaregistry.info/Elements/u/rightAscensionAndDeclination.en> ;
    reg:name "rightAscensionAndDeclination"@en ;
    reg:status <http://metadataregistry.org/uri/RegStatus/1001> ;
    a rdf:Property ;
    rdfs:isDefinedBy <http://rdaregistry.info/Elements/u/> ;
    rdfs:label "has right ascension and declination"@en ;
    rdfs:subPropertyOf <http://rdaregistry.info/Elements/u/P60109> ;
    skos:definition "Relates a resource to a system for identifying the location of a celestial object in the sky covered by the cartographic content of a resource using the angles of right ascension and declination."@en .

<http://rdaregistry.info/Elements/u/P60347>
    reg:lexicalAlias <http://rdaregistry.info/Elements/u/stringsOfCoordinatePairs.en> ;
    reg:name "stringsOfCoordinatePairs"@en ;
    reg:status <http://metadataregistry.org/uri/RegStatus/1001> ;
    a rdf:Property ;
    rdfs:isDefinedBy <http://rdaregistry.info/Elements/u/> ;
    rdfs:label "has strings of coordinate pairs"@en ;
    rdfs:subPropertyOf <http://rdaregistry.info/Elements/u/P60109> ;
    skos:definition "Relates a resource to a system for identifying the precise area covered by the cartographic content of a resource using coordinates for each vertex of a polygon."@en .

<http://rdaregistry.info/Elements/u/P60348>
    reg:lexicalAlias <http://rdaregistry.info/Elements/u/systemOfOrganization.en> ;
    reg:name "systemOfOrganization"@en ;
    reg:status <http://metadataregistry.org/uri/RegStatus/1001> ;
    a rdf:Property ;
    rdfs:isDefinedBy <http://rdaregistry.info/Elements/u/> ;
    rdfs:label "has system of organization"@en ;
    skos:definition "Relates a resource to a system of arranging materials in an archival resource or a collection."@en .

<http://rdaregistry.info/Elements/u/P60349>
    reg:hasSubproperty <http://rdaregistry.info/Elements/m/P30123> ;
    reg:lexicalAlias <http://rdaregistry.info/Elements/u/broadcastStandard.en> ;
    reg:name "broadcastStandard"@en ;
    reg:status <http://metadataregistry.org/uri/RegStatus/1001> ;
    a rdf:Property ;
    rdfs:isDefinedBy <http://rdaregistry.info/Elements/u/> ;
    rdfs:label "has broadcast standard"@en ;
    rdfs:subPropertyOf <http://rdaregistry.info/Elements/u/P60352> ;
    skos:definition "Relates a resource to a system used to format a video resource for television broadcast."@en .

<http://rdaregistry.info/Elements/u/P60350>
    reg:hasSubproperty <http://rdaregistry.info/Elements/m/P30124>, <http://rdaregistry.info/Elements/u/P60059>, <http://rdaregistry.info/Elements/u/P60093>, <http://rdaregistry.info/Elements/u/P60314>, <http://rdaregistry.info/Elements/u/P60323>, <http://rdaregistry.info/Elements/u/P60519>, <http://rdaregistry.info/Elements/u/P60551>, <http://rdaregistry.info/Elements/u/P60587> ;
    reg:lexicalAlias <http://rdaregistry.info/Elements/u/digitalFileCharacteristic.en> ;
    reg:name "digitalFileCharacteristic"@en ;
    reg:status <http://metadataregistry.org/uri/RegStatus/1001> ;
    a rdf:Property ;
    rdfs:isDefinedBy <http://rdaregistry.info/Elements/u/> ;
    rdfs:label "has digital file characteristic"@en ;
    skos:definition "Relates a resource to a technical specification relating to the digital encoding of text, image, audio, video, and other types of data in a resource."@en .

<http://rdaregistry.info/Elements/u/P60351>
    reg:hasSubproperty <http://rdaregistry.info/Elements/m/P30125>, <http://rdaregistry.info/Elements/u/P60481>, <http://rdaregistry.info/Elements/u/P60522>, <http://rdaregistry.info/Elements/u/P60532>, <http://rdaregistry.info/Elements/u/P60543>, <http://rdaregistry.info/Elements/u/P60552>, <http://rdaregistry.info/Elements/u/P60553>, <http://rdaregistry.info/Elements/u/P60586>, <http://rdaregistry.info/Elements/u/P60594> ;
    reg:lexicalAlias <http://rdaregistry.info/Elements/u/soundCharacteristic.en> ;
    reg:name "soundCharacteristic"@en ;
    reg:status <http://metadataregistry.org/uri/RegStatus/1001> ;
    a rdf:Property ;
    rdfs:isDefinedBy <http://rdaregistry.info/Elements/u/> ;
    rdfs:label "has sound characteristic"@en ;
    skos:definition "Relates a resource to a technical specification relating to the encoding of sound in a resource."@en .

<http://rdaregistry.info/Elements/u/P60352>
    reg:hasSubproperty <http://rdaregistry.info/Elements/m/P30126>, <http://rdaregistry.info/Elements/u/P60326>, <http://rdaregistry.info/Elements/u/P60349> ;
    reg:lexicalAlias <http://rdaregistry.info/Elements/u/videoCharacteristic.en> ;
    reg:name "videoCharacteristic"@en ;
    reg:status <http://metadataregistry.org/uri/RegStatus/1001> ;
    a rdf:Property ;
    rdfs:isDefinedBy <http://rdaregistry.info/Elements/u/> ;
    rdfs:label "has video characteristic"@en ;
    skos:definition "Relates a resource to a technical specification relating to the encoding of video images in a resource."@en .

<http://rdaregistry.info/Elements/u/P60353>
    reg:hasSubproperty <http://rdaregistry.info/Elements/m/P30127>, <http://rdaregistry.info/Elements/u/P60529>, <http://rdaregistry.info/Elements/u/P60585> ;
    reg:lexicalAlias <http://rdaregistry.info/Elements/u/projectionCharacteristicOfMotionPictureFilm.en> ;
    reg:name "projectionCharacteristicOfMotionPictureFilm"@en ;
    reg:status <http://metadataregistry.org/uri/RegStatus/1001> ;
    a rdf:Property ;
    rdfs:isDefinedBy <http://rdaregistry.info/Elements/u/> ;
    rdfs:label "has projection characteristic of motion picture film"@en ;
    skos:definition "Relates a resource to a technical specification relating to the projection of a motion picture film."@en .

<http://rdaregistry.info/Elements/u/P60354>
    reg:hasSubproperty <http://rdaregistry.info/Elements/e/P20066> ;
    reg:lexicalAlias <http://rdaregistry.info/Elements/u/adaptedAsATelevisionProgram.en> ;
    reg:name "adaptedAsATelevisionProgram"@en ;
    reg:status <http://metadataregistry.org/uri/RegStatus/1001> ;
    a rdf:Property ;
    rdfs:isDefinedBy <http://rdaregistry.info/Elements/u/> ;
    rdfs:label "is adapted as television program"@en ;
    rdfs:subPropertyOf <http://rdaregistry.info/Elements/u/P60260> ;
    owl:inverseOf <http://rdaregistry.info/Elements/u/P60230> ;
    skos:definition "Relates a resource to a television program based on the source resource."@en .

<http://rdaregistry.info/Elements/u/P60355>
    reg:hasSubproperty <http://rdaregistry.info/Elements/m/P30128> ;
    reg:lexicalAlias <http://rdaregistry.info/Elements/u/variantTitle.en> ;
    reg:name "variantTitle"@en ;
    reg:status <http://metadataregistry.org/uri/RegStatus/1001> ;
    a rdf:Property ;
    rdfs:isDefinedBy <http://rdaregistry.info/Elements/u/> ;
    rdfs:label "has variant title"@en ;
    rdfs:subPropertyOf <http://rdaregistry.info/Elements/u/P60369> ;
    skos:definition "Relates a resource to a title associated with a resource that differs from a title recorded as the preferred title, title proper, a parallel title proper, other title information, parallel other title information, earlier title proper, later title proper, key title, or abbreviated title."@en .

<http://rdaregistry.info/Elements/u/P60356>
    reg:hasSubproperty <http://rdaregistry.info/Elements/a/P50059> ;
    reg:lexicalAlias <http://rdaregistry.info/Elements/u/hereditaryTitle.en> ;
    reg:name "hereditaryTitle"@en ;
    reg:status <http://metadataregistry.org/uri/RegStatus/1001> ;
    a rdf:Property ;
    rdfs:isDefinedBy <http://rdaregistry.info/Elements/u/> ;
    rdfs:label "has hereditary title"@en ;
    skos:definition "Relates a resource to a title of nobility, etc., associated with an agent."@en .

<http://rdaregistry.info/Elements/u/P60357>
    reg:hasSubproperty <http://rdaregistry.info/Elements/m/P30129> ;
    reg:lexicalAlias <http://rdaregistry.info/Elements/u/laterTitleProper.en> ;
    reg:name "laterTitleProper"@en ;
    reg:status <http://metadataregistry.org/uri/RegStatus/1001> ;
    a rdf:Property ;
    rdfs:isDefinedBy <http://rdaregistry.info/Elements/u/> ;
    rdfs:label "has later title proper"@en ;
    rdfs:subPropertyOf <http://rdaregistry.info/Elements/u/P60369> ;
    skos:definition "Relates a resource to a title proper appearing on a later issue or part of a multipart monograph or serial that differs from that on the first or earliest issue or part."@en .

<http://rdaregistry.info/Elements/u/P60358>
    reg:hasSubproperty <http://rdaregistry.info/Elements/m/P30130> ;
    reg:lexicalAlias <http://rdaregistry.info/Elements/u/earlierTitleProper.en> ;
    reg:name "earlierTitleProper"@en ;
    reg:status <http://metadataregistry.org/uri/RegStatus/1001> ;
    a rdf:Property ;
    rdfs:isDefinedBy <http://rdaregistry.info/Elements/u/> ;
    rdfs:label "has earlier title proper"@en ;
    rdfs:subPropertyOf <http://rdaregistry.info/Elements/u/P60369> ;
    skos:definition "Relates a resource to a title proper appearing on an earlier iteration of an integrating resource that differs from that on the current iteration."@en .

<http://rdaregistry.info/Elements/u/P60359>
    reg:hasSubproperty <http://rdaregistry.info/Elements/m/P30131> ;
    reg:lexicalAlias <http://rdaregistry.info/Elements/u/abbreviatedTitle.en> ;
    reg:name "abbreviatedTitle"@en ;
    reg:status <http://metadataregistry.org/uri/RegStatus/1001> ;
    a rdf:Property ;
    rdfs:isDefinedBy <http://rdaregistry.info/Elements/u/> ;
    rdfs:label "has abbreviated title"@en ;
    rdfs:subPropertyOf <http://rdaregistry.info/Elements/u/P60369> ;
    skos:definition "Relates a resource to a title that has been abbreviated for purposes of indexing or identification."@en .

<http://rdaregistry.info/Elements/u/P60360>
    reg:hasSubproperty <http://rdaregistry.info/Elements/a/P50109> ;
    reg:lexicalAlias <http://rdaregistry.info/Elements/u/placeOfResidenceEtc.en> ;
    reg:name "placeOfResidenceEtc"@en ;
    reg:status <http://metadataregistry.org/uri/RegStatus/1001> ;
    a rdf:Property ;
    rdfs:isDefinedBy <http://rdaregistry.info/Elements/u/> ;
    rdfs:label "has place of residence, etc."@en ;
    skos:definition "Relates a resource to a town, city, province, state, and/or country in which an agent resides or has resided, or another significant place associated with the agent other than place of birth, place of death, or residence (e.g., a place where an agent has worked or studied)."@en .

<http://rdaregistry.info/Elements/u/P60361>
    reg:hasSubproperty <http://rdaregistry.info/Elements/e/P20067> ;
    reg:lexicalAlias <http://rdaregistry.info/Elements/u/adaptedAsAVideo.en> ;
    reg:name "adaptedAsAVideo"@en ;
    reg:status <http://metadataregistry.org/uri/RegStatus/1001> ;
    a rdf:Property ;
    rdfs:isDefinedBy <http://rdaregistry.info/Elements/u/> ;
    rdfs:label "is adapted as video"@en ;
    rdfs:subPropertyOf <http://rdaregistry.info/Elements/u/P60260> ;
    owl:inverseOf <http://rdaregistry.info/Elements/u/P60236> ;
    skos:definition "Relates a resource to a video based on the source resource."@en .

<http://rdaregistry.info/Elements/u/P60362>
    reg:hasSubproperty <http://rdaregistry.info/Elements/a/P50060> ;
    reg:lexicalAlias <http://rdaregistry.info/Elements/u/prominentMemberOfTheFamily.en> ;
    reg:name "prominentMemberOfTheFamily"@en ;
    reg:status <http://metadataregistry.org/uri/RegStatus/1001> ;
    a rdf:Property ;
    rdfs:isDefinedBy <http://rdaregistry.info/Elements/u/> ;
    rdfs:label "has prominent member of the agent"@en ;
    skos:definition "Relates a resource to a well-known individual who is a member of an agent."@en .

<http://rdaregistry.info/Elements/u/P60363>
    reg:hasSubproperty <http://rdaregistry.info/Elements/a/P50110> ;
    reg:lexicalAlias <http://rdaregistry.info/Elements/u/titleOfTheAgent.en> ;
    reg:name "titleOfTheAgent"@en ;
    reg:status <http://metadataregistry.org/uri/RegStatus/1001> ;
    a rdf:Property ;
    rdfs:isDefinedBy <http://rdaregistry.info/Elements/u/> ;
    rdfs:label "has title of the agent"@en ;
    skos:definition "Relates a resource to a word or phrase indicative of royalty, nobility, or ecclesiastical rank or office, a term of address for an agent of religious vocation, or another term indicative of rank, honour, or office."@en .

<http://rdaregistry.info/Elements/u/P60364>
    reg:hasSubproperty <http://rdaregistry.info/Elements/m/P30132> ;
    reg:lexicalAlias <http://rdaregistry.info/Elements/u/designationOfANamedRevisionOfAnEdition.en> ;
    reg:name "designationOfANamedRevisionOfAnEdition"@en ;
    reg:status <http://metadataregistry.org/uri/RegStatus/1001> ;
    a rdf:Property ;
    rdfs:isDefinedBy <http://rdaregistry.info/Elements/u/> ;
    rdfs:label "has designation of a named revision of an edition"@en ;
    skos:definition "Relates a resource to a word, character or group of words and/or characters, identifying a particular revision of a named edition."@en .

<http://rdaregistry.info/Elements/u/P60365>
    reg:hasSubproperty <http://rdaregistry.info/Elements/m/P30133> ;
    reg:lexicalAlias <http://rdaregistry.info/Elements/u/designationOfEdition.en> ;
    reg:name "designationOfEdition"@en ;
    reg:status <http://metadataregistry.org/uri/RegStatus/1001> ;
    a rdf:Property ;
    rdfs:isDefinedBy <http://rdaregistry.info/Elements/u/> ;
    rdfs:label "has designation of edition"@en ;
    skos:definition "Relates a resource to a word, character or group of words and/or characters, identifying the edition to which a resource belongs."@en .

<http://rdaregistry.info/Elements/u/P60366>
    reg:hasSubproperty <http://rdaregistry.info/Elements/u/P60548> ;
    reg:lexicalAlias <http://rdaregistry.info/Elements/u/nameOfThePlace.en> ;
    reg:name "nameOfThePlace"@en ;
    reg:status <http://metadataregistry.org/uri/RegStatus/1001> ;
    a rdf:Property ;
    rdfs:isDefinedBy <http://rdaregistry.info/Elements/u/> ;
    rdfs:label "has name of the place"@en ;
    skos:definition "Relates a resource to a word, character, or group of words and/or characters by which a place is known."@en .

<http://rdaregistry.info/Elements/u/P60367>
    reg:hasSubproperty <http://rdaregistry.info/Elements/u/P60588> ;
    reg:lexicalAlias <http://rdaregistry.info/Elements/u/titleOfTheResource.en> ;
    reg:name "titleOfTheResource"@en ;
    reg:status <http://metadataregistry.org/uri/RegStatus/1001> ;
    a rdf:Property ;
    rdfs:isDefinedBy <http://rdaregistry.info/Elements/u/> ;
    rdfs:label "has title of the resource"@en ;
    skos:definition "Relates a resource to a word, character, or group of words and/or characters by which a resource is known."@en .

<http://rdaregistry.info/Elements/u/P60368>
    reg:hasSubproperty <http://rdaregistry.info/Elements/a/P50032>, <http://rdaregistry.info/Elements/a/P50061>, <http://rdaregistry.info/Elements/a/P50111>, <http://rdaregistry.info/Elements/u/P60119>, <http://rdaregistry.info/Elements/u/P60549> ;
    reg:lexicalAlias <http://rdaregistry.info/Elements/u/nameOfTheAgent.en> ;
    reg:name "nameOfTheAgent"@en ;
    reg:status <http://metadataregistry.org/uri/RegStatus/1001> ;
    a rdf:Property ;
    rdfs:isDefinedBy <http://rdaregistry.info/Elements/u/> ;
    rdfs:label "has name of the agent"@en ;
    skos:definition "Relates a resource to a word, character, or group of words and/or characters by which an agent is known."@en .

<http://rdaregistry.info/Elements/u/P60369>
    reg:hasSubproperty <http://rdaregistry.info/Elements/m/P30134>, <http://rdaregistry.info/Elements/u/P60355>, <http://rdaregistry.info/Elements/u/P60357>, <http://rdaregistry.info/Elements/u/P60358>, <http://rdaregistry.info/Elements/u/P60359>, <http://rdaregistry.info/Elements/u/P60493>, <http://rdaregistry.info/Elements/u/P60507>, <http://rdaregistry.info/Elements/u/P60515>, <http://rdaregistry.info/Elements/u/P60589>, <http://rdaregistry.info/Elements/u/P60597> ;
    reg:lexicalAlias <http://rdaregistry.info/Elements/u/title.en> ;
    reg:name "title"@en ;
    reg:status <http://metadataregistry.org/uri/RegStatus/1001> ;
    a rdf:Property ;
    rdfs:isDefinedBy <http://rdaregistry.info/Elements/u/> ;
    rdfs:label "has title"@en ;
    skos:definition "Relates a resource to a word, character, or group of words and/or characters that names a resource or a resource contained in it."@en .

<http://rdaregistry.info/Elements/u/P60370>
    reg:hasSubproperty <http://rdaregistry.info/Elements/a/P50033>, <http://rdaregistry.info/Elements/a/P50108>, <http://rdaregistry.info/Elements/a/P50239> ;
    reg:lexicalAlias <http://rdaregistry.info/Elements/u/otherDesignationAssociatedWithTheAgent.en> ;
    reg:name "otherDesignationAssociatedWithTheAgent"@en ;
    reg:status <http://metadataregistry.org/uri/RegStatus/1001> ;
    a rdf:Property ;
    rdfs:isDefinedBy <http://rdaregistry.info/Elements/u/> ;
    rdfs:label "has other designation associated with the agent"@en ;
    skos:definition "Relates a resource to a word, phrase, or abbreviation indicating incorporation or legal status of an agent, or any term serving to differentiate the body from other corporate bodies, persons, etc., or a term other than a title that is associated with an agent’s name."@en .

<http://rdaregistry.info/Elements/u/P60371>
    reg:hasSubproperty <http://rdaregistry.info/Elements/e/P20068> ;
    reg:lexicalAlias <http://rdaregistry.info/Elements/u/writerOfAddedLyrics.en> ;
    reg:name "writerOfAddedLyrics"@en ;
    reg:status <http://metadataregistry.org/uri/RegStatus/1001> ;
    a rdf:Property ;
    rdfs:isDefinedBy <http://rdaregistry.info/Elements/u/> ;
    rdfs:label "has writer of added lyrics"@en ;
    rdfs:subPropertyOf <http://rdaregistry.info/Elements/u/P60380> ;
    owl:inverseOf <http://rdaregistry.info/Elements/u/P60600> ;
    skos:definition "Relates a resource to a writer of words added to a musical resource."@en .

<http://rdaregistry.info/Elements/u/P60372>
    reg:hasSubproperty <http://rdaregistry.info/Elements/e/P20069> ;
    reg:lexicalAlias <http://rdaregistry.info/Elements/u/summarizationOfTheContent.en> ;
    reg:name "summarizationOfTheContent"@en ;
    reg:status <http://metadataregistry.org/uri/RegStatus/1001> ;
    a rdf:Property ;
    rdfs:isDefinedBy <http://rdaregistry.info/Elements/u/> ;
    rdfs:label "has summarization of the content"@en ;
    skos:definition "Relates a resource to an abstract, summary, synopsis, etc., of the content of a resource."@en .

<http://rdaregistry.info/Elements/u/P60373>
    reg:lexicalAlias <http://rdaregistry.info/Elements/u/appellee.en> ;
    reg:name "appellee"@en ;
    reg:status <http://metadataregistry.org/uri/RegStatus/1001> ;
    a rdf:Property ;
    rdfs:isDefinedBy <http://rdaregistry.info/Elements/u/> ;
    rdfs:label "has appellee"@en ;
    rdfs:subPropertyOf <http://rdaregistry.info/Elements/u/P60374> ;
    owl:inverseOf <http://rdaregistry.info/Elements/u/P60601> ;
    skos:definition "Relates a resource to an agent against whom an appeal is taken on the decision of a lower court recorded in a legal resource of a higher court."@en .

<http://rdaregistry.info/Elements/u/P60374>
    reg:hasSubproperty <http://rdaregistry.info/Elements/i/P40023>, <http://rdaregistry.info/Elements/m/P30079>, <http://rdaregistry.info/Elements/u/P60060>, <http://rdaregistry.info/Elements/u/P60061>, <http://rdaregistry.info/Elements/u/P60062>, <http://rdaregistry.info/Elements/u/P60065>, <http://rdaregistry.info/Elements/u/P60097>, <http://rdaregistry.info/Elements/u/P60157>, <http://rdaregistry.info/Elements/u/P60373>, <http://rdaregistry.info/Elements/u/P60375>, <http://rdaregistry.info/Elements/u/P60376>, <http://rdaregistry.info/Elements/u/P60406>, <http://rdaregistry.info/Elements/u/P60421>, <http://rdaregistry.info/Elements/u/P60441>, <http://rdaregistry.info/Elements/u/P60449>, <http://rdaregistry.info/Elements/u/P60450>, <http://rdaregistry.info/Elements/u/P60451>, <http://rdaregistry.info/Elements/u/P60455>, <http://rdaregistry.info/Elements/u/P60456>, <http://rdaregistry.info/Elements/u/P60457>, <http://rdaregistry.info/Elements/u/P60458>, <http://rdaregistry.info/Elements/u/P60459>, <http://rdaregistry.info/Elements/u/P60460>, <http://rdaregistry.info/Elements/u/P60461>, <http://rdaregistry.info/Elements/u/P60462>, <http://rdaregistry.info/Elements/u/P60464>, <http://rdaregistry.info/Elements/u/P60466>, <http://rdaregistry.info/Elements/u/P60467>, <http://rdaregistry.info/Elements/u/P60815>, <http://rdaregistry.info/Elements/u/P60834>, <http://rdaregistry.info/Elements/u/P60836>, <http://rdaregistry.info/Elements/u/P60849>, <http://rdaregistry.info/Elements/u/P60869>, <http://rdaregistry.info/Elements/u/P60871> ;
    reg:lexicalAlias <http://rdaregistry.info/Elements/u/otherAgentAssociatedWithAResource.en> ;
    reg:name "otherAgentAssociatedWithAResource"@en ;
    reg:status <http://metadataregistry.org/uri/RegStatus/1001> ;
    a rdf:Property ;
    rdfs:isDefinedBy <http://rdaregistry.info/Elements/u/> ;
    rdfs:label "has other agent associated with a resource"@en ;
    owl:inverseOf <http://rdaregistry.info/Elements/u/P60602> ;
    skos:definition "Relates a resource to an agent other than a creator, custodian, owner, producer, publisher, distributor or manufacturer associated with a resource."@en ;
    skos:scopeNote "Includes book designers, platemakers, etc. Includes persons, etc., to whom correspondence is addressed, persons, etc., honoured by a festschrift, directors, cinematographers, sponsoring bodies, production companies, institutions, etc., hosting an exhibition or event, etc. Includes curators, binders, restorationists, etc."@en .

<http://rdaregistry.info/Elements/u/P60375>
    reg:lexicalAlias <http://rdaregistry.info/Elements/u/dedicator.en> ;
    reg:name "dedicator"@en ;
    reg:status <http://metadataregistry.org/uri/RegStatus/1001> ;
    a rdf:Property ;
    rdfs:isDefinedBy <http://rdaregistry.info/Elements/u/> ;
    rdfs:label "has dedicator"@en ;
    rdfs:subPropertyOf <http://rdaregistry.info/Elements/u/P60374> ;
    owl:inverseOf <http://rdaregistry.info/Elements/u/P60603> ;
    skos:definition "Relates a resource to an agent by whom a resource is dedicated."@en .

<http://rdaregistry.info/Elements/u/P60376>
    reg:hasSubproperty <http://rdaregistry.info/Elements/i/P40017>, <http://rdaregistry.info/Elements/u/P60066>, <http://rdaregistry.info/Elements/u/P60067> ;
    reg:lexicalAlias <http://rdaregistry.info/Elements/u/curator.en> ;
    reg:name "curator"@en ;
    reg:status <http://metadataregistry.org/uri/RegStatus/1001> ;
    a rdf:Property ;
    rdfs:isDefinedBy <http://rdaregistry.info/Elements/u/> ;
    rdfs:label "has curator"@en ;
    rdfs:subPropertyOf <http://rdaregistry.info/Elements/u/P60374> ;
    owl:inverseOf <http://rdaregistry.info/Elements/u/P60604> ;
    skos:definition "Relates a resource to an agent conceiving, aggregating, and/or organizing an exhibition, collection, or other resource."@en .

<http://rdaregistry.info/Elements/u/P60377>
    reg:hasSubproperty <http://rdaregistry.info/Elements/e/P20027> ;
    reg:lexicalAlias <http://rdaregistry.info/Elements/u/surveyor.en> ;
    reg:name "surveyor"@en ;
    reg:status <http://metadataregistry.org/uri/RegStatus/1001> ;
    a rdf:Property ;
    rdfs:isDefinedBy <http://rdaregistry.info/Elements/u/> ;
    rdfs:label "has surveyor"@en ;
    rdfs:subPropertyOf <http://rdaregistry.info/Elements/u/P60398> ;
    owl:inverseOf <http://rdaregistry.info/Elements/u/P60605> ;
    skos:definition "Relates a resource to an agent contributing to a cartographic resource by providing measurements or dimensional relationships for the geographic area represented."@en .

<http://rdaregistry.info/Elements/u/P60378>
    reg:hasSubproperty <http://rdaregistry.info/Elements/e/P20028> ;
    reg:lexicalAlias <http://rdaregistry.info/Elements/u/animator.en> ;
    reg:name "animator"@en ;
    reg:status <http://metadataregistry.org/uri/RegStatus/1001> ;
    a rdf:Property ;
    rdfs:isDefinedBy <http://rdaregistry.info/Elements/u/> ;
    rdfs:label "has animator"@en ;
    rdfs:subPropertyOf <http://rdaregistry.info/Elements/u/P60398> ;
    owl:inverseOf <http://rdaregistry.info/Elements/u/P60606> ;
    skos:definition "Relates a resource to an agent contributing to a moving image resource or computer program by giving apparent movement to inanimate objects or drawings."@en .

<http://rdaregistry.info/Elements/u/P60379>
    reg:hasSubproperty <http://rdaregistry.info/Elements/e/P20029> ;
    reg:lexicalAlias <http://rdaregistry.info/Elements/u/arrangerOfMusic.en> ;
    reg:name "arrangerOfMusic"@en ;
    reg:status <http://metadataregistry.org/uri/RegStatus/1001> ;
    a rdf:Property ;
    rdfs:isDefinedBy <http://rdaregistry.info/Elements/u/> ;
    rdfs:label "has arranger of music"@en ;
    rdfs:subPropertyOf <http://rdaregistry.info/Elements/u/P60398> ;
    owl:inverseOf <http://rdaregistry.info/Elements/u/P60607> ;
    skos:definition "Relates a resource to an agent contributing to a musical resource by rewriting the composition for a medium of performance different from that for which the resource was originally intended."@en .

<http://rdaregistry.info/Elements/u/P60380>
    reg:hasSubproperty <http://rdaregistry.info/Elements/e/P20030>, <http://rdaregistry.info/Elements/u/P60371> ;
    reg:lexicalAlias <http://rdaregistry.info/Elements/u/writerOfAddedText.en> ;
    reg:name "writerOfAddedText"@en ;
    reg:status <http://metadataregistry.org/uri/RegStatus/1001> ;
    a rdf:Property ;
    rdfs:isDefinedBy <http://rdaregistry.info/Elements/u/> ;
    rdfs:label "has writer of added text"@en ;
    rdfs:subPropertyOf <http://rdaregistry.info/Elements/u/P60392> ;
    owl:inverseOf <http://rdaregistry.info/Elements/u/P60608> ;
    skos:definition "Relates a resource to an agent contributing to a primarily non-textual resource by providing text for the non-textual resource (e.g., writing captions for photographs, descriptions of maps)."@en .

<http://rdaregistry.info/Elements/u/P60381>
    reg:hasSubproperty <http://rdaregistry.info/Elements/e/P20033> ;
    reg:lexicalAlias <http://rdaregistry.info/Elements/u/draftsman.en> ;
    reg:name "draftsman"@en ;
    reg:status <http://metadataregistry.org/uri/RegStatus/1001> ;
    a rdf:Property ;
    rdfs:isDefinedBy <http://rdaregistry.info/Elements/u/> ;
    rdfs:label "has draftsman"@en ;
    rdfs:subPropertyOf <http://rdaregistry.info/Elements/u/P60398> ;
    owl:inverseOf <http://rdaregistry.info/Elements/u/P60609> ;
    skos:definition "Relates a resource to an agent contributing to a resource by an architect, inventor, etc., by making detailed plans or drawings for buildings, ships, aircraft, machines, objects, etc."@en .

<http://rdaregistry.info/Elements/u/P60382>
    reg:hasSubproperty <http://rdaregistry.info/Elements/e/P20034> ;
    reg:lexicalAlias <http://rdaregistry.info/Elements/u/transcriber.en> ;
    reg:name "transcriber"@en ;
    reg:status <http://metadataregistry.org/uri/RegStatus/1001> ;
    a rdf:Property ;
    rdfs:isDefinedBy <http://rdaregistry.info/Elements/u/> ;
    rdfs:label "has transcriber"@en ;
    rdfs:subPropertyOf <http://rdaregistry.info/Elements/u/P60398> ;
    owl:inverseOf <http://rdaregistry.info/Elements/u/P60610> ;
    skos:definition "Relates a resource to an agent contributing to a resource by writing down or notating unwritten or unnotated content, or by changing it from one system of notation to another."@en .

<http://rdaregistry.info/Elements/u/P60383>
    reg:hasSubproperty <http://rdaregistry.info/Elements/e/P20035> ;
    reg:lexicalAlias <http://rdaregistry.info/Elements/u/musicalDirector.en> ;
    reg:name "musicalDirector"@en ;
    reg:status <http://metadataregistry.org/uri/RegStatus/1001> ;
    a rdf:Property ;
    rdfs:isDefinedBy <http://rdaregistry.info/Elements/u/> ;
    rdfs:label "has musical director"@en ;
    rdfs:subPropertyOf <http://rdaregistry.info/Elements/u/P60398> ;
    owl:inverseOf <http://rdaregistry.info/Elements/u/P60611> ;
    skos:definition "Relates a resource to an agent contributing to a resource by coordinating the activities of the composer, the sound editor, and sound mixers for a moving image production or for a musical or dramatic presentation or entertainment."@en .

<http://rdaregistry.info/Elements/u/P60384>
    reg:hasSubproperty <http://rdaregistry.info/Elements/e/P20036> ;
    reg:lexicalAlias <http://rdaregistry.info/Elements/u/costumeDesigner.en> ;
    reg:name "costumeDesigner"@en ;
    reg:status <http://metadataregistry.org/uri/RegStatus/1001> ;
    a rdf:Property ;
    rdfs:isDefinedBy <http://rdaregistry.info/Elements/u/> ;
    rdfs:label "has costume designer"@en ;
    rdfs:subPropertyOf <http://rdaregistry.info/Elements/u/P60398> ;
    owl:inverseOf <http://rdaregistry.info/Elements/u/P60612> ;
    skos:definition "Relates a resource to an agent contributing to a resource by designing the costumes for a moving image production or for a musical or dramatic presentation or entertainment."@en .

<http://rdaregistry.info/Elements/u/P60385>
    reg:hasSubproperty <http://rdaregistry.info/Elements/e/P20037> ;
    reg:lexicalAlias <http://rdaregistry.info/Elements/u/translator.en> ;
    reg:name "translator"@en ;
    reg:status <http://metadataregistry.org/uri/RegStatus/1001> ;
    a rdf:Property ;
    rdfs:isDefinedBy <http://rdaregistry.info/Elements/u/> ;
    rdfs:label "has translator"@en ;
    rdfs:subPropertyOf <http://rdaregistry.info/Elements/u/P60398> ;
    owl:inverseOf <http://rdaregistry.info/Elements/u/P60613> ;
    skos:definition "Relates a resource to an agent contributing to an expression of a resource by expressing the linguistic content of the resource in a language different from that of previous expressions of the original resource."@en .

<http://rdaregistry.info/Elements/u/P60386>
    reg:hasSubproperty <http://rdaregistry.info/Elements/e/P20038> ;
    reg:lexicalAlias <http://rdaregistry.info/Elements/u/artDirector.en> ;
    reg:name "artDirector"@en ;
    reg:status <http://metadataregistry.org/uri/RegStatus/1001> ;
    a rdf:Property ;
    rdfs:isDefinedBy <http://rdaregistry.info/Elements/u/> ;
    rdfs:label "has art director"@en ;
    rdfs:subPropertyOf <http://rdaregistry.info/Elements/u/P60398> ;
    owl:inverseOf <http://rdaregistry.info/Elements/u/P60614> ;
    skos:definition "Relates a resource to an agent contributing to a resource by overseeing the artists and craftspeople who build the sets for moving image productions."@en .

<http://rdaregistry.info/Elements/u/P60387>
    reg:hasSubproperty <http://rdaregistry.info/Elements/e/P20039>, <http://rdaregistry.info/Elements/u/P60141>, <http://rdaregistry.info/Elements/u/P60142>, <http://rdaregistry.info/Elements/u/P60143>, <http://rdaregistry.info/Elements/u/P60144>, <http://rdaregistry.info/Elements/u/P60145>, <http://rdaregistry.info/Elements/u/P60146>, <http://rdaregistry.info/Elements/u/P60147>, <http://rdaregistry.info/Elements/u/P60148>, <http://rdaregistry.info/Elements/u/P60149>, <http://rdaregistry.info/Elements/u/P60150>, <http://rdaregistry.info/Elements/u/P60151>, <http://rdaregistry.info/Elements/u/P60153>, <http://rdaregistry.info/Elements/u/P60154>, <http://rdaregistry.info/Elements/u/P60155>, <http://rdaregistry.info/Elements/u/P60156> ;
    reg:lexicalAlias <http://rdaregistry.info/Elements/u/performer.en> ;
    reg:name "performer"@en ;
    reg:status <http://metadataregistry.org/uri/RegStatus/1001> ;
    a rdf:Property ;
    rdfs:isDefinedBy <http://rdaregistry.info/Elements/u/> ;
    rdfs:label "has performer"@en ;
    rdfs:subPropertyOf <http://rdaregistry.info/Elements/u/P60398> ;
    owl:inverseOf <http://rdaregistry.info/Elements/u/P60615> ;
    skos:definition "Relates a resource to an agent contributing to a resource by performing music, acting, dancing, speaking, etc., often in a musical or dramatic presentation, etc."@en .

<http://rdaregistry.info/Elements/u/P60388>
    reg:hasSubproperty <http://rdaregistry.info/Elements/e/P20040> ;
    reg:lexicalAlias <http://rdaregistry.info/Elements/u/courtReporter.en> ;
    reg:name "courtReporter"@en ;
    reg:status <http://metadataregistry.org/uri/RegStatus/1001> ;
    a rdf:Property ;
    rdfs:isDefinedBy <http://rdaregistry.info/Elements/u/> ;
    rdfs:label "has court reporter"@en ;
    rdfs:subPropertyOf <http://rdaregistry.info/Elements/u/P60398> ;
    owl:inverseOf <http://rdaregistry.info/Elements/u/P60616> ;
    skos:definition "Relates a resource to an agent contributing to a resource by preparing a court's opinions for publication."@en .

<http://rdaregistry.info/Elements/u/P60389>
    reg:hasSubproperty <http://rdaregistry.info/Elements/e/P20041> ;
    reg:lexicalAlias <http://rdaregistry.info/Elements/u/writerOfPreface.en> ;
    reg:name "writerOfPreface"@en ;
    reg:status <http://metadataregistry.org/uri/RegStatus/1001> ;
    a rdf:Property ;
    rdfs:isDefinedBy <http://rdaregistry.info/Elements/u/> ;
    rdfs:label "has writer of preface"@en ;
    rdfs:subPropertyOf <http://rdaregistry.info/Elements/u/P60392> ;
    owl:inverseOf <http://rdaregistry.info/Elements/u/P60617> ;
    skos:definition "Relates a resource to an agent contributing to a resource by providing a preface to the original resource."@en .

<http://rdaregistry.info/Elements/u/P60390>
    reg:hasSubproperty <http://rdaregistry.info/Elements/e/P20044> ;
    reg:lexicalAlias <http://rdaregistry.info/Elements/u/writerOfAddedCommentary.en> ;
    reg:name "writerOfAddedCommentary"@en ;
    reg:status <http://metadataregistry.org/uri/RegStatus/1001> ;
    a rdf:Property ;
    rdfs:isDefinedBy <http://rdaregistry.info/Elements/u/> ;
    rdfs:label "has writer of added commentary"@en ;
    rdfs:subPropertyOf <http://rdaregistry.info/Elements/u/P60392> ;
    owl:inverseOf <http://rdaregistry.info/Elements/u/P60618> ;
    skos:definition "Relates a resource to an agent contributing to a resource by providing an interpretation or critical explanation of the original resource."@en .

<http://rdaregistry.info/Elements/u/P60391>
    reg:hasSubproperty <http://rdaregistry.info/Elements/e/P20045> ;
    reg:lexicalAlias <http://rdaregistry.info/Elements/u/writerOfIntroduction.en> ;
    reg:name "writerOfIntroduction"@en ;
    reg:status <http://metadataregistry.org/uri/RegStatus/1001> ;
    a rdf:Property ;
    rdfs:isDefinedBy <http://rdaregistry.info/Elements/u/> ;
    rdfs:label "has writer of introduction"@en ;
    rdfs:subPropertyOf <http://rdaregistry.info/Elements/u/P60392> ;
    owl:inverseOf <http://rdaregistry.info/Elements/u/P60619> ;
    skos:definition "Relates a resource to an agent contributing to a resource by providing an introduction to the original resource."@en .

<http://rdaregistry.info/Elements/u/P60392>
    reg:hasSubproperty <http://rdaregistry.info/Elements/e/P20046>, <http://rdaregistry.info/Elements/u/P60380>, <http://rdaregistry.info/Elements/u/P60389>, <http://rdaregistry.info/Elements/u/P60390>, <http://rdaregistry.info/Elements/u/P60391> ;
    reg:lexicalAlias <http://rdaregistry.info/Elements/u/writerOfSupplementaryTextualContent.en> ;
    reg:name "writerOfSupplementaryTextualContent"@en ;
    reg:status <http://metadataregistry.org/uri/RegStatus/1001> ;
    a rdf:Property ;
    rdfs:isDefinedBy <http://rdaregistry.info/Elements/u/> ;
    rdfs:label "has writer of supplementary textual content"@en ;
    rdfs:subPropertyOf <http://rdaregistry.info/Elements/u/P60398> ;
    owl:inverseOf <http://rdaregistry.info/Elements/u/P60620> ;
    skos:definition "Relates a resource to an agent contributing to a resource by providing supplementary textual content (e.g., an appendix, an introduction, a preface) to the original resource."@en .

<http://rdaregistry.info/Elements/u/P60393>
    reg:hasSubproperty <http://rdaregistry.info/Elements/e/P20048> ;
    reg:lexicalAlias <http://rdaregistry.info/Elements/u/editor.en> ;
    reg:name "editor"@en ;
    reg:status <http://metadataregistry.org/uri/RegStatus/1001> ;
    a rdf:Property ;
    rdfs:isDefinedBy <http://rdaregistry.info/Elements/u/> ;
    rdfs:label "has editor"@en ;
    rdfs:subPropertyOf <http://rdaregistry.info/Elements/u/P60398> ;
    owl:inverseOf <http://rdaregistry.info/Elements/u/P60621> ;
    skos:definition "Relates a resource to an agent contributing to a resource by revising or clarifying the content, or by selecting and putting together resources, or parts of resources, by one or more creators."@en .

<http://rdaregistry.info/Elements/u/P60394>
    reg:hasSubproperty <http://rdaregistry.info/Elements/e/P20049> ;
    reg:lexicalAlias <http://rdaregistry.info/Elements/u/abridger.en> ;
    reg:name "abridger"@en ;
    reg:status <http://metadataregistry.org/uri/RegStatus/1001> ;
    a rdf:Property ;
    rdfs:isDefinedBy <http://rdaregistry.info/Elements/u/> ;
    rdfs:label "has abridger"@en ;
    rdfs:subPropertyOf <http://rdaregistry.info/Elements/u/P60398> ;
    owl:inverseOf <http://rdaregistry.info/Elements/u/P60622> ;
    skos:definition "Relates a resource to an agent contributing to a resource by shortening or condensing the original resource but leaving the nature and content of the original resource substantially unchanged."@en .

<http://rdaregistry.info/Elements/u/P60395>
    reg:hasSubproperty <http://rdaregistry.info/Elements/e/P20050> ;
    reg:lexicalAlias <http://rdaregistry.info/Elements/u/recordingEngineer.en> ;
    reg:name "recordingEngineer"@en ;
    reg:status <http://metadataregistry.org/uri/RegStatus/1001> ;
    a rdf:Property ;
    rdfs:isDefinedBy <http://rdaregistry.info/Elements/u/> ;
    rdfs:label "has recording engineer"@en ;
    rdfs:subPropertyOf <http://rdaregistry.info/Elements/u/P60398> ;
    owl:inverseOf <http://rdaregistry.info/Elements/u/P60623> ;
    skos:definition "Relates a resource to an agent contributing to a resource by supervising the technical aspects of a sound or video recording session."@en .

<http://rdaregistry.info/Elements/u/P60396>
    reg:hasSubproperty <http://rdaregistry.info/Elements/e/P20051>, <http://rdaregistry.info/Elements/u/P60750> ;
    reg:lexicalAlias <http://rdaregistry.info/Elements/u/illustrator.en> ;
    reg:name "illustrator"@en ;
    reg:status <http://metadataregistry.org/uri/RegStatus/1001> ;
    a rdf:Property ;
    rdfs:isDefinedBy <http://rdaregistry.info/Elements/u/> ;
    rdfs:label "has illustrator"@en ;
    rdfs:subPropertyOf <http://rdaregistry.info/Elements/u/P60398> ;
    owl:inverseOf <http://rdaregistry.info/Elements/u/P60624> ;
    skos:definition "Relates a resource to an agent contributing to a resource by supplementing the primary content with drawings, diagrams, photographs, etc."@en .

<http://rdaregistry.info/Elements/u/P60397>
    reg:hasSubproperty <http://rdaregistry.info/Elements/e/P20052> ;
    reg:lexicalAlias <http://rdaregistry.info/Elements/u/recordist.en> ;
    reg:name "recordist"@en ;
    reg:status <http://metadataregistry.org/uri/RegStatus/1001> ;
    a rdf:Property ;
    rdfs:isDefinedBy <http://rdaregistry.info/Elements/u/> ;
    rdfs:label "has recordist"@en ;
    rdfs:subPropertyOf <http://rdaregistry.info/Elements/u/P60398> ;
    owl:inverseOf <http://rdaregistry.info/Elements/u/P60625> ;
    skos:definition "Relates a resource to an agent contributing to a resource by using a recording device to capture sound and/or video during a recording session, including field recordings of natural sounds, folkloric events, music, etc."@en .

<http://rdaregistry.info/Elements/u/P60398>
    reg:hasSubproperty <http://rdaregistry.info/Elements/e/P20053>, <http://rdaregistry.info/Elements/u/P60377>, <http://rdaregistry.info/Elements/u/P60378>, <http://rdaregistry.info/Elements/u/P60379>, <http://rdaregistry.info/Elements/u/P60381>, <http://rdaregistry.info/Elements/u/P60382>, <http://rdaregistry.info/Elements/u/P60383>, <http://rdaregistry.info/Elements/u/P60384>, <http://rdaregistry.info/Elements/u/P60385>, <http://rdaregistry.info/Elements/u/P60386>, <http://rdaregistry.info/Elements/u/P60387>, <http://rdaregistry.info/Elements/u/P60388>, <http://rdaregistry.info/Elements/u/P60392>, <http://rdaregistry.info/Elements/u/P60393>, <http://rdaregistry.info/Elements/u/P60394>, <http://rdaregistry.info/Elements/u/P60395>, <http://rdaregistry.info/Elements/u/P60396>, <http://rdaregistry.info/Elements/u/P60397>, <http://rdaregistry.info/Elements/u/P60399>, <http://rdaregistry.info/Elements/u/P60419>, <http://rdaregistry.info/Elements/u/P60422>, <http://rdaregistry.info/Elements/u/P60437>, <http://rdaregistry.info/Elements/u/P60446>, <http://rdaregistry.info/Elements/u/P60748>, <http://rdaregistry.info/Elements/u/P60749>, <http://rdaregistry.info/Elements/u/P60809>, <http://rdaregistry.info/Elements/u/P60811>, <http://rdaregistry.info/Elements/u/P60813>, <http://rdaregistry.info/Elements/u/P60824>, <http://rdaregistry.info/Elements/u/P60828>, <http://rdaregistry.info/Elements/u/P60838>, <http://rdaregistry.info/Elements/u/P60840>, <http://rdaregistry.info/Elements/u/P60851> ;
    reg:lexicalAlias <http://rdaregistry.info/Elements/u/contributor.en> ;
    reg:name "contributor"@en ;
    reg:status <http://metadataregistry.org/uri/RegStatus/1001> ;
    a rdf:Property ;
    rdfs:isDefinedBy <http://rdaregistry.info/Elements/u/> ;
    rdfs:label "has contributor"@en ;
    owl:inverseOf <http://rdaregistry.info/Elements/u/P60626> ;
    skos:definition "Relates a resource to an agent contributing to a resource."@en ;
    skos:scopeNote "Contributors include editors, translators, arrangers of music, performers, etc."@en .

<http://rdaregistry.info/Elements/u/P60399>
    reg:hasSubproperty <http://rdaregistry.info/Elements/e/P20031> ;
    reg:lexicalAlias <http://rdaregistry.info/Elements/u/stageDirector.en> ;
    reg:name "stageDirector"@en ;
    reg:status <http://metadataregistry.org/uri/RegStatus/1001> ;
    a rdf:Property ;
    rdfs:isDefinedBy <http://rdaregistry.info/Elements/u/> ;
    rdfs:label "has stage director"@en ;
    rdfs:subPropertyOf <http://rdaregistry.info/Elements/u/P60398> ;
    owl:inverseOf <http://rdaregistry.info/Elements/u/P60627> ;
    skos:definition "Relates a resource to an agent contributing to a stage resource through the general management and supervision of a performance."@en .

<http://rdaregistry.info/Elements/u/P60400>
    reg:hasSubproperty <http://rdaregistry.info/Elements/i/P40018>, <http://rdaregistry.info/Elements/u/P60068> ;
    reg:lexicalAlias <http://rdaregistry.info/Elements/u/currentOwner.en> ;
    reg:name "currentOwner"@en ;
    reg:status <http://metadataregistry.org/uri/RegStatus/1001> ;
    a rdf:Property ;
    rdfs:isDefinedBy <http://rdaregistry.info/Elements/u/> ;
    rdfs:label "has current owner"@en ;
    rdfs:subPropertyOf <http://rdaregistry.info/Elements/u/P60404> ;
    owl:inverseOf <http://rdaregistry.info/Elements/u/P60628> ;
    skos:definition "Relates a resource to an agent currently having legal possession of a resource."@en .

<http://rdaregistry.info/Elements/u/P60401>
    reg:hasSubproperty <http://rdaregistry.info/Elements/i/P40019>, <http://rdaregistry.info/Elements/u/P60091>, <http://rdaregistry.info/Elements/u/P60092> ;
    reg:lexicalAlias <http://rdaregistry.info/Elements/u/formerOwner.en> ;
    reg:name "formerOwner"@en ;
    reg:status <http://metadataregistry.org/uri/RegStatus/1001> ;
    a rdf:Property ;
    rdfs:isDefinedBy <http://rdaregistry.info/Elements/u/> ;
    rdfs:label "has former owner"@en ;
    rdfs:subPropertyOf <http://rdaregistry.info/Elements/u/P60404> ;
    owl:inverseOf <http://rdaregistry.info/Elements/u/P60630> ;
    skos:definition "Relates a resource to an agent formerly having legal possession of a resource."@en .

<http://rdaregistry.info/Elements/u/P60402>
    reg:hasSubproperty <http://rdaregistry.info/Elements/i/P40020> ;
    reg:lexicalAlias <http://rdaregistry.info/Elements/u/custodian.en> ;
    reg:name "custodian"@en ;
    reg:status <http://metadataregistry.org/uri/RegStatus/1001> ;
    a rdf:Property ;
    rdfs:isDefinedBy <http://rdaregistry.info/Elements/u/> ;
    rdfs:label "has custodian"@en ;
    owl:inverseOf <http://rdaregistry.info/Elements/u/P60631> ;
    skos:definition "Relates a resource to an agent having legal custody of a resource."@en .

<http://rdaregistry.info/Elements/u/P60404>
    reg:hasSubproperty <http://rdaregistry.info/Elements/i/P40021>, <http://rdaregistry.info/Elements/u/P60400>, <http://rdaregistry.info/Elements/u/P60401> ;
    reg:lexicalAlias <http://rdaregistry.info/Elements/u/owner.en> ;
    reg:name "owner"@en ;
    reg:status <http://metadataregistry.org/uri/RegStatus/1001> ;
    a rdf:Property ;
    rdfs:isDefinedBy <http://rdaregistry.info/Elements/u/> ;
    rdfs:label "has owner"@en ;
    owl:inverseOf <http://rdaregistry.info/Elements/u/P60632> ;
    skos:definition "Relates a resource to an agent having legal possession of a resource."@en .

<http://rdaregistry.info/Elements/u/P60406>
    reg:hasSubproperty <http://rdaregistry.info/Elements/i/P40022> ;
    reg:lexicalAlias <http://rdaregistry.info/Elements/u/honouree.en> ;
    reg:name "honouree"@en ;
    reg:status <http://metadataregistry.org/uri/RegStatus/1001> ;
    a rdf:Property ;
    rdfs:isDefinedBy <http://rdaregistry.info/Elements/u/> ;
    rdfs:label "has honouree"@en ;
    rdfs:subPropertyOf <http://rdaregistry.info/Elements/u/P60374> ;
    owl:inverseOf <http://rdaregistry.info/Elements/u/P60634> ;
    skos:altLabel "has honoree"@en ;
    skos:definition "Relates a resource to an agent honoured by a resource (e.g., the honouree of a festschrift)."@en .

<http://rdaregistry.info/Elements/u/P60407>
    reg:hasSubproperty <http://rdaregistry.info/Elements/m/P30067> ;
    reg:lexicalAlias <http://rdaregistry.info/Elements/u/broadcaster.en> ;
    reg:name "broadcaster"@en ;
    reg:status <http://metadataregistry.org/uri/RegStatus/1001> ;
    a rdf:Property ;
    rdfs:isDefinedBy <http://rdaregistry.info/Elements/u/> ;
    rdfs:label "has broadcaster"@en ;
    rdfs:subPropertyOf <http://rdaregistry.info/Elements/u/P60444> ;
    owl:inverseOf <http://rdaregistry.info/Elements/u/P60635> ;
    skos:definition "Relates a resource to an agent involved in broadcasting a resource to an audience via radio, television, webcast, etc."@en .

<http://rdaregistry.info/Elements/u/P60408>
    reg:hasSubproperty <http://rdaregistry.info/Elements/m/P30068> ;
    reg:lexicalAlias <http://rdaregistry.info/Elements/u/filmDistributor.en> ;
    reg:name "filmDistributor"@en ;
    reg:status <http://metadataregistry.org/uri/RegStatus/1001> ;
    a rdf:Property ;
    rdfs:isDefinedBy <http://rdaregistry.info/Elements/u/> ;
    rdfs:label "has film distributor"@en ;
    rdfs:subPropertyOf <http://rdaregistry.info/Elements/u/P60438> ;
    owl:inverseOf <http://rdaregistry.info/Elements/u/P60636> ;
    skos:definition "Relates a resource to an agent involved in distributing a moving image resource to theatres or other distribution channels."@en .

<http://rdaregistry.info/Elements/u/P60409>
    reg:hasSubproperty <http://rdaregistry.info/Elements/m/P30069> ;
    reg:lexicalAlias <http://rdaregistry.info/Elements/u/bookDesigner.en> ;
    reg:name "bookDesigner"@en ;
    reg:status <http://metadataregistry.org/uri/RegStatus/1001> ;
    a rdf:Property ;
    rdfs:isDefinedBy <http://rdaregistry.info/Elements/u/> ;
    rdfs:label "has book designer"@en ;
    rdfs:subPropertyOf <http://rdaregistry.info/Elements/u/P60443> ;
    owl:inverseOf <http://rdaregistry.info/Elements/u/P60637> ;
    skos:definition "Relates a resource to an agent involved in manufacturing a resource by being responsible for the entire graphic design of a book, including arrangement of type and illustration, choice of materials, and process used."@en .

<http://rdaregistry.info/Elements/u/P60410>
    reg:hasSubproperty <http://rdaregistry.info/Elements/m/P30070> ;
    reg:lexicalAlias <http://rdaregistry.info/Elements/u/engraver.en> ;
    reg:name "engraver"@en ;
    reg:status <http://metadataregistry.org/uri/RegStatus/1001> ;
    a rdf:Property ;
    rdfs:isDefinedBy <http://rdaregistry.info/Elements/u/> ;
    rdfs:label "has engraver"@en ;
    rdfs:subPropertyOf <http://rdaregistry.info/Elements/u/P60443> ;
    owl:inverseOf <http://rdaregistry.info/Elements/u/P60638> ;
    skos:definition "Relates a resource to an agent involved in manufacturing a resource by cutting letters, figures, etc., on a surface such as a wooden or metal plate used for printing."@en .

<http://rdaregistry.info/Elements/u/P60411>
    reg:hasSubproperty <http://rdaregistry.info/Elements/m/P30071> ;
    reg:lexicalAlias <http://rdaregistry.info/Elements/u/brailleEmbosser.en> ;
    reg:name "brailleEmbosser"@en ;
    reg:status <http://metadataregistry.org/uri/RegStatus/1001> ;
    a rdf:Property ;
    rdfs:isDefinedBy <http://rdaregistry.info/Elements/u/> ;
    rdfs:label "has braille embosser"@en ;
    rdfs:subPropertyOf <http://rdaregistry.info/Elements/u/P60443> ;
    owl:inverseOf <http://rdaregistry.info/Elements/u/P60639> ;
    skos:definition "Relates a resource to an agent involved in manufacturing a resource by embossing braille cells using a stylus, special embossing printer, or other device."@en .

<http://rdaregistry.info/Elements/u/P60412>
    reg:hasSubproperty <http://rdaregistry.info/Elements/m/P30072> ;
    reg:lexicalAlias <http://rdaregistry.info/Elements/u/printmaker.en> ;
    reg:name "printmaker"@en ;
    reg:status <http://metadataregistry.org/uri/RegStatus/1001> ;
    a rdf:Property ;
    rdfs:isDefinedBy <http://rdaregistry.info/Elements/u/> ;
    rdfs:label "has printmaker"@en ;
    rdfs:subPropertyOf <http://rdaregistry.info/Elements/u/P60443> ;
    owl:inverseOf <http://rdaregistry.info/Elements/u/P60640> ;
    skos:definition "Relates a resource to an agent involved in manufacturing a resource by making a relief, intaglio, or planographic printing surface."@en .

<http://rdaregistry.info/Elements/u/P60413>
    reg:hasSubproperty <http://rdaregistry.info/Elements/m/P30073> ;
    reg:lexicalAlias <http://rdaregistry.info/Elements/u/caster.en> ;
    reg:name "caster"@en ;
    reg:status <http://metadataregistry.org/uri/RegStatus/1001> ;
    a rdf:Property ;
    rdfs:isDefinedBy <http://rdaregistry.info/Elements/u/> ;
    rdfs:label "has caster"@en ;
    rdfs:subPropertyOf <http://rdaregistry.info/Elements/u/P60443> ;
    owl:inverseOf <http://rdaregistry.info/Elements/u/P60641> ;
    skos:definition "Relates a resource to an agent involved in manufacturing a resource by pouring a liquid or molten substance into a mold and leaving it to solidify to take the shape of the mold."@en .

<http://rdaregistry.info/Elements/u/P60414>
    reg:hasSubproperty <http://rdaregistry.info/Elements/m/P30074> ;
    reg:lexicalAlias <http://rdaregistry.info/Elements/u/lithographer.en> ;
    reg:name "lithographer"@en ;
    reg:status <http://metadataregistry.org/uri/RegStatus/1001> ;
    a rdf:Property ;
    rdfs:isDefinedBy <http://rdaregistry.info/Elements/u/> ;
    rdfs:label "has lithographer"@en ;
    rdfs:subPropertyOf <http://rdaregistry.info/Elements/u/P60443> ;
    owl:inverseOf <http://rdaregistry.info/Elements/u/P60642> ;
    skos:definition "Relates a resource to an agent involved in manufacturing a resource by preparing a stone or plate for lithographic printing, including a graphic artist creating a design directly on the surface from which printing will be done."@en .

<http://rdaregistry.info/Elements/u/P60415>
    reg:hasSubproperty <http://rdaregistry.info/Elements/m/P30075> ;
    reg:lexicalAlias <http://rdaregistry.info/Elements/u/platemaker.en> ;
    reg:name "platemaker"@en ;
    reg:status <http://metadataregistry.org/uri/RegStatus/1001> ;
    a rdf:Property ;
    rdfs:isDefinedBy <http://rdaregistry.info/Elements/u/> ;
    rdfs:label "has platemaker"@en ;
    rdfs:subPropertyOf <http://rdaregistry.info/Elements/u/P60443> ;
    owl:inverseOf <http://rdaregistry.info/Elements/u/P60643> ;
    skos:definition "Relates a resource to an agent involved in manufacturing a resource by preparing plates used in the production of printed images and/or text."@en .

<http://rdaregistry.info/Elements/u/P60416>
    reg:hasSubproperty <http://rdaregistry.info/Elements/m/P30076> ;
    reg:lexicalAlias <http://rdaregistry.info/Elements/u/etcher.en> ;
    reg:name "etcher"@en ;
    reg:status <http://metadataregistry.org/uri/RegStatus/1001> ;
    a rdf:Property ;
    rdfs:isDefinedBy <http://rdaregistry.info/Elements/u/> ;
    rdfs:label "has etcher"@en ;
    rdfs:subPropertyOf <http://rdaregistry.info/Elements/u/P60443> ;
    owl:inverseOf <http://rdaregistry.info/Elements/u/P60644> ;
    skos:definition "Relates a resource to an agent involved in manufacturing a resource by subjecting metal, glass, or some other surface used for printing, to acid or another corrosive substance."@en .

<http://rdaregistry.info/Elements/u/P60417>
    reg:hasSubproperty <http://rdaregistry.info/Elements/m/P30077> ;
    reg:lexicalAlias <http://rdaregistry.info/Elements/u/collotyper.en> ;
    reg:name "collotyper"@en ;
    reg:status <http://metadataregistry.org/uri/RegStatus/1001> ;
    a rdf:Property ;
    rdfs:isDefinedBy <http://rdaregistry.info/Elements/u/> ;
    rdfs:label "has collotyper"@en ;
    rdfs:subPropertyOf <http://rdaregistry.info/Elements/u/P60443> ;
    owl:inverseOf <http://rdaregistry.info/Elements/u/P60645> ;
    skos:definition "Relates a resource to an agent involved in manufacturing a resource using a photomechanical process for making prints directly from a hardened film of gelatin or other colloid that has ink-receptive and ink-repellent surfaces."@en .

<http://rdaregistry.info/Elements/u/P60418>
    reg:hasSubproperty <http://rdaregistry.info/Elements/m/P30078> ;
    reg:lexicalAlias <http://rdaregistry.info/Elements/u/printer.en> ;
    reg:name "printer"@en ;
    reg:status <http://metadataregistry.org/uri/RegStatus/1001> ;
    a rdf:Property ;
    rdfs:isDefinedBy <http://rdaregistry.info/Elements/u/> ;
    rdfs:label "has printer"@en ;
    rdfs:subPropertyOf <http://rdaregistry.info/Elements/u/P60443> ;
    owl:inverseOf <http://rdaregistry.info/Elements/u/P60646> ;
    skos:definition "Relates a resource to an agent involved in manufacturing a resource of printed text, notated music, etc., from type or plates, such as a book, newspaper, magazine, broadside, score, etc."@en .

<http://rdaregistry.info/Elements/u/P60419>
    reg:hasSubproperty <http://rdaregistry.info/Elements/e/P20054> ;
    reg:lexicalAlias <http://rdaregistry.info/Elements/u/presenter.en> ;
    reg:name "presenter"@en ;
    reg:status <http://metadataregistry.org/uri/RegStatus/1001> ;
    a rdf:Property ;
    rdfs:isDefinedBy <http://rdaregistry.info/Elements/u/> ;
    rdfs:label "has presenter"@en ;
    rdfs:subPropertyOf <http://rdaregistry.info/Elements/u/P60398> ;
    owl:inverseOf <http://rdaregistry.info/Elements/u/P60647> ;
    skos:definition "Relates a resource to an agent mentioned in an \"X presents\" credit for moving image materials and who is probably associated with production, finance, or distribution in some way."@en .

<http://rdaregistry.info/Elements/u/P60420>
    reg:lexicalAlias <http://rdaregistry.info/Elements/u/degreeSupervisor.en> ;
    reg:name "degreeSupervisor"@en ;
    reg:status <http://metadataregistry.org/uri/RegStatus/1001> ;
    a rdf:Property ;
    rdfs:isDefinedBy <http://rdaregistry.info/Elements/u/> ;
    rdfs:label "has degree supervisor"@en ;
    rdfs:subPropertyOf <http://rdaregistry.info/Elements/u/P60447> ;
    owl:inverseOf <http://rdaregistry.info/Elements/u/P60649> ;
    skos:definition "Relates a resource to an agent, such as an advisor or supervisor of thesis or dissertation research, overseeing either an academic degree or thesis."@en .

<http://rdaregistry.info/Elements/u/P60421>
    reg:hasSubproperty <http://rdaregistry.info/Elements/i/P40012> ;
    reg:lexicalAlias <http://rdaregistry.info/Elements/u/illuminator.en> ;
    reg:name "illuminator"@en ;
    reg:status <http://metadataregistry.org/uri/RegStatus/1001> ;
    a rdf:Property ;
    rdfs:isDefinedBy <http://rdaregistry.info/Elements/u/> ;
    rdfs:label "has illuminator"@en ;
    rdfs:subPropertyOf <http://rdaregistry.info/Elements/u/P60374> ;
    owl:inverseOf <http://rdaregistry.info/Elements/u/P60650> ;
    skos:definition "Relates a resource to an agent providing decoration to a specific resource using precious metals or color, often with elaborate designs and motifs."@en .

<http://rdaregistry.info/Elements/u/P60422>
    reg:hasSubproperty <http://rdaregistry.info/Elements/e/P20055> ;
    reg:lexicalAlias <http://rdaregistry.info/Elements/u/editorOfMovingImageResource.en> ;
    reg:name "editorOfMovingImageResource"@en ;
    reg:status <http://metadataregistry.org/uri/RegStatus/1001> ;
    a rdf:Property ;
    rdfs:isDefinedBy <http://rdaregistry.info/Elements/u/> ;
    rdfs:label "has editor of moving image work"@en ;
    rdfs:subPropertyOf <http://rdaregistry.info/Elements/u/P60398> ;
    owl:inverseOf <http://rdaregistry.info/Elements/u/P60651> ;
    skos:definition "Relates a resource to an agent responsible for assembling, arranging, and trimming film, video, or other moving image formats, including both visual and audio aspects."@en .

<http://rdaregistry.info/Elements/u/P60423>
    reg:lexicalAlias <http://rdaregistry.info/Elements/u/programmer.en> ;
    reg:name "programmer"@en ;
    reg:status <http://metadataregistry.org/uri/RegStatus/1001> ;
    a rdf:Property ;
    rdfs:isDefinedBy <http://rdaregistry.info/Elements/u/> ;
    rdfs:label "has programmer"@en ;
    rdfs:subPropertyOf <http://rdaregistry.info/Elements/u/P60447> ;
    owl:inverseOf <http://rdaregistry.info/Elements/u/P60652> ;
    skos:definition "Relates a resource to an agent responsible for creating a computer program."@en .

<http://rdaregistry.info/Elements/u/P60424>
    reg:lexicalAlias <http://rdaregistry.info/Elements/u/designer.en> ;
    reg:name "designer"@en ;
    reg:status <http://metadataregistry.org/uri/RegStatus/1001> ;
    a rdf:Property ;
    rdfs:isDefinedBy <http://rdaregistry.info/Elements/u/> ;
    rdfs:label "has designer"@en ;
    rdfs:subPropertyOf <http://rdaregistry.info/Elements/u/P60447> ;
    owl:inverseOf <http://rdaregistry.info/Elements/u/P60653> ;
    skos:definition "Relates a resource to an agent responsible for creating a design for an object."@en .

<http://rdaregistry.info/Elements/u/P60425>
    reg:hasSubproperty <http://rdaregistry.info/Elements/e/P20042> ;
    reg:lexicalAlias <http://rdaregistry.info/Elements/u/cartographer.en> ;
    reg:name "cartographer"@en ;
    reg:status <http://metadataregistry.org/uri/RegStatus/1001> ;
    a rdf:Property ;
    rdfs:isDefinedBy <http://rdaregistry.info/Elements/u/> ;
    rdfs:label "has cartographer"@en ;
    rdfs:subPropertyOf <http://rdaregistry.info/Elements/u/P60447> ;
    owl:inverseOf <http://rdaregistry.info/Elements/u/P60654> ;
    skos:definition "Relates a resource to an agent responsible for creating a map, atlas, globe, or other cartographic resource."@en .

<http://rdaregistry.info/Elements/u/P60426>
    reg:hasSubproperty <http://rdaregistry.info/Elements/e/P20026> ;
    reg:lexicalAlias <http://rdaregistry.info/Elements/u/composer.en> ;
    reg:name "composer"@en ;
    reg:status <http://metadataregistry.org/uri/RegStatus/1001> ;
    a rdf:Property ;
    rdfs:isDefinedBy <http://rdaregistry.info/Elements/u/> ;
    rdfs:label "has composer"@en ;
    rdfs:subPropertyOf <http://rdaregistry.info/Elements/u/P60447> ;
    owl:inverseOf <http://rdaregistry.info/Elements/u/P60655> ;
    skos:definition "Relates a resource to an agent responsible for creating a musical resource."@en .

<http://rdaregistry.info/Elements/u/P60427>
    reg:lexicalAlias <http://rdaregistry.info/Elements/u/inventor.en> ;
    reg:name "inventor"@en ;
    reg:status <http://metadataregistry.org/uri/RegStatus/1001> ;
    a rdf:Property ;
    rdfs:isDefinedBy <http://rdaregistry.info/Elements/u/> ;
    rdfs:label "has inventor"@en ;
    rdfs:subPropertyOf <http://rdaregistry.info/Elements/u/P60447> ;
    owl:inverseOf <http://rdaregistry.info/Elements/u/P60656> ;
    skos:definition "Relates a resource to an agent responsible for creating a new device or process."@en .

<http://rdaregistry.info/Elements/u/P60428>
    reg:lexicalAlias <http://rdaregistry.info/Elements/u/compiler.en> ;
    reg:name "compiler"@en ;
    reg:status <http://metadataregistry.org/uri/RegStatus/1001> ;
    a rdf:Property ;
    rdfs:isDefinedBy <http://rdaregistry.info/Elements/u/> ;
    rdfs:label "has compiler"@en ;
    rdfs:subPropertyOf <http://rdaregistry.info/Elements/u/P60447> ;
    owl:inverseOf <http://rdaregistry.info/Elements/u/P60657> ;
    skos:definition "Relates a resource to an agent responsible for creating a new resource (e.g., a bibliography, a directory) by selecting, arranging, aggregating, and editing data, information, etc."@en .

<http://rdaregistry.info/Elements/u/P60429>
    reg:hasSubproperty <http://rdaregistry.info/Elements/e/P20288> ;
    reg:lexicalAlias <http://rdaregistry.info/Elements/u/photographer.en> ;
    reg:name "photographer"@en ;
    reg:status <http://metadataregistry.org/uri/RegStatus/1001> ;
    a rdf:Property ;
    rdfs:isDefinedBy <http://rdaregistry.info/Elements/u/> ;
    rdfs:label "has photographer"@en ;
    rdfs:subPropertyOf <http://rdaregistry.info/Elements/u/P60447> ;
    owl:inverseOf <http://rdaregistry.info/Elements/u/P60658> ;
    skos:definition "Relates a resource to an agent responsible for creating a photographic resource."@en .

<http://rdaregistry.info/Elements/u/P60430>
    reg:hasSubproperty <http://rdaregistry.info/Elements/e/P20032> ;
    reg:lexicalAlias <http://rdaregistry.info/Elements/u/interviewer.en> ;
    reg:name "interviewer"@en ;
    reg:status <http://metadataregistry.org/uri/RegStatus/1001> ;
    a rdf:Property ;
    rdfs:isDefinedBy <http://rdaregistry.info/Elements/u/> ;
    rdfs:label "has interviewer"@en ;
    rdfs:subPropertyOf <http://rdaregistry.info/Elements/u/P60447> ;
    owl:inverseOf <http://rdaregistry.info/Elements/u/P60659> ;
    skos:definition "Relates a resource to an agent responsible for creating a resource by acting as an interviewer, reporter, pollster, or some other information gathering agent."@en .

<http://rdaregistry.info/Elements/u/P60431>
    reg:hasSubproperty <http://rdaregistry.info/Elements/u/P60475>, <http://rdaregistry.info/Elements/u/P60752>, <http://rdaregistry.info/Elements/u/P60753> ;
    reg:lexicalAlias <http://rdaregistry.info/Elements/u/artist.en> ;
    reg:name "artist"@en ;
    reg:status <http://metadataregistry.org/uri/RegStatus/1001> ;
    a rdf:Property ;
    rdfs:isDefinedBy <http://rdaregistry.info/Elements/u/> ;
    rdfs:label "has artist"@en ;
    rdfs:subPropertyOf <http://rdaregistry.info/Elements/u/P60447> ;
    owl:inverseOf <http://rdaregistry.info/Elements/u/P60660> ;
    skos:definition "Relates a resource to an agent responsible for creating a resource by conceiving, and often implementing, an original graphic design, drawing, painting, etc."@en .

<http://rdaregistry.info/Elements/u/P60432>
    reg:hasSubproperty <http://rdaregistry.info/Elements/e/P20047> ;
    reg:lexicalAlias <http://rdaregistry.info/Elements/u/interviewee.en> ;
    reg:name "interviewee"@en ;
    reg:status <http://metadataregistry.org/uri/RegStatus/1001> ;
    a rdf:Property ;
    rdfs:isDefinedBy <http://rdaregistry.info/Elements/u/> ;
    rdfs:label "has interviewee"@en ;
    rdfs:subPropertyOf <http://rdaregistry.info/Elements/u/P60447> ;
    owl:inverseOf <http://rdaregistry.info/Elements/u/P60661> ;
    skos:definition "Relates a resource to an agent responsible for creating a resource by responding to an interviewer, usually a reporter, pollster, or some other information gathering agent."@en .

<http://rdaregistry.info/Elements/u/P60433>
    reg:hasSubproperty <http://rdaregistry.info/Elements/e/P20043> ;
    reg:lexicalAlias <http://rdaregistry.info/Elements/u/choreographer.en> ;
    reg:name "choreographer"@en ;
    reg:status <http://metadataregistry.org/uri/RegStatus/1001> ;
    a rdf:Property ;
    rdfs:isDefinedBy <http://rdaregistry.info/Elements/u/> ;
    rdfs:label "has choreographer"@en ;
    rdfs:subPropertyOf <http://rdaregistry.info/Elements/u/P60447> ;
    owl:inverseOf <http://rdaregistry.info/Elements/u/P60662> ;
    skos:definition "Relates a resource to an agent responsible for creating a resource of movement."@en .

<http://rdaregistry.info/Elements/u/P60434>
    reg:hasSubproperty <http://rdaregistry.info/Elements/u/P60476>, <http://rdaregistry.info/Elements/u/P60477>, <http://rdaregistry.info/Elements/u/P60478>, <http://rdaregistry.info/Elements/u/P60751> ;
    reg:lexicalAlias <http://rdaregistry.info/Elements/u/author.en> ;
    reg:name "author"@en ;
    reg:status <http://metadataregistry.org/uri/RegStatus/1001> ;
    a rdf:Property ;
    rdfs:isDefinedBy <http://rdaregistry.info/Elements/u/> ;
    rdfs:label "has author"@en ;
    rdfs:subPropertyOf <http://rdaregistry.info/Elements/u/P60447> ;
    owl:inverseOf <http://rdaregistry.info/Elements/u/P60663> ;
    skos:definition "Relates a resource to an agent responsible for creating a resource that is primarily textual in content, regardless of media type (e.g., printed text, spoken word, electronic text, tactile text) or genre (e.g., poems, novels, screenplays, blogs)."@en .

<http://rdaregistry.info/Elements/u/P60435>
    reg:hasSubproperty <http://rdaregistry.info/Elements/u/P60473> ;
    reg:lexicalAlias <http://rdaregistry.info/Elements/u/architect.en> ;
    reg:name "architect"@en ;
    reg:status <http://metadataregistry.org/uri/RegStatus/1001> ;
    a rdf:Property ;
    rdfs:isDefinedBy <http://rdaregistry.info/Elements/u/> ;
    rdfs:label "has architect"@en ;
    rdfs:subPropertyOf <http://rdaregistry.info/Elements/u/P60447> ;
    owl:inverseOf <http://rdaregistry.info/Elements/u/P60664> ;
    skos:definition "Relates a resource to an agent responsible for creating an architectural design, including a pictorial representation intended to show how a building, etc., will look when completed."@en .

<http://rdaregistry.info/Elements/u/P60436>
    reg:lexicalAlias <http://rdaregistry.info/Elements/u/filmmaker.en> ;
    reg:name "filmmaker"@en ;
    reg:status <http://metadataregistry.org/uri/RegStatus/1001> ;
    a rdf:Property ;
    rdfs:isDefinedBy <http://rdaregistry.info/Elements/u/> ;
    rdfs:label "has filmmaker"@en ;
    rdfs:subPropertyOf <http://rdaregistry.info/Elements/u/P60447> ;
    owl:inverseOf <http://rdaregistry.info/Elements/u/P60665> ;
    skos:definition "Relates a resource to an agent responsible for creating an independent or personal film."@en .

<http://rdaregistry.info/Elements/u/P60437>
    reg:hasSubproperty <http://rdaregistry.info/Elements/e/P20056> ;
    reg:lexicalAlias <http://rdaregistry.info/Elements/u/productionDesigner.en> ;
    reg:name "productionDesigner"@en ;
    reg:status <http://metadataregistry.org/uri/RegStatus/1001> ;
    a rdf:Property ;
    rdfs:isDefinedBy <http://rdaregistry.info/Elements/u/> ;
    rdfs:label "has production designer"@en ;
    rdfs:subPropertyOf <http://rdaregistry.info/Elements/u/P60398> ;
    owl:inverseOf <http://rdaregistry.info/Elements/u/P60666> ;
    skos:definition "Relates a resource to an agent responsible for designing the overall visual appearance of a moving image production."@en .

<http://rdaregistry.info/Elements/u/P60438>
    reg:hasSubproperty <http://rdaregistry.info/Elements/m/P30080>, <http://rdaregistry.info/Elements/u/P60408> ;
    reg:lexicalAlias <http://rdaregistry.info/Elements/u/distributor.en> ;
    reg:name "distributor"@en ;
    reg:status <http://metadataregistry.org/uri/RegStatus/1001> ;
    a rdf:Property ;
    rdfs:isDefinedBy <http://rdaregistry.info/Elements/u/> ;
    rdfs:label "has distributor"@en ;
    owl:inverseOf <http://rdaregistry.info/Elements/u/P60667> ;
    skos:definition "Relates a resource to an agent responsible for distributing a resource."@en .

<http://rdaregistry.info/Elements/u/P60440>
    reg:hasSubproperty <http://rdaregistry.info/Elements/m/P30081> ;
    reg:lexicalAlias <http://rdaregistry.info/Elements/u/producerOfAnUnpublishedResource.en> ;
    reg:name "producerOfAnUnpublishedResource"@en ;
    reg:status <http://metadataregistry.org/uri/RegStatus/1001> ;
    a rdf:Property ;
    rdfs:isDefinedBy <http://rdaregistry.info/Elements/u/> ;
    rdfs:label "has producer of an unpublished resource"@en ;
    skos:definition "Relates a resource to an agent responsible for inscribing, fabricating, constructing, etc., a resource in an unpublished form."@en .

<http://rdaregistry.info/Elements/u/P60441>
    reg:hasSubproperty <http://rdaregistry.info/Elements/u/P60169>, <http://rdaregistry.info/Elements/u/P60170>, <http://rdaregistry.info/Elements/u/P60171> ;
    reg:lexicalAlias <http://rdaregistry.info/Elements/u/producer.en> ;
    reg:name "producer"@en ;
    reg:status <http://metadataregistry.org/uri/RegStatus/1001> ;
    a rdf:Property ;
    rdfs:isDefinedBy <http://rdaregistry.info/Elements/u/> ;
    rdfs:label "has producer"@en ;
    rdfs:subPropertyOf <http://rdaregistry.info/Elements/u/P60374> ;
    owl:inverseOf <http://rdaregistry.info/Elements/u/P60668> ;
    skos:definition "Relates a resource to an agent responsible for most of the business aspects of a production for screen, sound recording, television, webcast, etc. the producer is generally responsible for fund raising, managing the production, hiring key personnel, arranging for distributors, etc."@en .

<http://rdaregistry.info/Elements/u/P60442>
    reg:status <http://metadataregistry.org/uri/RegStatus/1008> ;
    rdfs:isDefinedBy <http://rdaregistry.info/Elements/u/> .

<http://rdaregistry.info/Elements/u/P60443>
    reg:hasSubproperty <http://rdaregistry.info/Elements/m/P30082>, <http://rdaregistry.info/Elements/u/P60409>, <http://rdaregistry.info/Elements/u/P60410>, <http://rdaregistry.info/Elements/u/P60411>, <http://rdaregistry.info/Elements/u/P60412>, <http://rdaregistry.info/Elements/u/P60413>, <http://rdaregistry.info/Elements/u/P60414>, <http://rdaregistry.info/Elements/u/P60415>, <http://rdaregistry.info/Elements/u/P60416>, <http://rdaregistry.info/Elements/u/P60417>, <http://rdaregistry.info/Elements/u/P60418>, <http://rdaregistry.info/Elements/u/P60746> ;
    reg:lexicalAlias <http://rdaregistry.info/Elements/u/manufacturer.en> ;
    reg:name "manufacturer"@en ;
    reg:status <http://metadataregistry.org/uri/RegStatus/1001> ;
    a rdf:Property ;
    rdfs:isDefinedBy <http://rdaregistry.info/Elements/u/> ;
    rdfs:label "has manufacturer"@en ;
    owl:inverseOf <http://rdaregistry.info/Elements/u/P60669> ;
    skos:definition "Relates a resource to an agent responsible for printing, duplicating, casting, etc., a resource in a published form."@en .

<http://rdaregistry.info/Elements/u/P60444>
    reg:hasSubproperty <http://rdaregistry.info/Elements/m/P30083>, <http://rdaregistry.info/Elements/u/P60407> ;
    reg:lexicalAlias <http://rdaregistry.info/Elements/u/publisher.en> ;
    reg:name "publisher"@en ;
    reg:status <http://metadataregistry.org/uri/RegStatus/1001> ;
    a rdf:Property ;
    rdfs:isDefinedBy <http://rdaregistry.info/Elements/u/> ;
    rdfs:label "has publisher"@en ;
    owl:inverseOf <http://rdaregistry.info/Elements/u/P60670> ;
    skos:definition "Relates a resource to an agent responsible for publishing, releasing, or issuing a resource."@en .

<http://rdaregistry.info/Elements/u/P60446>
    reg:hasSubproperty <http://rdaregistry.info/Elements/e/P20058> ;
    reg:lexicalAlias <http://rdaregistry.info/Elements/u/minuteTaker.en> ;
    reg:name "minuteTaker"@en ;
    reg:status <http://metadataregistry.org/uri/RegStatus/1001> ;
    a rdf:Property ;
    rdfs:isDefinedBy <http://rdaregistry.info/Elements/u/> ;
    rdfs:label "has minute taker"@en ;
    rdfs:subPropertyOf <http://rdaregistry.info/Elements/u/P60398> ;
    owl:inverseOf <http://rdaregistry.info/Elements/u/P60671> ;
    skos:definition "Relates a resource to an agent responsible for recording the minutes of a meeting."@en .

<http://rdaregistry.info/Elements/u/P60447>
    reg:hasSubproperty <http://rdaregistry.info/Elements/u/P60045>, <http://rdaregistry.info/Elements/u/P60096>, <http://rdaregistry.info/Elements/u/P60420>, <http://rdaregistry.info/Elements/u/P60423>, <http://rdaregistry.info/Elements/u/P60424>, <http://rdaregistry.info/Elements/u/P60425>, <http://rdaregistry.info/Elements/u/P60426>, <http://rdaregistry.info/Elements/u/P60427>, <http://rdaregistry.info/Elements/u/P60428>, <http://rdaregistry.info/Elements/u/P60429>, <http://rdaregistry.info/Elements/u/P60430>, <http://rdaregistry.info/Elements/u/P60431>, <http://rdaregistry.info/Elements/u/P60432>, <http://rdaregistry.info/Elements/u/P60433>, <http://rdaregistry.info/Elements/u/P60434>, <http://rdaregistry.info/Elements/u/P60435>, <http://rdaregistry.info/Elements/u/P60436>, <http://rdaregistry.info/Elements/u/P60463>, <http://rdaregistry.info/Elements/u/P60465>, <http://rdaregistry.info/Elements/u/P60826> ;
    reg:lexicalAlias <http://rdaregistry.info/Elements/u/creator.en> ;
    reg:name "creator"@en ;
    reg:status <http://metadataregistry.org/uri/RegStatus/1001> ;
    a rdf:Property ;
    rdfs:isDefinedBy <http://rdaregistry.info/Elements/u/> ;
    rdfs:label "has creator"@en ;
    owl:inverseOf <http://rdaregistry.info/Elements/u/P60672> ;
    skos:definition "Relates a resource to an agent responsible for the creation of a resource"@en .

<http://rdaregistry.info/Elements/u/P60449>
    reg:hasSubproperty <http://rdaregistry.info/Elements/u/P60084>, <http://rdaregistry.info/Elements/u/P60085>, <http://rdaregistry.info/Elements/u/P60086> ;
    reg:lexicalAlias <http://rdaregistry.info/Elements/u/director.en> ;
    reg:name "director"@en ;
    reg:status <http://metadataregistry.org/uri/RegStatus/1001> ;
    a rdf:Property ;
    rdfs:isDefinedBy <http://rdaregistry.info/Elements/u/> ;
    rdfs:label "has director"@en ;
    rdfs:subPropertyOf <http://rdaregistry.info/Elements/u/P60374> ;
    owl:inverseOf <http://rdaregistry.info/Elements/u/P60452> ;
    skos:definition "Relates a resource to an agent responsible for the general management and supervision of a filmed performance, a radio or television program, etc."@en .

<http://rdaregistry.info/Elements/u/P60450>
    reg:hasSubproperty <http://rdaregistry.info/Elements/e/P20289>, <http://rdaregistry.info/Elements/i/P40024> ;
    reg:lexicalAlias <http://rdaregistry.info/Elements/u/restorationist.en> ;
    reg:name "restorationist"@en ;
    reg:status <http://metadataregistry.org/uri/RegStatus/1001> ;
    a rdf:Property ;
    rdfs:isDefinedBy <http://rdaregistry.info/Elements/u/> ;
    rdfs:label "has restorationist"@en ;
    rdfs:subPropertyOf <http://rdaregistry.info/Elements/u/P60374> ;
    owl:inverseOf <http://rdaregistry.info/Elements/u/P60674> ;
    skos:definition "Relates a resource to an agent responsible for the set of technical, editorial, and intellectual procedures aimed at compensating for the degradation of a resource by bringing it back to a state as close as possible to its original condition."@en .

<http://rdaregistry.info/Elements/u/P60451>
    reg:lexicalAlias <http://rdaregistry.info/Elements/u/sponsoringBody.en> ;
    reg:name "sponsoringBody"@en ;
    reg:status <http://metadataregistry.org/uri/RegStatus/1001> ;
    a rdf:Property ;
    rdfs:isDefinedBy <http://rdaregistry.info/Elements/u/> ;
    rdfs:label "has sponsoring body"@en ;
    rdfs:subPropertyOf <http://rdaregistry.info/Elements/u/P60374> ;
    owl:inverseOf <http://rdaregistry.info/Elements/u/P60675> ;
    skos:definition "Relates a resource to an agent sponsoring some aspect of a resource, e.g., funding research, sponsoring an event."@en .

<http://rdaregistry.info/Elements/u/P60452>
    reg:hasSubproperty <http://rdaregistry.info/Elements/u/P60009>, <http://rdaregistry.info/Elements/u/P60010>, <http://rdaregistry.info/Elements/u/P60011> ;
    reg:lexicalAlias <http://rdaregistry.info/Elements/u/directorOfPhotography.en> ;
    reg:name "directorOfPhotography"@en ;
    reg:status <http://metadataregistry.org/uri/RegStatus/1001> ;
    a rdf:Property ;
    rdfs:isDefinedBy <http://rdaregistry.info/Elements/u/> ;
    rdfs:label "has director of photography"@en ;
    rdfs:subPropertyOf <http://rdaregistry.info/Elements/u/P60374> ;
    owl:inverseOf <http://rdaregistry.info/Elements/u/P60678> ;
    skos:definition "Relates a resource to an agent that captures images, either electronically or on film or video stock, and often selects and arranges the lighting. the director of photography for a movie is also called the chief cinematographer."@en .

<http://rdaregistry.info/Elements/u/P60454>
    reg:hasSubproperty <http://rdaregistry.info/Elements/a/P50218>, <http://rdaregistry.info/Elements/a/P50219>, <http://rdaregistry.info/Elements/a/P50220>, <http://rdaregistry.info/Elements/u/P60633>, <http://rdaregistry.info/Elements/u/P60737>, <http://rdaregistry.info/Elements/u/P60853>, <http://rdaregistry.info/Elements/u/P60854>, <http://rdaregistry.info/Elements/u/P60855>, <http://rdaregistry.info/Elements/u/P60856>, <http://rdaregistry.info/Elements/u/P60861>, <http://rdaregistry.info/Elements/u/P60862>, <http://rdaregistry.info/Elements/u/P60863> ;
    reg:lexicalAlias <http://rdaregistry.info/Elements/u/relatedAgent.en> ;
    reg:name "relatedAgent"@en ;
    reg:status <http://metadataregistry.org/uri/RegStatus/1001> ;
    a rdf:Property ;
    rdfs:isDefinedBy <http://rdaregistry.info/Elements/u/> ;
    rdfs:label "has related agent"@en ;
    skos:definition "Relates an agent to an agent that is associated with the agent being identified."@en .

<http://rdaregistry.info/Elements/u/P60455>
    reg:hasSubproperty <http://rdaregistry.info/Elements/i/P40025> ;
    reg:lexicalAlias <http://rdaregistry.info/Elements/u/dedicatee.en> ;
    reg:name "dedicatee"@en ;
    reg:status <http://metadataregistry.org/uri/RegStatus/1001> ;
    a rdf:Property ;
    rdfs:isDefinedBy <http://rdaregistry.info/Elements/u/> ;
    rdfs:label "has dedicatee"@en ;
    rdfs:subPropertyOf <http://rdaregistry.info/Elements/u/P60374> ;
    owl:inverseOf <http://rdaregistry.info/Elements/u/P60689> ;
    skos:definition "Relates a resource to an agent to whom a resource is dedicated."@en .

<http://rdaregistry.info/Elements/u/P60456>
    reg:lexicalAlias <http://rdaregistry.info/Elements/u/addressee.en> ;
    reg:name "addressee"@en ;
    reg:status <http://metadataregistry.org/uri/RegStatus/1001> ;
    a rdf:Property ;
    rdfs:isDefinedBy <http://rdaregistry.info/Elements/u/> ;
    rdfs:label "has addressee"@en ;
    rdfs:subPropertyOf <http://rdaregistry.info/Elements/u/P60374> ;
    owl:inverseOf <http://rdaregistry.info/Elements/u/P60690> ;
    skos:definition "Relates a resource to an agent to whom a resource or part of a resource is addressed."@en .

<http://rdaregistry.info/Elements/u/P60457>
    reg:lexicalAlias <http://rdaregistry.info/Elements/u/appellant.en> ;
    reg:name "appellant"@en ;
    reg:status <http://metadataregistry.org/uri/RegStatus/1001> ;
    a rdf:Property ;
    rdfs:isDefinedBy <http://rdaregistry.info/Elements/u/> ;
    rdfs:label "has appellant"@en ;
    rdfs:subPropertyOf <http://rdaregistry.info/Elements/u/P60374> ;
    owl:inverseOf <http://rdaregistry.info/Elements/u/P60691> ;
    skos:definition "Relates a resource to an agent who appeals the decision of a lower court recorded in a legal resource of a higher court."@en .

<http://rdaregistry.info/Elements/u/P60458>
    reg:hasSubproperty <http://rdaregistry.info/Elements/i/P40013> ;
    reg:lexicalAlias <http://rdaregistry.info/Elements/u/binder.en> ;
    reg:name "binder"@en ;
    reg:status <http://metadataregistry.org/uri/RegStatus/1001> ;
    a rdf:Property ;
    rdfs:isDefinedBy <http://rdaregistry.info/Elements/u/> ;
    rdfs:label "has binder"@en ;
    rdfs:subPropertyOf <http://rdaregistry.info/Elements/u/P60374> ;
    owl:inverseOf <http://rdaregistry.info/Elements/u/P60692> ;
    skos:definition "Relates a resource to an agent who binds a resource."@en .

<http://rdaregistry.info/Elements/u/P60459>
    reg:lexicalAlias <http://rdaregistry.info/Elements/u/plaintiff.en> ;
    reg:name "plaintiff"@en ;
    reg:status <http://metadataregistry.org/uri/RegStatus/1001> ;
    a rdf:Property ;
    rdfs:isDefinedBy <http://rdaregistry.info/Elements/u/> ;
    rdfs:label "has plaintiff"@en ;
    rdfs:subPropertyOf <http://rdaregistry.info/Elements/u/P60374> ;
    owl:inverseOf <http://rdaregistry.info/Elements/u/P60693> ;
    skos:definition "Relates a resource to an agent who brings a suit in a civil proceeding."@en .

<http://rdaregistry.info/Elements/u/P60460>
    reg:hasSubproperty <http://rdaregistry.info/Elements/i/P40014> ;
    reg:lexicalAlias <http://rdaregistry.info/Elements/u/inscriber.en> ;
    reg:name "inscriber"@en ;
    reg:status <http://metadataregistry.org/uri/RegStatus/1001> ;
    a rdf:Property ;
    rdfs:isDefinedBy <http://rdaregistry.info/Elements/u/> ;
    rdfs:label "has inscriber"@en ;
    rdfs:subPropertyOf <http://rdaregistry.info/Elements/u/P60374> ;
    owl:inverseOf <http://rdaregistry.info/Elements/u/P60695> ;
    skos:definition "Relates a resource to an agent who has written a statement of dedication or gift on a resource."@en .

<http://rdaregistry.info/Elements/u/P60461>
    reg:lexicalAlias <http://rdaregistry.info/Elements/u/judge.en> ;
    reg:name "judge"@en ;
    reg:status <http://metadataregistry.org/uri/RegStatus/1001> ;
    a rdf:Property ;
    rdfs:isDefinedBy <http://rdaregistry.info/Elements/u/> ;
    rdfs:label "has judge"@en ;
    rdfs:subPropertyOf <http://rdaregistry.info/Elements/u/P60374> ;
    owl:inverseOf <http://rdaregistry.info/Elements/u/P60696> ;
    skos:definition "Relates a resource to an agent who hears and decides on legal matters in court."@en .

<http://rdaregistry.info/Elements/u/P60462>
    reg:hasSubproperty <http://rdaregistry.info/Elements/w/P10285>, <http://rdaregistry.info/Elements/w/P10286> ;
    reg:lexicalAlias <http://rdaregistry.info/Elements/u/defendant.en> ;
    reg:name "defendant"@en ;
    reg:status <http://metadataregistry.org/uri/RegStatus/1001> ;
    a rdf:Property ;
    rdfs:isDefinedBy <http://rdaregistry.info/Elements/u/> ;
    rdfs:label "has defendant"@en ;
    rdfs:subPropertyOf <http://rdaregistry.info/Elements/u/P60374> ;
    owl:inverseOf <http://rdaregistry.info/Elements/u/P60698> ;
    skos:definition "Relates a resource to an agent who is accused in a criminal proceeding or sued in a civil proceeding."@en .

<http://rdaregistry.info/Elements/u/P60463>
    reg:lexicalAlias <http://rdaregistry.info/Elements/u/praeses.en> ;
    reg:name "praeses"@en ;
    reg:status <http://metadataregistry.org/uri/RegStatus/1001> ;
    a rdf:Property ;
    rdfs:isDefinedBy <http://rdaregistry.info/Elements/u/> ;
    rdfs:label "has praeses"@en ;
    rdfs:subPropertyOf <http://rdaregistry.info/Elements/u/P60447> ;
    owl:inverseOf <http://rdaregistry.info/Elements/u/P60699> ;
    skos:definition "Relates a resource to an agent who is the faculty moderator of an academic disputation, normally proposing a thesis and participating in the ensuing disputation."@en .

<http://rdaregistry.info/Elements/u/P60464>
    reg:hasSubproperty <http://rdaregistry.info/Elements/i/P40015> ;
    reg:lexicalAlias <http://rdaregistry.info/Elements/u/annotator.en> ;
    reg:name "annotator"@en ;
    reg:status <http://metadataregistry.org/uri/RegStatus/1001> ;
    a rdf:Property ;
    rdfs:isDefinedBy <http://rdaregistry.info/Elements/u/> ;
    rdfs:label "has annotator"@en ;
    rdfs:subPropertyOf <http://rdaregistry.info/Elements/u/P60374> ;
    owl:inverseOf <http://rdaregistry.info/Elements/u/P60700> ;
    skos:definition "Relates a resource to an agent who makes manuscript annotations on a resource."@en .

<http://rdaregistry.info/Elements/u/P60465>
    reg:lexicalAlias <http://rdaregistry.info/Elements/u/consultant.en> ;
    reg:name "consultant"@en ;
    reg:status <http://metadataregistry.org/uri/RegStatus/1001> ;
    a rdf:Property ;
    rdfs:isDefinedBy <http://rdaregistry.info/Elements/u/> ;
    rdfs:label "has consultant"@en ;
    rdfs:subPropertyOf <http://rdaregistry.info/Elements/u/P60447> ;
    owl:inverseOf <http://rdaregistry.info/Elements/u/P60701> ;
    skos:definition "Relates a resource to an agent who provides consultation services, and often makes recommendations, for another person, family or corporate body that is represented as the creator of a resource."@en .

<http://rdaregistry.info/Elements/u/P60466>
    reg:hasSubproperty <http://rdaregistry.info/Elements/i/P40016> ;
    reg:lexicalAlias <http://rdaregistry.info/Elements/u/autographer.en> ;
    reg:name "autographer"@en ;
    reg:status <http://metadataregistry.org/uri/RegStatus/1001> ;
    a rdf:Property ;
    rdfs:isDefinedBy <http://rdaregistry.info/Elements/u/> ;
    rdfs:label "has autographer"@en ;
    rdfs:subPropertyOf <http://rdaregistry.info/Elements/u/P60374> ;
    owl:inverseOf <http://rdaregistry.info/Elements/u/P60702> ;
    skos:definition "Relates a resource to an agent whose manuscript signature appears on a resource."@en .

<http://rdaregistry.info/Elements/u/P60467>
    reg:lexicalAlias <http://rdaregistry.info/Elements/u/issuingBody.en> ;
    reg:name "issuingBody"@en ;
    reg:status <http://metadataregistry.org/uri/RegStatus/1001> ;
    a rdf:Property ;
    rdfs:isDefinedBy <http://rdaregistry.info/Elements/u/> ;
    rdfs:label "has issuing body"@en ;
    rdfs:subPropertyOf <http://rdaregistry.info/Elements/u/P60374> ;
    owl:inverseOf <http://rdaregistry.info/Elements/u/P60703> ;
    skos:definition "Relates a resource to an agent, family or corporate body issuing a resource, such as an official organ of the body."@en .

<http://rdaregistry.info/Elements/u/P60468>
    reg:hasSubproperty <http://rdaregistry.info/Elements/a/P50104> ;
    reg:lexicalAlias <http://rdaregistry.info/Elements/u/professionOrOccupation.en> ;
    reg:name "professionOrOccupation"@en ;
    reg:status <http://metadataregistry.org/uri/RegStatus/1001> ;
    a rdf:Property ;
    rdfs:isDefinedBy <http://rdaregistry.info/Elements/u/> ;
    rdfs:label "has profession or occupation"@en ;
    skos:definition "Relates a resource to an agent's vocation or avocation."@en .

<http://rdaregistry.info/Elements/u/P60469>
    reg:hasSubproperty <http://rdaregistry.info/Elements/i/P40027>, <http://rdaregistry.info/Elements/m/P30136> ;
    reg:lexicalAlias <http://rdaregistry.info/Elements/u/electronicReproductionOf.en> ;
    reg:name "electronicReproductionOf"@en ;
    reg:status <http://metadataregistry.org/uri/RegStatus/1001> ;
    a rdf:Property ;
    rdfs:isDefinedBy <http://rdaregistry.info/Elements/u/> ;
    rdfs:label "is electronic reproduction of"@en ;
    rdfs:subPropertyOf <http://rdaregistry.info/Elements/u/P60297> ;
    owl:inverseOf <http://rdaregistry.info/Elements/u/P60083> ;
    skos:definition "Relates a resource to a resource in an analog format that is transferred to a digital format."@en .

<http://rdaregistry.info/Elements/u/P60470>
    reg:hasSubproperty <http://rdaregistry.info/Elements/e/P20071>, <http://rdaregistry.info/Elements/i/P40028>, <http://rdaregistry.info/Elements/m/P30137>, <http://rdaregistry.info/Elements/m/P30214>, <http://rdaregistry.info/Elements/u/P60122>, <http://rdaregistry.info/Elements/u/P60123>, <http://rdaregistry.info/Elements/u/P60124>, <http://rdaregistry.info/Elements/u/P60125>, <http://rdaregistry.info/Elements/u/P60126>, <http://rdaregistry.info/Elements/u/P60127>, <http://rdaregistry.info/Elements/u/P60128>, <http://rdaregistry.info/Elements/u/P60129>, <http://rdaregistry.info/Elements/u/P60130>, <http://rdaregistry.info/Elements/u/P60131>, <http://rdaregistry.info/Elements/u/P60132>, <http://rdaregistry.info/Elements/u/P60133>, <http://rdaregistry.info/Elements/u/P60134>, <http://rdaregistry.info/Elements/u/P60135>, <http://rdaregistry.info/Elements/u/P60136>, <http://rdaregistry.info/Elements/u/P60137>, <http://rdaregistry.info/Elements/u/P60868> ;
    reg:lexicalAlias <http://rdaregistry.info/Elements/u/noteOnResource.en> ;
    reg:name "noteOnResource"@en ;
    reg:status <http://metadataregistry.org/uri/RegStatus/1001> ;
    a rdf:Property ;
    rdfs:isDefinedBy <http://rdaregistry.info/Elements/u/> ;
    rdfs:label "has note on resource"@en ;
    skos:definition "Relates a resource to an annotation providing additional information about content recorded as a resource attribute."@en .

<http://rdaregistry.info/Elements/u/P60471>
    reg:status <http://metadataregistry.org/uri/RegStatus/1008> ;
    rdfs:isDefinedBy <http://rdaregistry.info/Elements/u/> .

<http://rdaregistry.info/Elements/u/P60472>
    reg:lexicalAlias <http://rdaregistry.info/Elements/u/epoch.en> ;
    reg:name "epoch"@en ;
    reg:status <http://metadataregistry.org/uri/RegStatus/1001> ;
    a rdf:Property ;
    rdfs:isDefinedBy <http://rdaregistry.info/Elements/u/> ;
    rdfs:label "has epoch"@en ;
    skos:definition "Relates a resource to an arbitrary moment in time to which measurements of position for a body or orientation for an orbit are referred."@en .

<http://rdaregistry.info/Elements/u/P60473>
    reg:lexicalAlias <http://rdaregistry.info/Elements/u/landscapeArchitect.en> ;
    reg:name "landscapeArchitect"@en ;
    reg:status <http://metadataregistry.org/uri/RegStatus/1001> ;
    a rdf:Property ;
    rdfs:isDefinedBy <http://rdaregistry.info/Elements/u/> ;
    rdfs:label "has landscape architect"@en ;
    rdfs:subPropertyOf <http://rdaregistry.info/Elements/u/P60435> ;
    owl:inverseOf <http://rdaregistry.info/Elements/u/P60704> ;
    skos:definition "Relates a resource to an architect responsible for creating landscape resources."@en .

<http://rdaregistry.info/Elements/u/P60474>
    reg:hasSubproperty <http://rdaregistry.info/Elements/e/P20197> ;
    reg:lexicalAlias <http://rdaregistry.info/Elements/u/findingAidFor.en> ;
    reg:name "findingAidFor"@en ;
    reg:status <http://metadataregistry.org/uri/RegStatus/1001> ;
    a rdf:Property ;
    rdfs:isDefinedBy <http://rdaregistry.info/Elements/u/> ;
    rdfs:label "is finding aid for"@en ;
    rdfs:subPropertyOf <http://rdaregistry.info/Elements/u/P60307> ;
    owl:inverseOf <http://rdaregistry.info/Elements/u/P60262> ;
    skos:definition "Relates a resource to an archival collection that is described in a finding aid, i.e., a guide to the organization, arrangement, and contents of the collection."@en .

<http://rdaregistry.info/Elements/u/P60475>
    reg:lexicalAlias <http://rdaregistry.info/Elements/u/sculptor.en> ;
    reg:name "sculptor"@en ;
    reg:status <http://metadataregistry.org/uri/RegStatus/1001> ;
    a rdf:Property ;
    rdfs:isDefinedBy <http://rdaregistry.info/Elements/u/> ;
    rdfs:label "has sculptor"@en ;
    rdfs:subPropertyOf <http://rdaregistry.info/Elements/u/P60431> ;
    owl:inverseOf <http://rdaregistry.info/Elements/u/P60705> ;
    skos:definition "Relates a resource to an artist responsible for creating a three-dimensional resource by modeling, carving, or similar technique."@en .

<http://rdaregistry.info/Elements/u/P60476>
    reg:lexicalAlias <http://rdaregistry.info/Elements/u/screenwriter.en> ;
    reg:name "screenwriter"@en ;
    reg:status <http://metadataregistry.org/uri/RegStatus/1001> ;
    a rdf:Property ;
    rdfs:isDefinedBy <http://rdaregistry.info/Elements/u/> ;
    rdfs:label "has screenwriter"@en ;
    rdfs:subPropertyOf <http://rdaregistry.info/Elements/u/P60434> ;
    owl:inverseOf <http://rdaregistry.info/Elements/u/P60706> ;
    skos:definition "Relates a resource to an author of a screenplay, script, or scene."@en .

<http://rdaregistry.info/Elements/u/P60477>
    reg:lexicalAlias <http://rdaregistry.info/Elements/u/lyricist.en> ;
    reg:name "lyricist"@en ;
    reg:status <http://metadataregistry.org/uri/RegStatus/1001> ;
    a rdf:Property ;
    rdfs:isDefinedBy <http://rdaregistry.info/Elements/u/> ;
    rdfs:label "has lyricist"@en ;
    rdfs:subPropertyOf <http://rdaregistry.info/Elements/u/P60434> ;
    owl:inverseOf <http://rdaregistry.info/Elements/u/P60707> ;
    skos:definition "Relates a resource to an author of the words of a popular song, including a song or songs from a musical."@en .

<http://rdaregistry.info/Elements/u/P60478>
    reg:lexicalAlias <http://rdaregistry.info/Elements/u/librettist.en> ;
    reg:name "librettist"@en ;
    reg:status <http://metadataregistry.org/uri/RegStatus/1001> ;
    a rdf:Property ;
    rdfs:isDefinedBy <http://rdaregistry.info/Elements/u/> ;
    rdfs:label "has librettist"@en ;
    rdfs:subPropertyOf <http://rdaregistry.info/Elements/u/P60434> ;
    owl:inverseOf <http://rdaregistry.info/Elements/u/P60708> ;
    skos:definition "Relates a resource to an author of the words of an opera or other musical stage resource or an oratorio."@en .

<http://rdaregistry.info/Elements/u/P60479>
    reg:hasSubproperty <http://rdaregistry.info/Elements/e/P20198> ;
    reg:lexicalAlias <http://rdaregistry.info/Elements/u/replacementInPartOf.en> ;
    reg:name "replacementInPartOf"@en ;
    reg:status <http://metadataregistry.org/uri/RegStatus/1001> ;
    a rdf:Property ;
    rdfs:isDefinedBy <http://rdaregistry.info/Elements/u/> ;
    rdfs:label "is replacement in part of"@en ;
    rdfs:subPropertyOf <http://rdaregistry.info/Elements/u/P60261> ;
    owl:inverseOf <http://rdaregistry.info/Elements/u/P60103> ;
    skos:definition "Relates a resource to an earlier resource whose content has been partially replaced by a later resource, usually because the later resource contains updated or new information that makes the earlier resource obsolete."@en .

<http://rdaregistry.info/Elements/u/P60480>
    reg:hasSubproperty <http://rdaregistry.info/Elements/e/P20199> ;
    reg:lexicalAlias <http://rdaregistry.info/Elements/u/replacementOf.en> ;
    reg:name "replacementOf"@en ;
    reg:status <http://metadataregistry.org/uri/RegStatus/1001> ;
    a rdf:Property ;
    rdfs:isDefinedBy <http://rdaregistry.info/Elements/u/> ;
    rdfs:label "is replacement of"@en ;
    rdfs:subPropertyOf <http://rdaregistry.info/Elements/u/P60261> ;
    owl:inverseOf <http://rdaregistry.info/Elements/u/P60104> ;
    skos:definition "Relates a resource to an earlier resource whose content has been replaced by a later resource, usually because the later resource contains updated or new information that makes the earlier resource obsolete."@en .

<http://rdaregistry.info/Elements/u/P60481>
    reg:hasSubproperty <http://rdaregistry.info/Elements/m/P30138> ;
    reg:lexicalAlias <http://rdaregistry.info/Elements/u/specialPlaybackCharacteristic.en> ;
    reg:name "specialPlaybackCharacteristic"@en ;
    reg:status <http://metadataregistry.org/uri/RegStatus/1001> ;
    a rdf:Property ;
    rdfs:isDefinedBy <http://rdaregistry.info/Elements/u/> ;
    rdfs:label "has special playback characteristic"@en ;
    rdfs:subPropertyOf <http://rdaregistry.info/Elements/u/P60351> ;
    skos:definition "Relates a resource to an equalization system, noise reduction system, etc., used in making an audio recording."@en .

<http://rdaregistry.info/Elements/u/P60482>
    reg:hasSubproperty <http://rdaregistry.info/Elements/a/P50034> ;
    reg:lexicalAlias <http://rdaregistry.info/Elements/u/associatedInstitution.en> ;
    reg:name "associatedInstitution"@en ;
    reg:status <http://metadataregistry.org/uri/RegStatus/1001> ;
    a rdf:Property ;
    rdfs:isDefinedBy <http://rdaregistry.info/Elements/u/> ;
    rdfs:label "has associated institution"@en ;
    skos:definition "Relates a resource to an institution commonly associated with an agent."@en .

<http://rdaregistry.info/Elements/u/P60483>
    reg:lexicalAlias <http://rdaregistry.info/Elements/u/grantingInstitutionOrFaculty.en> ;
    reg:name "grantingInstitutionOrFaculty"@en ;
    reg:status <http://metadataregistry.org/uri/RegStatus/1001> ;
    a rdf:Property ;
    rdfs:isDefinedBy <http://rdaregistry.info/Elements/u/> ;
    rdfs:label "has granting institution or faculty"@en ;
    skos:definition "Relates a resource to an institution or faculty conferring an academic degree on a candidate."@en .

<http://rdaregistry.info/Elements/u/P60484>
    reg:hasSubproperty <http://rdaregistry.info/Elements/a/P50035>, <http://rdaregistry.info/Elements/a/P50064> ;
    reg:lexicalAlias <http://rdaregistry.info/Elements/u/agentHistory.en> ;
    reg:name "agentHistory"@en ;
    reg:status <http://metadataregistry.org/uri/RegStatus/1001> ;
    a rdf:Property ;
    rdfs:isDefinedBy <http://rdaregistry.info/Elements/u/> ;
    rdfs:label "has agent history"@en ;
    skos:definition "Relates a resource to biographical or historical information about the agent."@en .

<http://rdaregistry.info/Elements/u/P60485>
    reg:hasSubproperty <http://rdaregistry.info/Elements/e/P20206> ;
    reg:lexicalAlias <http://rdaregistry.info/Elements/u/supplementaryContent.en> ;
    reg:name "supplementaryContent"@en ;
    reg:status <http://metadataregistry.org/uri/RegStatus/1001> ;
    a rdf:Property ;
    rdfs:isDefinedBy <http://rdaregistry.info/Elements/u/> ;
    rdfs:label "has supplementary content"@en ;
    skos:definition "Relates a resource to content (e.g., an index, a bibliography, an appendix) intended to supplement the primary content of a resource."@en .

<http://rdaregistry.info/Elements/u/P60486>
    reg:hasSubproperty <http://rdaregistry.info/Elements/e/P20207> ;
    reg:lexicalAlias <http://rdaregistry.info/Elements/u/illustrativeContent.en> ;
    reg:name "illustrativeContent"@en ;
    reg:status <http://metadataregistry.org/uri/RegStatus/1001> ;
    a rdf:Property ;
    rdfs:isDefinedBy <http://rdaregistry.info/Elements/u/> ;
    rdfs:label "has illustrative content"@en ;
    skos:definition "Relates a resource to content intended to illustrate the primary content of a resource."@en .

<http://rdaregistry.info/Elements/u/P60487>
    reg:hasSubproperty <http://rdaregistry.info/Elements/e/P20208> ;
    reg:lexicalAlias <http://rdaregistry.info/Elements/u/accessibilityContent.en> ;
    reg:name "accessibilityContent"@en ;
    reg:status <http://metadataregistry.org/uri/RegStatus/1001> ;
    a rdf:Property ;
    rdfs:isDefinedBy <http://rdaregistry.info/Elements/u/> ;
    rdfs:label "has accessibility content"@en ;
    skos:definition "Relates a resource to content that assists those with a sensory impairment in the greater understanding of content which their impairment prevents them fully seeing or hearing."@en .

<http://rdaregistry.info/Elements/u/P60488>
    reg:hasSubproperty <http://rdaregistry.info/Elements/e/P20209> ;
    reg:lexicalAlias <http://rdaregistry.info/Elements/u/formatOfNotatedMusic.en> ;
    reg:name "formatOfNotatedMusic"@en ;
    reg:status <http://metadataregistry.org/uri/RegStatus/1001> ;
    a rdf:Property ;
    rdfs:isDefinedBy <http://rdaregistry.info/Elements/u/> ;
    rdfs:label "has format of notated music"@en ;
    skos:definition "Relates a resource to the musical or physical layout of the content of a resource that is presented in the form of musical notation."@en .

<http://rdaregistry.info/Elements/u/P60489>
    reg:lexicalAlias <http://rdaregistry.info/Elements/u/dissertationOrThesisInformation.en> ;
    reg:name "dissertationOrThesisInformation"@en ;
    reg:status <http://metadataregistry.org/uri/RegStatus/1001> ;
    a rdf:Property ;
    rdfs:isDefinedBy <http://rdaregistry.info/Elements/u/> ;
    rdfs:label "has dissertation or thesis information"@en ;
    skos:definition "Relates a resource to information about a resource presented as part of the formal requirements for an academic degree."@en .

<http://rdaregistry.info/Elements/u/P60490>
    reg:hasSubproperty <http://rdaregistry.info/Elements/m/P30141> ;
    reg:lexicalAlias <http://rdaregistry.info/Elements/u/contactInformation.en> ;
    reg:name "contactInformation"@en ;
    reg:status <http://metadataregistry.org/uri/RegStatus/1001> ;
    a rdf:Property ;
    rdfs:isDefinedBy <http://rdaregistry.info/Elements/u/> ;
    rdfs:label "has contact information"@en ;
    skos:definition "Relates a resource to information about an organization, etc., from which a resource may be obtained."@en .

<http://rdaregistry.info/Elements/u/P60491>
    reg:lexicalAlias <http://rdaregistry.info/Elements/u/historyOfTheResource.en> ;
    reg:name "historyOfTheResource"@en ;
    reg:status <http://metadataregistry.org/uri/RegStatus/1001> ;
    a rdf:Property ;
    rdfs:isDefinedBy <http://rdaregistry.info/Elements/u/> ;
    rdfs:label "has history of the resource"@en ;
    skos:definition "Relates a resource to information about the history of a resource."@en .

<http://rdaregistry.info/Elements/u/P60492>
    reg:hasSubproperty <http://rdaregistry.info/Elements/a/P50113> ;
    reg:lexicalAlias <http://rdaregistry.info/Elements/u/biographicalInformation.en> ;
    reg:name "biographicalInformation"@en ;
    reg:status <http://metadataregistry.org/uri/RegStatus/1001> ;
    a rdf:Property ;
    rdfs:isDefinedBy <http://rdaregistry.info/Elements/u/> ;
    rdfs:label "has biographical information"@en ;
    skos:definition "Relates a resource to information about the life or history of an agent."@en .

<http://rdaregistry.info/Elements/u/P60493>
    reg:hasSubproperty <http://rdaregistry.info/Elements/m/P30142> ;
    reg:lexicalAlias <http://rdaregistry.info/Elements/u/otherTitleInformation.en> ;
    reg:name "otherTitleInformation"@en ;
    reg:status <http://metadataregistry.org/uri/RegStatus/1001> ;
    a rdf:Property ;
    rdfs:isDefinedBy <http://rdaregistry.info/Elements/u/> ;
    rdfs:label "has other title information"@en ;
    rdfs:subPropertyOf <http://rdaregistry.info/Elements/u/P60369> ;
    skos:definition "Relates a resource to information that appears in conjunction with, and is subordinate to, the title proper of a resource."@en .

<http://rdaregistry.info/Elements/u/P60494>
    reg:hasSubproperty <http://rdaregistry.info/Elements/m/P30143> ;
    reg:lexicalAlias <http://rdaregistry.info/Elements/u/otherTitleInformationOfSeries.en> ;
    reg:name "otherTitleInformationOfSeries"@en ;
    reg:status <http://metadataregistry.org/uri/RegStatus/1001> ;
    a rdf:Property ;
    rdfs:isDefinedBy <http://rdaregistry.info/Elements/u/> ;
    rdfs:label "has other title information of series"@en ;
    skos:definition "Relates a resource to information that appears in conjunction with, and is subordinate to, the title proper of a series."@en .

<http://rdaregistry.info/Elements/u/P60495>
    reg:hasSubproperty <http://rdaregistry.info/Elements/m/P30144> ;
    reg:lexicalAlias <http://rdaregistry.info/Elements/u/otherTitleInformationOfSubseries.en> ;
    reg:name "otherTitleInformationOfSubseries"@en ;
    reg:status <http://metadataregistry.org/uri/RegStatus/1001> ;
    a rdf:Property ;
    rdfs:isDefinedBy <http://rdaregistry.info/Elements/u/> ;
    rdfs:label "has other title information of subseries"@en ;
    skos:definition "Relates a resource to information that appears in conjunction with, and is subordinate to, the title proper of a subseries."@en .

<http://rdaregistry.info/Elements/u/P60496>
    reg:hasSubproperty <http://rdaregistry.info/Elements/i/P40047>, <http://rdaregistry.info/Elements/m/P30145> ;
    reg:lexicalAlias <http://rdaregistry.info/Elements/u/restrictionsOnAccess.en> ;
    reg:name "restrictionsOnAccess"@en ;
    reg:status <http://metadataregistry.org/uri/RegStatus/1001> ;
    a rdf:Property ;
    rdfs:isDefinedBy <http://rdaregistry.info/Elements/u/> ;
    rdfs:label "has restrictions on access"@en ;
    skos:definition "Relates a resource to limitations placed on access to a resource."@en .

<http://rdaregistry.info/Elements/u/P60497>
    reg:hasSubproperty <http://rdaregistry.info/Elements/i/P40048>, <http://rdaregistry.info/Elements/m/P30146> ;
    reg:lexicalAlias <http://rdaregistry.info/Elements/u/restrictionsOnUse.en> ;
    reg:name "restrictionsOnUse"@en ;
    reg:status <http://metadataregistry.org/uri/RegStatus/1001> ;
    a rdf:Property ;
    rdfs:isDefinedBy <http://rdaregistry.info/Elements/u/> ;
    rdfs:label "has restrictions on use"@en ;
    skos:definition "Relates a resource to limitations placed on uses such as reproduction, publication, exhibition, etc."@en .

<http://rdaregistry.info/Elements/u/P60498>
    reg:hasSubproperty <http://rdaregistry.info/Elements/e/P20210> ;
    reg:lexicalAlias <http://rdaregistry.info/Elements/u/otherDetailsOfCartographicContent.en> ;
    reg:name "otherDetailsOfCartographicContent"@en ;
    reg:status <http://metadataregistry.org/uri/RegStatus/1001> ;
    a rdf:Property ;
    rdfs:isDefinedBy <http://rdaregistry.info/Elements/u/> ;
    rdfs:label "has other details of cartographic content"@en ;
    skos:definition "Relates a resource to mathematical data and other features of the cartographic content of a resource not recorded in statements of scale, projection, and coordinates."@en .

<http://rdaregistry.info/Elements/u/P60499>
    reg:hasSubproperty <http://rdaregistry.info/Elements/m/P30147> ;
    reg:lexicalAlias <http://rdaregistry.info/Elements/u/numericAndOrAlphabeticDesignationOfFirstIssueOrPartOfSequence.en> ;
    reg:name "numericAndOrAlphabeticDesignationOfFirstIssueOrPartOfSequence"@en ;
    reg:status <http://metadataregistry.org/uri/RegStatus/1001> ;
    a rdf:Property ;
    rdfs:isDefinedBy <http://rdaregistry.info/Elements/u/> ;
    rdfs:label "has numeric and/or alphabetic designation of first issue or part of sequence"@en ;
    rdfs:subPropertyOf <http://rdaregistry.info/Elements/u/P60533> ;
    skos:definition "Relates a resource to numbering presented in numeric and/or alphabetic form on the first issue or part of a sequence of numbering for a serial."@en .

<http://rdaregistry.info/Elements/u/P60500>
    reg:hasSubproperty <http://rdaregistry.info/Elements/m/P30148> ;
    reg:lexicalAlias <http://rdaregistry.info/Elements/u/numericAndOrAlphabeticDesignationOfLastIssueOrPartOfSequence.en> ;
    reg:name "numericAndOrAlphabeticDesignationOfLastIssueOrPartOfSequence"@en ;
    reg:status <http://metadataregistry.org/uri/RegStatus/1001> ;
    a rdf:Property ;
    rdfs:isDefinedBy <http://rdaregistry.info/Elements/u/> ;
    rdfs:label "has numeric and/or alphabetic designation of last issue or part of sequence"@en ;
    rdfs:subPropertyOf <http://rdaregistry.info/Elements/u/P60533> ;
    skos:definition "Relates a resource to numbering presented in numeric and/or alphabetic form on the last issue or part of a sequence of numbering for a serial."@en .

<http://rdaregistry.info/Elements/u/P60501>
    reg:hasSubproperty <http://rdaregistry.info/Elements/m/P30149> ;
    reg:lexicalAlias <http://rdaregistry.info/Elements/u/chronologicalDesignationOfFirstIssueOrPartOfSequence.en> ;
    reg:name "chronologicalDesignationOfFirstIssueOrPartOfSequence"@en ;
    reg:status <http://metadataregistry.org/uri/RegStatus/1001> ;
    a rdf:Property ;
    rdfs:isDefinedBy <http://rdaregistry.info/Elements/u/> ;
    rdfs:label "has chronological designation of first issue or part of sequence"@en ;
    rdfs:subPropertyOf <http://rdaregistry.info/Elements/u/P60533> ;
    skos:definition "Relates a resource to numbering presented in the form of a date (e.g., a year; year and month; month, day, and year) on the first issue or part of a sequence of numbering for a serial."@en .

<http://rdaregistry.info/Elements/u/P60502>
    reg:hasSubproperty <http://rdaregistry.info/Elements/m/P30150> ;
    reg:lexicalAlias <http://rdaregistry.info/Elements/u/chronologicalDesignationOfLastIssueOrPartOfSequence.en> ;
    reg:name "chronologicalDesignationOfLastIssueOrPartOfSequence"@en ;
    reg:status <http://metadataregistry.org/uri/RegStatus/1001> ;
    a rdf:Property ;
    rdfs:isDefinedBy <http://rdaregistry.info/Elements/u/> ;
    rdfs:label "has chronological designation of last issue or part of sequence"@en ;
    rdfs:subPropertyOf <http://rdaregistry.info/Elements/u/P60533> ;
    skos:definition "Relates a resource to numbering presented in the form of a date (e.g., a year; year and month; month, day, and year) on the last issue or part of a sequence of numbering for a serial."@en .

<http://rdaregistry.info/Elements/u/P60503>
    reg:hasSubproperty <http://rdaregistry.info/Elements/e/P20200> ;
    reg:lexicalAlias <http://rdaregistry.info/Elements/u/splitInto.en> ;
    reg:name "splitInto"@en ;
    reg:status <http://metadataregistry.org/uri/RegStatus/1001> ;
    a rdf:Property ;
    rdfs:isDefinedBy <http://rdaregistry.info/Elements/u/> ;
    rdfs:label "is split into"@en ;
    rdfs:subPropertyOf <http://rdaregistry.info/Elements/u/P60278> ;
    owl:inverseOf <http://rdaregistry.info/Elements/u/P60276> ;
    skos:definition "Relates a resource to one of two or more resources resulting from the division of an earlier resource into separate resources."@en .

<http://rdaregistry.info/Elements/u/P60504>
    reg:hasSubproperty <http://rdaregistry.info/Elements/e/P20212> ;
    reg:lexicalAlias <http://rdaregistry.info/Elements/u/mergedToForm.en> ;
    reg:name "mergedToForm"@en ;
    reg:status <http://metadataregistry.org/uri/RegStatus/1001> ;
    a rdf:Property ;
    rdfs:isDefinedBy <http://rdaregistry.info/Elements/u/> ;
    rdfs:label "is merged to form"@en ;
    rdfs:subPropertyOf <http://rdaregistry.info/Elements/u/P60278> ;
    owl:inverseOf <http://rdaregistry.info/Elements/u/P60505> ;
    skos:definition "Relates a resource to a resource formed from the coming together of two or more resources."@en .

<http://rdaregistry.info/Elements/u/P60505>
    reg:hasSubproperty <http://rdaregistry.info/Elements/e/P20201> ;
    reg:lexicalAlias <http://rdaregistry.info/Elements/u/mergerOf.en> ;
    reg:name "mergerOf"@en ;
    reg:status <http://metadataregistry.org/uri/RegStatus/1001> ;
    a rdf:Property ;
    rdfs:isDefinedBy <http://rdaregistry.info/Elements/u/> ;
    rdfs:label "is merger of"@en ;
    rdfs:subPropertyOf <http://rdaregistry.info/Elements/u/P60261> ;
    owl:inverseOf <http://rdaregistry.info/Elements/u/P60504> ;
    skos:definition "Relates a resource to a resource that came together with one or more other resources to form the new resource."@en .

<http://rdaregistry.info/Elements/u/P60506>
    reg:lexicalAlias <http://rdaregistry.info/Elements/u/equinox.en> ;
    reg:name "equinox"@en ;
    reg:status <http://metadataregistry.org/uri/RegStatus/1001> ;
    a rdf:Property ;
    rdfs:isDefinedBy <http://rdaregistry.info/Elements/u/> ;
    rdfs:label "has equinox"@en ;
    skos:definition "Relates a resource to one of two points of intersection of the ecliptic and the celestial equator, occupied by the sun when its declination is 0°."@en .

<http://rdaregistry.info/Elements/u/P60507>
    reg:hasSubproperty <http://rdaregistry.info/Elements/m/P30151> ;
    reg:lexicalAlias <http://rdaregistry.info/Elements/u/parallelOtherTitleInformation.en> ;
    reg:name "parallelOtherTitleInformation"@en ;
    reg:status <http://metadataregistry.org/uri/RegStatus/1001> ;
    a rdf:Property ;
    rdfs:isDefinedBy <http://rdaregistry.info/Elements/u/> ;
    rdfs:label "has parallel other title information"@en ;
    rdfs:subPropertyOf <http://rdaregistry.info/Elements/u/P60369> ;
    skos:definition "Relates a resource to other title information in a language and/or script that differs from that recorded in the other title information element."@en .

<http://rdaregistry.info/Elements/u/P60508>
    reg:hasSubproperty <http://rdaregistry.info/Elements/m/P30152> ;
    reg:lexicalAlias <http://rdaregistry.info/Elements/u/parallelOtherTitleInformationOfSeries.en> ;
    reg:name "parallelOtherTitleInformationOfSeries"@en ;
    reg:status <http://metadataregistry.org/uri/RegStatus/1001> ;
    a rdf:Property ;
    rdfs:isDefinedBy <http://rdaregistry.info/Elements/u/> ;
    rdfs:label "has parallel other title information of series"@en ;
    skos:definition "Relates a resource to other title information of a series in a language and/or script that differs from that recorded in the other title information of series element."@en .

<http://rdaregistry.info/Elements/u/P60509>
    reg:hasSubproperty <http://rdaregistry.info/Elements/m/P30153> ;
    reg:lexicalAlias <http://rdaregistry.info/Elements/u/parallelOtherTitleInformationOfSubseries.en> ;
    reg:name "parallelOtherTitleInformationOfSubseries"@en ;
    reg:status <http://metadataregistry.org/uri/RegStatus/1001> ;
    a rdf:Property ;
    rdfs:isDefinedBy <http://rdaregistry.info/Elements/u/> ;
    rdfs:label "has parallel other title information of subseries"@en ;
    skos:definition "Relates a resource to other title information of a subseries in a language and/or script that differs from that recorded in the other title information of subseries element."@en .

<http://rdaregistry.info/Elements/u/P60510>
    reg:hasSubproperty <http://rdaregistry.info/Elements/e/P20213> ;
    reg:lexicalAlias <http://rdaregistry.info/Elements/u/additionalScaleInformation.en> ;
    reg:name "additionalScaleInformation"@en ;
    reg:status <http://metadataregistry.org/uri/RegStatus/1001> ;
    a rdf:Property ;
    rdfs:isDefinedBy <http://rdaregistry.info/Elements/u/> ;
    rdfs:label "has additional scale information"@en ;
    rdfs:subPropertyOf <http://rdaregistry.info/Elements/u/P60565> ;
    skos:definition "Relates a resource to supplemental information about scale such as a statement of comparative measurements or limitation of the scale to particular parts of the content of a resource."@en .

<http://rdaregistry.info/Elements/u/P60511>
    reg:hasSubproperty <http://rdaregistry.info/Elements/m/P30154> ;
    reg:lexicalAlias <http://rdaregistry.info/Elements/u/uniformResourceLocator.en> ;
    reg:name "uniformResourceLocator"@en ;
    reg:status <http://metadataregistry.org/uri/RegStatus/1001> ;
    a rdf:Property ;
    rdfs:isDefinedBy <http://rdaregistry.info/Elements/u/> ;
    rdfs:label "has uniform resource locator"@en ;
    skos:definition "Relates a resource to the address of a remote access resource."@en .

<http://rdaregistry.info/Elements/u/P60512>
    reg:hasSubproperty <http://rdaregistry.info/Elements/a/P50036>, <http://rdaregistry.info/Elements/a/P50114> ;
    reg:lexicalAlias <http://rdaregistry.info/Elements/u/addressOfTheAgent.en> ;
    reg:name "addressOfTheAgent"@en ;
    reg:status <http://metadataregistry.org/uri/RegStatus/1001> ;
    a rdf:Property ;
    rdfs:isDefinedBy <http://rdaregistry.info/Elements/u/> ;
    rdfs:label "has address of the agent"@en ;
    skos:definition "Relates a resource to the address of an agent's place of residence, business, or employer, headquarters or offices, or an e-mail or internet address."@en .

<http://rdaregistry.info/Elements/u/P60513>
    reg:hasSubproperty <http://rdaregistry.info/Elements/m/P30155> ;
    reg:lexicalAlias <http://rdaregistry.info/Elements/u/layout.en> ;
    reg:name "layout"@en ;
    reg:status <http://metadataregistry.org/uri/RegStatus/1001> ;
    a rdf:Property ;
    rdfs:isDefinedBy <http://rdaregistry.info/Elements/u/> ;
    rdfs:label "has layout"@en ;
    skos:definition "Relates a resource to the arrangement of text, images, tactile notation, etc., in a resource."@en .

<http://rdaregistry.info/Elements/u/P60514>
    reg:lexicalAlias <http://rdaregistry.info/Elements/u/yearDegreeGranted.en> ;
    reg:name "yearDegreeGranted"@en ;
    reg:status <http://metadataregistry.org/uri/RegStatus/1001> ;
    a rdf:Property ;
    rdfs:isDefinedBy <http://rdaregistry.info/Elements/u/> ;
    rdfs:label "has year degree granted"@en ;
    skos:definition "Relates a resource to the calendar year in which a granting institution or faculty conferred an academic degree on a candidate."@en .

<http://rdaregistry.info/Elements/u/P60515>
    reg:hasSubproperty <http://rdaregistry.info/Elements/m/P30156> ;
    reg:lexicalAlias <http://rdaregistry.info/Elements/u/titleProper.en> ;
    reg:name "titleProper"@en ;
    reg:status <http://metadataregistry.org/uri/RegStatus/1001> ;
    a rdf:Property ;
    rdfs:isDefinedBy <http://rdaregistry.info/Elements/u/> ;
    rdfs:label "has title proper"@en ;
    rdfs:subPropertyOf <http://rdaregistry.info/Elements/u/P60369> ;
    skos:definition "Relates a resource to the chief name of a resource (i.e., the title normally used when citing the resource)."@en .

<http://rdaregistry.info/Elements/u/P60516>
    reg:hasSubproperty <http://rdaregistry.info/Elements/m/P30157> ;
    reg:lexicalAlias <http://rdaregistry.info/Elements/u/titleProperOfSeries.en> ;
    reg:name "titleProperOfSeries"@en ;
    reg:status <http://metadataregistry.org/uri/RegStatus/1001> ;
    a rdf:Property ;
    rdfs:isDefinedBy <http://rdaregistry.info/Elements/u/> ;
    rdfs:label "has title proper of series"@en ;
    skos:definition "Relates a resource to the chief name of a series (i.e., the title normally used when citing the series)."@en .

<http://rdaregistry.info/Elements/u/P60517>
    reg:hasSubproperty <http://rdaregistry.info/Elements/m/P30158> ;
    reg:lexicalAlias <http://rdaregistry.info/Elements/u/titleProperOfSubseries.en> ;
    reg:name "titleProperOfSubseries"@en ;
    reg:status <http://metadataregistry.org/uri/RegStatus/1001> ;
    a rdf:Property ;
    rdfs:isDefinedBy <http://rdaregistry.info/Elements/u/> ;
    rdfs:label "has title proper of subseries"@en ;
    skos:definition "Relates a resource to the chief name of a subseries (i.e., the title normally used when citing the subseries)."@en .

<http://rdaregistry.info/Elements/u/P60518>
    reg:lexicalAlias <http://rdaregistry.info/Elements/u/coverageOfTheContent.en> ;
    reg:name "coverageOfTheContent"@en ;
    reg:status <http://metadataregistry.org/uri/RegStatus/1001> ;
    a rdf:Property ;
    rdfs:isDefinedBy <http://rdaregistry.info/Elements/u/> ;
    rdfs:label "has coverage of the content"@en ;
    skos:definition "Relates a resource to the chronological or geographic coverage of the content of a resource."@en .

<http://rdaregistry.info/Elements/u/P60519>
    reg:hasSubproperty <http://rdaregistry.info/Elements/m/P30159> ;
    reg:lexicalAlias <http://rdaregistry.info/Elements/u/resolution.en> ;
    reg:name "resolution"@en ;
    reg:status <http://metadataregistry.org/uri/RegStatus/1001> ;
    a rdf:Property ;
    rdfs:isDefinedBy <http://rdaregistry.info/Elements/u/> ;
    rdfs:label "has resolution"@en ;
    rdfs:subPropertyOf <http://rdaregistry.info/Elements/u/P60350> ;
    skos:definition "Relates a resource to the clarity or fineness of detail in a digital image, expressed by the measurement of the image in pixels, etc."@en .

<http://rdaregistry.info/Elements/u/P60520>
    reg:lexicalAlias <http://rdaregistry.info/Elements/u/intendedAudience.en> ;
    reg:name "intendedAudience"@en ;
    reg:status <http://metadataregistry.org/uri/RegStatus/1001> ;
    a rdf:Property ;
    rdfs:isDefinedBy <http://rdaregistry.info/Elements/u/> ;
    rdfs:label "has intended audience"@en ;
    skos:definition "Relates a resource to the class of user for which the content of a resource is intended, or for whom the content is considered suitable."@en .

<http://rdaregistry.info/Elements/u/P60521>
    reg:hasSubproperty <http://rdaregistry.info/Elements/m/P30160> ;
    reg:lexicalAlias <http://rdaregistry.info/Elements/u/termsOfAvailability.en> ;
    reg:name "termsOfAvailability"@en ;
    reg:status <http://metadataregistry.org/uri/RegStatus/1001> ;
    a rdf:Property ;
    rdfs:isDefinedBy <http://rdaregistry.info/Elements/u/> ;
    rdfs:label "has terms of availability"@en ;
    skos:definition "Relates a resource to the conditions under which the publisher, distributor, etc., will normally supply a resource or the price of a resource."@en .

<http://rdaregistry.info/Elements/u/P60522>
    reg:hasSubproperty <http://rdaregistry.info/Elements/m/P30161> ;
    reg:lexicalAlias <http://rdaregistry.info/Elements/u/trackConfiguration.en> ;
    reg:name "trackConfiguration"@en ;
    reg:status <http://metadataregistry.org/uri/RegStatus/1001> ;
    a rdf:Property ;
    rdfs:isDefinedBy <http://rdaregistry.info/Elements/u/> ;
    rdfs:label "has track configuration"@en ;
    rdfs:subPropertyOf <http://rdaregistry.info/Elements/u/P60351> ;
    skos:definition "Relates a resource to the configuration of the audio track on a sound-track film (e.g., centre track)."@en .

<http://rdaregistry.info/Elements/u/P60523>
    reg:lexicalAlias <http://rdaregistry.info/Elements/u/placeOfOriginOfTheResource.en> ;
    reg:name "placeOfOriginOfTheResource"@en ;
    reg:status <http://metadataregistry.org/uri/RegStatus/1001> ;
    a rdf:Property ;
    rdfs:isDefinedBy <http://rdaregistry.info/Elements/u/> ;
    rdfs:label "has place of origin of the resource"@en ;
    skos:definition "Relates a resource to the country or other territorial jurisdiction from which a resource originated."@en .

<http://rdaregistry.info/Elements/u/P60524>
    reg:hasSubproperty <http://rdaregistry.info/Elements/a/P50037> ;
    reg:lexicalAlias <http://rdaregistry.info/Elements/u/dateOfEstablishment.en> ;
    reg:name "dateOfEstablishment"@en ;
    reg:status <http://metadataregistry.org/uri/RegStatus/1001> ;
    a rdf:Property ;
    rdfs:isDefinedBy <http://rdaregistry.info/Elements/u/> ;
    rdfs:label "has date of establishment"@en ;
    rdfs:subPropertyOf <http://rdaregistry.info/Elements/u/P60324> ;
    skos:definition "Relates a resource to the date on which an agent was established or founded."@en .

<http://rdaregistry.info/Elements/u/P60525>
    reg:hasSubproperty <http://rdaregistry.info/Elements/a/P50038> ;
    reg:lexicalAlias <http://rdaregistry.info/Elements/u/dateOfTermination.en> ;
    reg:name "dateOfTermination"@en ;
    reg:status <http://metadataregistry.org/uri/RegStatus/1001> ;
    a rdf:Property ;
    rdfs:isDefinedBy <http://rdaregistry.info/Elements/u/> ;
    rdfs:label "has date of termination"@en ;
    rdfs:subPropertyOf <http://rdaregistry.info/Elements/u/P60324> ;
    skos:definition "Relates a resource to the date on which an agent was terminated or dissolved."@en .

<http://rdaregistry.info/Elements/u/P60526>
    reg:hasSubproperty <http://rdaregistry.info/Elements/a/P50039> ;
    reg:lexicalAlias <http://rdaregistry.info/Elements/u/dateOfConferenceEtc.en> ;
    reg:name "dateOfConferenceEtc"@en ;
    reg:status <http://metadataregistry.org/uri/RegStatus/1001> ;
    a rdf:Property ;
    rdfs:isDefinedBy <http://rdaregistry.info/Elements/u/> ;
    rdfs:label "has date of conference, etc."@en ;
    rdfs:subPropertyOf <http://rdaregistry.info/Elements/u/P60324> ;
    skos:definition "Relates a resource to the date or range of dates on which a conference, congress, meeting, exhibition, fair, festival, etc., was held."@en .

<http://rdaregistry.info/Elements/u/P60527>
    reg:hasSubproperty <http://rdaregistry.info/Elements/e/P20214> ;
    reg:lexicalAlias <http://rdaregistry.info/Elements/u/dateOfResource.en> ;
    reg:name "dateOfResource"@en ;
    reg:status <http://metadataregistry.org/uri/RegStatus/1001> ;
    a rdf:Property ;
    rdfs:isDefinedBy <http://rdaregistry.info/Elements/u/> ;
    rdfs:label "has date of resource"@en ;
    skos:definition "Relates a resource to the earliest date associated with a resource."@en .

<http://rdaregistry.info/Elements/u/P60528>
    reg:hasSubproperty <http://rdaregistry.info/Elements/m/P30162> ;
    reg:lexicalAlias <http://rdaregistry.info/Elements/u/equipmentOrSystemRequirement.en> ;
    reg:name "equipmentOrSystemRequirement"@en ;
    reg:status <http://metadataregistry.org/uri/RegStatus/1001> ;
    a rdf:Property ;
    rdfs:isDefinedBy <http://rdaregistry.info/Elements/u/> ;
    rdfs:label "has equipment or system requirement"@en ;
    skos:definition "Relates a resource to the equipment or system required for use, playback, etc., of an analog, digital, etc., resource."@en .

<http://rdaregistry.info/Elements/u/P60529>
    reg:hasSubproperty <http://rdaregistry.info/Elements/m/P30163> ;
    reg:lexicalAlias <http://rdaregistry.info/Elements/u/presentationFormat.en> ;
    reg:name "presentationFormat"@en ;
    reg:status <http://metadataregistry.org/uri/RegStatus/1001> ;
    a rdf:Property ;
    rdfs:isDefinedBy <http://rdaregistry.info/Elements/u/> ;
    rdfs:label "has presentation format"@en ;
    rdfs:subPropertyOf <http://rdaregistry.info/Elements/u/P60353> ;
    skos:definition "Relates a resource to the format used in the production of a projected image (e.g., Cinerama, IMAX)."@en .

<http://rdaregistry.info/Elements/u/P60530>
    reg:hasSubproperty <http://rdaregistry.info/Elements/a/P50115> ;
    reg:lexicalAlias <http://rdaregistry.info/Elements/u/fullerFormOfName.en> ;
    reg:name "fullerFormOfName"@en ;
    reg:status <http://metadataregistry.org/uri/RegStatus/1001> ;
    a rdf:Property ;
    rdfs:isDefinedBy <http://rdaregistry.info/Elements/u/> ;
    rdfs:label "has fuller form of name"@en ;
    skos:definition "Relates a resource to the full form of a part of a name represented only by an initial or abbreviation in the form chosen as the preferred name, or a part of the name not included in the form chosen as the preferred name."@en .

<http://rdaregistry.info/Elements/u/P60531>
    reg:hasSubproperty <http://rdaregistry.info/Elements/a/P50116> ;
    reg:lexicalAlias <http://rdaregistry.info/Elements/u/gender.en> ;
    reg:name "gender"@en ;
    reg:status <http://metadataregistry.org/uri/RegStatus/1001> ;
    a rdf:Property ;
    rdfs:isDefinedBy <http://rdaregistry.info/Elements/u/> ;
    rdfs:label "has gender"@en ;
    skos:definition "Relates a resource to the gender with which an agent identifies."@en .

<http://rdaregistry.info/Elements/u/P60532>
    reg:hasSubproperty <http://rdaregistry.info/Elements/m/P30164> ;
    reg:lexicalAlias <http://rdaregistry.info/Elements/u/grooveCharacteristic.en> ;
    reg:name "grooveCharacteristic"@en ;
    reg:status <http://metadataregistry.org/uri/RegStatus/1001> ;
    a rdf:Property ;
    rdfs:isDefinedBy <http://rdaregistry.info/Elements/u/> ;
    rdfs:label "has groove characteristic"@en ;
    rdfs:subPropertyOf <http://rdaregistry.info/Elements/u/P60351> ;
    skos:definition "Relates a resource to the groove width of an analog disc or the groove pitch of an analog cylinder."@en .

<http://rdaregistry.info/Elements/u/P60533>
    reg:hasSubproperty <http://rdaregistry.info/Elements/m/P30165>, <http://rdaregistry.info/Elements/u/P60499>, <http://rdaregistry.info/Elements/u/P60500>, <http://rdaregistry.info/Elements/u/P60501>, <http://rdaregistry.info/Elements/u/P60502>, <http://rdaregistry.info/Elements/u/P60818>, <http://rdaregistry.info/Elements/u/P60819>, <http://rdaregistry.info/Elements/u/P60820>, <http://rdaregistry.info/Elements/u/P60821> ;
    reg:lexicalAlias <http://rdaregistry.info/Elements/u/numberingOfSerials.en> ;
    reg:name "numberingOfSerials"@en ;
    reg:status <http://metadataregistry.org/uri/RegStatus/1001> ;
    a rdf:Property ;
    rdfs:isDefinedBy <http://rdaregistry.info/Elements/u/> ;
    rdfs:label "has numbering of serials"@en ;
    skos:definition "Relates a resource to the identification of each of the issues or parts of a serial."@en .

<http://rdaregistry.info/Elements/u/P60534>
    reg:hasSubproperty <http://rdaregistry.info/Elements/m/P30166> ;
    reg:lexicalAlias <http://rdaregistry.info/Elements/u/issnOfSeries.en> ;
    reg:name "issnOfSeries"@en ;
    reg:status <http://metadataregistry.org/uri/RegStatus/1001> ;
    a rdf:Property ;
    rdfs:isDefinedBy <http://rdaregistry.info/Elements/u/> ;
    rdfs:label "has ISSN of series"@en ;
    skos:definition "Relates a resource to the identifier assigned to a series by an ISSN registration agency."@en .

<http://rdaregistry.info/Elements/u/P60535>
    reg:hasSubproperty <http://rdaregistry.info/Elements/m/P30167> ;
    reg:lexicalAlias <http://rdaregistry.info/Elements/u/issnOfSubseries.en> ;
    reg:name "issnOfSubseries"@en ;
    reg:status <http://metadataregistry.org/uri/RegStatus/1001> ;
    a rdf:Property ;
    rdfs:isDefinedBy <http://rdaregistry.info/Elements/u/> ;
    rdfs:label "has ISSN of subseries"@en ;
    skos:definition "Relates a resource to the identifier assigned to a subseries by an ISSN registration agency."@en .

<http://rdaregistry.info/Elements/u/P60536>
    reg:lexicalAlias <http://rdaregistry.info/Elements/u/mediumOfPerformance.en> ;
    reg:name "mediumOfPerformance"@en ;
    reg:status <http://metadataregistry.org/uri/RegStatus/1001> ;
    a rdf:Property ;
    rdfs:isDefinedBy <http://rdaregistry.info/Elements/u/> ;
    rdfs:label "has medium of performance"@en ;
    skos:definition "Relates a resource to the instrument, instruments, voice, voices, etc., for which a musical resource was originally conceived."@en .

<http://rdaregistry.info/Elements/u/P60537>
    reg:hasSubproperty <http://rdaregistry.info/Elements/e/P20215> ;
    reg:lexicalAlias <http://rdaregistry.info/Elements/u/mediumOfPerformanceOfMusicalContent.en> ;
    reg:name "mediumOfPerformanceOfMusicalContent"@en ;
    reg:status <http://metadataregistry.org/uri/RegStatus/1001> ;
    a rdf:Property ;
    rdfs:isDefinedBy <http://rdaregistry.info/Elements/u/> ;
    rdfs:label "has medium of performance of musical content"@en ;
    skos:definition "Relates a resource to the instrument, instruments, voice, voices, etc., used (or intended to be used) for performance of musical content."@en .

<http://rdaregistry.info/Elements/u/P60538>
    reg:hasSubproperty <http://rdaregistry.info/Elements/m/P30168> ;
    reg:lexicalAlias <http://rdaregistry.info/Elements/u/frequency.en> ;
    reg:name "frequency"@en ;
    reg:status <http://metadataregistry.org/uri/RegStatus/1001> ;
    a rdf:Property ;
    rdfs:isDefinedBy <http://rdaregistry.info/Elements/u/> ;
    rdfs:label "has frequency"@en ;
    skos:definition "Relates a resource to the intervals at which the issues or parts of a serial or the updates to an integrating resource are issued."@en .

<http://rdaregistry.info/Elements/u/P60539>
    reg:hasSubproperty <http://rdaregistry.info/Elements/m/P30169>, <http://rdaregistry.info/Elements/u/P60540>, <http://rdaregistry.info/Elements/u/P60541> ;
    reg:lexicalAlias <http://rdaregistry.info/Elements/u/dimensions.en> ;
    reg:name "dimensions"@en ;
    reg:status <http://metadataregistry.org/uri/RegStatus/1001> ;
    a rdf:Property ;
    rdfs:isDefinedBy <http://rdaregistry.info/Elements/u/> ;
    rdfs:label "has dimensions"@en ;
    skos:definition "Relates a resource to the measurements of the carrier or carriers and/or the container of a resource."@en .

<http://rdaregistry.info/Elements/u/P60540>
    reg:hasSubproperty <http://rdaregistry.info/Elements/m/P30170> ;
    reg:lexicalAlias <http://rdaregistry.info/Elements/u/dimensionsOfMapEtc.en> ;
    reg:name "dimensionsOfMapEtc"@en ;
    reg:status <http://metadataregistry.org/uri/RegStatus/1001> ;
    a rdf:Property ;
    rdfs:isDefinedBy <http://rdaregistry.info/Elements/u/> ;
    rdfs:label "has dimensions of map, etc."@en ;
    rdfs:subPropertyOf <http://rdaregistry.info/Elements/u/P60539> ;
    skos:definition "Relates a resource to the measurements of the face of a map, etc."@en .

<http://rdaregistry.info/Elements/u/P60541>
    reg:hasSubproperty <http://rdaregistry.info/Elements/m/P30171> ;
    reg:lexicalAlias <http://rdaregistry.info/Elements/u/dimensionsOfStillImage.en> ;
    reg:name "dimensionsOfStillImage"@en ;
    reg:status <http://metadataregistry.org/uri/RegStatus/1001> ;
    a rdf:Property ;
    rdfs:isDefinedBy <http://rdaregistry.info/Elements/u/> ;
    rdfs:label "has dimensions of still image"@en ;
    rdfs:subPropertyOf <http://rdaregistry.info/Elements/u/P60539> ;
    skos:definition "Relates a resource to the measurements of the pictorial area of a still image."@en .

<http://rdaregistry.info/Elements/u/P60542>
    reg:hasSubproperty <http://rdaregistry.info/Elements/e/P20216> ;
    reg:lexicalAlias <http://rdaregistry.info/Elements/u/projectionOfCartographicContent.en> ;
    reg:name "projectionOfCartographicContent"@en ;
    reg:status <http://metadataregistry.org/uri/RegStatus/1001> ;
    a rdf:Property ;
    rdfs:isDefinedBy <http://rdaregistry.info/Elements/u/> ;
    rdfs:label "has projection of cartographic content"@en ;
    skos:definition "Relates a resource to the method or system used to represent the surface of the earth or of a celestial sphere on a plane."@en .

<http://rdaregistry.info/Elements/u/P60543>
    reg:hasSubproperty <http://rdaregistry.info/Elements/m/P30172> ;
    reg:lexicalAlias <http://rdaregistry.info/Elements/u/typeOfRecording.en> ;
    reg:name "typeOfRecording"@en ;
    reg:status <http://metadataregistry.org/uri/RegStatus/1001> ;
    a rdf:Property ;
    rdfs:isDefinedBy <http://rdaregistry.info/Elements/u/> ;
    rdfs:label "has type of recording"@en ;
    rdfs:subPropertyOf <http://rdaregistry.info/Elements/u/P60351> ;
    skos:definition "Relates a resource to the method used to encode audio content for playback (e.g., analog or digital)."@en .

<http://rdaregistry.info/Elements/u/P60544>
    reg:hasSubproperty <http://rdaregistry.info/Elements/m/P30173> ;
    reg:lexicalAlias <http://rdaregistry.info/Elements/u/distributorsName.en> ;
    reg:name "distributorsName"@en ;
    reg:status <http://metadataregistry.org/uri/RegStatus/1001> ;
    a rdf:Property ;
    rdfs:isDefinedBy <http://rdaregistry.info/Elements/u/> ;
    rdfs:label "has distributor’s name"@en ;
    skos:definition "Relates a resource to the name of an agent responsible for distributing a resource in a published form."@en .

<http://rdaregistry.info/Elements/u/P60545>
    reg:hasSubproperty <http://rdaregistry.info/Elements/m/P30174> ;
    reg:lexicalAlias <http://rdaregistry.info/Elements/u/producersName.en> ;
    reg:name "producersName"@en ;
    reg:status <http://metadataregistry.org/uri/RegStatus/1001> ;
    a rdf:Property ;
    rdfs:isDefinedBy <http://rdaregistry.info/Elements/u/> ;
    rdfs:label "has producer’s name"@en ;
    skos:definition "Relates a resource to the name of an agent responsible for inscribing, fabricating, constructing, etc., a resource in an unpublished form."@en .

<http://rdaregistry.info/Elements/u/P60546>
    reg:hasSubproperty <http://rdaregistry.info/Elements/m/P30175> ;
    reg:lexicalAlias <http://rdaregistry.info/Elements/u/manufacturersName.en> ;
    reg:name "manufacturersName"@en ;
    reg:status <http://metadataregistry.org/uri/RegStatus/1001> ;
    a rdf:Property ;
    rdfs:isDefinedBy <http://rdaregistry.info/Elements/u/> ;
    rdfs:label "has manufacturer’s name"@en ;
    skos:definition "Relates a resource to the name of an agent responsible for printing, duplicating, casting, etc., a resource in a published form."@en .

<http://rdaregistry.info/Elements/u/P60547>
    reg:hasSubproperty <http://rdaregistry.info/Elements/m/P30176> ;
    reg:lexicalAlias <http://rdaregistry.info/Elements/u/publishersName.en> ;
    reg:name "publishersName"@en ;
    reg:status <http://metadataregistry.org/uri/RegStatus/1001> ;
    a rdf:Property ;
    rdfs:isDefinedBy <http://rdaregistry.info/Elements/u/> ;
    rdfs:label "has publisher’s name"@en ;
    skos:definition "Relates a resource to the name of an agent responsible for publishing, releasing, or issuing a resource."@en .

<http://rdaregistry.info/Elements/u/P60548>
    reg:lexicalAlias <http://rdaregistry.info/Elements/u/preferredNameForThePlace.en> ;
    reg:name "preferredNameForThePlace"@en ;
    reg:status <http://metadataregistry.org/uri/RegStatus/1001> ;
    a rdf:Property ;
    rdfs:isDefinedBy <http://rdaregistry.info/Elements/u/> ;
    rdfs:label "has preferred name for the place"@en ;
    rdfs:subPropertyOf <http://rdaregistry.info/Elements/u/P60366> ;
    skos:definition "Relates a resource to the name or form of name chosen to identify a place."@en .

<http://rdaregistry.info/Elements/u/P60549>
    reg:hasSubproperty <http://rdaregistry.info/Elements/a/P50041>, <http://rdaregistry.info/Elements/a/P50065>, <http://rdaregistry.info/Elements/a/P50117> ;
    reg:lexicalAlias <http://rdaregistry.info/Elements/u/preferredNameForTheAgent.en> ;
    reg:name "preferredNameForTheAgent"@en ;
    reg:status <http://metadataregistry.org/uri/RegStatus/1001> ;
    a rdf:Property ;
    rdfs:isDefinedBy <http://rdaregistry.info/Elements/u/> ;
    rdfs:label "has preferred name for the agent"@en ;
    rdfs:subPropertyOf <http://rdaregistry.info/Elements/u/P60368> ;
    skos:definition "Relates a resource to the name or form of name chosen to identify the agent. it is also the basis for the authorized access point representing that body."@en .

<http://rdaregistry.info/Elements/u/P60550>
    reg:hasSubproperty <http://rdaregistry.info/Elements/m/P30177>, <http://rdaregistry.info/Elements/m/P30178>, <http://rdaregistry.info/Elements/m/P30179>, <http://rdaregistry.info/Elements/m/P30180>, <http://rdaregistry.info/Elements/m/P30181>, <http://rdaregistry.info/Elements/m/P30182> ;
    reg:lexicalAlias <http://rdaregistry.info/Elements/u/extent.en> ;
    reg:name "extent"@en ;
    reg:status <http://metadataregistry.org/uri/RegStatus/1001> ;
    a rdf:Property ;
    rdfs:isDefinedBy <http://rdaregistry.info/Elements/u/> ;
    rdfs:label "has extent"@en ;
    skos:definition "Relates a resource to the number and type of units and/or subunits making up a resource."@en .

<http://rdaregistry.info/Elements/u/P60551>
    reg:hasSubproperty <http://rdaregistry.info/Elements/m/P30183> ;
    reg:lexicalAlias <http://rdaregistry.info/Elements/u/fileSize.en> ;
    reg:name "fileSize"@en ;
    reg:status <http://metadataregistry.org/uri/RegStatus/1001> ;
    a rdf:Property ;
    rdfs:isDefinedBy <http://rdaregistry.info/Elements/u/> ;
    rdfs:label "has file size"@en ;
    rdfs:subPropertyOf <http://rdaregistry.info/Elements/u/P60350> ;
    skos:definition "Relates a resource to the number of bytes in a digital file."@en .

<http://rdaregistry.info/Elements/u/P60552>
    reg:hasSubproperty <http://rdaregistry.info/Elements/m/P30184> ;
    reg:lexicalAlias <http://rdaregistry.info/Elements/u/configurationOfPlaybackChannels.en> ;
    reg:name "configurationOfPlaybackChannels"@en ;
    reg:status <http://metadataregistry.org/uri/RegStatus/1001> ;
    a rdf:Property ;
    rdfs:isDefinedBy <http://rdaregistry.info/Elements/u/> ;
    rdfs:label "has configuration of playback channels"@en ;
    rdfs:subPropertyOf <http://rdaregistry.info/Elements/u/P60351> ;
    skos:definition "Relates a resource to the number of sound channels used to make a recording (e.g., one channel for a monophonic recording, two channels for a stereophonic recording)."@en .

<http://rdaregistry.info/Elements/u/P60553>
    reg:hasSubproperty <http://rdaregistry.info/Elements/m/P30185> ;
    reg:lexicalAlias <http://rdaregistry.info/Elements/u/tapeConfiguration.en> ;
    reg:name "tapeConfiguration"@en ;
    reg:status <http://metadataregistry.org/uri/RegStatus/1001> ;
    a rdf:Property ;
    rdfs:isDefinedBy <http://rdaregistry.info/Elements/u/> ;
    rdfs:label "has tape configuration"@en ;
    rdfs:subPropertyOf <http://rdaregistry.info/Elements/u/P60351> ;
    skos:definition "Relates a resource to the number of tracks on an audiotape."@en .

<http://rdaregistry.info/Elements/u/P60554>
    reg:hasSubproperty <http://rdaregistry.info/Elements/m/P30186> ;
    reg:lexicalAlias <http://rdaregistry.info/Elements/u/mount.en> ;
    reg:name "mount"@en ;
    reg:status <http://metadataregistry.org/uri/RegStatus/1001> ;
    a rdf:Property ;
    rdfs:isDefinedBy <http://rdaregistry.info/Elements/u/> ;
    rdfs:label "has mount"@en ;
    skos:definition "Relates a resource to the physical material used for the support or backing to which the base material of a resource has been attached."@en .

<http://rdaregistry.info/Elements/u/P60555>
    reg:hasSubproperty <http://rdaregistry.info/Elements/e/P20217> ;
    reg:lexicalAlias <http://rdaregistry.info/Elements/u/placeAndDateOfCapture.en> ;
    reg:name "placeAndDateOfCapture"@en ;
    reg:status <http://metadataregistry.org/uri/RegStatus/1001> ;
    a rdf:Property ;
    rdfs:isDefinedBy <http://rdaregistry.info/Elements/u/> ;
    rdfs:label "has place and date of capture"@en ;
    skos:definition "Relates a resource to the place and date associated with the capture (i.e., recording, filming, etc.) of the content of a resource."@en .

<http://rdaregistry.info/Elements/u/P60556>
    reg:hasSubproperty <http://rdaregistry.info/Elements/e/P20218> ;
    reg:lexicalAlias <http://rdaregistry.info/Elements/u/placeOfCapture.en> ;
    reg:name "placeOfCapture"@en ;
    reg:status <http://metadataregistry.org/uri/RegStatus/1001> ;
    a rdf:Property ;
    rdfs:isDefinedBy <http://rdaregistry.info/Elements/u/> ;
    rdfs:label "has place of capture"@en ;
    skos:definition "Relates a resource to the place associated with the capture (i.e., recording, filming, etc.) of the content of a resource."@en .

<http://rdaregistry.info/Elements/u/P60557>
    reg:hasSubproperty <http://rdaregistry.info/Elements/e/P20219> ;
    reg:lexicalAlias <http://rdaregistry.info/Elements/u/duration.en> ;
    reg:name "duration"@en ;
    reg:status <http://metadataregistry.org/uri/RegStatus/1001> ;
    a rdf:Property ;
    rdfs:isDefinedBy <http://rdaregistry.info/Elements/u/> ;
    rdfs:label "has duration"@en ;
    skos:definition "Relates a resource to the playing time, running time, etc., of the content of a resource."@en .

<http://rdaregistry.info/Elements/u/P60558>
    reg:hasSubproperty <http://rdaregistry.info/Elements/e/P20224> ;
    reg:lexicalAlias <http://rdaregistry.info/Elements/u/colourContent.en> ;
    reg:name "colourContent"@en ;
    reg:status <http://metadataregistry.org/uri/RegStatus/1001> ;
    a rdf:Property ;
    rdfs:isDefinedBy <http://rdaregistry.info/Elements/u/> ;
    rdfs:label "has colour content"@en ;
    skos:altLabel "has color content"@en ;
    skos:definition "Relates a resource to the presence of colour, tone, etc., in the content of a resource. colour content is also the specific colours, tones, etc., (including black and white) present in the content of a resource."@en .

<http://rdaregistry.info/Elements/u/P60559>
    reg:hasSubproperty <http://rdaregistry.info/Elements/e/P20225> ;
    reg:lexicalAlias <http://rdaregistry.info/Elements/u/soundContent.en> ;
    reg:name "soundContent"@en ;
    reg:status <http://metadataregistry.org/uri/RegStatus/1001> ;
    a rdf:Property ;
    rdfs:isDefinedBy <http://rdaregistry.info/Elements/u/> ;
    rdfs:label "has sound content"@en ;
    skos:definition "Relates a resource to the presence of sound in a resource other than one that consists primarily of recorded sound."@en .

<http://rdaregistry.info/Elements/u/P60560>
    reg:hasSubproperty <http://rdaregistry.info/Elements/m/P30187>, <http://rdaregistry.info/Elements/u/P60561>, <http://rdaregistry.info/Elements/u/P60562> ;
    reg:lexicalAlias <http://rdaregistry.info/Elements/u/productionMethod.en> ;
    reg:name "productionMethod"@en ;
    reg:status <http://metadataregistry.org/uri/RegStatus/1001> ;
    a rdf:Property ;
    rdfs:isDefinedBy <http://rdaregistry.info/Elements/u/> ;
    rdfs:label "has production method"@en ;
    skos:definition "Relates a resource to the process used to produce a resource."@en .

<http://rdaregistry.info/Elements/u/P60561>
    reg:hasSubproperty <http://rdaregistry.info/Elements/m/P30188> ;
    reg:lexicalAlias <http://rdaregistry.info/Elements/u/productionMethodForTactileResource.en> ;
    reg:name "productionMethodForTactileResource"@en ;
    reg:status <http://metadataregistry.org/uri/RegStatus/1001> ;
    a rdf:Property ;
    rdfs:isDefinedBy <http://rdaregistry.info/Elements/u/> ;
    rdfs:label "has production method for tactile resource"@en ;
    rdfs:subPropertyOf <http://rdaregistry.info/Elements/u/P60560> ;
    skos:definition "Relates a resource to the process used to produce a tactile resource (e.g., embossing, thermoform)."@en .

<http://rdaregistry.info/Elements/u/P60562>
    reg:hasSubproperty <http://rdaregistry.info/Elements/m/P30189> ;
    reg:lexicalAlias <http://rdaregistry.info/Elements/u/productionMethodForManuscript.en> ;
    reg:name "productionMethodForManuscript"@en ;
    reg:status <http://metadataregistry.org/uri/RegStatus/1001> ;
    a rdf:Property ;
    rdfs:isDefinedBy <http://rdaregistry.info/Elements/u/> ;
    rdfs:label "has production method for manuscript"@en ;
    rdfs:subPropertyOf <http://rdaregistry.info/Elements/u/P60560> ;
    skos:definition "Relates a resource to the process used to produce an original manuscript or a copy."@en .

<http://rdaregistry.info/Elements/u/P60563>
    reg:hasSubproperty <http://rdaregistry.info/Elements/e/P20226> ;
    reg:lexicalAlias <http://rdaregistry.info/Elements/u/horizontalScaleOfCartographicContent.en> ;
    reg:name "horizontalScaleOfCartographicContent"@en ;
    reg:status <http://metadataregistry.org/uri/RegStatus/1001> ;
    a rdf:Property ;
    rdfs:isDefinedBy <http://rdaregistry.info/Elements/u/> ;
    rdfs:label "has horizontal scale of cartographic content"@en ;
    rdfs:subPropertyOf <http://rdaregistry.info/Elements/u/P60565> ;
    skos:definition "Relates a resource to the ratio of horizontal distances in the cartographic content of a resource to the actual distances they represent."@en .

<http://rdaregistry.info/Elements/u/P60564>
    reg:hasSubproperty <http://rdaregistry.info/Elements/e/P20227> ;
    reg:lexicalAlias <http://rdaregistry.info/Elements/u/scaleOfStillImageOrThreeDimensionalForm.en> ;
    reg:name "scaleOfStillImageOrThreeDimensionalForm"@en ;
    reg:status <http://metadataregistry.org/uri/RegStatus/1001> ;
    a rdf:Property ;
    rdfs:isDefinedBy <http://rdaregistry.info/Elements/u/> ;
    rdfs:label "has scale of still image or three-dimensional form"@en ;
    rdfs:subPropertyOf <http://rdaregistry.info/Elements/u/P60565> ;
    skos:definition "Relates a resource to the ratio of the dimensions of a still image or three-dimensional form contained or embodied in a resource to the dimensions of the entity it represents."@en .

<http://rdaregistry.info/Elements/u/P60565>
    reg:hasSubproperty <http://rdaregistry.info/Elements/e/P20228>, <http://rdaregistry.info/Elements/u/P60510>, <http://rdaregistry.info/Elements/u/P60563>, <http://rdaregistry.info/Elements/u/P60564>, <http://rdaregistry.info/Elements/u/P60579> ;
    reg:lexicalAlias <http://rdaregistry.info/Elements/u/scale.en> ;
    reg:name "scale"@en ;
    reg:status <http://metadataregistry.org/uri/RegStatus/1001> ;
    a rdf:Property ;
    rdfs:isDefinedBy <http://rdaregistry.info/Elements/u/> ;
    rdfs:label "has scale"@en ;
    skos:definition "Relates a resource to the ratio of the dimensions of an image or three-dimensional form contained or embodied in a resource to the dimensions of the entity it represents."@en .

<http://rdaregistry.info/Elements/u/P60566>
    reg:hasSubproperty <http://rdaregistry.info/Elements/e/P20229> ;
    reg:lexicalAlias <http://rdaregistry.info/Elements/u/aspectRatio.en> ;
    reg:name "aspectRatio"@en ;
    reg:status <http://metadataregistry.org/uri/RegStatus/1001> ;
    a rdf:Property ;
    rdfs:isDefinedBy <http://rdaregistry.info/Elements/u/> ;
    rdfs:label "has aspect ratio"@en ;
    skos:definition "Relates a resource to the ratio of the width to the height of a moving image."@en .

<http://rdaregistry.info/Elements/u/P60567>
    reg:hasSubproperty <http://rdaregistry.info/Elements/m/P30190> ;
    reg:lexicalAlias <http://rdaregistry.info/Elements/u/generationOfAudioRecording.en> ;
    reg:name "generationOfAudioRecording"@en ;
    reg:status <http://metadataregistry.org/uri/RegStatus/1001> ;
    a rdf:Property ;
    rdfs:isDefinedBy <http://rdaregistry.info/Elements/u/> ;
    rdfs:label "has generation of audio recording"@en ;
    rdfs:subPropertyOf <http://rdaregistry.info/Elements/u/P60568> ;
    skos:definition "Relates a resource to the relationship between an original audio carrier and the carrier of a reproduction made from the original (e.g., a tape duplication master, a test pressing)."@en .

<http://rdaregistry.info/Elements/u/P60568>
    reg:hasSubproperty <http://rdaregistry.info/Elements/m/P30191>, <http://rdaregistry.info/Elements/u/P60567>, <http://rdaregistry.info/Elements/u/P60569>, <http://rdaregistry.info/Elements/u/P60570>, <http://rdaregistry.info/Elements/u/P60571>, <http://rdaregistry.info/Elements/u/P60572> ;
    reg:lexicalAlias <http://rdaregistry.info/Elements/u/generation.en> ;
    reg:name "generation"@en ;
    reg:status <http://metadataregistry.org/uri/RegStatus/1001> ;
    a rdf:Property ;
    rdfs:isDefinedBy <http://rdaregistry.info/Elements/u/> ;
    rdfs:label "has generation"@en ;
    skos:definition "Relates a resource to the relationship between an original carrier and the carrier of a reproduction made from the original (e.g., a first generation camera master, a second generation printing master)."@en .

<http://rdaregistry.info/Elements/u/P60569>
    reg:hasSubproperty <http://rdaregistry.info/Elements/m/P30192> ;
    reg:lexicalAlias <http://rdaregistry.info/Elements/u/generationOfDigitalResource.en> ;
    reg:name "generationOfDigitalResource"@en ;
    reg:status <http://metadataregistry.org/uri/RegStatus/1001> ;
    a rdf:Property ;
    rdfs:isDefinedBy <http://rdaregistry.info/Elements/u/> ;
    rdfs:label "has generation of digital resource"@en ;
    rdfs:subPropertyOf <http://rdaregistry.info/Elements/u/P60568> ;
    skos:definition "Relates a resource to the relationship between an original carrier of a digital resource and the carrier of a reproduction made from the original (e.g., a derivative master)."@en .

<http://rdaregistry.info/Elements/u/P60570>
    reg:hasSubproperty <http://rdaregistry.info/Elements/m/P30193> ;
    reg:lexicalAlias <http://rdaregistry.info/Elements/u/generationOfMotionPictureFilm.en> ;
    reg:name "generationOfMotionPictureFilm"@en ;
    reg:status <http://metadataregistry.org/uri/RegStatus/1001> ;
    a rdf:Property ;
    rdfs:isDefinedBy <http://rdaregistry.info/Elements/u/> ;
    rdfs:label "has generation of motion picture film"@en ;
    rdfs:subPropertyOf <http://rdaregistry.info/Elements/u/P60568> ;
    skos:definition "Relates a resource to the relationship between an original carrier of a motion picture film resource and the carrier of a reproduction made from the original (e.g., a reference print)."@en .

<http://rdaregistry.info/Elements/u/P60571>
    reg:hasSubproperty <http://rdaregistry.info/Elements/m/P30194> ;
    reg:lexicalAlias <http://rdaregistry.info/Elements/u/generationOfVideotape.en> ;
    reg:name "generationOfVideotape"@en ;
    reg:status <http://metadataregistry.org/uri/RegStatus/1001> ;
    a rdf:Property ;
    rdfs:isDefinedBy <http://rdaregistry.info/Elements/u/> ;
    rdfs:label "has generation of videotape"@en ;
    rdfs:subPropertyOf <http://rdaregistry.info/Elements/u/P60568> ;
    skos:definition "Relates a resource to the relationship between an original carrier of a videotape resource and the carrier of a reproduction made from the original (e.g., a show copy)."@en .

<http://rdaregistry.info/Elements/u/P60572>
    reg:hasSubproperty <http://rdaregistry.info/Elements/m/P30195> ;
    reg:lexicalAlias <http://rdaregistry.info/Elements/u/generationOfMicroform.en> ;
    reg:name "generationOfMicroform"@en ;
    reg:status <http://metadataregistry.org/uri/RegStatus/1001> ;
    a rdf:Property ;
    rdfs:isDefinedBy <http://rdaregistry.info/Elements/u/> ;
    rdfs:label "has generation of microform"@en ;
    rdfs:subPropertyOf <http://rdaregistry.info/Elements/u/P60568> ;
    skos:definition "Relates a resource to the relationship between an original microform carrier and the carrier of a reproduction made from the original (e.g., a printing master)."@en .

<http://rdaregistry.info/Elements/u/P60573>
    reg:hasSubproperty <http://rdaregistry.info/Elements/m/P30196> ;
    reg:lexicalAlias <http://rdaregistry.info/Elements/u/polarity.en> ;
    reg:name "polarity"@en ;
    reg:status <http://metadataregistry.org/uri/RegStatus/1001> ;
    a rdf:Property ;
    rdfs:isDefinedBy <http://rdaregistry.info/Elements/u/> ;
    rdfs:label "has polarity"@en ;
    skos:definition "Relates a resource to the relationship of the colours and tones in an image to the colours and tones of the object reproduced (e.g., positive, negative)."@en .

<http://rdaregistry.info/Elements/u/P60574>
    reg:hasSubproperty <http://rdaregistry.info/Elements/e/P20137> ;
    reg:lexicalAlias <http://rdaregistry.info/Elements/u/absorptionOf.en> ;
    reg:name "absorptionOf"@en ;
    reg:status <http://metadataregistry.org/uri/RegStatus/1001> ;
    a rdf:Property ;
    rdfs:isDefinedBy <http://rdaregistry.info/Elements/u/> ;
    rdfs:label "is absorption of"@en ;
    rdfs:subPropertyOf <http://rdaregistry.info/Elements/u/P60261> ;
    owl:inverseOf <http://rdaregistry.info/Elements/u/P60247> ;
    skos:definition "Relates a resource to the resource that has been incorporated into another resource."@en .

<http://rdaregistry.info/Elements/u/P60575>
    reg:hasSubproperty <http://rdaregistry.info/Elements/e/P20138> ;
    reg:lexicalAlias <http://rdaregistry.info/Elements/u/absorptionInPartOf.en> ;
    reg:name "absorptionInPartOf"@en ;
    reg:status <http://metadataregistry.org/uri/RegStatus/1001> ;
    a rdf:Property ;
    rdfs:isDefinedBy <http://rdaregistry.info/Elements/u/> ;
    rdfs:label "is absorption in part of"@en ;
    rdfs:subPropertyOf <http://rdaregistry.info/Elements/u/P60261> ;
    owl:inverseOf <http://rdaregistry.info/Elements/u/P60248> ;
    skos:definition "Relates a resource to the resource that has been partially incorporated into another resource."@en .

<http://rdaregistry.info/Elements/u/P60576>
    reg:hasSubproperty <http://rdaregistry.info/Elements/e/P20149> ;
    reg:lexicalAlias <http://rdaregistry.info/Elements/u/continuationOf.en> ;
    reg:name "continuationOf"@en ;
    reg:status <http://metadataregistry.org/uri/RegStatus/1001> ;
    a rdf:Property ;
    rdfs:isDefinedBy <http://rdaregistry.info/Elements/u/> ;
    rdfs:label "is continuation of"@en ;
    rdfs:subPropertyOf <http://rdaregistry.info/Elements/u/P60261> ;
    owl:inverseOf <http://rdaregistry.info/Elements/u/P60306> ;
    skos:definition "Relates a resource to the resource that is continued by the content of a later resource under a new title."@en .

<http://rdaregistry.info/Elements/u/P60577>
    reg:lexicalAlias <http://rdaregistry.info/Elements/u/sequelTo.en> ;
    reg:name "sequelTo"@en ;
    reg:status <http://metadataregistry.org/uri/RegStatus/1001> ;
    a rdf:Property ;
    rdfs:isDefinedBy <http://rdaregistry.info/Elements/u/> ;
    rdfs:label "is sequel to"@en ;
    rdfs:subPropertyOf <http://rdaregistry.info/Elements/u/P60261> ;
    owl:inverseOf <http://rdaregistry.info/Elements/u/P60102> ;
    skos:definition "Relates a resource to the resource whose narrative is continued by the later resource."@en .

<http://rdaregistry.info/Elements/u/P60578>
    reg:hasSubproperty <http://rdaregistry.info/Elements/m/P30197> ;
    reg:lexicalAlias <http://rdaregistry.info/Elements/u/bookFormat.en> ;
    reg:name "bookFormat"@en ;
    reg:status <http://metadataregistry.org/uri/RegStatus/1001> ;
    a rdf:Property ;
    rdfs:isDefinedBy <http://rdaregistry.info/Elements/u/> ;
    rdfs:label "has book format"@en ;
    skos:definition "Relates a resource to the result of folding a printed sheet to form a gathering of leaves (e.g., a sheet folded once to form a folio, twice to form a quarto, three times to form an octavo, etc.)."@en .

<http://rdaregistry.info/Elements/u/P60579>
    reg:hasSubproperty <http://rdaregistry.info/Elements/e/P20230> ;
    reg:lexicalAlias <http://rdaregistry.info/Elements/u/verticalScaleOfCartographicContent.en> ;
    reg:name "verticalScaleOfCartographicContent"@en ;
    reg:status <http://metadataregistry.org/uri/RegStatus/1001> ;
    a rdf:Property ;
    rdfs:isDefinedBy <http://rdaregistry.info/Elements/u/> ;
    rdfs:label "has vertical scale of cartographic content"@en ;
    rdfs:subPropertyOf <http://rdaregistry.info/Elements/u/P60565> ;
    skos:definition "Relates a resource to the scale of elevation or vertical dimension of the cartographic content of a resource."@en .

<http://rdaregistry.info/Elements/u/P60580>
    reg:lexicalAlias <http://rdaregistry.info/Elements/u/key.en> ;
    reg:name "key"@en ;
    reg:status <http://metadataregistry.org/uri/RegStatus/1001> ;
    a rdf:Property ;
    rdfs:isDefinedBy <http://rdaregistry.info/Elements/u/> ;
    rdfs:label "has key"@en ;
    skos:definition "Relates a resource to the set of pitch relationships that establishes the tonal centre, or principal tonal centre, of a musical resource."@en .

<http://rdaregistry.info/Elements/u/P60581>
    reg:hasSubproperty <http://rdaregistry.info/Elements/m/P30198> ;
    reg:lexicalAlias <http://rdaregistry.info/Elements/u/reductionRatio.en> ;
    reg:name "reductionRatio"@en ;
    reg:status <http://metadataregistry.org/uri/RegStatus/1001> ;
    a rdf:Property ;
    rdfs:isDefinedBy <http://rdaregistry.info/Elements/u/> ;
    rdfs:label "has reduction ratio"@en ;
    skos:definition "Relates a resource to the size of a micro-image in relation to the original from which it was produced."@en .

<http://rdaregistry.info/Elements/u/P60582>
    reg:hasSubproperty <http://rdaregistry.info/Elements/m/P30199> ;
    reg:lexicalAlias <http://rdaregistry.info/Elements/u/fontSize.en> ;
    reg:name "fontSize"@en ;
    reg:status <http://metadataregistry.org/uri/RegStatus/1001> ;
    a rdf:Property ;
    rdfs:isDefinedBy <http://rdaregistry.info/Elements/u/> ;
    rdfs:label "has font size"@en ;
    skos:definition "Relates a resource to the size of the type used to represent the characters and symbols in a resource."@en .

<http://rdaregistry.info/Elements/u/P60583>
    reg:hasSubproperty <http://rdaregistry.info/Elements/i/P40050> ;
    reg:lexicalAlias <http://rdaregistry.info/Elements/u/immediateSourceOfAcquisitionOfItem.en> ;
    reg:name "immediateSourceOfAcquisitionOfItem"@en ;
    reg:status <http://metadataregistry.org/uri/RegStatus/1001> ;
    a rdf:Property ;
    rdfs:isDefinedBy <http://rdaregistry.info/Elements/u/> ;
    rdfs:label "has immediate source of acquisition of resource"@en ;
    skos:definition "Relates a resource to the source from which the agency directly acquired a resource and the circumstances under which it was received."@en .

<http://rdaregistry.info/Elements/u/P60584>
    reg:lexicalAlias <http://rdaregistry.info/Elements/u/natureOfTheContent.en> ;
    reg:name "natureOfTheContent"@en ;
    reg:status <http://metadataregistry.org/uri/RegStatus/1001> ;
    a rdf:Property ;
    rdfs:isDefinedBy <http://rdaregistry.info/Elements/u/> ;
    rdfs:label "has nature of the content"@en ;
    skos:definition "Relates a resource to the specific character of the primary content of a resource (e.g., legal articles, interim report)."@en .

<http://rdaregistry.info/Elements/u/P60585>
    reg:hasSubproperty <http://rdaregistry.info/Elements/m/P30200> ;
    reg:lexicalAlias <http://rdaregistry.info/Elements/u/projectionSpeed.en> ;
    reg:name "projectionSpeed"@en ;
    reg:status <http://metadataregistry.org/uri/RegStatus/1001> ;
    a rdf:Property ;
    rdfs:isDefinedBy <http://rdaregistry.info/Elements/u/> ;
    rdfs:label "has projection speed"@en ;
    rdfs:subPropertyOf <http://rdaregistry.info/Elements/u/P60353> ;
    skos:definition "Relates a resource to the speed at which a projected carrier must be operated to produce the moving image intended."@en .

<http://rdaregistry.info/Elements/u/P60586>
    reg:hasSubproperty <http://rdaregistry.info/Elements/m/P30201> ;
    reg:lexicalAlias <http://rdaregistry.info/Elements/u/playingSpeed.en> ;
    reg:name "playingSpeed"@en ;
    reg:status <http://metadataregistry.org/uri/RegStatus/1001> ;
    a rdf:Property ;
    rdfs:isDefinedBy <http://rdaregistry.info/Elements/u/> ;
    rdfs:label "has playing speed"@en ;
    rdfs:subPropertyOf <http://rdaregistry.info/Elements/u/P60351> ;
    skos:definition "Relates a resource to the speed at which an audio carrier must be operated to produce the sound intended."@en .

<http://rdaregistry.info/Elements/u/P60587>
    reg:hasSubproperty <http://rdaregistry.info/Elements/m/P30202> ;
    reg:lexicalAlias <http://rdaregistry.info/Elements/u/encodedBitrate.en> ;
    reg:name "encodedBitrate"@en ;
    reg:status <http://metadataregistry.org/uri/RegStatus/1001> ;
    a rdf:Property ;
    rdfs:isDefinedBy <http://rdaregistry.info/Elements/u/> ;
    rdfs:label "has encoded bitrate"@en ;
    rdfs:subPropertyOf <http://rdaregistry.info/Elements/u/P60350> ;
    owl:inverseOf <http://rdaregistry.info/Elements/u/P60858> ;
    skos:definition "Relates a resource to the speed at which streaming audio, video, etc., is designed to play."@en .

<http://rdaregistry.info/Elements/u/P60588>
    reg:lexicalAlias <http://rdaregistry.info/Elements/u/preferredTitleForTheResource.en> ;
    reg:name "preferredTitleForTheResource"@en ;
    reg:status <http://metadataregistry.org/uri/RegStatus/1001> ;
    a rdf:Property ;
    rdfs:isDefinedBy <http://rdaregistry.info/Elements/u/> ;
    rdfs:label "has preferred title for the resource"@en ;
    rdfs:subPropertyOf <http://rdaregistry.info/Elements/u/P60367> ;
    owl:inverseOf <http://rdaregistry.info/Elements/u/P60857> ;
    skos:definition "Relates a resource to the title or form of title chosen to identify the resource."@en .

<http://rdaregistry.info/Elements/u/P60589>
    reg:hasSubproperty <http://rdaregistry.info/Elements/m/P30203> ;
    reg:lexicalAlias <http://rdaregistry.info/Elements/u/parallelTitleProper.en> ;
    reg:name "parallelTitleProper"@en ;
    reg:status <http://metadataregistry.org/uri/RegStatus/1001> ;
    a rdf:Property ;
    rdfs:isDefinedBy <http://rdaregistry.info/Elements/u/> ;
    rdfs:label "has parallel title proper"@en ;
    rdfs:subPropertyOf <http://rdaregistry.info/Elements/u/P60369> ;
    skos:definition "Relates a resource to the title proper in another language and/or script."@en .

<http://rdaregistry.info/Elements/u/P60590>
    reg:hasSubproperty <http://rdaregistry.info/Elements/m/P30204> ;
    reg:lexicalAlias <http://rdaregistry.info/Elements/u/parallelTitleProperOfSeries.en> ;
    reg:name "parallelTitleProperOfSeries"@en ;
    reg:status <http://metadataregistry.org/uri/RegStatus/1001> ;
    a rdf:Property ;
    rdfs:isDefinedBy <http://rdaregistry.info/Elements/u/> ;
    rdfs:label "has parallel title proper of series"@en ;
    skos:definition "Relates a resource to the title proper of a series in another language and/or script."@en .

<http://rdaregistry.info/Elements/u/P60591>
    reg:hasSubproperty <http://rdaregistry.info/Elements/m/P30205> ;
    reg:lexicalAlias <http://rdaregistry.info/Elements/u/parallelTitleProperOfSubseries.en> ;
    reg:name "parallelTitleProperOfSubseries"@en ;
    reg:status <http://metadataregistry.org/uri/RegStatus/1001> ;
    a rdf:Property ;
    rdfs:isDefinedBy <http://rdaregistry.info/Elements/u/> ;
    rdfs:label "has parallel title proper of subseries"@en ;
    skos:definition "Relates a resource to the title proper of a subseries in another language and/or script."@en .

<http://rdaregistry.info/Elements/u/P60592>
    reg:hasSubproperty <http://rdaregistry.info/Elements/a/P50118> ;
    reg:lexicalAlias <http://rdaregistry.info/Elements/u/placeOfDeath.en> ;
    reg:name "placeOfDeath"@en ;
    reg:status <http://metadataregistry.org/uri/RegStatus/1001> ;
    a rdf:Property ;
    rdfs:isDefinedBy <http://rdaregistry.info/Elements/u/> ;
    rdfs:label "has place of death"@en ;
    skos:definition "Relates a resource to the town, city, province, state, and/or country in which an agent died."@en .

<http://rdaregistry.info/Elements/u/P60593>
    reg:hasSubproperty <http://rdaregistry.info/Elements/a/P50119> ;
    reg:lexicalAlias <http://rdaregistry.info/Elements/u/placeOfBirth.en> ;
    reg:name "placeOfBirth"@en ;
    reg:status <http://metadataregistry.org/uri/RegStatus/1001> ;
    a rdf:Property ;
    rdfs:isDefinedBy <http://rdaregistry.info/Elements/u/> ;
    rdfs:label "has place of birth"@en ;
    skos:definition "Relates a resource to the town, city, province, state, and/or country in which an agent was born."@en .

<http://rdaregistry.info/Elements/u/P60594>
    reg:hasSubproperty <http://rdaregistry.info/Elements/m/P30206> ;
    reg:lexicalAlias <http://rdaregistry.info/Elements/u/recordingMedium.en> ;
    reg:name "recordingMedium"@en ;
    reg:status <http://metadataregistry.org/uri/RegStatus/1001> ;
    a rdf:Property ;
    rdfs:isDefinedBy <http://rdaregistry.info/Elements/u/> ;
    rdfs:label "has recording medium"@en ;
    rdfs:subPropertyOf <http://rdaregistry.info/Elements/u/P60351> ;
    skos:definition "Relates a resource to the type of medium used to record sound on an audio carrier (e.g., magnetic, optical)."@en .

<http://rdaregistry.info/Elements/u/P60595>
    reg:status <http://metadataregistry.org/uri/RegStatus/1008> ;
    rdfs:isDefinedBy <http://rdaregistry.info/Elements/u/> .

<http://rdaregistry.info/Elements/u/P60596>
    reg:hasSubproperty <http://rdaregistry.info/Elements/m/P30208> ;
    reg:lexicalAlias <http://rdaregistry.info/Elements/u/baseMaterial.en> ;
    reg:name "baseMaterial"@en ;
    reg:status <http://metadataregistry.org/uri/RegStatus/1001> ;
    a rdf:Property ;
    rdfs:isDefinedBy <http://rdaregistry.info/Elements/u/> ;
    rdfs:label "has base material"@en ;
    skos:definition "Relates a resource to the underlying physical material of a resource."@en .

<http://rdaregistry.info/Elements/u/P60597>
    reg:hasSubproperty <http://rdaregistry.info/Elements/m/P30209> ;
    reg:lexicalAlias <http://rdaregistry.info/Elements/u/keyTitle.en> ;
    reg:name "keyTitle"@en ;
    reg:status <http://metadataregistry.org/uri/RegStatus/1001> ;
    a rdf:Property ;
    rdfs:isDefinedBy <http://rdaregistry.info/Elements/u/> ;
    rdfs:label "has key title"@en ;
    rdfs:subPropertyOf <http://rdaregistry.info/Elements/u/P60369> ;
    skos:definition "Relates a resource to the unique name assigned to a resource by an issn registration agency."@en .

<http://rdaregistry.info/Elements/u/P60598>
    reg:hasSubproperty <http://rdaregistry.info/Elements/a/P50120> ;
    reg:lexicalAlias <http://rdaregistry.info/Elements/u/dateOfDeath.en> ;
    reg:name "dateOfDeath"@en ;
    reg:status <http://metadataregistry.org/uri/RegStatus/1001> ;
    a rdf:Property ;
    rdfs:isDefinedBy <http://rdaregistry.info/Elements/u/> ;
    rdfs:label "has date of death"@en ;
    rdfs:subPropertyOf <http://rdaregistry.info/Elements/u/P60324> ;
    skos:definition "Relates a resource to the year an agent died."@en .

<http://rdaregistry.info/Elements/u/P60599>
    reg:hasSubproperty <http://rdaregistry.info/Elements/a/P50121> ;
    reg:lexicalAlias <http://rdaregistry.info/Elements/u/dateOfBirth.en> ;
    reg:name "dateOfBirth"@en ;
    reg:status <http://metadataregistry.org/uri/RegStatus/1001> ;
    a rdf:Property ;
    rdfs:isDefinedBy <http://rdaregistry.info/Elements/u/> ;
    rdfs:label "has date of birth"@en ;
    rdfs:subPropertyOf <http://rdaregistry.info/Elements/u/P60324> ;
    skos:definition "Relates a resource to the year an agent was born."@en .

<http://rdaregistry.info/Elements/u/P60600>
    reg:hasSubproperty <http://rdaregistry.info/Elements/a/P50216> ;
    reg:lexicalAlias <http://rdaregistry.info/Elements/u/writerOfAddedLyricsOf.en> ;
    reg:name "writerOfAddedLyricsOf"@en ;
    reg:status <http://metadataregistry.org/uri/RegStatus/1001> ;
    a rdf:Property ;
    rdfs:isDefinedBy <http://rdaregistry.info/Elements/u/> ;
    rdfs:label "is writer of added lyrics of"@en ;
    rdfs:subPropertyOf <http://rdaregistry.info/Elements/u/P60608> ;
    owl:inverseOf <http://rdaregistry.info/Elements/u/P60371> ;
    skos:definition "Relates a writer of words added to a musical resource to the resource."@en .

<http://rdaregistry.info/Elements/u/P60601>
    reg:hasSubproperty <http://rdaregistry.info/Elements/a/P50002>, <http://rdaregistry.info/Elements/a/P50085>, <http://rdaregistry.info/Elements/a/P50087> ;
    reg:lexicalAlias <http://rdaregistry.info/Elements/u/appelleeOf.en> ;
    reg:name "appelleeOf"@en ;
    reg:status <http://metadataregistry.org/uri/RegStatus/1001> ;
    a rdf:Property ;
    rdfs:isDefinedBy <http://rdaregistry.info/Elements/u/> ;
    rdfs:label "is appellee of"@en ;
    rdfs:subPropertyOf <http://rdaregistry.info/Elements/u/P60602> ;
    owl:inverseOf <http://rdaregistry.info/Elements/u/P60373> ;
    skos:definition "Relates an agent against whom an appeal is taken on the decision of a lower court recorded in a legal resource of a higher court to the resource."@en .

<http://rdaregistry.info/Elements/u/P60602>
    reg:hasSubproperty <http://rdaregistry.info/Elements/a/P50131>, <http://rdaregistry.info/Elements/a/P50181>, <http://rdaregistry.info/Elements/a/P50182>, <http://rdaregistry.info/Elements/u/P60002>, <http://rdaregistry.info/Elements/u/P60003>, <http://rdaregistry.info/Elements/u/P60004>, <http://rdaregistry.info/Elements/u/P60005>, <http://rdaregistry.info/Elements/u/P60015>, <http://rdaregistry.info/Elements/u/P60032>, <http://rdaregistry.info/Elements/u/P60601>, <http://rdaregistry.info/Elements/u/P60603>, <http://rdaregistry.info/Elements/u/P60604>, <http://rdaregistry.info/Elements/u/P60634>, <http://rdaregistry.info/Elements/u/P60650>, <http://rdaregistry.info/Elements/u/P60668>, <http://rdaregistry.info/Elements/u/P60673>, <http://rdaregistry.info/Elements/u/P60674>, <http://rdaregistry.info/Elements/u/P60675>, <http://rdaregistry.info/Elements/u/P60678>, <http://rdaregistry.info/Elements/u/P60689>, <http://rdaregistry.info/Elements/u/P60690>, <http://rdaregistry.info/Elements/u/P60691>, <http://rdaregistry.info/Elements/u/P60692>, <http://rdaregistry.info/Elements/u/P60693>, <http://rdaregistry.info/Elements/u/P60695>, <http://rdaregistry.info/Elements/u/P60696>, <http://rdaregistry.info/Elements/u/P60698>, <http://rdaregistry.info/Elements/u/P60700>, <http://rdaregistry.info/Elements/u/P60702>, <http://rdaregistry.info/Elements/u/P60703>, <http://rdaregistry.info/Elements/u/P60816>, <http://rdaregistry.info/Elements/u/P60835>, <http://rdaregistry.info/Elements/u/P60837>, <http://rdaregistry.info/Elements/u/P60850>, <http://rdaregistry.info/Elements/u/P60870>, <http://rdaregistry.info/Elements/u/P60872> ;
    reg:lexicalAlias <http://rdaregistry.info/Elements/u/otherAgentAssociatedWithAResourceOf.en> ;
    reg:name "otherAgentAssociatedWithAResourceOf"@en ;
    reg:status <http://metadataregistry.org/uri/RegStatus/1001> ;
    a rdf:Property ;
    rdfs:isDefinedBy <http://rdaregistry.info/Elements/u/> ;
    rdfs:label "is other agent associated with a resource of"@en ;
    owl:inverseOf <http://rdaregistry.info/Elements/u/P60374> ;
    skos:definition "Relates an agent other than a creator, custodian, owner, producer, publisher, distributor or manufacturer associated with a resource to the resource."@en .

<http://rdaregistry.info/Elements/u/P60603>
    reg:hasSubproperty <http://rdaregistry.info/Elements/a/P50132> ;
    reg:lexicalAlias <http://rdaregistry.info/Elements/u/dedicatorOf.en> ;
    reg:name "dedicatorOf"@en ;
    reg:status <http://metadataregistry.org/uri/RegStatus/1001> ;
    a rdf:Property ;
    rdfs:isDefinedBy <http://rdaregistry.info/Elements/u/> ;
    rdfs:label "is dedicator of"@en ;
    rdfs:subPropertyOf <http://rdaregistry.info/Elements/u/P60602> ;
    owl:inverseOf <http://rdaregistry.info/Elements/u/P60375> ;
    skos:definition "Relates an agent by whom a resource is dedicated to the resource."@en .

<http://rdaregistry.info/Elements/u/P60604>
    reg:hasSubproperty <http://rdaregistry.info/Elements/a/P50133>, <http://rdaregistry.info/Elements/u/P60006>, <http://rdaregistry.info/Elements/u/P60007> ;
    reg:lexicalAlias <http://rdaregistry.info/Elements/u/curatorOf.en> ;
    reg:name "curatorOf"@en ;
    reg:status <http://metadataregistry.org/uri/RegStatus/1001> ;
    a rdf:Property ;
    rdfs:isDefinedBy <http://rdaregistry.info/Elements/u/> ;
    rdfs:label "is curator of"@en ;
    rdfs:subPropertyOf <http://rdaregistry.info/Elements/u/P60602> ;
    owl:inverseOf <http://rdaregistry.info/Elements/u/P60376> ;
    skos:definition "Relates an agent conceiving, aggregating, and/or organizing an exhibition, collection, or other resource to the resource."@en .

<http://rdaregistry.info/Elements/u/P60605>
    reg:hasSubproperty <http://rdaregistry.info/Elements/a/P50135> ;
    reg:lexicalAlias <http://rdaregistry.info/Elements/u/surveyorOf.en> ;
    reg:name "surveyorOf"@en ;
    reg:status <http://metadataregistry.org/uri/RegStatus/1001> ;
    a rdf:Property ;
    rdfs:isDefinedBy <http://rdaregistry.info/Elements/u/> ;
    rdfs:label "is surveyor of"@en ;
    rdfs:subPropertyOf <http://rdaregistry.info/Elements/u/P60626> ;
    owl:inverseOf <http://rdaregistry.info/Elements/u/P60377> ;
    skos:definition "Relates an agent contributing to a cartographic resource by providing measurements or dimensional relationships for the geographic area represented to the resource."@en .

<http://rdaregistry.info/Elements/u/P60606>
    reg:hasSubproperty <http://rdaregistry.info/Elements/a/P50136> ;
    reg:lexicalAlias <http://rdaregistry.info/Elements/u/animatorOf.en> ;
    reg:name "animatorOf"@en ;
    reg:status <http://metadataregistry.org/uri/RegStatus/1001> ;
    a rdf:Property ;
    rdfs:isDefinedBy <http://rdaregistry.info/Elements/u/> ;
    rdfs:label "is animator of"@en ;
    rdfs:subPropertyOf <http://rdaregistry.info/Elements/u/P60626> ;
    owl:inverseOf <http://rdaregistry.info/Elements/u/P60378> ;
    skos:definition "Relates an agent contributing to a moving image resource or computer program by giving apparent movement to inanimate objects or drawings to the resource."@en .

<http://rdaregistry.info/Elements/u/P60607>
    reg:hasSubproperty <http://rdaregistry.info/Elements/a/P50137> ;
    reg:lexicalAlias <http://rdaregistry.info/Elements/u/arrangerOfMusicOf.en> ;
    reg:name "arrangerOfMusicOf"@en ;
    reg:status <http://metadataregistry.org/uri/RegStatus/1001> ;
    a rdf:Property ;
    rdfs:isDefinedBy <http://rdaregistry.info/Elements/u/> ;
    rdfs:label "is arranger of music of"@en ;
    rdfs:subPropertyOf <http://rdaregistry.info/Elements/u/P60626> ;
    owl:inverseOf <http://rdaregistry.info/Elements/u/P60379> ;
    skos:definition "Relates an agent contributing to a musical resource by rewriting the composition for a medium of performance different from that for which the resource was originally intended to the resource."@en .

<http://rdaregistry.info/Elements/u/P60608>
    reg:hasSubproperty <http://rdaregistry.info/Elements/a/P50138>, <http://rdaregistry.info/Elements/u/P60600> ;
    reg:lexicalAlias <http://rdaregistry.info/Elements/u/writerOfAddedTextOf.en> ;
    reg:name "writerOfAddedTextOf"@en ;
    reg:status <http://metadataregistry.org/uri/RegStatus/1001> ;
    a rdf:Property ;
    rdfs:isDefinedBy <http://rdaregistry.info/Elements/u/> ;
    rdfs:label "is writer of added text of"@en ;
    rdfs:subPropertyOf <http://rdaregistry.info/Elements/u/P60620> ;
    owl:inverseOf <http://rdaregistry.info/Elements/u/P60380> ;
    skos:definition "Relates an agent contributing to a primarily non-textual resource by providing text for the non-textual resource (e.g., writing captions for photographs, descriptions of maps) to the resource."@en .

<http://rdaregistry.info/Elements/u/P60609>
    reg:hasSubproperty <http://rdaregistry.info/Elements/a/P50141> ;
    reg:lexicalAlias <http://rdaregistry.info/Elements/u/draftsmanOf.en> ;
    reg:name "draftsmanOf"@en ;
    reg:status <http://metadataregistry.org/uri/RegStatus/1001> ;
    a rdf:Property ;
    rdfs:isDefinedBy <http://rdaregistry.info/Elements/u/> ;
    rdfs:label "is draftsman of"@en ;
    rdfs:subPropertyOf <http://rdaregistry.info/Elements/u/P60626> ;
    owl:inverseOf <http://rdaregistry.info/Elements/u/P60381> ;
    skos:definition "Relates an agent contributing to a resource by an architect, inventor, etc., by making detailed plans or drawings for buildings, ships, aircraft, machines, objects, etc. to the resource."@en .

<http://rdaregistry.info/Elements/u/P60610>
    reg:hasSubproperty <http://rdaregistry.info/Elements/a/P50142> ;
    reg:lexicalAlias <http://rdaregistry.info/Elements/u/transcriberOf.en> ;
    reg:name "transcriberOf"@en ;
    reg:status <http://metadataregistry.org/uri/RegStatus/1001> ;
    a rdf:Property ;
    rdfs:isDefinedBy <http://rdaregistry.info/Elements/u/> ;
    rdfs:label "is transcriber of"@en ;
    rdfs:subPropertyOf <http://rdaregistry.info/Elements/u/P60626> ;
    owl:inverseOf <http://rdaregistry.info/Elements/u/P60382> ;
    skos:definition "Relates an agent contributing to a resource by writing down or notating previously unwritten or unnotated content, or by changing it from one system of notation to another to the resource."@en .

<http://rdaregistry.info/Elements/u/P60611>
    reg:hasSubproperty <http://rdaregistry.info/Elements/a/P50143> ;
    reg:lexicalAlias <http://rdaregistry.info/Elements/u/musicalDirectorOf.en> ;
    reg:name "musicalDirectorOf"@en ;
    reg:status <http://metadataregistry.org/uri/RegStatus/1001> ;
    a rdf:Property ;
    rdfs:isDefinedBy <http://rdaregistry.info/Elements/u/> ;
    rdfs:label "is musical director of"@en ;
    rdfs:subPropertyOf <http://rdaregistry.info/Elements/u/P60626> ;
    owl:inverseOf <http://rdaregistry.info/Elements/u/P60383> ;
    skos:definition "Relates an agent contributing to a resource by coordinating the activities of the composer, the sound editor, and sound mixers for a moving image production or for a musical or dramatic presentation or entertainment to the resource."@en .

<http://rdaregistry.info/Elements/u/P60612>
    reg:hasSubproperty <http://rdaregistry.info/Elements/a/P50144> ;
    reg:lexicalAlias <http://rdaregistry.info/Elements/u/costumeDesignerOf.en> ;
    reg:name "costumeDesignerOf"@en ;
    reg:status <http://metadataregistry.org/uri/RegStatus/1001> ;
    a rdf:Property ;
    rdfs:isDefinedBy <http://rdaregistry.info/Elements/u/> ;
    rdfs:label "is costume designer of"@en ;
    rdfs:subPropertyOf <http://rdaregistry.info/Elements/u/P60626> ;
    owl:inverseOf <http://rdaregistry.info/Elements/u/P60384> ;
    skos:definition "Relates an agent contributing to a resource by designing the costumes for a moving image production or for a musical or dramatic presentation or entertainment to the resource."@en .

<http://rdaregistry.info/Elements/u/P60613>
    reg:hasSubproperty <http://rdaregistry.info/Elements/a/P50145> ;
    reg:lexicalAlias <http://rdaregistry.info/Elements/u/translatorOf.en> ;
    reg:name "translatorOf"@en ;
    reg:status <http://metadataregistry.org/uri/RegStatus/1001> ;
    a rdf:Property ;
    rdfs:isDefinedBy <http://rdaregistry.info/Elements/u/> ;
    rdfs:label "is translator of"@en ;
    rdfs:subPropertyOf <http://rdaregistry.info/Elements/u/P60626> ;
    owl:inverseOf <http://rdaregistry.info/Elements/u/P60385> ;
    skos:definition "Relates an agent contributing to a resource by expressing the linguistic content of the resource in a language different from that of previous expressions of the original resource to the resource."@en .

<http://rdaregistry.info/Elements/u/P60614>
    reg:hasSubproperty <http://rdaregistry.info/Elements/a/P50146> ;
    reg:lexicalAlias <http://rdaregistry.info/Elements/u/artDirectorOf.en> ;
    reg:name "artDirectorOf"@en ;
    reg:status <http://metadataregistry.org/uri/RegStatus/1001> ;
    a rdf:Property ;
    rdfs:isDefinedBy <http://rdaregistry.info/Elements/u/> ;
    rdfs:label "is art director of"@en ;
    rdfs:subPropertyOf <http://rdaregistry.info/Elements/u/P60626> ;
    owl:inverseOf <http://rdaregistry.info/Elements/u/P60386> ;
    skos:definition "Relates an agent contributing to a resource by overseeing the artists and craftspeople who build the sets for moving image productions to the resource."@en .

<http://rdaregistry.info/Elements/u/P60615>
    reg:hasSubproperty <http://rdaregistry.info/Elements/a/P50147>, <http://rdaregistry.info/Elements/u/P60016>, <http://rdaregistry.info/Elements/u/P60017>, <http://rdaregistry.info/Elements/u/P60018>, <http://rdaregistry.info/Elements/u/P60019>, <http://rdaregistry.info/Elements/u/P60020>, <http://rdaregistry.info/Elements/u/P60021>, <http://rdaregistry.info/Elements/u/P60022>, <http://rdaregistry.info/Elements/u/P60023>, <http://rdaregistry.info/Elements/u/P60024>, <http://rdaregistry.info/Elements/u/P60025>, <http://rdaregistry.info/Elements/u/P60026>, <http://rdaregistry.info/Elements/u/P60028>, <http://rdaregistry.info/Elements/u/P60029>, <http://rdaregistry.info/Elements/u/P60030>, <http://rdaregistry.info/Elements/u/P60031> ;
    reg:lexicalAlias <http://rdaregistry.info/Elements/u/performerOf.en> ;
    reg:name "performerOf"@en ;
    reg:status <http://metadataregistry.org/uri/RegStatus/1001> ;
    a rdf:Property ;
    rdfs:isDefinedBy <http://rdaregistry.info/Elements/u/> ;
    rdfs:label "is performer of"@en ;
    rdfs:subPropertyOf <http://rdaregistry.info/Elements/u/P60626> ;
    owl:inverseOf <http://rdaregistry.info/Elements/u/P60387> ;
    skos:definition "Relates an agent contributing to a resource by performing music, acting, dancing, speaking, etc., often in a musical or dramatic presentation, etc. to the resource."@en .

<http://rdaregistry.info/Elements/u/P60616>
    reg:hasSubproperty <http://rdaregistry.info/Elements/a/P50148> ;
    reg:lexicalAlias <http://rdaregistry.info/Elements/u/courtReporterOf.en> ;
    reg:name "courtReporterOf"@en ;
    reg:status <http://metadataregistry.org/uri/RegStatus/1001> ;
    a rdf:Property ;
    rdfs:isDefinedBy <http://rdaregistry.info/Elements/u/> ;
    rdfs:label "is court reporter of"@en ;
    rdfs:subPropertyOf <http://rdaregistry.info/Elements/u/P60626> ;
    owl:inverseOf <http://rdaregistry.info/Elements/u/P60388> ;
    skos:definition "Relates an agent contributing to a resource by preparing a court's opinions for publication to the resource."@en .

<http://rdaregistry.info/Elements/u/P60617>
    reg:hasSubproperty <http://rdaregistry.info/Elements/a/P50149> ;
    reg:lexicalAlias <http://rdaregistry.info/Elements/u/writerOfPrefaceOf.en> ;
    reg:name "writerOfPrefaceOf"@en ;
    reg:status <http://metadataregistry.org/uri/RegStatus/1001> ;
    a rdf:Property ;
    rdfs:isDefinedBy <http://rdaregistry.info/Elements/u/> ;
    rdfs:label "is writer of introduction of"@en ;
    rdfs:subPropertyOf <http://rdaregistry.info/Elements/u/P60620> ;
    owl:inverseOf <http://rdaregistry.info/Elements/u/P60389> ;
    skos:definition "Relates an agent contributing to a resource by providing an introduction to the original resource to the resource."@en .

<http://rdaregistry.info/Elements/u/P60618>
    reg:hasSubproperty <http://rdaregistry.info/Elements/a/P50152> ;
    reg:lexicalAlias <http://rdaregistry.info/Elements/u/writerOfAddedCommentaryOf.en> ;
    reg:name "writerOfAddedCommentaryOf"@en ;
    reg:status <http://metadataregistry.org/uri/RegStatus/1001> ;
    a rdf:Property ;
    rdfs:isDefinedBy <http://rdaregistry.info/Elements/u/> ;
    rdfs:label "is writer of added commentary of"@en ;
    rdfs:subPropertyOf <http://rdaregistry.info/Elements/u/P60620> ;
    owl:inverseOf <http://rdaregistry.info/Elements/u/P60390> ;
    skos:definition "Relates an agent contributing to a resource by providing an interpretation or critical explanation of the original resource to the resource."@en .

<http://rdaregistry.info/Elements/u/P60619>
    reg:hasSubproperty <http://rdaregistry.info/Elements/a/P50153> ;
    reg:lexicalAlias <http://rdaregistry.info/Elements/u/writerOfIntroductionOf.en> ;
    reg:name "writerOfIntroductionOf"@en ;
    reg:status <http://metadataregistry.org/uri/RegStatus/1001> ;
    a rdf:Property ;
    rdfs:isDefinedBy <http://rdaregistry.info/Elements/u/> ;
    rdfs:label "is writer of afterword of"@en ;
    rdfs:subPropertyOf <http://rdaregistry.info/Elements/u/P60620> ;
    owl:inverseOf <http://rdaregistry.info/Elements/u/P60391> ;
    skos:definition "Relates an agent contributing to a resource by providing an afterword to the original resource to the resource."@en .

<http://rdaregistry.info/Elements/u/P60620>
    reg:hasSubproperty <http://rdaregistry.info/Elements/a/P50154>, <http://rdaregistry.info/Elements/u/P60608>, <http://rdaregistry.info/Elements/u/P60617>, <http://rdaregistry.info/Elements/u/P60618>, <http://rdaregistry.info/Elements/u/P60619> ;
    reg:lexicalAlias <http://rdaregistry.info/Elements/u/writerOfSupplementaryTextualContentOf.en> ;
    reg:name "writerOfSupplementaryTextualContentOf"@en ;
    reg:status <http://metadataregistry.org/uri/RegStatus/1001> ;
    a rdf:Property ;
    rdfs:isDefinedBy <http://rdaregistry.info/Elements/u/> ;
    rdfs:label "is writer of postface of"@en ;
    rdfs:subPropertyOf <http://rdaregistry.info/Elements/u/P60626> ;
    owl:inverseOf <http://rdaregistry.info/Elements/u/P60392> ;
    skos:definition "Relates an agent contributing to a resource by providing a postface to the original resource to the resource."@en .

<http://rdaregistry.info/Elements/u/P60621>
    reg:hasSubproperty <http://rdaregistry.info/Elements/a/P50156> ;
    reg:lexicalAlias <http://rdaregistry.info/Elements/u/editorOf.en> ;
    reg:name "editorOf"@en ;
    reg:status <http://metadataregistry.org/uri/RegStatus/1001> ;
    a rdf:Property ;
    rdfs:isDefinedBy <http://rdaregistry.info/Elements/u/> ;
    rdfs:label "is editor of"@en ;
    rdfs:subPropertyOf <http://rdaregistry.info/Elements/u/P60626> ;
    owl:inverseOf <http://rdaregistry.info/Elements/u/P60393> ;
    skos:definition "Relates an agent contributing to a resource by revising or clarifying the content, e.g., adding an introduction, notes, or other critical matter to the resource."@en .

<http://rdaregistry.info/Elements/u/P60622>
    reg:hasSubproperty <http://rdaregistry.info/Elements/a/P50157> ;
    reg:lexicalAlias <http://rdaregistry.info/Elements/u/abridgerOf.en> ;
    reg:name "abridgerOf"@en ;
    reg:status <http://metadataregistry.org/uri/RegStatus/1001> ;
    a rdf:Property ;
    rdfs:isDefinedBy <http://rdaregistry.info/Elements/u/> ;
    rdfs:label "is abridger of"@en ;
    rdfs:subPropertyOf <http://rdaregistry.info/Elements/u/P60626> ;
    owl:inverseOf <http://rdaregistry.info/Elements/u/P60394> ;
    skos:definition "Relates an agent contributing to a resource by shortening or condensing the original resource but leaving the nature and content of the original resource substantially unchanged to the resource."@en .

<http://rdaregistry.info/Elements/u/P60623>
    reg:hasSubproperty <http://rdaregistry.info/Elements/a/P50158> ;
    reg:lexicalAlias <http://rdaregistry.info/Elements/u/recordingEngineerOf.en> ;
    reg:name "recordingEngineerOf"@en ;
    reg:status <http://metadataregistry.org/uri/RegStatus/1001> ;
    a rdf:Property ;
    rdfs:isDefinedBy <http://rdaregistry.info/Elements/u/> ;
    rdfs:label "is recording engineer of"@en ;
    rdfs:subPropertyOf <http://rdaregistry.info/Elements/u/P60626> ;
    owl:inverseOf <http://rdaregistry.info/Elements/u/P60395> ;
    skos:definition "Relates an agent contributing to a resource by supervising the technical aspects of a sound or video recording session to the resource."@en .

<http://rdaregistry.info/Elements/u/P60624>
    reg:hasSubproperty <http://rdaregistry.info/Elements/a/P50159>, <http://rdaregistry.info/Elements/u/P60756> ;
    reg:lexicalAlias <http://rdaregistry.info/Elements/u/illustratorOf.en> ;
    reg:name "illustratorOf"@en ;
    reg:status <http://metadataregistry.org/uri/RegStatus/1001> ;
    a rdf:Property ;
    rdfs:isDefinedBy <http://rdaregistry.info/Elements/u/> ;
    rdfs:label "is illustrator of"@en ;
    rdfs:subPropertyOf <http://rdaregistry.info/Elements/u/P60626> ;
    owl:inverseOf <http://rdaregistry.info/Elements/u/P60396> ;
    skos:definition "Relates an agent contributing to a resource by supplementing the primary content with drawings, diagrams, photographs, etc. to the resource."@en .

<http://rdaregistry.info/Elements/u/P60625>
    reg:hasSubproperty <http://rdaregistry.info/Elements/a/P50160> ;
    reg:lexicalAlias <http://rdaregistry.info/Elements/u/recordistOf.en> ;
    reg:name "recordistOf"@en ;
    reg:status <http://metadataregistry.org/uri/RegStatus/1001> ;
    a rdf:Property ;
    rdfs:isDefinedBy <http://rdaregistry.info/Elements/u/> ;
    rdfs:label "is recordist of"@en ;
    rdfs:subPropertyOf <http://rdaregistry.info/Elements/u/P60626> ;
    owl:inverseOf <http://rdaregistry.info/Elements/u/P60397> ;
    skos:definition "Relates an agent contributing to a resource by using a recording device to capture sound and/or video during a recording session, including field recordings of natural sounds, folkloric events, music, etc. to the resource."@en .

<http://rdaregistry.info/Elements/u/P60626>
    reg:hasSubproperty <http://rdaregistry.info/Elements/a/P50161>, <http://rdaregistry.info/Elements/u/P60605>, <http://rdaregistry.info/Elements/u/P60606>, <http://rdaregistry.info/Elements/u/P60607>, <http://rdaregistry.info/Elements/u/P60609>, <http://rdaregistry.info/Elements/u/P60610>, <http://rdaregistry.info/Elements/u/P60611>, <http://rdaregistry.info/Elements/u/P60612>, <http://rdaregistry.info/Elements/u/P60613>, <http://rdaregistry.info/Elements/u/P60614>, <http://rdaregistry.info/Elements/u/P60615>, <http://rdaregistry.info/Elements/u/P60616>, <http://rdaregistry.info/Elements/u/P60620>, <http://rdaregistry.info/Elements/u/P60621>, <http://rdaregistry.info/Elements/u/P60622>, <http://rdaregistry.info/Elements/u/P60623>, <http://rdaregistry.info/Elements/u/P60624>, <http://rdaregistry.info/Elements/u/P60625>, <http://rdaregistry.info/Elements/u/P60627>, <http://rdaregistry.info/Elements/u/P60647>, <http://rdaregistry.info/Elements/u/P60651>, <http://rdaregistry.info/Elements/u/P60666>, <http://rdaregistry.info/Elements/u/P60671>, <http://rdaregistry.info/Elements/u/P60754>, <http://rdaregistry.info/Elements/u/P60755>, <http://rdaregistry.info/Elements/u/P60810>, <http://rdaregistry.info/Elements/u/P60812>, <http://rdaregistry.info/Elements/u/P60814>, <http://rdaregistry.info/Elements/u/P60825>, <http://rdaregistry.info/Elements/u/P60829>, <http://rdaregistry.info/Elements/u/P60839>, <http://rdaregistry.info/Elements/u/P60841>, <http://rdaregistry.info/Elements/u/P60852> ;
    reg:lexicalAlias <http://rdaregistry.info/Elements/u/contributorOf.en> ;
    reg:name "contributorOf"@en ;
    reg:status <http://metadataregistry.org/uri/RegStatus/1001> ;
    a rdf:Property ;
    rdfs:isDefinedBy <http://rdaregistry.info/Elements/u/> ;
    rdfs:label "is contributor of"@en ;
    owl:inverseOf <http://rdaregistry.info/Elements/u/P60398> ;
    skos:definition "Relates an agent contributing to an expression to the resource."@en .

<http://rdaregistry.info/Elements/u/P60627>
    reg:hasSubproperty <http://rdaregistry.info/Elements/a/P50139> ;
    reg:lexicalAlias <http://rdaregistry.info/Elements/u/stageDirectorOf.en> ;
    reg:name "stageDirectorOf"@en ;
    reg:status <http://metadataregistry.org/uri/RegStatus/1001> ;
    a rdf:Property ;
    rdfs:isDefinedBy <http://rdaregistry.info/Elements/u/> ;
    rdfs:label "is stage director of"@en ;
    rdfs:subPropertyOf <http://rdaregistry.info/Elements/u/P60626> ;
    owl:inverseOf <http://rdaregistry.info/Elements/u/P60399> ;
    skos:definition "Relates an agent contributing to a stage resource through the general management and supervision of a performance to the resource."@en .

<http://rdaregistry.info/Elements/u/P60628>
    reg:hasSubproperty <http://rdaregistry.info/Elements/a/P50162>, <http://rdaregistry.info/Elements/u/P60008> ;
    reg:lexicalAlias <http://rdaregistry.info/Elements/u/currentOwnerOf.en> ;
    reg:name "currentOwnerOf"@en ;
    reg:status <http://metadataregistry.org/uri/RegStatus/1001> ;
    a rdf:Property ;
    rdfs:isDefinedBy <http://rdaregistry.info/Elements/u/> ;
    rdfs:label "is current owner of"@en ;
    rdfs:subPropertyOf <http://rdaregistry.info/Elements/u/P60632> ;
    owl:inverseOf <http://rdaregistry.info/Elements/u/P60400> ;
    skos:definition "Relates an agent currently having legal possession of a resource to the resource."@en .

<http://rdaregistry.info/Elements/u/P60629>
    reg:hasSubproperty <http://rdaregistry.info/Elements/a/P50026> ;
    reg:lexicalAlias <http://rdaregistry.info/Elements/u/employee.en> ;
    reg:name "employee"@en ;
    reg:status <http://metadataregistry.org/uri/RegStatus/1001> ;
    a rdf:Property ;
    rdfs:isDefinedBy <http://rdaregistry.info/Elements/u/> ;
    rdfs:label "has employee"@en ;
    owl:inverseOf <http://rdaregistry.info/Elements/u/P60679> ;
    skos:definition "Relates an agent employed by the agent to the agent."@en .

<http://rdaregistry.info/Elements/u/P60630>
    reg:hasSubproperty <http://rdaregistry.info/Elements/a/P50163>, <http://rdaregistry.info/Elements/u/P60012>, <http://rdaregistry.info/Elements/u/P60013> ;
    reg:lexicalAlias <http://rdaregistry.info/Elements/u/formerOwnerOf.en> ;
    reg:name "formerOwnerOf"@en ;
    reg:status <http://metadataregistry.org/uri/RegStatus/1001> ;
    a rdf:Property ;
    rdfs:isDefinedBy <http://rdaregistry.info/Elements/u/> ;
    rdfs:label "is former owner of"@en ;
    rdfs:subPropertyOf <http://rdaregistry.info/Elements/u/P60632> ;
    owl:inverseOf <http://rdaregistry.info/Elements/u/P60401> ;
    skos:definition "Relates an agent formerly having legal possession of a resource to the resource."@en .

<http://rdaregistry.info/Elements/u/P60631>
    reg:hasSubproperty <http://rdaregistry.info/Elements/a/P50164> ;
    reg:lexicalAlias <http://rdaregistry.info/Elements/u/custodianOf.en> ;
    reg:name "custodianOf"@en ;
    reg:status <http://metadataregistry.org/uri/RegStatus/1001> ;
    a rdf:Property ;
    rdfs:isDefinedBy <http://rdaregistry.info/Elements/u/> ;
    rdfs:label "is custodian of"@en ;
    owl:inverseOf <http://rdaregistry.info/Elements/u/P60402> ;
    skos:definition "Relates an agent having legal custody of a resource to the resource."@en .

<http://rdaregistry.info/Elements/u/P60632>
    reg:hasSubproperty <http://rdaregistry.info/Elements/a/P50165>, <http://rdaregistry.info/Elements/u/P60628>, <http://rdaregistry.info/Elements/u/P60630> ;
    reg:lexicalAlias <http://rdaregistry.info/Elements/u/ownerOf.en> ;
    reg:name "ownerOf"@en ;
    reg:status <http://metadataregistry.org/uri/RegStatus/1001> ;
    a rdf:Property ;
    rdfs:isDefinedBy <http://rdaregistry.info/Elements/u/> ;
    rdfs:label "is owner of"@en ;
    owl:inverseOf <http://rdaregistry.info/Elements/u/P60404> ;
    skos:definition "Relates an agent having legal possession of a resource to the resource."@en .

<http://rdaregistry.info/Elements/u/P60633>
    reg:hasSubproperty <http://rdaregistry.info/Elements/a/P50027>, <http://rdaregistry.info/Elements/u/P60864>, <http://rdaregistry.info/Elements/u/P60866> ;
    reg:lexicalAlias <http://rdaregistry.info/Elements/u/officer.en> ;
    reg:name "officer"@en ;
    reg:status <http://metadataregistry.org/uri/RegStatus/1001> ;
    a rdf:Property ;
    rdfs:isDefinedBy <http://rdaregistry.info/Elements/u/> ;
    rdfs:label "has officer"@en ;
    rdfs:subPropertyOf <http://rdaregistry.info/Elements/u/P60454> ;
    owl:inverseOf <http://rdaregistry.info/Elements/u/P60737> ;
    skos:definition "Relates an agent holding an office in or commanding the agent to the agent."@en .

<http://rdaregistry.info/Elements/u/P60634>
    reg:hasSubproperty <http://rdaregistry.info/Elements/a/P50166>, <http://rdaregistry.info/Elements/a/P50167> ;
    reg:lexicalAlias <http://rdaregistry.info/Elements/u/honoureeOf.en> ;
    reg:name "honoureeOf"@en ;
    reg:status <http://metadataregistry.org/uri/RegStatus/1001> ;
    a rdf:Property ;
    rdfs:isDefinedBy <http://rdaregistry.info/Elements/u/> ;
    rdfs:label "is honouree of"@en ;
    rdfs:subPropertyOf <http://rdaregistry.info/Elements/u/P60602> ;
    owl:inverseOf <http://rdaregistry.info/Elements/u/P60406> ;
    skos:altLabel "is honoree of"@en ;
    skos:definition "Relates an agent honoured by a resource (e.g., the honouree of a festschrift) to the resource."@en .

<http://rdaregistry.info/Elements/u/P60635>
    reg:hasSubproperty <http://rdaregistry.info/Elements/a/P50168> ;
    reg:lexicalAlias <http://rdaregistry.info/Elements/u/broadcasterOf.en> ;
    reg:name "broadcasterOf"@en ;
    reg:status <http://metadataregistry.org/uri/RegStatus/1001> ;
    a rdf:Property ;
    rdfs:isDefinedBy <http://rdaregistry.info/Elements/u/> ;
    rdfs:label "is broadcaster of"@en ;
    rdfs:subPropertyOf <http://rdaregistry.info/Elements/u/P60670> ;
    owl:inverseOf <http://rdaregistry.info/Elements/u/P60407> ;
    skos:definition "Relates an agent involved in broadcasting a resource to an audience via radio, television, webcast, etc. to the resource."@en .

<http://rdaregistry.info/Elements/u/P60636>
    reg:hasSubproperty <http://rdaregistry.info/Elements/a/P50169> ;
    reg:lexicalAlias <http://rdaregistry.info/Elements/u/filmDistributorOf.en> ;
    reg:name "filmDistributorOf"@en ;
    reg:status <http://metadataregistry.org/uri/RegStatus/1001> ;
    a rdf:Property ;
    rdfs:isDefinedBy <http://rdaregistry.info/Elements/u/> ;
    rdfs:label "is film distributor of"@en ;
    rdfs:subPropertyOf <http://rdaregistry.info/Elements/u/P60667> ;
    owl:inverseOf <http://rdaregistry.info/Elements/u/P60408> ;
    skos:definition "Relates an agent involved in distributing a moving image resource to theatres or other distribution channels to the resource."@en .

<http://rdaregistry.info/Elements/u/P60637>
    reg:hasSubproperty <http://rdaregistry.info/Elements/a/P50170> ;
    reg:lexicalAlias <http://rdaregistry.info/Elements/u/bookDesignerOf.en> ;
    reg:name "bookDesignerOf"@en ;
    reg:status <http://metadataregistry.org/uri/RegStatus/1001> ;
    a rdf:Property ;
    rdfs:isDefinedBy <http://rdaregistry.info/Elements/u/> ;
    rdfs:label "is book designer of"@en ;
    rdfs:subPropertyOf <http://rdaregistry.info/Elements/u/P60669> ;
    owl:inverseOf <http://rdaregistry.info/Elements/u/P60409> ;
    skos:definition "Relates an agent involved in manufacturing a resource by being responsible for the entire graphic design of a book, including arrangement of type and illustration, choice of materials, and process used to the resource."@en .

<http://rdaregistry.info/Elements/u/P60638>
    reg:hasSubproperty <http://rdaregistry.info/Elements/a/P50171> ;
    reg:lexicalAlias <http://rdaregistry.info/Elements/u/engraverOf.en> ;
    reg:name "engraverOf"@en ;
    reg:status <http://metadataregistry.org/uri/RegStatus/1001> ;
    a rdf:Property ;
    rdfs:isDefinedBy <http://rdaregistry.info/Elements/u/> ;
    rdfs:label "is engraver of"@en ;
    rdfs:subPropertyOf <http://rdaregistry.info/Elements/u/P60669> ;
    owl:inverseOf <http://rdaregistry.info/Elements/u/P60410> ;
    skos:definition "Relates an agent involved in manufacturing a resource by cutting letters, figures, etc., on a surface such as a wooden or metal plate used for printing to the resource."@en .

<http://rdaregistry.info/Elements/u/P60639>
    reg:hasSubproperty <http://rdaregistry.info/Elements/a/P50172> ;
    reg:lexicalAlias <http://rdaregistry.info/Elements/u/brailleEmbosserOf.en> ;
    reg:name "brailleEmbosserOf"@en ;
    reg:status <http://metadataregistry.org/uri/RegStatus/1001> ;
    a rdf:Property ;
    rdfs:isDefinedBy <http://rdaregistry.info/Elements/u/> ;
    rdfs:label "is braille embosser of"@en ;
    rdfs:subPropertyOf <http://rdaregistry.info/Elements/u/P60669> ;
    owl:inverseOf <http://rdaregistry.info/Elements/u/P60411> ;
    skos:definition "Relates an agent involved in manufacturing a resource by embossing braille cells using a stylus, special embossing printer, or other device to the resource."@en .

<http://rdaregistry.info/Elements/u/P60640>
    reg:hasSubproperty <http://rdaregistry.info/Elements/a/P50173> ;
    reg:lexicalAlias <http://rdaregistry.info/Elements/u/printmakerOf.en> ;
    reg:name "printmakerOf"@en ;
    reg:status <http://metadataregistry.org/uri/RegStatus/1001> ;
    a rdf:Property ;
    rdfs:isDefinedBy <http://rdaregistry.info/Elements/u/> ;
    rdfs:label "is printmaker of"@en ;
    rdfs:subPropertyOf <http://rdaregistry.info/Elements/u/P60669> ;
    owl:inverseOf <http://rdaregistry.info/Elements/u/P60412> ;
    skos:definition "Relates an agent involved in manufacturing a resource by making a relief, intaglio, or planographic printing surface to the resource."@en .

<http://rdaregistry.info/Elements/u/P60641>
    reg:hasSubproperty <http://rdaregistry.info/Elements/a/P50174> ;
    reg:lexicalAlias <http://rdaregistry.info/Elements/u/casterOf.en> ;
    reg:name "casterOf"@en ;
    reg:status <http://metadataregistry.org/uri/RegStatus/1001> ;
    a rdf:Property ;
    rdfs:isDefinedBy <http://rdaregistry.info/Elements/u/> ;
    rdfs:label "is caster of"@en ;
    rdfs:subPropertyOf <http://rdaregistry.info/Elements/u/P60669> ;
    owl:inverseOf <http://rdaregistry.info/Elements/u/P60413> ;
    skos:definition "Relates an agent involved in manufacturing a resource by pouring a liquid or molten substance into a mold and leaving it to solidify to take the shape of the mold to the resource."@en .

<http://rdaregistry.info/Elements/u/P60642>
    reg:hasSubproperty <http://rdaregistry.info/Elements/a/P50175> ;
    reg:lexicalAlias <http://rdaregistry.info/Elements/u/lithographerOf.en> ;
    reg:name "lithographerOf"@en ;
    reg:status <http://metadataregistry.org/uri/RegStatus/1001> ;
    a rdf:Property ;
    rdfs:isDefinedBy <http://rdaregistry.info/Elements/u/> ;
    rdfs:label "is lithographer of"@en ;
    rdfs:subPropertyOf <http://rdaregistry.info/Elements/u/P60669> ;
    owl:inverseOf <http://rdaregistry.info/Elements/u/P60414> ;
    skos:definition "Relates an agent involved in manufacturing a resource by preparing a stone or plate for lithographic printing, including a graphic artist creating a design directly on the surface from which printing will be done to the resource."@en .

<http://rdaregistry.info/Elements/u/P60643>
    reg:hasSubproperty <http://rdaregistry.info/Elements/a/P50176> ;
    reg:lexicalAlias <http://rdaregistry.info/Elements/u/platemakerOf.en> ;
    reg:name "platemakerOf"@en ;
    reg:status <http://metadataregistry.org/uri/RegStatus/1001> ;
    a rdf:Property ;
    rdfs:isDefinedBy <http://rdaregistry.info/Elements/u/> ;
    rdfs:label "is platemaker of"@en ;
    rdfs:subPropertyOf <http://rdaregistry.info/Elements/u/P60669> ;
    owl:inverseOf <http://rdaregistry.info/Elements/u/P60415> ;
    skos:definition "Relates an agent involved in manufacturing a resource by preparing plates used in the production of printed images and/or text to the resource."@en .

<http://rdaregistry.info/Elements/u/P60644>
    reg:hasSubproperty <http://rdaregistry.info/Elements/a/P50177> ;
    reg:lexicalAlias <http://rdaregistry.info/Elements/u/etcherOf.en> ;
    reg:name "etcherOf"@en ;
    reg:status <http://metadataregistry.org/uri/RegStatus/1001> ;
    a rdf:Property ;
    rdfs:isDefinedBy <http://rdaregistry.info/Elements/u/> ;
    rdfs:label "is etcher of"@en ;
    rdfs:subPropertyOf <http://rdaregistry.info/Elements/u/P60669> ;
    owl:inverseOf <http://rdaregistry.info/Elements/u/P60416> ;
    skos:definition "Relates an agent involved in manufacturing a resource by subjecting metal, glass, or some other surface used for printing, to acid or another corrosive substance to the resource."@en .

<http://rdaregistry.info/Elements/u/P60645>
    reg:hasSubproperty <http://rdaregistry.info/Elements/a/P50178> ;
    reg:lexicalAlias <http://rdaregistry.info/Elements/u/collotyperOf.en> ;
    reg:name "collotyperOf"@en ;
    reg:status <http://metadataregistry.org/uri/RegStatus/1001> ;
    a rdf:Property ;
    rdfs:isDefinedBy <http://rdaregistry.info/Elements/u/> ;
    rdfs:label "is collotyper of"@en ;
    rdfs:subPropertyOf <http://rdaregistry.info/Elements/u/P60669> ;
    owl:inverseOf <http://rdaregistry.info/Elements/u/P60417> ;
    skos:definition "Relates an agent involved in manufacturing a resource using a photomechanical process for making prints directly from a hardened film of gelatin or other colloid that has ink-receptive and ink-repellent surfaces to the resource."@en .

<http://rdaregistry.info/Elements/u/P60646>
    reg:hasSubproperty <http://rdaregistry.info/Elements/a/P50179> ;
    reg:lexicalAlias <http://rdaregistry.info/Elements/u/printerOf.en> ;
    reg:name "printerOf"@en ;
    reg:status <http://metadataregistry.org/uri/RegStatus/1001> ;
    a rdf:Property ;
    rdfs:isDefinedBy <http://rdaregistry.info/Elements/u/> ;
    rdfs:label "is printer of"@en ;
    rdfs:subPropertyOf <http://rdaregistry.info/Elements/u/P60669> ;
    owl:inverseOf <http://rdaregistry.info/Elements/u/P60418> ;
    skos:definition "Relates an agent involved in manufacturing a resource of printed text, notated music, etc., from type or plates, such as a book, newspaper, magazine, broadside, score, etc. to the resource."@en .

<http://rdaregistry.info/Elements/u/P60647>
    reg:hasSubproperty <http://rdaregistry.info/Elements/a/P50180> ;
    reg:lexicalAlias <http://rdaregistry.info/Elements/u/presenterOf.en> ;
    reg:name "presenterOf"@en ;
    reg:status <http://metadataregistry.org/uri/RegStatus/1001> ;
    a rdf:Property ;
    rdfs:isDefinedBy <http://rdaregistry.info/Elements/u/> ;
    rdfs:label "is presenter of"@en ;
    rdfs:subPropertyOf <http://rdaregistry.info/Elements/u/P60626> ;
    owl:inverseOf <http://rdaregistry.info/Elements/u/P60419> ;
    skos:definition "Relates an agent mentioned in an \"X presents\" credit for moving image materials and who is probably associated with production, finance, or distribution in some way to the resource."@en .

<http://rdaregistry.info/Elements/u/P60648>
    reg:hasSubproperty <http://rdaregistry.info/Elements/a/P50056>, <http://rdaregistry.info/Elements/a/P50095>, <http://rdaregistry.info/Elements/a/P50230> ;
    reg:lexicalAlias <http://rdaregistry.info/Elements/u/memberOf.en> ;
    reg:name "memberOf"@en ;
    reg:status <http://metadataregistry.org/uri/RegStatus/1001> ;
    a rdf:Property ;
    rdfs:isDefinedBy <http://rdaregistry.info/Elements/u/> ;
    rdfs:label "has member of"@en ;
    owl:inverseOf <http://rdaregistry.info/Elements/u/P60697> ;
    skos:definition "Relates an agent of which the agent is a member to the agent."@en .

<http://rdaregistry.info/Elements/u/P60649>
    reg:hasSubproperty <http://rdaregistry.info/Elements/a/P50091> ;
    reg:lexicalAlias <http://rdaregistry.info/Elements/u/degreeSupervisorOf.en> ;
    reg:name "degreeSupervisorOf"@en ;
    reg:status <http://metadataregistry.org/uri/RegStatus/1001> ;
    a rdf:Property ;
    rdfs:isDefinedBy <http://rdaregistry.info/Elements/u/> ;
    rdfs:label "is degree supervisor of"@en ;
    rdfs:subPropertyOf <http://rdaregistry.info/Elements/u/P60672> ;
    owl:inverseOf <http://rdaregistry.info/Elements/u/P60420> ;
    skos:definition "Relates an agent, such as an advisor or supervisor of thesis or dissertation research, overseeing either an academic degree or thesis to the resource."@en .

<http://rdaregistry.info/Elements/u/P60650>
    reg:hasSubproperty <http://rdaregistry.info/Elements/a/P50092> ;
    reg:lexicalAlias <http://rdaregistry.info/Elements/u/illuminatorOf.en> ;
    reg:name "illuminatorOf"@en ;
    reg:status <http://metadataregistry.org/uri/RegStatus/1001> ;
    a rdf:Property ;
    rdfs:isDefinedBy <http://rdaregistry.info/Elements/u/> ;
    rdfs:label "is illuminator of"@en ;
    rdfs:subPropertyOf <http://rdaregistry.info/Elements/u/P60602> ;
    owl:inverseOf <http://rdaregistry.info/Elements/u/P60421> ;
    skos:definition "Relates an agent providing decoration to a specific resource using precious metals or color, often with elaborate designs and motifs to the resource."@en .

<http://rdaregistry.info/Elements/u/P60651>
    reg:hasSubproperty <http://rdaregistry.info/Elements/a/P50183> ;
    reg:lexicalAlias <http://rdaregistry.info/Elements/u/editorOfMovingImageResourceOf.en> ;
    reg:name "editorOfMovingImageResourceOf"@en ;
    reg:status <http://metadataregistry.org/uri/RegStatus/1001> ;
    a rdf:Property ;
    rdfs:isDefinedBy <http://rdaregistry.info/Elements/u/> ;
    rdfs:label "is editor of moving image work of"@en ;
    rdfs:subPropertyOf <http://rdaregistry.info/Elements/u/P60626> ;
    owl:inverseOf <http://rdaregistry.info/Elements/u/P60422> ;
    skos:definition "Relates an agent responsible for assembling, arranging, and trimming film, video, or other moving image formats, including both visual and audio aspects to the resource."@en .

<http://rdaregistry.info/Elements/u/P60652>
    reg:hasSubproperty <http://rdaregistry.info/Elements/a/P50184> ;
    reg:lexicalAlias <http://rdaregistry.info/Elements/u/programmerOf.en> ;
    reg:name "programmerOf"@en ;
    reg:status <http://metadataregistry.org/uri/RegStatus/1001> ;
    a rdf:Property ;
    rdfs:isDefinedBy <http://rdaregistry.info/Elements/u/> ;
    rdfs:label "is programmer of"@en ;
    rdfs:subPropertyOf <http://rdaregistry.info/Elements/u/P60672> ;
    owl:inverseOf <http://rdaregistry.info/Elements/u/P60423> ;
    skos:definition "Relates an agent responsible for creating a computer program to the resource."@en .

<http://rdaregistry.info/Elements/u/P60653>
    reg:hasSubproperty <http://rdaregistry.info/Elements/a/P50185> ;
    reg:lexicalAlias <http://rdaregistry.info/Elements/u/designerOf.en> ;
    reg:name "designerOf"@en ;
    reg:status <http://metadataregistry.org/uri/RegStatus/1001> ;
    a rdf:Property ;
    rdfs:isDefinedBy <http://rdaregistry.info/Elements/u/> ;
    rdfs:label "is designer of"@en ;
    rdfs:subPropertyOf <http://rdaregistry.info/Elements/u/P60672> ;
    owl:inverseOf <http://rdaregistry.info/Elements/u/P60424> ;
    skos:definition "Relates an agent responsible for creating a design for an object to the resource."@en .

<http://rdaregistry.info/Elements/u/P60654>
    reg:hasSubproperty <http://rdaregistry.info/Elements/a/P50150>, <http://rdaregistry.info/Elements/a/P50186> ;
    reg:lexicalAlias <http://rdaregistry.info/Elements/u/cartographerOf.en> ;
    reg:name "cartographerOf"@en ;
    reg:status <http://metadataregistry.org/uri/RegStatus/1001> ;
    a rdf:Property ;
    rdfs:isDefinedBy <http://rdaregistry.info/Elements/u/> ;
    rdfs:label "is cartographer of"@en ;
    rdfs:subPropertyOf <http://rdaregistry.info/Elements/u/P60672> ;
    owl:inverseOf <http://rdaregistry.info/Elements/u/P60425> ;
    skos:definition "Relates an agent responsible for creating a map, atlas, globe, or other cartographic resource to the resource."@en .

<http://rdaregistry.info/Elements/u/P60655>
    reg:hasSubproperty <http://rdaregistry.info/Elements/a/P50134>, <http://rdaregistry.info/Elements/a/P50187> ;
    reg:lexicalAlias <http://rdaregistry.info/Elements/u/composerOf.en> ;
    reg:name "composerOf"@en ;
    reg:status <http://metadataregistry.org/uri/RegStatus/1001> ;
    a rdf:Property ;
    rdfs:isDefinedBy <http://rdaregistry.info/Elements/u/> ;
    rdfs:label "is composer of"@en ;
    rdfs:subPropertyOf <http://rdaregistry.info/Elements/u/P60672> ;
    owl:inverseOf <http://rdaregistry.info/Elements/u/P60426> ;
    skos:definition "Relates an agent responsible for creating a musical resource to the resource."@en .

<http://rdaregistry.info/Elements/u/P60656>
    reg:hasSubproperty <http://rdaregistry.info/Elements/a/P50188> ;
    reg:lexicalAlias <http://rdaregistry.info/Elements/u/inventorOf.en> ;
    reg:name "inventorOf"@en ;
    reg:status <http://metadataregistry.org/uri/RegStatus/1001> ;
    a rdf:Property ;
    rdfs:isDefinedBy <http://rdaregistry.info/Elements/u/> ;
    rdfs:label "is inventor of"@en ;
    rdfs:subPropertyOf <http://rdaregistry.info/Elements/u/P60672> ;
    owl:inverseOf <http://rdaregistry.info/Elements/u/P60427> ;
    skos:definition "Relates an agent responsible for creating a new device or process to the resource."@en .

<http://rdaregistry.info/Elements/u/P60657>
    reg:hasSubproperty <http://rdaregistry.info/Elements/a/P50189> ;
    reg:lexicalAlias <http://rdaregistry.info/Elements/u/compilerOf.en> ;
    reg:name "compilerOf"@en ;
    reg:status <http://metadataregistry.org/uri/RegStatus/1001> ;
    a rdf:Property ;
    rdfs:isDefinedBy <http://rdaregistry.info/Elements/u/> ;
    rdfs:label "is compiler of"@en ;
    rdfs:subPropertyOf <http://rdaregistry.info/Elements/u/P60672> ;
    owl:inverseOf <http://rdaregistry.info/Elements/u/P60428> ;
    skos:definition "Relates an agent responsible for creating a new resource (e.g., a bibliography, a directory) by selecting, arranging, aggregating, and editing data, information, etc. to the resource."@en .

<http://rdaregistry.info/Elements/u/P60658>
    reg:hasSubproperty <http://rdaregistry.info/Elements/a/P50190>, <http://rdaregistry.info/Elements/a/P50272> ;
    reg:lexicalAlias <http://rdaregistry.info/Elements/u/photographerOf.en> ;
    reg:name "photographerOf"@en ;
    reg:status <http://metadataregistry.org/uri/RegStatus/1001> ;
    a rdf:Property ;
    rdfs:isDefinedBy <http://rdaregistry.info/Elements/u/> ;
    rdfs:label "is photographer of"@en ;
    rdfs:subPropertyOf <http://rdaregistry.info/Elements/u/P60672> ;
    owl:inverseOf <http://rdaregistry.info/Elements/u/P60429> ;
    skos:definition "Relates an agent responsible for creating a photographic resource to the resource."@en .

<http://rdaregistry.info/Elements/u/P60659>
    reg:hasSubproperty <http://rdaregistry.info/Elements/a/P50140>, <http://rdaregistry.info/Elements/a/P50191> ;
    reg:lexicalAlias <http://rdaregistry.info/Elements/u/interviewerOf.en> ;
    reg:name "interviewerOf"@en ;
    reg:status <http://metadataregistry.org/uri/RegStatus/1001> ;
    a rdf:Property ;
    rdfs:isDefinedBy <http://rdaregistry.info/Elements/u/> ;
    rdfs:label "is interviewer of"@en ;
    rdfs:subPropertyOf <http://rdaregistry.info/Elements/u/P60672> ;
    owl:inverseOf <http://rdaregistry.info/Elements/u/P60430> ;
    skos:definition "Relates an agent responsible for creating a resource by acting as an interviewer, reporter, pollster, or some other information gathering agent to the resource."@en .

<http://rdaregistry.info/Elements/u/P60660>
    reg:hasSubproperty <http://rdaregistry.info/Elements/a/P50192>, <http://rdaregistry.info/Elements/u/P60705>, <http://rdaregistry.info/Elements/u/P60758>, <http://rdaregistry.info/Elements/u/P60759> ;
    reg:lexicalAlias <http://rdaregistry.info/Elements/u/artistOf.en> ;
    reg:name "artistOf"@en ;
    reg:status <http://metadataregistry.org/uri/RegStatus/1001> ;
    a rdf:Property ;
    rdfs:isDefinedBy <http://rdaregistry.info/Elements/u/> ;
    rdfs:label "is artist of"@en ;
    rdfs:subPropertyOf <http://rdaregistry.info/Elements/u/P60672> ;
    owl:inverseOf <http://rdaregistry.info/Elements/u/P60431> ;
    skos:definition "Relates an agent responsible for creating a resource by conceiving, and often implementing, an original graphic design, drawing, painting, etc. to the resource."@en .

<http://rdaregistry.info/Elements/u/P60661>
    reg:hasSubproperty <http://rdaregistry.info/Elements/a/P50155>, <http://rdaregistry.info/Elements/a/P50193> ;
    reg:lexicalAlias <http://rdaregistry.info/Elements/u/intervieweeOf.en> ;
    reg:name "intervieweeOf"@en ;
    reg:status <http://metadataregistry.org/uri/RegStatus/1001> ;
    a rdf:Property ;
    rdfs:isDefinedBy <http://rdaregistry.info/Elements/u/> ;
    rdfs:label "is interviewee of"@en ;
    rdfs:subPropertyOf <http://rdaregistry.info/Elements/u/P60672> ;
    owl:inverseOf <http://rdaregistry.info/Elements/u/P60432> ;
    skos:definition "Relates an agent responsible for creating a resource by responding to an interviewer, usually a reporter, pollster, or some other information gathering agent to the resource."@en .

<http://rdaregistry.info/Elements/u/P60662>
    reg:hasSubproperty <http://rdaregistry.info/Elements/a/P50151>, <http://rdaregistry.info/Elements/a/P50194> ;
    reg:lexicalAlias <http://rdaregistry.info/Elements/u/choreographerOf.en> ;
    reg:name "choreographerOf"@en ;
    reg:status <http://metadataregistry.org/uri/RegStatus/1001> ;
    a rdf:Property ;
    rdfs:isDefinedBy <http://rdaregistry.info/Elements/u/> ;
    rdfs:label "is choreographer of"@en ;
    rdfs:subPropertyOf <http://rdaregistry.info/Elements/u/P60672> ;
    owl:inverseOf <http://rdaregistry.info/Elements/u/P60433> ;
    skos:definition "Relates an agent responsible for creating a resource of movement to the resource."@en .

<http://rdaregistry.info/Elements/u/P60663>
    reg:hasSubproperty <http://rdaregistry.info/Elements/a/P50195>, <http://rdaregistry.info/Elements/u/P60706>, <http://rdaregistry.info/Elements/u/P60707>, <http://rdaregistry.info/Elements/u/P60708>, <http://rdaregistry.info/Elements/u/P60757> ;
    reg:lexicalAlias <http://rdaregistry.info/Elements/u/authorOf.en> ;
    reg:name "authorOf"@en ;
    reg:status <http://metadataregistry.org/uri/RegStatus/1001> ;
    a rdf:Property ;
    rdfs:isDefinedBy <http://rdaregistry.info/Elements/u/> ;
    rdfs:label "is author of"@en ;
    rdfs:subPropertyOf <http://rdaregistry.info/Elements/u/P60672> ;
    owl:inverseOf <http://rdaregistry.info/Elements/u/P60434> ;
    skos:definition "Relates an agent responsible for creating a resource that is primarily textual in content, regardless of media type (e.g., printed text, spoken word, electronic text, tactile text) or genre (e.g., poems, novels, screenplays, blogs) to the resource."@en .

<http://rdaregistry.info/Elements/u/P60664>
    reg:hasSubproperty <http://rdaregistry.info/Elements/a/P50196>, <http://rdaregistry.info/Elements/u/P60704> ;
    reg:lexicalAlias <http://rdaregistry.info/Elements/u/architectOf.en> ;
    reg:name "architectOf"@en ;
    reg:status <http://metadataregistry.org/uri/RegStatus/1001> ;
    a rdf:Property ;
    rdfs:isDefinedBy <http://rdaregistry.info/Elements/u/> ;
    rdfs:label "is architect of"@en ;
    rdfs:subPropertyOf <http://rdaregistry.info/Elements/u/P60672> ;
    owl:inverseOf <http://rdaregistry.info/Elements/u/P60435> ;
    skos:definition "Relates an agent responsible for creating an architectural design, including a pictorial representation intended to show how a building, etc., will look when completed to the resource."@en .

<http://rdaregistry.info/Elements/u/P60665>
    reg:hasSubproperty <http://rdaregistry.info/Elements/a/P50197> ;
    reg:lexicalAlias <http://rdaregistry.info/Elements/u/filmmakerOf.en> ;
    reg:name "filmmakerOf"@en ;
    reg:status <http://metadataregistry.org/uri/RegStatus/1001> ;
    a rdf:Property ;
    rdfs:isDefinedBy <http://rdaregistry.info/Elements/u/> ;
    rdfs:label "is filmmaker of"@en ;
    rdfs:subPropertyOf <http://rdaregistry.info/Elements/u/P60672> ;
    owl:inverseOf <http://rdaregistry.info/Elements/u/P60436> ;
    skos:definition "Relates an agent responsible for creating an independent or personal film to the resource."@en .

<http://rdaregistry.info/Elements/u/P60666>
    reg:hasSubproperty <http://rdaregistry.info/Elements/a/P50198> ;
    reg:lexicalAlias <http://rdaregistry.info/Elements/u/productionDesignerOf.en> ;
    reg:name "productionDesignerOf"@en ;
    reg:status <http://metadataregistry.org/uri/RegStatus/1001> ;
    a rdf:Property ;
    rdfs:isDefinedBy <http://rdaregistry.info/Elements/u/> ;
    rdfs:label "is production designer of"@en ;
    rdfs:subPropertyOf <http://rdaregistry.info/Elements/u/P60626> ;
    owl:inverseOf <http://rdaregistry.info/Elements/u/P60437> ;
    skos:definition "Relates an agent responsible for designing the overall visual appearance of a moving image production to the resource."@en .

<http://rdaregistry.info/Elements/u/P60667>
    reg:hasSubproperty <http://rdaregistry.info/Elements/a/P50199>, <http://rdaregistry.info/Elements/u/P60636> ;
    reg:lexicalAlias <http://rdaregistry.info/Elements/u/distributorOf.en> ;
    reg:name "distributorOf"@en ;
    reg:status <http://metadataregistry.org/uri/RegStatus/1001> ;
    a rdf:Property ;
    rdfs:isDefinedBy <http://rdaregistry.info/Elements/u/> ;
    rdfs:label "is distributor of"@en ;
    owl:inverseOf <http://rdaregistry.info/Elements/u/P60438> ;
    skos:definition "Relates an agent responsible for distributing a resource to the resource."@en .

<http://rdaregistry.info/Elements/u/P60668>
    reg:hasSubproperty <http://rdaregistry.info/Elements/a/P50201>, <http://rdaregistry.info/Elements/u/P60033>, <http://rdaregistry.info/Elements/u/P60034>, <http://rdaregistry.info/Elements/u/P60035> ;
    reg:lexicalAlias <http://rdaregistry.info/Elements/u/producerOf.en> ;
    reg:name "producerOf"@en ;
    reg:status <http://metadataregistry.org/uri/RegStatus/1001> ;
    a rdf:Property ;
    rdfs:isDefinedBy <http://rdaregistry.info/Elements/u/> ;
    rdfs:label "is producer of"@en ;
    rdfs:subPropertyOf <http://rdaregistry.info/Elements/u/P60602> ;
    owl:inverseOf <http://rdaregistry.info/Elements/u/P60441> ;
    skos:definition "Relates an agent responsible for most of the business aspects of a production for screen, sound recording, television, webcast, etc. the producer is generally responsible for fund raising, managing the production, hiring key personnel, arranging for distributors, etc. to the resource."@en .

<http://rdaregistry.info/Elements/u/P60669>
    reg:hasSubproperty <http://rdaregistry.info/Elements/a/P50202>, <http://rdaregistry.info/Elements/u/P60637>, <http://rdaregistry.info/Elements/u/P60638>, <http://rdaregistry.info/Elements/u/P60639>, <http://rdaregistry.info/Elements/u/P60640>, <http://rdaregistry.info/Elements/u/P60641>, <http://rdaregistry.info/Elements/u/P60642>, <http://rdaregistry.info/Elements/u/P60643>, <http://rdaregistry.info/Elements/u/P60644>, <http://rdaregistry.info/Elements/u/P60645>, <http://rdaregistry.info/Elements/u/P60646>, <http://rdaregistry.info/Elements/u/P60747> ;
    reg:lexicalAlias <http://rdaregistry.info/Elements/u/manufacturerOf.en> ;
    reg:name "manufacturerOf"@en ;
    reg:status <http://metadataregistry.org/uri/RegStatus/1001> ;
    a rdf:Property ;
    rdfs:isDefinedBy <http://rdaregistry.info/Elements/u/> ;
    rdfs:label "is manufacturer of"@en ;
    owl:inverseOf <http://rdaregistry.info/Elements/u/P60443> ;
    skos:definition "Relates an agent responsible for printing, duplicating, casting, etc., a resource in a published form to the resource."@en .

<http://rdaregistry.info/Elements/u/P60670>
    reg:hasSubproperty <http://rdaregistry.info/Elements/a/P50203>, <http://rdaregistry.info/Elements/u/P60635> ;
    reg:lexicalAlias <http://rdaregistry.info/Elements/u/publisherOf.en> ;
    reg:name "publisherOf"@en ;
    reg:status <http://metadataregistry.org/uri/RegStatus/1001> ;
    a rdf:Property ;
    rdfs:isDefinedBy <http://rdaregistry.info/Elements/u/> ;
    rdfs:label "is publisher of"@en ;
    owl:inverseOf <http://rdaregistry.info/Elements/u/P60444> ;
    skos:definition "Relates an agent responsible for publishing, releasing, or issuing a resource to the resource."@en .

<http://rdaregistry.info/Elements/u/P60671>
    reg:hasSubproperty <http://rdaregistry.info/Elements/a/P50212> ;
    reg:lexicalAlias <http://rdaregistry.info/Elements/u/minuteTakerOf.en> ;
    reg:name "minuteTakerOf"@en ;
    reg:status <http://metadataregistry.org/uri/RegStatus/1001> ;
    a rdf:Property ;
    rdfs:isDefinedBy <http://rdaregistry.info/Elements/u/> ;
    rdfs:label "is minute taker of"@en ;
    rdfs:subPropertyOf <http://rdaregistry.info/Elements/u/P60626> ;
    owl:inverseOf <http://rdaregistry.info/Elements/u/P60446> ;
    skos:definition "Relates an agent responsible for recording the minutes of a meeting to the resource."@en .

<http://rdaregistry.info/Elements/u/P60672>
    reg:hasSubproperty <http://rdaregistry.info/Elements/a/P50204>, <http://rdaregistry.info/Elements/u/P60001>, <http://rdaregistry.info/Elements/u/P60014>, <http://rdaregistry.info/Elements/u/P60649>, <http://rdaregistry.info/Elements/u/P60652>, <http://rdaregistry.info/Elements/u/P60653>, <http://rdaregistry.info/Elements/u/P60654>, <http://rdaregistry.info/Elements/u/P60655>, <http://rdaregistry.info/Elements/u/P60656>, <http://rdaregistry.info/Elements/u/P60657>, <http://rdaregistry.info/Elements/u/P60658>, <http://rdaregistry.info/Elements/u/P60659>, <http://rdaregistry.info/Elements/u/P60660>, <http://rdaregistry.info/Elements/u/P60661>, <http://rdaregistry.info/Elements/u/P60662>, <http://rdaregistry.info/Elements/u/P60663>, <http://rdaregistry.info/Elements/u/P60664>, <http://rdaregistry.info/Elements/u/P60665>, <http://rdaregistry.info/Elements/u/P60699>, <http://rdaregistry.info/Elements/u/P60701>, <http://rdaregistry.info/Elements/u/P60827> ;
    reg:lexicalAlias <http://rdaregistry.info/Elements/u/creatorOf.en> ;
    reg:name "creatorOf"@en ;
    reg:status <http://metadataregistry.org/uri/RegStatus/1001> ;
    a rdf:Property ;
    rdfs:isDefinedBy <http://rdaregistry.info/Elements/u/> ;
    rdfs:label "is creator of"@en ;
    owl:inverseOf <http://rdaregistry.info/Elements/u/P60447> ;
    skos:definition "Relates an agent responsible for the creation of a resourc to the resource."@en .

<http://rdaregistry.info/Elements/u/P60673>
    reg:hasSubproperty <http://rdaregistry.info/Elements/a/P50205> ;
    reg:lexicalAlias <http://rdaregistry.info/Elements/u/directorOf.en> ;
    reg:name "directorOf"@en ;
    reg:status <http://metadataregistry.org/uri/RegStatus/1001> ;
    a rdf:Property ;
    rdfs:isDefinedBy <http://rdaregistry.info/Elements/u/> ;
    rdfs:label "is director of"@en ;
    rdfs:subPropertyOf <http://rdaregistry.info/Elements/u/P60602> ;
    owl:inverseOf <http://rdaregistry.info/Elements/u/P60449> ;
    skos:definition "Relates an agent responsible for the general management and supervision of a filmed performance, a radio or television program, etc. to the resource."@en .

<http://rdaregistry.info/Elements/u/P60674>
    reg:hasSubproperty <http://rdaregistry.info/Elements/a/P50206>, <http://rdaregistry.info/Elements/a/P50273> ;
    reg:lexicalAlias <http://rdaregistry.info/Elements/u/restorationistOf.en> ;
    reg:name "restorationistOf"@en ;
    reg:status <http://metadataregistry.org/uri/RegStatus/1001> ;
    a rdf:Property ;
    rdfs:isDefinedBy <http://rdaregistry.info/Elements/u/> ;
    rdfs:label "is restorationist of"@en ;
    rdfs:subPropertyOf <http://rdaregistry.info/Elements/u/P60602> ;
    owl:inverseOf <http://rdaregistry.info/Elements/u/P60450> ;
    skos:definition "Relates an agent responsible for the set of technical, editorial, and intellectual procedures aimed at compensating for the degradation of a resource by bringing it back to a state as close as possible to its original condition to the resource."@en .

<http://rdaregistry.info/Elements/u/P60675>
    reg:hasSubproperty <http://rdaregistry.info/Elements/a/P50226> ;
    reg:lexicalAlias <http://rdaregistry.info/Elements/u/sponsoringBodyOf.en> ;
    reg:name "sponsoringBodyOf"@en ;
    reg:status <http://metadataregistry.org/uri/RegStatus/1001> ;
    a rdf:Property ;
    rdfs:isDefinedBy <http://rdaregistry.info/Elements/u/> ;
    rdfs:label "is sponsoring body of"@en ;
    rdfs:subPropertyOf <http://rdaregistry.info/Elements/u/P60602> ;
    owl:inverseOf <http://rdaregistry.info/Elements/u/P60451> ;
    skos:definition "Relates an agent sponsoring some aspect of a resource, e.g., funding research, sponsoring an event to the resource."@en .

<http://rdaregistry.info/Elements/u/P60676>
    reg:hasSubproperty <http://rdaregistry.info/Elements/a/P50015>, <http://rdaregistry.info/Elements/a/P50021>, <http://rdaregistry.info/Elements/a/P50028> ;
    reg:lexicalAlias <http://rdaregistry.info/Elements/u/sponsor.en> ;
    reg:name "sponsor"@en ;
    reg:status <http://metadataregistry.org/uri/RegStatus/1001> ;
    a rdf:Property ;
    rdfs:isDefinedBy <http://rdaregistry.info/Elements/u/> ;
    rdfs:label "has sponsor"@en ;
    owl:inverseOf <http://rdaregistry.info/Elements/u/P60688> ;
    skos:definition "Relates an agent sponsoring the agent to the agent."@en .

<http://rdaregistry.info/Elements/u/P60678>
    reg:hasSubproperty <http://rdaregistry.info/Elements/a/P50207> ;
    reg:lexicalAlias <http://rdaregistry.info/Elements/u/directorOfPhotographyOf.en> ;
    reg:name "directorOfPhotographyOf"@en ;
    reg:status <http://metadataregistry.org/uri/RegStatus/1001> ;
    a rdf:Property ;
    rdfs:isDefinedBy <http://rdaregistry.info/Elements/u/> ;
    rdfs:label "is director of photography of"@en ;
    rdfs:subPropertyOf <http://rdaregistry.info/Elements/u/P60602> ;
    owl:inverseOf <http://rdaregistry.info/Elements/u/P60452> ;
    skos:definition "Relates an agent that captures images, either electronically or on film or video stock, and often selects and arranges the lighting. the director of photography for a movie is also called the chief cinematographer to the resource."@en .

<http://rdaregistry.info/Elements/u/P60679>
    reg:hasSubproperty <http://rdaregistry.info/Elements/a/P50096> ;
    reg:lexicalAlias <http://rdaregistry.info/Elements/u/employer.en> ;
    reg:name "employer"@en ;
    reg:status <http://metadataregistry.org/uri/RegStatus/1001> ;
    a rdf:Property ;
    rdfs:isDefinedBy <http://rdaregistry.info/Elements/u/> ;
    rdfs:label "has employer"@en ;
    owl:inverseOf <http://rdaregistry.info/Elements/u/P60629> ;
    skos:definition "Relates an agent that employs the agent to the agent."@en .

<http://rdaregistry.info/Elements/u/P60680>
    reg:hasSubproperty <http://rdaregistry.info/Elements/a/P50008> ;
    reg:lexicalAlias <http://rdaregistry.info/Elements/u/hierarchicalSuperior.en> ;
    reg:name "hierarchicalSuperior"@en ;
    reg:status <http://metadataregistry.org/uri/RegStatus/1001> ;
    a rdf:Property ;
    rdfs:isDefinedBy <http://rdaregistry.info/Elements/u/> ;
    rdfs:label "has hierarchical superior"@en ;
    owl:inverseOf <http://rdaregistry.info/Elements/u/P60681> ;
    skos:definition "Relates an agent that is hierarchically superior to the other agent to the agent."@en .

<http://rdaregistry.info/Elements/u/P60681>
    reg:hasSubproperty <http://rdaregistry.info/Elements/a/P50010> ;
    reg:lexicalAlias <http://rdaregistry.info/Elements/u/hierarchicalSubordinate.en> ;
    reg:name "hierarchicalSubordinate"@en ;
    reg:status <http://metadataregistry.org/uri/RegStatus/1001> ;
    a rdf:Property ;
    rdfs:isDefinedBy <http://rdaregistry.info/Elements/u/> ;
    rdfs:label "has hierarchical subordinate"@en ;
    owl:inverseOf <http://rdaregistry.info/Elements/u/P60680> ;
    skos:definition "Relates an agent that is subordinate to the other agent to the agent."@en .

<http://rdaregistry.info/Elements/u/P60682>
    reg:hasSubproperty <http://rdaregistry.info/Elements/a/P50011> ;
    reg:lexicalAlias <http://rdaregistry.info/Elements/u/mergee.en> ;
    reg:name "mergee"@en ;
    reg:status <http://metadataregistry.org/uri/RegStatus/1001> ;
    a rdf:Property ;
    rdfs:isDefinedBy <http://rdaregistry.info/Elements/u/> ;
    rdfs:label "has mergee"@en ;
    owl:inverseOf <http://rdaregistry.info/Elements/u/P60682> ;
    skos:definition "Relates a agent that merged with the other agent to form a third to the agent."@en .

<http://rdaregistry.info/Elements/u/P60683>
    reg:hasSubproperty <http://rdaregistry.info/Elements/a/P50012>, <http://rdaregistry.info/Elements/a/P50055> ;
    reg:lexicalAlias <http://rdaregistry.info/Elements/u/predecessor.en> ;
    reg:name "predecessor"@en ;
    reg:status <http://metadataregistry.org/uri/RegStatus/1001> ;
    a rdf:Property ;
    rdfs:isDefinedBy <http://rdaregistry.info/Elements/u/> ;
    rdfs:label "has predecessor"@en ;
    owl:inverseOf <http://rdaregistry.info/Elements/u/P60686> ;
    skos:definition "Relates an agent that precedes the other agent to the agent."@en .

<http://rdaregistry.info/Elements/u/P60684>
    reg:hasSubproperty <http://rdaregistry.info/Elements/a/P50013> ;
    reg:lexicalAlias <http://rdaregistry.info/Elements/u/productOfAMerger.en> ;
    reg:name "productOfAMerger"@en ;
    reg:status <http://metadataregistry.org/uri/RegStatus/1001> ;
    a rdf:Property ;
    rdfs:isDefinedBy <http://rdaregistry.info/Elements/u/> ;
    rdfs:label "has product of merger"@en ;
    owl:inverseOf <http://rdaregistry.info/Elements/u/P60736> ;
    skos:definition "Relates a agent that resulted from a merger of two or more other agents to the agent."@en .

<http://rdaregistry.info/Elements/u/P60685>
    reg:hasSubproperty <http://rdaregistry.info/Elements/a/P50014> ;
    reg:lexicalAlias <http://rdaregistry.info/Elements/u/productOfASplit.en> ;
    reg:name "productOfASplit"@en ;
    reg:status <http://metadataregistry.org/uri/RegStatus/1001> ;
    a rdf:Property ;
    rdfs:isDefinedBy <http://rdaregistry.info/Elements/u/> ;
    rdfs:label "has product of split"@en ;
    owl:inverseOf <http://rdaregistry.info/Elements/u/P60733> ;
    skos:definition "Relates a agent that resulted from a split or division of the other agent to the agent."@en .

<http://rdaregistry.info/Elements/u/P60686>
    reg:hasSubproperty <http://rdaregistry.info/Elements/a/P50016>, <http://rdaregistry.info/Elements/a/P50053>, <http://rdaregistry.info/Elements/a/P50099> ;
    reg:lexicalAlias <http://rdaregistry.info/Elements/u/successor.en> ;
    reg:name "successor"@en ;
    reg:status <http://metadataregistry.org/uri/RegStatus/1001> ;
    a rdf:Property ;
    rdfs:isDefinedBy <http://rdaregistry.info/Elements/u/> ;
    rdfs:label "has successor"@en ;
    owl:inverseOf <http://rdaregistry.info/Elements/u/P60683> ;
    skos:definition "Relates an agent that succeeds or follows the other agent to the agent."@en .

<http://rdaregistry.info/Elements/u/P60687>
    reg:hasSubproperty <http://rdaregistry.info/Elements/a/P50017>, <http://rdaregistry.info/Elements/a/P50062>, <http://rdaregistry.info/Elements/a/P50112> ;
    reg:lexicalAlias <http://rdaregistry.info/Elements/u/foundedEntity.en> ;
    reg:name "foundedEntity"@en ;
    reg:status <http://metadataregistry.org/uri/RegStatus/1001> ;
    a rdf:Property ;
    rdfs:isDefinedBy <http://rdaregistry.info/Elements/u/> ;
    rdfs:label "has founded entity"@en ;
    owl:inverseOf <http://rdaregistry.info/Elements/u/P60694> ;
    skos:definition "Relates an agent that the agent founded to the agent."@en .

<http://rdaregistry.info/Elements/u/P60688>
    reg:hasSubproperty <http://rdaregistry.info/Elements/a/P50009>, <http://rdaregistry.info/Elements/a/P50063> ;
    reg:lexicalAlias <http://rdaregistry.info/Elements/u/sponsoredEntity.en> ;
    reg:name "sponsoredEntity"@en ;
    reg:status <http://metadataregistry.org/uri/RegStatus/1001> ;
    a rdf:Property ;
    rdfs:isDefinedBy <http://rdaregistry.info/Elements/u/> ;
    rdfs:label "has sponsored entity"@en ;
    owl:inverseOf <http://rdaregistry.info/Elements/u/P60676> ;
    skos:definition "Relates an agent that the agent sponsors to the agent."@en .

<http://rdaregistry.info/Elements/u/P60689>
    reg:hasSubproperty <http://rdaregistry.info/Elements/a/P50208>, <http://rdaregistry.info/Elements/a/P50210> ;
    reg:lexicalAlias <http://rdaregistry.info/Elements/u/dedicateeOf.en> ;
    reg:name "dedicateeOf"@en ;
    reg:status <http://metadataregistry.org/uri/RegStatus/1001> ;
    a rdf:Property ;
    rdfs:isDefinedBy <http://rdaregistry.info/Elements/u/> ;
    rdfs:label "is dedicatee of"@en ;
    rdfs:subPropertyOf <http://rdaregistry.info/Elements/u/P60602> ;
    owl:inverseOf <http://rdaregistry.info/Elements/u/P60455> ;
    skos:definition "Relates an agent to whom a resource is dedicated to the resource."@en .

<http://rdaregistry.info/Elements/u/P60690>
    reg:hasSubproperty <http://rdaregistry.info/Elements/a/P50209> ;
    reg:lexicalAlias <http://rdaregistry.info/Elements/u/addresseeOf.en> ;
    reg:name "addresseeOf"@en ;
    reg:status <http://metadataregistry.org/uri/RegStatus/1001> ;
    a rdf:Property ;
    rdfs:isDefinedBy <http://rdaregistry.info/Elements/u/> ;
    rdfs:label "is addressee of"@en ;
    rdfs:subPropertyOf <http://rdaregistry.info/Elements/u/P60602> ;
    owl:inverseOf <http://rdaregistry.info/Elements/u/P60456> ;
    skos:definition "Relates an agent to whom a resource or part of a resource is addressed to the resource."@en .

<http://rdaregistry.info/Elements/u/P60691>
    reg:hasSubproperty <http://rdaregistry.info/Elements/a/P50042>, <http://rdaregistry.info/Elements/a/P50088>, <http://rdaregistry.info/Elements/a/P50122> ;
    reg:lexicalAlias <http://rdaregistry.info/Elements/u/appellantOf.en> ;
    reg:name "appellantOf"@en ;
    reg:status <http://metadataregistry.org/uri/RegStatus/1001> ;
    a rdf:Property ;
    rdfs:isDefinedBy <http://rdaregistry.info/Elements/u/> ;
    rdfs:label "is appellant of"@en ;
    rdfs:subPropertyOf <http://rdaregistry.info/Elements/u/P60602> ;
    owl:inverseOf <http://rdaregistry.info/Elements/u/P60457> ;
    skos:definition "Relates an agent who appeals the decision of a lower court recorded in a legal resource of a higher court to the resource."@en .

<http://rdaregistry.info/Elements/u/P60692>
    reg:hasSubproperty <http://rdaregistry.info/Elements/a/P50123> ;
    reg:lexicalAlias <http://rdaregistry.info/Elements/u/binderOf.en> ;
    reg:name "binderOf"@en ;
    reg:status <http://metadataregistry.org/uri/RegStatus/1001> ;
    a rdf:Property ;
    rdfs:isDefinedBy <http://rdaregistry.info/Elements/u/> ;
    rdfs:label "is binder of"@en ;
    rdfs:subPropertyOf <http://rdaregistry.info/Elements/u/P60602> ;
    owl:inverseOf <http://rdaregistry.info/Elements/u/P60458> ;
    skos:definition "Relates an agent who binds a resource to the resource."@en .

<http://rdaregistry.info/Elements/u/P60693>
    reg:hasSubproperty <http://rdaregistry.info/Elements/a/P50043>, <http://rdaregistry.info/Elements/a/P50089>, <http://rdaregistry.info/Elements/a/P50124> ;
    reg:lexicalAlias <http://rdaregistry.info/Elements/u/plaintiffOf.en> ;
    reg:name "plaintiffOf"@en ;
    reg:status <http://metadataregistry.org/uri/RegStatus/1001> ;
    a rdf:Property ;
    rdfs:isDefinedBy <http://rdaregistry.info/Elements/u/> ;
    rdfs:label "is plaintiff of"@en ;
    rdfs:subPropertyOf <http://rdaregistry.info/Elements/u/P60602> ;
    owl:inverseOf <http://rdaregistry.info/Elements/u/P60459> ;
    skos:definition "Relates an agent who brings a suit in a civil proceeding to the resource."@en .

<http://rdaregistry.info/Elements/u/P60694>
    reg:hasSubproperty <http://rdaregistry.info/Elements/a/P50007>, <http://rdaregistry.info/Elements/a/P50020>, <http://rdaregistry.info/Elements/a/P50029> ;
    reg:lexicalAlias <http://rdaregistry.info/Elements/u/founder.en> ;
    reg:name "founder"@en ;
    reg:status <http://metadataregistry.org/uri/RegStatus/1001> ;
    a rdf:Property ;
    rdfs:isDefinedBy <http://rdaregistry.info/Elements/u/> ;
    rdfs:label "has founder"@en ;
    owl:inverseOf <http://rdaregistry.info/Elements/u/P60687> ;
    skos:definition "Relates an agent who founded the agent to the agent."@en .

<http://rdaregistry.info/Elements/u/P60695>
    reg:hasSubproperty <http://rdaregistry.info/Elements/a/P50125> ;
    reg:lexicalAlias <http://rdaregistry.info/Elements/u/inscriberOf.en> ;
    reg:name "inscriberOf"@en ;
    reg:status <http://metadataregistry.org/uri/RegStatus/1001> ;
    a rdf:Property ;
    rdfs:isDefinedBy <http://rdaregistry.info/Elements/u/> ;
    rdfs:label "is inscriber of"@en ;
    rdfs:subPropertyOf <http://rdaregistry.info/Elements/u/P60602> ;
    owl:inverseOf <http://rdaregistry.info/Elements/u/P60460> ;
    skos:definition "Relates an agent who has written a statement of dedication or gift on a resource to the resource."@en .

<http://rdaregistry.info/Elements/u/P60696>
    reg:hasSubproperty <http://rdaregistry.info/Elements/a/P50126> ;
    reg:lexicalAlias <http://rdaregistry.info/Elements/u/judgeOf.en> ;
    reg:name "judgeOf"@en ;
    reg:status <http://metadataregistry.org/uri/RegStatus/1001> ;
    a rdf:Property ;
    rdfs:isDefinedBy <http://rdaregistry.info/Elements/u/> ;
    rdfs:label "is judge of"@en ;
    rdfs:subPropertyOf <http://rdaregistry.info/Elements/u/P60602> ;
    owl:inverseOf <http://rdaregistry.info/Elements/u/P60461> ;
    skos:definition "Relates an agent who hears and decides on legal matters in court to the resource."@en .

<http://rdaregistry.info/Elements/u/P60697>
    reg:hasSubproperty <http://rdaregistry.info/Elements/a/P50030>, <http://rdaregistry.info/Elements/a/P50231>, <http://rdaregistry.info/Elements/a/P50233> ;
    reg:lexicalAlias <http://rdaregistry.info/Elements/u/member.en> ;
    reg:name "member"@en ;
    reg:status <http://metadataregistry.org/uri/RegStatus/1001> ;
    a rdf:Property ;
    rdfs:isDefinedBy <http://rdaregistry.info/Elements/u/> ;
    rdfs:label "has member"@en ;
    owl:inverseOf <http://rdaregistry.info/Elements/u/P60648> ;
    skos:definition "Relates an agent who is a member of the agent to the agent."@en .

<http://rdaregistry.info/Elements/u/P60698>
    reg:hasSubproperty <http://rdaregistry.info/Elements/a/P50090>, <http://rdaregistry.info/Elements/a/P50258>, <http://rdaregistry.info/Elements/a/P50259> ;
    reg:lexicalAlias <http://rdaregistry.info/Elements/u/defendantOf.en> ;
    reg:name "defendantOf"@en ;
    reg:status <http://metadataregistry.org/uri/RegStatus/1001> ;
    a rdf:Property ;
    rdfs:isDefinedBy <http://rdaregistry.info/Elements/u/> ;
    rdfs:label "is defendant of"@en ;
    rdfs:subPropertyOf <http://rdaregistry.info/Elements/u/P60602> ;
    owl:inverseOf <http://rdaregistry.info/Elements/u/P60462> ;
    skos:definition "Relates an agent who is accused in a criminal proceeding or sued in a civil proceeding to the resource."@en .

<http://rdaregistry.info/Elements/u/P60699>
    reg:hasSubproperty <http://rdaregistry.info/Elements/a/P50127> ;
    reg:lexicalAlias <http://rdaregistry.info/Elements/u/praesesOf.en> ;
    reg:name "praesesOf"@en ;
    reg:status <http://metadataregistry.org/uri/RegStatus/1001> ;
    a rdf:Property ;
    rdfs:isDefinedBy <http://rdaregistry.info/Elements/u/> ;
    rdfs:label "is praeses of"@en ;
    rdfs:subPropertyOf <http://rdaregistry.info/Elements/u/P60672> ;
    owl:inverseOf <http://rdaregistry.info/Elements/u/P60463> ;
    skos:definition "Relates an agent who is the faculty moderator of an academic disputation, normally proposing a thesis and participating in the ensuing disputation to the resource."@en .

<http://rdaregistry.info/Elements/u/P60700>
    reg:hasSubproperty <http://rdaregistry.info/Elements/a/P50128> ;
    reg:lexicalAlias <http://rdaregistry.info/Elements/u/annotatorOf.en> ;
    reg:name "annotatorOf"@en ;
    reg:status <http://metadataregistry.org/uri/RegStatus/1001> ;
    a rdf:Property ;
    rdfs:isDefinedBy <http://rdaregistry.info/Elements/u/> ;
    rdfs:label "is annotator of"@en ;
    rdfs:subPropertyOf <http://rdaregistry.info/Elements/u/P60602> ;
    owl:inverseOf <http://rdaregistry.info/Elements/u/P60464> ;
    skos:definition "Relates an agent who makes manuscript annotations on a resource to the resource."@en .

<http://rdaregistry.info/Elements/u/P60701>
    reg:hasSubproperty <http://rdaregistry.info/Elements/a/P50211> ;
    reg:lexicalAlias <http://rdaregistry.info/Elements/u/consultantOf.en> ;
    reg:name "consultantOf"@en ;
    reg:status <http://metadataregistry.org/uri/RegStatus/1001> ;
    a rdf:Property ;
    rdfs:isDefinedBy <http://rdaregistry.info/Elements/u/> ;
    rdfs:label "is consultant of"@en ;
    rdfs:subPropertyOf <http://rdaregistry.info/Elements/u/P60672> ;
    owl:inverseOf <http://rdaregistry.info/Elements/u/P60465> ;
    skos:definition "Relates an agent who provides consultation services, and often makes recommendations, for another person, family or corporate body that is represented as the creator of a resource to the resource."@en .

<http://rdaregistry.info/Elements/u/P60702>
    reg:hasSubproperty <http://rdaregistry.info/Elements/a/P50129> ;
    reg:lexicalAlias <http://rdaregistry.info/Elements/u/autographerOf.en> ;
    reg:name "autographerOf"@en ;
    reg:status <http://metadataregistry.org/uri/RegStatus/1001> ;
    a rdf:Property ;
    rdfs:isDefinedBy <http://rdaregistry.info/Elements/u/> ;
    rdfs:label "is autographer of"@en ;
    rdfs:subPropertyOf <http://rdaregistry.info/Elements/u/P60602> ;
    owl:inverseOf <http://rdaregistry.info/Elements/u/P60466> ;
    skos:definition "Relates an agent whose manuscript signature appears on a resource to the resource."@en .

<http://rdaregistry.info/Elements/u/P60703>
    reg:hasSubproperty <http://rdaregistry.info/Elements/a/P50130> ;
    reg:lexicalAlias <http://rdaregistry.info/Elements/u/issuingBodyOf.en> ;
    reg:name "issuingBodyOf"@en ;
    reg:status <http://metadataregistry.org/uri/RegStatus/1001> ;
    a rdf:Property ;
    rdfs:isDefinedBy <http://rdaregistry.info/Elements/u/> ;
    rdfs:label "is issuing body of"@en ;
    rdfs:subPropertyOf <http://rdaregistry.info/Elements/u/P60602> ;
    owl:inverseOf <http://rdaregistry.info/Elements/u/P60467> ;
    skos:definition "Relates an agent, family or corporate body issuing a resource, such as an official organ of the body to the resource."@en .

<http://rdaregistry.info/Elements/u/P60704>
    reg:hasSubproperty <http://rdaregistry.info/Elements/a/P50221> ;
    reg:lexicalAlias <http://rdaregistry.info/Elements/u/landscapeArchitectOf.en> ;
    reg:name "landscapeArchitectOf"@en ;
    reg:status <http://metadataregistry.org/uri/RegStatus/1001> ;
    a rdf:Property ;
    rdfs:isDefinedBy <http://rdaregistry.info/Elements/u/> ;
    rdfs:label "is landscape architect of"@en ;
    rdfs:subPropertyOf <http://rdaregistry.info/Elements/u/P60664> ;
    owl:inverseOf <http://rdaregistry.info/Elements/u/P60473> ;
    skos:definition "Relates an architect responsible for creating landscape resources to the resource."@en .

<http://rdaregistry.info/Elements/u/P60705>
    reg:hasSubproperty <http://rdaregistry.info/Elements/a/P50222> ;
    reg:lexicalAlias <http://rdaregistry.info/Elements/u/sculptorOf.en> ;
    reg:name "sculptorOf"@en ;
    reg:status <http://metadataregistry.org/uri/RegStatus/1001> ;
    a rdf:Property ;
    rdfs:isDefinedBy <http://rdaregistry.info/Elements/u/> ;
    rdfs:label "is sculptor of"@en ;
    rdfs:subPropertyOf <http://rdaregistry.info/Elements/u/P60660> ;
    owl:inverseOf <http://rdaregistry.info/Elements/u/P60475> ;
    skos:definition "Relates an artist responsible for creating a three-dimensional resource by modeling, carving, or similar technique to the resource."@en .

<http://rdaregistry.info/Elements/u/P60706>
    reg:hasSubproperty <http://rdaregistry.info/Elements/a/P50223> ;
    reg:lexicalAlias <http://rdaregistry.info/Elements/u/screenwriterOf.en> ;
    reg:name "screenwriterOf"@en ;
    reg:status <http://metadataregistry.org/uri/RegStatus/1001> ;
    a rdf:Property ;
    rdfs:isDefinedBy <http://rdaregistry.info/Elements/u/> ;
    rdfs:label "is screenwriter of"@en ;
    rdfs:subPropertyOf <http://rdaregistry.info/Elements/u/P60663> ;
    owl:inverseOf <http://rdaregistry.info/Elements/u/P60476> ;
    skos:definition "Relates an author of a screenplay, script, or scene to the resource."@en .

<http://rdaregistry.info/Elements/u/P60707>
    reg:hasSubproperty <http://rdaregistry.info/Elements/a/P50224> ;
    reg:lexicalAlias <http://rdaregistry.info/Elements/u/lyricistOf.en> ;
    reg:name "lyricistOf"@en ;
    reg:status <http://metadataregistry.org/uri/RegStatus/1001> ;
    a rdf:Property ;
    rdfs:isDefinedBy <http://rdaregistry.info/Elements/u/> ;
    rdfs:label "is lyricist of"@en ;
    rdfs:subPropertyOf <http://rdaregistry.info/Elements/u/P60663> ;
    owl:inverseOf <http://rdaregistry.info/Elements/u/P60477> ;
    skos:definition "Relates an author of the words of a popular song, including a song or songs from a musical to the resource."@en .

<http://rdaregistry.info/Elements/u/P60708>
    reg:hasSubproperty <http://rdaregistry.info/Elements/a/P50225> ;
    reg:lexicalAlias <http://rdaregistry.info/Elements/u/librettistOf.en> ;
    reg:name "librettistOf"@en ;
    reg:status <http://metadataregistry.org/uri/RegStatus/1001> ;
    a rdf:Property ;
    rdfs:isDefinedBy <http://rdaregistry.info/Elements/u/> ;
    rdfs:label "is librettist of"@en ;
    rdfs:subPropertyOf <http://rdaregistry.info/Elements/u/P60663> ;
    owl:inverseOf <http://rdaregistry.info/Elements/u/P60478> ;
    skos:definition "Relates an author of the words of an opera or other musical stage resource or an oratorio to the resource."@en .

<http://rdaregistry.info/Elements/u/P60709>
    reg:hasSubproperty <http://rdaregistry.info/Elements/e/P20232>, <http://rdaregistry.info/Elements/i/P40051>, <http://rdaregistry.info/Elements/m/P30210>, <http://rdaregistry.info/Elements/u/P60196>, <http://rdaregistry.info/Elements/u/P60198>, <http://rdaregistry.info/Elements/u/P60204>, <http://rdaregistry.info/Elements/u/P60307> ;
    reg:lexicalAlias <http://rdaregistry.info/Elements/u/accompanyingResourceRelationshipWith.en> ;
    reg:name "accompanyingResourceRelationshipWith"@en ;
    reg:status <http://metadataregistry.org/uri/RegStatus/1001> ;
    a rdf:Property ;
    rdfs:isDefinedBy <http://rdaregistry.info/Elements/u/> ;
    rdfs:label "has accompanying resource relationship with"@en ;
    owl:inverseOf <http://rdaregistry.info/Elements/u/P60709> ;
    skos:definition "Relates a resource to a resource that is an augmentation of, or is augmented by, or is complemented by, or accompanies, or is accompanied by the resource."@en .

<http://rdaregistry.info/Elements/u/P60710>
    reg:hasSubproperty <http://rdaregistry.info/Elements/e/P20233>, <http://rdaregistry.info/Elements/u/P60250>, <http://rdaregistry.info/Elements/u/P60305> ;
    reg:lexicalAlias <http://rdaregistry.info/Elements/u/derivativeResourceRelationshipWith.en> ;
    reg:name "derivativeResourceRelationshipWith"@en ;
    reg:status <http://metadataregistry.org/uri/RegStatus/1001> ;
    a rdf:Property ;
    rdfs:isDefinedBy <http://rdaregistry.info/Elements/u/> ;
    rdfs:label "has derivative resource relationship with"@en ;
    owl:inverseOf <http://rdaregistry.info/Elements/u/P60710> ;
    skos:definition "Relates a resource to a resource that is based on or is a derivative of the resource."@en .

<http://rdaregistry.info/Elements/u/P60711>
    reg:hasSubproperty <http://rdaregistry.info/Elements/u/P60190>, <http://rdaregistry.info/Elements/u/P60215> ;
    reg:status <http://metadataregistry.org/uri/RegStatus/1008> ;
    rdfs:isDefinedBy <http://rdaregistry.info/Elements/u/> .

<http://rdaregistry.info/Elements/u/P60712>
    reg:hasSubproperty <http://rdaregistry.info/Elements/i/P40053>, <http://rdaregistry.info/Elements/m/P30212>, <http://rdaregistry.info/Elements/u/P60191> ;
    reg:lexicalAlias <http://rdaregistry.info/Elements/u/equivalentResourceRelationshipWith.en> ;
    reg:name "equivalentResourceRelationshipWith"@en ;
    reg:status <http://metadataregistry.org/uri/RegStatus/1001> ;
    a rdf:Property ;
    rdfs:isDefinedBy <http://rdaregistry.info/Elements/u/> ;
    rdfs:label "has equivalent resource relationship with"@en ;
    owl:inverseOf <http://rdaregistry.info/Elements/u/P60712> ;
    skos:definition "Relates a resource to a resource that is equivalent to the resource."@en .

<http://rdaregistry.info/Elements/u/P60713>
    reg:hasSubproperty <http://rdaregistry.info/Elements/e/P20235>, <http://rdaregistry.info/Elements/u/P60261>, <http://rdaregistry.info/Elements/u/P60278> ;
    reg:lexicalAlias <http://rdaregistry.info/Elements/u/sequentialResourceRelationshipWith.en> ;
    reg:name "sequentialResourceRelationshipWith"@en ;
    reg:status <http://metadataregistry.org/uri/RegStatus/1001> ;
    a rdf:Property ;
    rdfs:isDefinedBy <http://rdaregistry.info/Elements/u/> ;
    rdfs:label "has sequential resource relationship with"@en ;
    owl:inverseOf <http://rdaregistry.info/Elements/u/P60713> ;
    skos:definition "Relates a resource to a resource that is preceded by or succeeded by the resource."@en .

<http://rdaregistry.info/Elements/u/P60714>
    reg:hasSubproperty <http://rdaregistry.info/Elements/e/P20236>, <http://rdaregistry.info/Elements/i/P40054>, <http://rdaregistry.info/Elements/m/P30213>, <http://rdaregistry.info/Elements/u/P60101>, <http://rdaregistry.info/Elements/u/P60249> ;
    reg:lexicalAlias <http://rdaregistry.info/Elements/u/wholePartResourceRelationshipWith.en> ;
    reg:name "wholePartResourceRelationshipWith"@en ;
    reg:status <http://metadataregistry.org/uri/RegStatus/1001> ;
    a rdf:Property ;
    rdfs:isDefinedBy <http://rdaregistry.info/Elements/u/> ;
    rdfs:label "has whole-part resource relationship with"@en ;
    owl:inverseOf <http://rdaregistry.info/Elements/u/P60714> ;
    skos:definition "Relates a resource to a resource that is contained in or contains the resource."@en .

<http://rdaregistry.info/Elements/u/P60715>
    reg:hasSubproperty <http://rdaregistry.info/Elements/e/P20237> ;
    reg:lexicalAlias <http://rdaregistry.info/Elements/u/writerOfAfterword.en> ;
    reg:name "writerOfAfterword"@en ;
    reg:status <http://metadataregistry.org/uri/RegStatus/1001> ;
    a rdf:Property ;
    rdfs:isDefinedBy <http://rdaregistry.info/Elements/u/> ;
    rdfs:label "has writer of afterword"@en ;
    rdfs:subPropertyOf <http://rdaregistry.info/Elements/u/P60392> ;
    owl:inverseOf <http://rdaregistry.info/Elements/u/P60717> ;
    skos:definition "Relates a resource to an agent contributing to a resource by providing an afterword to the original resource."@en .

<http://rdaregistry.info/Elements/u/P60716>
    reg:hasSubproperty <http://rdaregistry.info/Elements/e/P20238> ;
    reg:lexicalAlias <http://rdaregistry.info/Elements/u/writerOfPostface.en> ;
    reg:name "writerOfPostface"@en ;
    reg:status <http://metadataregistry.org/uri/RegStatus/1001> ;
    a rdf:Property ;
    rdfs:isDefinedBy <http://rdaregistry.info/Elements/u/> ;
    rdfs:label "has writer of postface"@en ;
    rdfs:subPropertyOf <http://rdaregistry.info/Elements/u/P60392> ;
    owl:inverseOf <http://rdaregistry.info/Elements/u/P60718> ;
    skos:definition "Relates a resource to an agent contributing to a resource by providing a postface to the original resource."@en .

<http://rdaregistry.info/Elements/u/P60717>
    reg:hasSubproperty <http://rdaregistry.info/Elements/a/P50227> ;
    reg:lexicalAlias <http://rdaregistry.info/Elements/u/writerOfAfterwordOf.en> ;
    reg:name "writerOfAfterwordOf"@en ;
    reg:status <http://metadataregistry.org/uri/RegStatus/1001> ;
    a rdf:Property ;
    rdfs:isDefinedBy <http://rdaregistry.info/Elements/u/> ;
    rdfs:label "is writer of preface of"@en ;
    rdfs:subPropertyOf <http://rdaregistry.info/Elements/u/P60620> ;
    owl:inverseOf <http://rdaregistry.info/Elements/u/P60715> ;
    skos:definition "Relates an agent contributing to a resource by providing a preface to the original resource to the resource."@en .

<http://rdaregistry.info/Elements/u/P60718>
    reg:hasSubproperty <http://rdaregistry.info/Elements/a/P50228> ;
    reg:lexicalAlias <http://rdaregistry.info/Elements/u/writerOfPostfaceOf.en> ;
    reg:name "writerOfPostfaceOf"@en ;
    reg:status <http://metadataregistry.org/uri/RegStatus/1001> ;
    a rdf:Property ;
    rdfs:isDefinedBy <http://rdaregistry.info/Elements/u/> ;
    rdfs:label "is writer of supplementary textual content of"@en ;
    rdfs:subPropertyOf <http://rdaregistry.info/Elements/u/P60620> ;
    owl:inverseOf <http://rdaregistry.info/Elements/u/P60716> ;
    skos:definition "Relates an agent contributing to a resource by providing supplementary textual content (e.g., an appendix, an introduction, a preface) to the original resource to the resource."@en .

<http://rdaregistry.info/Elements/u/P60719>
    reg:hasSubproperty <http://rdaregistry.info/Elements/e/P20239> ;
    reg:lexicalAlias <http://rdaregistry.info/Elements/u/musicalTheatreAdaptationOf.en> ;
    reg:name "musicalTheatreAdaptationOf"@en ;
    reg:status <http://metadataregistry.org/uri/RegStatus/1001> ;
    a rdf:Property ;
    rdfs:isDefinedBy <http://rdaregistry.info/Elements/u/> ;
    rdfs:label "is musical theatre adaptation of"@en ;
    rdfs:subPropertyOf <http://rdaregistry.info/Elements/u/P60241> ;
    owl:inverseOf <http://rdaregistry.info/Elements/u/P60721> ;
    skos:definition "Relates a resource to a resource that has been adapted as a musical theatre resource."@en .

<http://rdaregistry.info/Elements/u/P60720>
    reg:hasSubproperty <http://rdaregistry.info/Elements/e/P20240> ;
    reg:lexicalAlias <http://rdaregistry.info/Elements/u/operaAdaptationOf.en> ;
    reg:name "operaAdaptationOf"@en ;
    reg:status <http://metadataregistry.org/uri/RegStatus/1001> ;
    a rdf:Property ;
    rdfs:isDefinedBy <http://rdaregistry.info/Elements/u/> ;
    rdfs:label "is opera adaptation of"@en ;
    rdfs:subPropertyOf <http://rdaregistry.info/Elements/u/P60241> ;
    owl:inverseOf <http://rdaregistry.info/Elements/u/P60722> ;
    skos:definition "Relates a resource to a resource that has been adapted as opera."@en .

<http://rdaregistry.info/Elements/u/P60721>
    reg:hasSubproperty <http://rdaregistry.info/Elements/e/P20241> ;
    reg:lexicalAlias <http://rdaregistry.info/Elements/u/adaptedAsMusicalTheatre.en> ;
    reg:name "adaptedAsMusicalTheatre"@en ;
    reg:status <http://metadataregistry.org/uri/RegStatus/1001> ;
    a rdf:Property ;
    rdfs:isDefinedBy <http://rdaregistry.info/Elements/u/> ;
    rdfs:label "is adapted as musical theatre"@en ;
    rdfs:subPropertyOf <http://rdaregistry.info/Elements/u/P60260> ;
    owl:inverseOf <http://rdaregistry.info/Elements/u/P60719> ;
    skos:definition "Relates a resource to a musical theatre resource based on the source resource."@en .

<http://rdaregistry.info/Elements/u/P60722>
    reg:hasSubproperty <http://rdaregistry.info/Elements/e/P20242> ;
    reg:lexicalAlias <http://rdaregistry.info/Elements/u/adaptedAsOpera.en> ;
    reg:name "adaptedAsOpera"@en ;
    reg:status <http://metadataregistry.org/uri/RegStatus/1001> ;
    a rdf:Property ;
    rdfs:isDefinedBy <http://rdaregistry.info/Elements/u/> ;
    rdfs:label "is adapted as opera"@en ;
    rdfs:subPropertyOf <http://rdaregistry.info/Elements/u/P60260> ;
    owl:inverseOf <http://rdaregistry.info/Elements/u/P60720> ;
    skos:definition "Relates a resource to an opera based on the source resource."@en .

<http://rdaregistry.info/Elements/u/P60723>
    reg:hasSubproperty <http://rdaregistry.info/Elements/e/P20243>, <http://rdaregistry.info/Elements/u/P60118>, <http://rdaregistry.info/Elements/w/P10237> ;
    reg:lexicalAlias <http://rdaregistry.info/Elements/u/music.en> ;
    reg:name "music"@en ;
    reg:status <http://metadataregistry.org/uri/RegStatus/1001> ;
    a rdf:Property ;
    rdfs:isDefinedBy <http://rdaregistry.info/Elements/u/> ;
    rdfs:label "is music"@en ;
    rdfs:subPropertyOf <http://rdaregistry.info/Elements/u/P60198> ;
    owl:inverseOf <http://rdaregistry.info/Elements/u/P60724> ;
    skos:definition "Relates a resource to a musical resource that is used in a motion picture, play, television program, etc."@en .

<http://rdaregistry.info/Elements/u/P60724>
    reg:hasSubproperty <http://rdaregistry.info/Elements/e/P20244>, <http://rdaregistry.info/Elements/u/P60202>, <http://rdaregistry.info/Elements/w/P10238> ;
    reg:lexicalAlias <http://rdaregistry.info/Elements/u/musicFor.en> ;
    reg:name "musicFor"@en ;
    reg:status <http://metadataregistry.org/uri/RegStatus/1001> ;
    a rdf:Property ;
    rdfs:isDefinedBy <http://rdaregistry.info/Elements/u/> ;
    rdfs:label "is music for"@en ;
    rdfs:subPropertyOf <http://rdaregistry.info/Elements/u/P60198> ;
    owl:inverseOf <http://rdaregistry.info/Elements/u/P60723> ;
    skos:definition "Relates a resource to a resource such as a motion picture, play, television program, etc. that uses the musical resource."@en .

<http://rdaregistry.info/Elements/u/P60725>
    reg:hasSubproperty <http://rdaregistry.info/Elements/e/P20245> ;
    reg:lexicalAlias <http://rdaregistry.info/Elements/u/videoMusic.en> ;
    reg:name "videoMusic"@en ;
    reg:status <http://metadataregistry.org/uri/RegStatus/1001> ;
    a rdf:Property ;
    rdfs:isDefinedBy <http://rdaregistry.info/Elements/u/> ;
    rdfs:label "is video music"@en ;
    rdfs:subPropertyOf <http://rdaregistry.info/Elements/u/P60723> ;
    owl:inverseOf <http://rdaregistry.info/Elements/u/P60726> ;
    skos:definition "Relates a resource to a musical resource that is used in a video."@en .

<http://rdaregistry.info/Elements/u/P60726>
    reg:hasSubproperty <http://rdaregistry.info/Elements/e/P20246> ;
    reg:lexicalAlias <http://rdaregistry.info/Elements/u/musicForVideo.en> ;
    reg:name "musicForVideo"@en ;
    reg:status <http://metadataregistry.org/uri/RegStatus/1001> ;
    a rdf:Property ;
    rdfs:isDefinedBy <http://rdaregistry.info/Elements/u/> ;
    rdfs:label "is music for video"@en ;
    rdfs:subPropertyOf <http://rdaregistry.info/Elements/u/P60724> ;
    owl:inverseOf <http://rdaregistry.info/Elements/u/P60725> ;
    skos:definition "Relates a resource to a resource that uses the musical resource in a video."@en .

<http://rdaregistry.info/Elements/u/P60727>
    reg:hasSubproperty <http://rdaregistry.info/Elements/e/P20247> ;
    reg:lexicalAlias <http://rdaregistry.info/Elements/u/televisionProgramMusic.en> ;
    reg:name "televisionProgramMusic"@en ;
    reg:status <http://metadataregistry.org/uri/RegStatus/1001> ;
    a rdf:Property ;
    rdfs:isDefinedBy <http://rdaregistry.info/Elements/u/> ;
    rdfs:label "is television program music"@en ;
    rdfs:subPropertyOf <http://rdaregistry.info/Elements/u/P60723> ;
    owl:inverseOf <http://rdaregistry.info/Elements/u/P60728> ;
    skos:definition "Relates a resource to a musical resource that is used in a television program."@en .

<http://rdaregistry.info/Elements/u/P60728>
    reg:hasSubproperty <http://rdaregistry.info/Elements/e/P20248> ;
    reg:lexicalAlias <http://rdaregistry.info/Elements/u/musicForTelevisionProgram.en> ;
    reg:name "musicForTelevisionProgram"@en ;
    reg:status <http://metadataregistry.org/uri/RegStatus/1001> ;
    a rdf:Property ;
    rdfs:isDefinedBy <http://rdaregistry.info/Elements/u/> ;
    rdfs:label "is music for television program"@en ;
    rdfs:subPropertyOf <http://rdaregistry.info/Elements/u/P60724> ;
    owl:inverseOf <http://rdaregistry.info/Elements/u/P60727> ;
    skos:definition "Relates a resource to a resource that uses the musical resource in a television program."@en .

<http://rdaregistry.info/Elements/u/P60729>
    reg:hasSubproperty <http://rdaregistry.info/Elements/e/P20249> ;
    reg:lexicalAlias <http://rdaregistry.info/Elements/u/radioProgramMusic.en> ;
    reg:name "radioProgramMusic"@en ;
    reg:status <http://metadataregistry.org/uri/RegStatus/1001> ;
    a rdf:Property ;
    rdfs:isDefinedBy <http://rdaregistry.info/Elements/u/> ;
    rdfs:label "is radio program music"@en ;
    rdfs:subPropertyOf <http://rdaregistry.info/Elements/u/P60723> ;
    owl:inverseOf <http://rdaregistry.info/Elements/u/P60730> ;
    skos:definition "Relates a resource to a musical resource that is used in a radio program."@en .

<http://rdaregistry.info/Elements/u/P60730>
    reg:hasSubproperty <http://rdaregistry.info/Elements/e/P20250> ;
    reg:lexicalAlias <http://rdaregistry.info/Elements/u/musicForRadioProgram.en> ;
    reg:name "musicForRadioProgram"@en ;
    reg:status <http://metadataregistry.org/uri/RegStatus/1001> ;
    a rdf:Property ;
    rdfs:isDefinedBy <http://rdaregistry.info/Elements/u/> ;
    rdfs:label "is music for radio program"@en ;
    rdfs:subPropertyOf <http://rdaregistry.info/Elements/u/P60724> ;
    owl:inverseOf <http://rdaregistry.info/Elements/u/P60729> ;
    skos:definition "Relates a resource to a resource that uses the musical resource in a radio program."@en .

<http://rdaregistry.info/Elements/u/P60731>
    reg:hasSubproperty <http://rdaregistry.info/Elements/e/P20251> ;
    reg:lexicalAlias <http://rdaregistry.info/Elements/u/musicForMotionPicture.en> ;
    reg:name "musicForMotionPicture"@en ;
    reg:status <http://metadataregistry.org/uri/RegStatus/1001> ;
    a rdf:Property ;
    rdfs:isDefinedBy <http://rdaregistry.info/Elements/u/> ;
    rdfs:label "is music for motion picture"@en ;
    rdfs:subPropertyOf <http://rdaregistry.info/Elements/u/P60723> ;
    owl:inverseOf <http://rdaregistry.info/Elements/u/P60732> ;
    skos:definition "Relates a resource to a resource that uses the musical resource in a motion picture."@en .

<http://rdaregistry.info/Elements/u/P60732>
    reg:hasSubproperty <http://rdaregistry.info/Elements/e/P20252> ;
    reg:lexicalAlias <http://rdaregistry.info/Elements/u/motionPictureMusic.en> ;
    reg:name "motionPictureMusic"@en ;
    reg:status <http://metadataregistry.org/uri/RegStatus/1001> ;
    a rdf:Property ;
    rdfs:isDefinedBy <http://rdaregistry.info/Elements/u/> ;
    rdfs:label "is motion picture music"@en ;
    rdfs:subPropertyOf <http://rdaregistry.info/Elements/u/P60724> ;
    owl:inverseOf <http://rdaregistry.info/Elements/u/P60731> ;
    skos:definition "Relates a resource to a musical resource that is used in a motion picture."@en .

<http://rdaregistry.info/Elements/u/P60733>
    reg:hasSubproperty <http://rdaregistry.info/Elements/a/P50229> ;
    reg:lexicalAlias <http://rdaregistry.info/Elements/u/predecessorOfSplit.en> ;
    reg:name "predecessorOfSplit"@en ;
    reg:status <http://metadataregistry.org/uri/RegStatus/1001> ;
    a rdf:Property ;
    rdfs:isDefinedBy <http://rdaregistry.info/Elements/u/> ;
    rdfs:label "has predecessor of split"@en ;
    owl:inverseOf <http://rdaregistry.info/Elements/u/P60685> ;
    skos:definition "Relates an agent that split or divided into the other agent to the agent."@en .

<http://rdaregistry.info/Elements/u/P60736>
    reg:hasSubproperty <http://rdaregistry.info/Elements/a/P50232> ;
    reg:lexicalAlias <http://rdaregistry.info/Elements/u/componentOfAMerger.en> ;
    reg:name "componentOfAMerger"@en ;
    reg:status <http://metadataregistry.org/uri/RegStatus/1001> ;
    a rdf:Property ;
    rdfs:isDefinedBy <http://rdaregistry.info/Elements/u/> ;
    rdfs:label "has component of a merger"@en ;
    owl:inverseOf <http://rdaregistry.info/Elements/u/P60684> ;
    skos:definition "Relates an agent that formed the other agent by merging with one or more other agents to the agent."@en .

<http://rdaregistry.info/Elements/u/P60737>
    reg:hasSubproperty <http://rdaregistry.info/Elements/a/P50234>, <http://rdaregistry.info/Elements/u/P60865>, <http://rdaregistry.info/Elements/u/P60867> ;
    reg:lexicalAlias <http://rdaregistry.info/Elements/u/officerOf.en> ;
    reg:name "officerOf"@en ;
    reg:status <http://metadataregistry.org/uri/RegStatus/1001> ;
    a rdf:Property ;
    rdfs:isDefinedBy <http://rdaregistry.info/Elements/u/> ;
    rdfs:label "has officer of"@en ;
    rdfs:subPropertyOf <http://rdaregistry.info/Elements/u/P60454> ;
    owl:inverseOf <http://rdaregistry.info/Elements/u/P60633> ;
    skos:definition "Relates an agent to an agent holding an office in or commanding the agent."@en .

<http://rdaregistry.info/Elements/u/P60738>
    reg:lexicalAlias <http://rdaregistry.info/Elements/u/broaderAffiliatedAgent.en> ;
    reg:name "broaderAffiliatedAgent"@en ;
    reg:status <http://metadataregistry.org/uri/RegStatus/1001> ;
    a rdf:Property ;
    rdfs:isDefinedBy <http://rdaregistry.info/Elements/u/> ;
    rdfs:label "has broader affiliated agent"@en ;
    skos:definition "Relates an agent that acts for the local affiliated agent and others at a broader organizational level to the agent."@en .

<http://rdaregistry.info/Elements/u/P60739>
    reg:lexicalAlias <http://rdaregistry.info/Elements/u/localAffiliate.en> ;
    reg:name "localAffiliate"@en ;
    reg:status <http://metadataregistry.org/uri/RegStatus/1001> ;
    a rdf:Property ;
    rdfs:isDefinedBy <http://rdaregistry.info/Elements/u/> ;
    rdfs:label "has local affiliate"@en ;
    skos:definition "Relates a local agent affiliated with the broader agent which acts for it and others at a broader organizational level to the agent."@en .

<http://rdaregistry.info/Elements/u/P60740>
    reg:lexicalAlias <http://rdaregistry.info/Elements/u/choreography.en> ;
    reg:name "choreography"@en ;
    reg:status <http://metadataregistry.org/uri/RegStatus/1001> ;
    a rdf:Property ;
    rdfs:isDefinedBy <http://rdaregistry.info/Elements/u/> ;
    rdfs:label "is choreography"@en ;
    rdfs:subPropertyOf <http://rdaregistry.info/Elements/u/P60198> ;
    owl:inverseOf <http://rdaregistry.info/Elements/u/P60741> ;
    skos:definition "Relates a resource to a resource that provides the choreography for use in the related resource."@en .

<http://rdaregistry.info/Elements/u/P60741>
    reg:lexicalAlias <http://rdaregistry.info/Elements/u/choreographyFor.en> ;
    reg:name "choreographyFor"@en ;
    reg:status <http://metadataregistry.org/uri/RegStatus/1001> ;
    a rdf:Property ;
    rdfs:isDefinedBy <http://rdaregistry.info/Elements/u/> ;
    rdfs:label "is choreography for"@en ;
    rdfs:subPropertyOf <http://rdaregistry.info/Elements/u/P60198> ;
    owl:inverseOf <http://rdaregistry.info/Elements/u/P60740> ;
    skos:definition "Relates a resource to a resource that uses the choreography of the related resource."@en .

<http://rdaregistry.info/Elements/u/P60742>
    reg:lexicalAlias <http://rdaregistry.info/Elements/u/adaptedAsGraphicNovel.en> ;
    reg:name "adaptedAsGraphicNovel"@en ;
    reg:status <http://metadataregistry.org/uri/RegStatus/1001> ;
    a rdf:Property ;
    rdfs:isDefinedBy <http://rdaregistry.info/Elements/u/> ;
    rdfs:label "is adapted as graphic novel"@en ;
    rdfs:subPropertyOf <http://rdaregistry.info/Elements/u/P60260> ;
    owl:inverseOf <http://rdaregistry.info/Elements/u/P60743> ;
    skos:definition "Relates a resource to a graphic novel based on the source resource"@en .

<http://rdaregistry.info/Elements/u/P60743>
    reg:lexicalAlias <http://rdaregistry.info/Elements/u/graphicNovelizationOf.en> ;
    reg:name "graphicNovelizationOf"@en ;
    reg:status <http://metadataregistry.org/uri/RegStatus/1001> ;
    a rdf:Property ;
    rdfs:isDefinedBy <http://rdaregistry.info/Elements/u/> ;
    rdfs:label "is graphic novelization of"@en ;
    rdfs:subPropertyOf <http://rdaregistry.info/Elements/u/P60241> ;
    owl:inverseOf <http://rdaregistry.info/Elements/u/P60742> ;
    skos:definition "Relates a resource to a resource that has been adapated as a graphic novel."@en .

<http://rdaregistry.info/Elements/u/P60744>
    reg:lexicalAlias <http://rdaregistry.info/Elements/u/adaptedAsVideoGame.en> ;
    reg:name "adaptedAsVideoGame"@en ;
    reg:status <http://metadataregistry.org/uri/RegStatus/1001> ;
    a rdf:Property ;
    rdfs:isDefinedBy <http://rdaregistry.info/Elements/u/> ;
    rdfs:label "is adapted as video game"@en ;
    rdfs:subPropertyOf <http://rdaregistry.info/Elements/u/P60260> ;
    owl:inverseOf <http://rdaregistry.info/Elements/u/P60745> ;
    skos:definition "Relates a resource to relates a resource to a video game based on the source resource."@en .

<http://rdaregistry.info/Elements/u/P60745>
    reg:lexicalAlias <http://rdaregistry.info/Elements/u/videoGameAdaptationOf.en> ;
    reg:name "videoGameAdaptationOf"@en ;
    reg:status <http://metadataregistry.org/uri/RegStatus/1001> ;
    a rdf:Property ;
    rdfs:isDefinedBy <http://rdaregistry.info/Elements/u/> ;
    rdfs:label "is video game adaptation of"@en ;
    rdfs:subPropertyOf <http://rdaregistry.info/Elements/u/P60241> ;
    owl:inverseOf <http://rdaregistry.info/Elements/u/P60744> ;
    skos:definition "Relates a resource to a resource that has been adapted as a video game."@en .

<http://rdaregistry.info/Elements/u/P60746>
    reg:lexicalAlias <http://rdaregistry.info/Elements/u/papermaker.en> ;
    reg:name "papermaker"@en ;
    reg:status <http://metadataregistry.org/uri/RegStatus/1001> ;
    a rdf:Property ;
    rdfs:isDefinedBy <http://rdaregistry.info/Elements/u/> ;
    rdfs:label "has papermaker"@en ;
    rdfs:subPropertyOf <http://rdaregistry.info/Elements/u/P60443> ;
    owl:inverseOf <http://rdaregistry.info/Elements/u/P60747> ;
    skos:definition "Relates a resource to an agent responsible for the production of paper used to manufacture a resource."@en .

<http://rdaregistry.info/Elements/u/P60747>
    reg:lexicalAlias <http://rdaregistry.info/Elements/u/papermakerOf.en> ;
    reg:name "papermakerOf"@en ;
    reg:status <http://metadataregistry.org/uri/RegStatus/1001> ;
    a rdf:Property ;
    rdfs:isDefinedBy <http://rdaregistry.info/Elements/u/> ;
    rdfs:label "is papermaker of"@en ;
    rdfs:subPropertyOf <http://rdaregistry.info/Elements/u/P60669> ;
    owl:inverseOf <http://rdaregistry.info/Elements/u/P60746> ;
    skos:definition "Relates an agent responsible for the production of paper used to manufacture a resource to the resource."@en .

<http://rdaregistry.info/Elements/u/P60748>
    reg:lexicalAlias <http://rdaregistry.info/Elements/u/visualEffectsProvider.en> ;
    reg:name "visualEffectsProvider"@en ;
    reg:status <http://metadataregistry.org/uri/RegStatus/1001> ;
    a rdf:Property ;
    rdfs:isDefinedBy <http://rdaregistry.info/Elements/u/> ;
    rdfs:label "has visual effects provider"@en ;
    rdfs:subPropertyOf <http://rdaregistry.info/Elements/u/P60398> ;
    owl:inverseOf <http://rdaregistry.info/Elements/u/P60754> ;
    skos:definition "Relates a resource to an agent contributing to an expression of a moving image resource by designing and creating post-production visual effects."@en .

<http://rdaregistry.info/Elements/u/P60749>
    reg:lexicalAlias <http://rdaregistry.info/Elements/u/specialEffectsProvider.en> ;
    reg:name "specialEffectsProvider"@en ;
    reg:status <http://metadataregistry.org/uri/RegStatus/1001> ;
    a rdf:Property ;
    rdfs:isDefinedBy <http://rdaregistry.info/Elements/u/> ;
    rdfs:label "has special effects provider"@en ;
    rdfs:subPropertyOf <http://rdaregistry.info/Elements/u/P60398> ;
    owl:inverseOf <http://rdaregistry.info/Elements/u/P60755> ;
    skos:definition "Relates a resource to an agent contributing to a moving image or audio resource by designing and creating on-set special effects (on-set mechanical effects and in-camera optical effects)."@en .

<http://rdaregistry.info/Elements/u/P60750>
    reg:lexicalAlias <http://rdaregistry.info/Elements/u/letterer.en> ;
    reg:name "letterer"@en ;
    reg:status <http://metadataregistry.org/uri/RegStatus/1001> ;
    a rdf:Property ;
    rdfs:isDefinedBy <http://rdaregistry.info/Elements/u/> ;
    rdfs:label "has letterer"@en ;
    rdfs:subPropertyOf <http://rdaregistry.info/Elements/u/P60396> ;
    owl:inverseOf <http://rdaregistry.info/Elements/u/P60756> ;
    skos:definition "Relates a resource to an illustrator contributing to a comic book, graphic novel, etc., by drawing the text and graphic sound effects."@en .

<http://rdaregistry.info/Elements/u/P60751>
    reg:lexicalAlias <http://rdaregistry.info/Elements/u/rapporteur.en> ;
    reg:name "rapporteur"@en ;
    reg:status <http://metadataregistry.org/uri/RegStatus/1001> ;
    a rdf:Property ;
    rdfs:isDefinedBy <http://rdaregistry.info/Elements/u/> ;
    rdfs:label "has rapporteur"@en ;
    rdfs:subPropertyOf <http://rdaregistry.info/Elements/u/P60434> ;
    owl:inverseOf <http://rdaregistry.info/Elements/u/P60757> ;
    skos:definition "Relates a resource to an author who is appointed by an organization to report on the proceedings of its meetings."@en .

<http://rdaregistry.info/Elements/u/P60752>
    reg:lexicalAlias <http://rdaregistry.info/Elements/u/calligrapher.en> ;
    reg:name "calligrapher"@en ;
    reg:status <http://metadataregistry.org/uri/RegStatus/1001> ;
    a rdf:Property ;
    rdfs:isDefinedBy <http://rdaregistry.info/Elements/u/> ;
    rdfs:label "has calligrapher"@en ;
    rdfs:subPropertyOf <http://rdaregistry.info/Elements/u/P60431> ;
    owl:inverseOf <http://rdaregistry.info/Elements/u/P60758> ;
    skos:definition "Relates a resource to an artist responsible for creating a resource of calligraphy where the focus of interest lies in the aesthetic value of its penmanship or graphic artistry, regardless of whether the same person, etc., also authored the inscribed text."@en .

<http://rdaregistry.info/Elements/u/P60753>
    reg:lexicalAlias <http://rdaregistry.info/Elements/u/bookArtist.en> ;
    reg:name "bookArtist"@en ;
    reg:status <http://metadataregistry.org/uri/RegStatus/1001> ;
    a rdf:Property ;
    rdfs:isDefinedBy <http://rdaregistry.info/Elements/u/> ;
    rdfs:label "has book artist"@en ;
    rdfs:subPropertyOf <http://rdaregistry.info/Elements/u/P60431> ;
    owl:inverseOf <http://rdaregistry.info/Elements/u/P60759> ;
    skos:definition "Relates a resource to an artist responsible for creating art resources that exploit the book form or alter its physical structure as part of the content of the resource."@en .

<http://rdaregistry.info/Elements/u/P60754>
    reg:lexicalAlias <http://rdaregistry.info/Elements/u/visualEffectsProviderOf.en> ;
    reg:name "visualEffectsProviderOf"@en ;
    reg:status <http://metadataregistry.org/uri/RegStatus/1001> ;
    a rdf:Property ;
    rdfs:isDefinedBy <http://rdaregistry.info/Elements/u/> ;
    rdfs:label "is visual effects provider of"@en ;
    rdfs:subPropertyOf <http://rdaregistry.info/Elements/u/P60626> ;
    owl:inverseOf <http://rdaregistry.info/Elements/u/P60748> ;
    skos:definition "Relates an agent contributing to an expression of a moving image resource by designing and creating post-production visual effects to the resource."@en .

<http://rdaregistry.info/Elements/u/P60755>
    reg:lexicalAlias <http://rdaregistry.info/Elements/u/specialEffectsProviderOf.en> ;
    reg:name "specialEffectsProviderOf"@en ;
    reg:status <http://metadataregistry.org/uri/RegStatus/1001> ;
    a rdf:Property ;
    rdfs:isDefinedBy <http://rdaregistry.info/Elements/u/> ;
    rdfs:label "is special effects provider of"@en ;
    rdfs:subPropertyOf <http://rdaregistry.info/Elements/u/P60626> ;
    owl:inverseOf <http://rdaregistry.info/Elements/u/P60749> ;
    skos:definition "Relates an agent contributing to a moving image or audio resource by designing and creating on-set special effects (on-set mechanical effects and in-camera optical effects) to the resource."@en .

<http://rdaregistry.info/Elements/u/P60756>
    reg:lexicalAlias <http://rdaregistry.info/Elements/u/lettererOf.en> ;
    reg:name "lettererOf"@en ;
    reg:status <http://metadataregistry.org/uri/RegStatus/1001> ;
    a rdf:Property ;
    rdfs:isDefinedBy <http://rdaregistry.info/Elements/u/> ;
    rdfs:label "is letterer of"@en ;
    rdfs:subPropertyOf <http://rdaregistry.info/Elements/u/P60624> ;
    owl:inverseOf <http://rdaregistry.info/Elements/u/P60750> ;
    skos:definition "Relates an illustrator contributing to a comic book, graphic novel, etc., by drawing the text and graphic sound effects to the resource."@en .

<http://rdaregistry.info/Elements/u/P60757>
    reg:lexicalAlias <http://rdaregistry.info/Elements/u/rapporteurOf.en> ;
    reg:name "rapporteurOf"@en ;
    reg:status <http://metadataregistry.org/uri/RegStatus/1001> ;
    a rdf:Property ;
    rdfs:isDefinedBy <http://rdaregistry.info/Elements/u/> ;
    rdfs:label "is rapporteur of"@en ;
    rdfs:subPropertyOf <http://rdaregistry.info/Elements/u/P60663> ;
    owl:inverseOf <http://rdaregistry.info/Elements/u/P60751> ;
    skos:definition "Relates an author who is appointed by an organization to report on the proceedings of its meetings to the resource."@en .

<http://rdaregistry.info/Elements/u/P60758>
    reg:lexicalAlias <http://rdaregistry.info/Elements/u/calligrapherOf.en> ;
    reg:name "calligrapherOf"@en ;
    reg:status <http://metadataregistry.org/uri/RegStatus/1001> ;
    a rdf:Property ;
    rdfs:isDefinedBy <http://rdaregistry.info/Elements/u/> ;
    rdfs:label "is calligrapher of"@en ;
    rdfs:subPropertyOf <http://rdaregistry.info/Elements/u/P60660> ;
    owl:inverseOf <http://rdaregistry.info/Elements/u/P60752> ;
    skos:definition "Relates an artist responsible for creating a resource of calligraphy where the focus of interest lies in the aesthetic value of its penmanship or graphic artistry, regardless of whether the same person, etc., also authored the inscribed text to the resource."@en .

<http://rdaregistry.info/Elements/u/P60759>
    reg:lexicalAlias <http://rdaregistry.info/Elements/u/bookArtistOf.en> ;
    reg:name "bookArtistOf"@en ;
    reg:status <http://metadataregistry.org/uri/RegStatus/1001> ;
    a rdf:Property ;
    rdfs:isDefinedBy <http://rdaregistry.info/Elements/u/> ;
    rdfs:label "is book artist of"@en ;
    rdfs:subPropertyOf <http://rdaregistry.info/Elements/u/P60660> ;
    owl:inverseOf <http://rdaregistry.info/Elements/u/P60753> ;
    skos:definition "Relates an artist responsible for creating art resources that exploit the book form or alter its physical structure as part of the content of the resource to the resource."@en .

<http://rdaregistry.info/Elements/u/P60760>
    reg:lexicalAlias <http://rdaregistry.info/Elements/u/detailsOfAspectRatio.en> ;
    reg:name "detailsOfAspectRatio"@en ;
    reg:status <http://metadataregistry.org/uri/RegStatus/1001> ;
    a rdf:Property ;
    rdfs:isDefinedBy <http://rdaregistry.info/Elements/u/> ;
    rdfs:label "has details of aspect ratio"@en ;
    skos:definition "Relates a resource to details of the ratio of the width to the height of a moving image."@en .

<http://rdaregistry.info/Elements/u/P60761>
    reg:lexicalAlias <http://rdaregistry.info/Elements/u/detailsOfColourContent.en> ;
    reg:name "detailsOfColourContent"@en ;
    reg:status <http://metadataregistry.org/uri/RegStatus/1001> ;
    a rdf:Property ;
    rdfs:isDefinedBy <http://rdaregistry.info/Elements/u/> ;
    rdfs:label "has details of colour content"@en ;
    skos:altLabel "has details of color content"@en ;
    skos:definition "Relates a resource to details of the presence of colour, tone, etc., in the content of a resource, and the specific colours, tones, etc., (including black and white) present."@en .

<http://rdaregistry.info/Elements/u/P60762>
    reg:lexicalAlias <http://rdaregistry.info/Elements/u/detailsOfFormOfMusicalNotation.en> ;
    reg:name "detailsOfFormOfMusicalNotation"@en ;
    reg:status <http://metadataregistry.org/uri/RegStatus/1001> ;
    a rdf:Property ;
    rdfs:isDefinedBy <http://rdaregistry.info/Elements/u/> ;
    rdfs:label "has details of form of musical notation"@en ;
    skos:definition "Relates a resource to details of the set of characters and/or symbols used to express the musical content of a resource."@en .

<http://rdaregistry.info/Elements/u/P60763>
    reg:lexicalAlias <http://rdaregistry.info/Elements/u/detailsOfFormOfNotatedMovement.en> ;
    reg:name "detailsOfFormOfNotatedMovement"@en ;
    reg:status <http://metadataregistry.org/uri/RegStatus/1001> ;
    a rdf:Property ;
    rdfs:isDefinedBy <http://rdaregistry.info/Elements/u/> ;
    rdfs:label "has details of form of notated movement"@en ;
    skos:definition "Relates a resource to details of the set of characters and/or symbols used to express the movement content of a resource."@en .

<http://rdaregistry.info/Elements/u/P60764>
    reg:lexicalAlias <http://rdaregistry.info/Elements/u/detailsOfFormatOfNotatedMusic.en> ;
    reg:name "detailsOfFormatOfNotatedMusic"@en ;
    reg:status <http://metadataregistry.org/uri/RegStatus/1001> ;
    a rdf:Property ;
    rdfs:isDefinedBy <http://rdaregistry.info/Elements/u/> ;
    rdfs:label "has details of format of notated music"@en ;
    skos:definition "Relates a resource to details of the musical or physical layout of the content of a resource that is presented in the form of musical notation."@en .

<http://rdaregistry.info/Elements/u/P60765>
    reg:lexicalAlias <http://rdaregistry.info/Elements/u/detailsOfFormOfTactileNotation.en> ;
    reg:name "detailsOfFormOfTactileNotation"@en ;
    reg:status <http://metadataregistry.org/uri/RegStatus/1001> ;
    a rdf:Property ;
    rdfs:isDefinedBy <http://rdaregistry.info/Elements/u/> ;
    rdfs:label "has details of form of tactile notation"@en ;
    skos:definition "Relates a resource to details of the set of characters and/or symbols used to express the content of a resource in a form that can be perceived through touch."@en .

<http://rdaregistry.info/Elements/u/P60766>
    reg:lexicalAlias <http://rdaregistry.info/Elements/u/detailsOfScript.en> ;
    reg:name "detailsOfScript"@en ;
    reg:status <http://metadataregistry.org/uri/RegStatus/1001> ;
    a rdf:Property ;
    rdfs:isDefinedBy <http://rdaregistry.info/Elements/u/> ;
    rdfs:label "has details of script"@en ;
    skos:definition "Relates a resource to details of set of characters and/or symbols used to express the written language content of a resource."@en .

<http://rdaregistry.info/Elements/u/P60767>
    reg:hasSubproperty <http://rdaregistry.info/Elements/u/P60774> ;
    reg:lexicalAlias <http://rdaregistry.info/Elements/u/detailsOfAppliedMaterial.en> ;
    reg:name "detailsOfAppliedMaterial"@en ;
    reg:status <http://metadataregistry.org/uri/RegStatus/1001> ;
    a rdf:Property ;
    rdfs:isDefinedBy <http://rdaregistry.info/Elements/u/> ;
    rdfs:label "has details of applied material"@en ;
    skos:definition "Relates a resource to details of a physical or chemical substance applied to a base material of a resource."@en .

<http://rdaregistry.info/Elements/u/P60768>
    reg:lexicalAlias <http://rdaregistry.info/Elements/u/detailsOfBaseMaterial.en> ;
    reg:name "detailsOfBaseMaterial"@en ;
    reg:status <http://metadataregistry.org/uri/RegStatus/1001> ;
    a rdf:Property ;
    rdfs:isDefinedBy <http://rdaregistry.info/Elements/u/> ;
    rdfs:label "has details of base material"@en ;
    skos:definition "Relates a resource to details of the underlying physical material of a resource."@en .

<http://rdaregistry.info/Elements/u/P60769>
    reg:lexicalAlias <http://rdaregistry.info/Elements/u/detailsOfBookFormat.en> ;
    reg:name "detailsOfBookFormat"@en ;
    reg:status <http://metadataregistry.org/uri/RegStatus/1001> ;
    a rdf:Property ;
    rdfs:isDefinedBy <http://rdaregistry.info/Elements/u/> ;
    rdfs:label "has details of book format"@en ;
    skos:definition "Relates a resource to details of the result of folding a printed sheet to form a gathering of leaves (e.g., a sheet folded once to form a folio, twice to form a quarto, three times to form an octavo, etc.)."@en .

<http://rdaregistry.info/Elements/u/P60770>
    reg:lexicalAlias <http://rdaregistry.info/Elements/u/detailsOfBroadcastStandard.en> ;
    reg:name "detailsOfBroadcastStandard"@en ;
    reg:status <http://metadataregistry.org/uri/RegStatus/1001> ;
    a rdf:Property ;
    rdfs:isDefinedBy <http://rdaregistry.info/Elements/u/> ;
    rdfs:label "has details of broadcast standard"@en ;
    rdfs:subPropertyOf <http://rdaregistry.info/Elements/u/P60801> ;
    skos:definition "Relates a resource to details of a system used to format a video resource for television broadcast."@en .

<http://rdaregistry.info/Elements/u/P60771>
    reg:lexicalAlias <http://rdaregistry.info/Elements/u/detailsOfConfigurationOfPlaybackChannels.en> ;
    reg:name "detailsOfConfigurationOfPlaybackChannels"@en ;
    reg:status <http://metadataregistry.org/uri/RegStatus/1001> ;
    a rdf:Property ;
    rdfs:isDefinedBy <http://rdaregistry.info/Elements/u/> ;
    rdfs:label "has details of configuration of playback channels"@en ;
    rdfs:subPropertyOf <http://rdaregistry.info/Elements/u/P60796> ;
    skos:definition "Relates a resource to details of the number of sound channels used to make a recording (e.g., one channel for a monophonic recording, two channels for a stereophonic recording)."@en .

<http://rdaregistry.info/Elements/u/P60772>
    reg:hasSubproperty <http://rdaregistry.info/Elements/u/P60773>, <http://rdaregistry.info/Elements/u/P60775>, <http://rdaregistry.info/Elements/u/P60776> ;
    reg:lexicalAlias <http://rdaregistry.info/Elements/u/detailsOfDigitalFileCharacteristic.en> ;
    reg:name "detailsOfDigitalFileCharacteristic"@en ;
    reg:status <http://metadataregistry.org/uri/RegStatus/1001> ;
    a rdf:Property ;
    rdfs:isDefinedBy <http://rdaregistry.info/Elements/u/> ;
    rdfs:label "has details of digital file characteristic"@en ;
    skos:definition "Relates a resource to details of a technical specification relating to the digital encoding of text, image, audio, video, and other types of data in a resource."@en .

<http://rdaregistry.info/Elements/u/P60773>
    reg:lexicalAlias <http://rdaregistry.info/Elements/u/detailsOfDigitalRepresentationOfCartographicContent.en> ;
    reg:name "detailsOfDigitalRepresentationOfCartographicContent"@en ;
    reg:status <http://metadataregistry.org/uri/RegStatus/1001> ;
    a rdf:Property ;
    rdfs:isDefinedBy <http://rdaregistry.info/Elements/u/> ;
    rdfs:label "has details of digital representation of cartographic content"@en ;
    rdfs:subPropertyOf <http://rdaregistry.info/Elements/u/P60772> ;
    skos:definition "Relates a resource to details of the encoding of geospatial information in a cartographic resource (e.g., topology level, compression)."@en .

<http://rdaregistry.info/Elements/u/P60774>
    reg:lexicalAlias <http://rdaregistry.info/Elements/u/detailsOfEmulsionOnMicrofilmAndMicrofiche.en> ;
    reg:name "detailsOfEmulsionOnMicrofilmAndMicrofiche"@en ;
    reg:status <http://metadataregistry.org/uri/RegStatus/1001> ;
    a rdf:Property ;
    rdfs:isDefinedBy <http://rdaregistry.info/Elements/u/> ;
    rdfs:label "has details of emulsion on microfilm and microfiche"@en ;
    rdfs:subPropertyOf <http://rdaregistry.info/Elements/u/P60767> ;
    skos:definition "Relates a resource to details of a suspension of light-sensitive chemicals used as a coating on a microfilm or microfiche (e.g., silver halide)."@en .

<http://rdaregistry.info/Elements/u/P60775>
    reg:lexicalAlias <http://rdaregistry.info/Elements/u/detailsOfEncodingFormat.en> ;
    reg:name "detailsOfEncodingFormat"@en ;
    reg:status <http://metadataregistry.org/uri/RegStatus/1001> ;
    a rdf:Property ;
    rdfs:isDefinedBy <http://rdaregistry.info/Elements/u/> ;
    rdfs:label "has details of encoding format"@en ;
    rdfs:subPropertyOf <http://rdaregistry.info/Elements/u/P60772> ;
    skos:definition "Relates a resource to details of a schema, standard, etc., used to encode the digital content of a resource."@en .

<http://rdaregistry.info/Elements/u/P60776>
    reg:lexicalAlias <http://rdaregistry.info/Elements/u/detailsOfFileType.en> ;
    reg:name "detailsOfFileType"@en ;
    reg:status <http://metadataregistry.org/uri/RegStatus/1001> ;
    a rdf:Property ;
    rdfs:isDefinedBy <http://rdaregistry.info/Elements/u/> ;
    rdfs:label "has details of file type"@en ;
    rdfs:subPropertyOf <http://rdaregistry.info/Elements/u/P60772> ;
    skos:definition "Relates a resource to details of a general type of data content encoded in a computer file."@en .

<http://rdaregistry.info/Elements/u/P60777>
    reg:lexicalAlias <http://rdaregistry.info/Elements/u/detailsOfFontSize.en> ;
    reg:name "detailsOfFontSize"@en ;
    reg:status <http://metadataregistry.org/uri/RegStatus/1001> ;
    a rdf:Property ;
    rdfs:isDefinedBy <http://rdaregistry.info/Elements/u/> ;
    rdfs:label "has details of font size"@en ;
    skos:definition "Relates a resource to details of the size of the type used to represent the characters and symbols in a resource."@en .

<http://rdaregistry.info/Elements/u/P60778>
    reg:lexicalAlias <http://rdaregistry.info/Elements/u/detailsOfGenerationOfAudioRecording.en> ;
    reg:name "detailsOfGenerationOfAudioRecording"@en ;
    reg:status <http://metadataregistry.org/uri/RegStatus/1001> ;
    a rdf:Property ;
    rdfs:isDefinedBy <http://rdaregistry.info/Elements/u/> ;
    rdfs:label "has details of generation of audio recording"@en ;
    rdfs:subPropertyOf <http://rdaregistry.info/Elements/u/P60803> ;
    skos:definition "Relates a resource to details of the relationship between an original audio carrier and the carrier of a reproduction made from the original (e.g., a tape duplication master, a test pressing)."@en .

<http://rdaregistry.info/Elements/u/P60779>
    reg:lexicalAlias <http://rdaregistry.info/Elements/u/detailsOfGenerationOfDigitalResource.en> ;
    reg:name "detailsOfGenerationOfDigitalResource"@en ;
    reg:status <http://metadataregistry.org/uri/RegStatus/1001> ;
    a rdf:Property ;
    rdfs:isDefinedBy <http://rdaregistry.info/Elements/u/> ;
    rdfs:label "has details of generation of digital resource"@en ;
    rdfs:subPropertyOf <http://rdaregistry.info/Elements/u/P60803> ;
    skos:definition "Relates a resource to details of the relationship between an original carrier of a digital resource and the carrier of a reproduction made from the original (e.g., a derivative master)."@en .

<http://rdaregistry.info/Elements/u/P60780>
    reg:lexicalAlias <http://rdaregistry.info/Elements/u/detailsOfGenerationOfMicroform.en> ;
    reg:name "detailsOfGenerationOfMicroform"@en ;
    reg:status <http://metadataregistry.org/uri/RegStatus/1001> ;
    a rdf:Property ;
    rdfs:isDefinedBy <http://rdaregistry.info/Elements/u/> ;
    rdfs:label "has details of generation of microform"@en ;
    rdfs:subPropertyOf <http://rdaregistry.info/Elements/u/P60803> ;
    skos:definition "Relates a resource to details of the relationship between an original microform carrier and the carrier of a reproduction made from the original (e.g., a printing master)."@en .

<http://rdaregistry.info/Elements/u/P60781>
    reg:lexicalAlias <http://rdaregistry.info/Elements/u/detailsOfGenerationOfMotionPictureFilm.en> ;
    reg:name "detailsOfGenerationOfMotionPictureFilm"@en ;
    reg:status <http://metadataregistry.org/uri/RegStatus/1001> ;
    a rdf:Property ;
    rdfs:isDefinedBy <http://rdaregistry.info/Elements/u/> ;
    rdfs:label "has details of generation of motion picture film"@en ;
    rdfs:subPropertyOf <http://rdaregistry.info/Elements/u/P60803> ;
    skos:definition "Relates a resource to details of the relationship between an original carrier of a motion picture film resource and the carrier of a reproduction made from the original (e.g., a reference print)."@en .

<http://rdaregistry.info/Elements/u/P60782>
    reg:lexicalAlias <http://rdaregistry.info/Elements/u/detailsOfGenerationOfVideotape.en> ;
    reg:name "detailsOfGenerationOfVideotape"@en ;
    reg:status <http://metadataregistry.org/uri/RegStatus/1001> ;
    a rdf:Property ;
    rdfs:isDefinedBy <http://rdaregistry.info/Elements/u/> ;
    rdfs:label "has details of generation of videotape"@en ;
    rdfs:subPropertyOf <http://rdaregistry.info/Elements/u/P60803> ;
    skos:definition "Relates a resource to details of the relationship between an original carrier of a videotape resource and the carrier of a reproduction made from the original (e.g., a show copy)."@en .

<http://rdaregistry.info/Elements/u/P60783>
    reg:lexicalAlias <http://rdaregistry.info/Elements/u/detailsOfGrooveCharacteristic.en> ;
    reg:name "detailsOfGrooveCharacteristic"@en ;
    reg:status <http://metadataregistry.org/uri/RegStatus/1001> ;
    a rdf:Property ;
    rdfs:isDefinedBy <http://rdaregistry.info/Elements/u/> ;
    rdfs:label "has details of groove characteristic"@en ;
    rdfs:subPropertyOf <http://rdaregistry.info/Elements/u/P60796> ;
    skos:definition "Relates a resource to details of the groove width of an analog disc or the groove pitch of an analog cylinder."@en .

<http://rdaregistry.info/Elements/u/P60784>
    reg:lexicalAlias <http://rdaregistry.info/Elements/u/detailsOfLayout.en> ;
    reg:name "detailsOfLayout"@en ;
    reg:status <http://metadataregistry.org/uri/RegStatus/1001> ;
    a rdf:Property ;
    rdfs:isDefinedBy <http://rdaregistry.info/Elements/u/> ;
    rdfs:label "has details of layout"@en ;
    skos:definition "Relates a resource to details of the arrangement of text, images, tactile notation, etc., in a resource."@en .

<http://rdaregistry.info/Elements/u/P60785>
    reg:lexicalAlias <http://rdaregistry.info/Elements/u/detailsOfMount.en> ;
    reg:name "detailsOfMount"@en ;
    reg:status <http://metadataregistry.org/uri/RegStatus/1001> ;
    a rdf:Property ;
    rdfs:isDefinedBy <http://rdaregistry.info/Elements/u/> ;
    rdfs:label "has details of mount"@en ;
    skos:definition "Relates a resource to details of the physical material used for the support or backing to which the base material of a resource has been attached."@en .

<http://rdaregistry.info/Elements/u/P60786>
    reg:lexicalAlias <http://rdaregistry.info/Elements/u/detailsOfPlayingSpeed.en> ;
    reg:name "detailsOfPlayingSpeed"@en ;
    reg:status <http://metadataregistry.org/uri/RegStatus/1001> ;
    a rdf:Property ;
    rdfs:isDefinedBy <http://rdaregistry.info/Elements/u/> ;
    rdfs:label "has details of playing speed"@en ;
    skos:definition "Relates a resource to details of the speed at which an audio carrier must be operated to produce the sound intended."@en .

<http://rdaregistry.info/Elements/u/P60787>
    reg:lexicalAlias <http://rdaregistry.info/Elements/u/detailsOfPolarity.en> ;
    reg:name "detailsOfPolarity"@en ;
    reg:status <http://metadataregistry.org/uri/RegStatus/1001> ;
    a rdf:Property ;
    rdfs:isDefinedBy <http://rdaregistry.info/Elements/u/> ;
    rdfs:label "has details of polarity"@en ;
    skos:definition "Relates a resource to details of the relationship of the colours and tones in an image to the colours and tones of the object reproduced (e.g., positive, negative)."@en .

<http://rdaregistry.info/Elements/u/P60788>
    reg:lexicalAlias <http://rdaregistry.info/Elements/u/detailsOfPresentationFormat.en> ;
    reg:name "detailsOfPresentationFormat"@en ;
    reg:status <http://metadataregistry.org/uri/RegStatus/1001> ;
    a rdf:Property ;
    rdfs:isDefinedBy <http://rdaregistry.info/Elements/u/> ;
    rdfs:label "has details of presentation format"@en ;
    skos:definition "Relates a resource to details of the format used in the production of a projected image (e.g., cinerama, imax)."@en .

<http://rdaregistry.info/Elements/u/P60789>
    reg:hasSubproperty <http://rdaregistry.info/Elements/u/P60790>, <http://rdaregistry.info/Elements/u/P60791> ;
    reg:lexicalAlias <http://rdaregistry.info/Elements/u/detailsOfProductionMethod.en> ;
    reg:name "detailsOfProductionMethod"@en ;
    reg:status <http://metadataregistry.org/uri/RegStatus/1001> ;
    a rdf:Property ;
    rdfs:isDefinedBy <http://rdaregistry.info/Elements/u/> ;
    rdfs:label "has details of production method"@en ;
    skos:definition "Relates a resource to details of the process used to produce a resource."@en .

<http://rdaregistry.info/Elements/u/P60790>
    reg:lexicalAlias <http://rdaregistry.info/Elements/u/detailsOfProductionMethodForManuscript.en> ;
    reg:name "detailsOfProductionMethodForManuscript"@en ;
    reg:status <http://metadataregistry.org/uri/RegStatus/1001> ;
    a rdf:Property ;
    rdfs:isDefinedBy <http://rdaregistry.info/Elements/u/> ;
    rdfs:label "has details of production method for manuscript"@en ;
    rdfs:subPropertyOf <http://rdaregistry.info/Elements/u/P60789> ;
    skos:definition "Relates a resource to details of the process used to produce an original manuscript or a copy."@en .

<http://rdaregistry.info/Elements/u/P60791>
    reg:lexicalAlias <http://rdaregistry.info/Elements/u/detailsOfProductionMethodForTactileResource.en> ;
    reg:name "detailsOfProductionMethodForTactileResource"@en ;
    reg:status <http://metadataregistry.org/uri/RegStatus/1001> ;
    a rdf:Property ;
    rdfs:isDefinedBy <http://rdaregistry.info/Elements/u/> ;
    rdfs:label "has details of production method for tactile resource"@en ;
    rdfs:subPropertyOf <http://rdaregistry.info/Elements/u/P60789> ;
    skos:definition "Relates a resource to details of the process used to produce a tactile resource (e.g., embossing, thermoform)."@en .

<http://rdaregistry.info/Elements/u/P60792>
    reg:hasSubproperty <http://rdaregistry.info/Elements/u/P60793> ;
    reg:lexicalAlias <http://rdaregistry.info/Elements/u/detailsOfProjectionCharacteristicOfMotionPictureFilm.en> ;
    reg:name "detailsOfProjectionCharacteristicOfMotionPictureFilm"@en ;
    reg:status <http://metadataregistry.org/uri/RegStatus/1001> ;
    a rdf:Property ;
    rdfs:isDefinedBy <http://rdaregistry.info/Elements/u/> ;
    rdfs:label "has details of projection characteristic of motion picture film"@en ;
    skos:definition "Relates a resource to details of a technical specification relating to the projection of a motion picture film."@en .

<http://rdaregistry.info/Elements/u/P60793>
    reg:lexicalAlias <http://rdaregistry.info/Elements/u/detailsOfProjectionSpeed.en> ;
    reg:name "detailsOfProjectionSpeed"@en ;
    reg:status <http://metadataregistry.org/uri/RegStatus/1001> ;
    a rdf:Property ;
    rdfs:isDefinedBy <http://rdaregistry.info/Elements/u/> ;
    rdfs:label "has details of projection speed"@en ;
    rdfs:subPropertyOf <http://rdaregistry.info/Elements/u/P60792> ;
    skos:definition "Relates a resource to details of the speed at which a projected carrier must be operated to produce the moving image intended."@en .

<http://rdaregistry.info/Elements/u/P60794>
    reg:lexicalAlias <http://rdaregistry.info/Elements/u/detailsOfRecordingMedium.en> ;
    reg:name "detailsOfRecordingMedium"@en ;
    reg:status <http://metadataregistry.org/uri/RegStatus/1001> ;
    a rdf:Property ;
    rdfs:isDefinedBy <http://rdaregistry.info/Elements/u/> ;
    rdfs:label "has details of recording medium"@en ;
    rdfs:subPropertyOf <http://rdaregistry.info/Elements/u/P60796> ;
    skos:definition "Relates a resource to details of the type of medium used to record sound on an audio carrier (e.g., magnetic, optical)."@en .

<http://rdaregistry.info/Elements/u/P60795>
    reg:lexicalAlias <http://rdaregistry.info/Elements/u/detailsOfReductionRatio.en> ;
    reg:name "detailsOfReductionRatio"@en ;
    reg:status <http://metadataregistry.org/uri/RegStatus/1001> ;
    a rdf:Property ;
    rdfs:isDefinedBy <http://rdaregistry.info/Elements/u/> ;
    rdfs:label "has details of reduction ratio"@en ;
    skos:definition "Relates a resource to details of the size of a micro-image in relation to the original from which it was produced."@en .

<http://rdaregistry.info/Elements/u/P60796>
    reg:hasSubproperty <http://rdaregistry.info/Elements/u/P60771>, <http://rdaregistry.info/Elements/u/P60783>, <http://rdaregistry.info/Elements/u/P60794>, <http://rdaregistry.info/Elements/u/P60797>, <http://rdaregistry.info/Elements/u/P60798>, <http://rdaregistry.info/Elements/u/P60799>, <http://rdaregistry.info/Elements/u/P60800> ;
    reg:lexicalAlias <http://rdaregistry.info/Elements/u/detailsOfSoundCharacteristic.en> ;
    reg:name "detailsOfSoundCharacteristic"@en ;
    reg:status <http://metadataregistry.org/uri/RegStatus/1001> ;
    a rdf:Property ;
    rdfs:isDefinedBy <http://rdaregistry.info/Elements/u/> ;
    rdfs:label "has details of sound characteristic"@en ;
    skos:definition "Relates a resource to details of a technical specification relating to the encoding of sound in a resource."@en .

<http://rdaregistry.info/Elements/u/P60797>
    reg:lexicalAlias <http://rdaregistry.info/Elements/u/detailsOfSpecialPlaybackCharacteristic.en> ;
    reg:name "detailsOfSpecialPlaybackCharacteristic"@en ;
    reg:status <http://metadataregistry.org/uri/RegStatus/1001> ;
    a rdf:Property ;
    rdfs:isDefinedBy <http://rdaregistry.info/Elements/u/> ;
    rdfs:label "has details of special playback characteristic"@en ;
    rdfs:subPropertyOf <http://rdaregistry.info/Elements/u/P60796> ;
    skos:definition "Relates a resource to details of an equalization system, noise reduction system, etc., used in making an audio recording."@en .

<http://rdaregistry.info/Elements/u/P60798>
    reg:lexicalAlias <http://rdaregistry.info/Elements/u/detailsOfTapeConfiguration.en> ;
    reg:name "detailsOfTapeConfiguration"@en ;
    reg:status <http://metadataregistry.org/uri/RegStatus/1001> ;
    a rdf:Property ;
    rdfs:isDefinedBy <http://rdaregistry.info/Elements/u/> ;
    rdfs:label "has details of tape configuration"@en ;
    rdfs:subPropertyOf <http://rdaregistry.info/Elements/u/P60796> ;
    skos:definition "Relates a resource to details of the number of tracks on an audiotape."@en .

<http://rdaregistry.info/Elements/u/P60799>
    reg:lexicalAlias <http://rdaregistry.info/Elements/u/detailsOfTrackConfiguration.en> ;
    reg:name "detailsOfTrackConfiguration"@en ;
    reg:status <http://metadataregistry.org/uri/RegStatus/1001> ;
    a rdf:Property ;
    rdfs:isDefinedBy <http://rdaregistry.info/Elements/u/> ;
    rdfs:label "has details of track configuration"@en ;
    rdfs:subPropertyOf <http://rdaregistry.info/Elements/u/P60796> ;
    skos:definition "Relates a resource to details of the configuration of the audio track on a sound-track film (e.g., centre track)."@en .

<http://rdaregistry.info/Elements/u/P60800>
    reg:lexicalAlias <http://rdaregistry.info/Elements/u/detailsOfTypeOfRecording.en> ;
    reg:name "detailsOfTypeOfRecording"@en ;
    reg:status <http://metadataregistry.org/uri/RegStatus/1001> ;
    a rdf:Property ;
    rdfs:isDefinedBy <http://rdaregistry.info/Elements/u/> ;
    rdfs:label "has details of type of recording"@en ;
    rdfs:subPropertyOf <http://rdaregistry.info/Elements/u/P60796> ;
    skos:definition "Relates a resource to details of the method used to encode audio content for playback (e.g., analog or digital)."@en .

<http://rdaregistry.info/Elements/u/P60801>
    reg:hasSubproperty <http://rdaregistry.info/Elements/u/P60770>, <http://rdaregistry.info/Elements/u/P60802> ;
    reg:lexicalAlias <http://rdaregistry.info/Elements/u/detailsOfVideoCharacteristic.en> ;
    reg:name "detailsOfVideoCharacteristic"@en ;
    reg:status <http://metadataregistry.org/uri/RegStatus/1001> ;
    a rdf:Property ;
    rdfs:isDefinedBy <http://rdaregistry.info/Elements/u/> ;
    rdfs:label "has details of video characteristic"@en ;
    skos:definition "Relates a resource to details of a technical specification relating to the encoding of video images in a resource."@en .

<http://rdaregistry.info/Elements/u/P60802>
    reg:lexicalAlias <http://rdaregistry.info/Elements/u/detailsOfVideoFormat.en> ;
    reg:name "detailsOfVideoFormat"@en ;
    reg:status <http://metadataregistry.org/uri/RegStatus/1001> ;
    a rdf:Property ;
    rdfs:isDefinedBy <http://rdaregistry.info/Elements/u/> ;
    rdfs:label "has details of video format"@en ;
    rdfs:subPropertyOf <http://rdaregistry.info/Elements/u/P60801> ;
    skos:definition "Relates a resource to details of a standard, etc., used to encode the analog video content of a resource."@en .

<http://rdaregistry.info/Elements/u/P60803>
    reg:hasSubproperty <http://rdaregistry.info/Elements/u/P60778>, <http://rdaregistry.info/Elements/u/P60779>, <http://rdaregistry.info/Elements/u/P60780>, <http://rdaregistry.info/Elements/u/P60781>, <http://rdaregistry.info/Elements/u/P60782> ;
    reg:lexicalAlias <http://rdaregistry.info/Elements/u/detailsOfGeneration.en> ;
    reg:name "detailsOfGeneration"@en ;
    reg:status <http://metadataregistry.org/uri/RegStatus/1001> ;
    a rdf:Property ;
    rdfs:isDefinedBy <http://rdaregistry.info/Elements/u/> ;
    rdfs:label "has details of generation"@en ;
    skos:definition "Relates a resource to details of the relationship between an original carrier and the carrier of a reproduction made from the original (e.g., a first generation camera master, a second generation printing master)."@en .

<http://rdaregistry.info/Elements/u/P60804>
    reg:lexicalAlias <http://rdaregistry.info/Elements/u/detailsOfIllustrativeContent.en> ;
    reg:name "detailsOfIllustrativeContent"@en ;
    reg:status <http://metadataregistry.org/uri/RegStatus/1001> ;
    a rdf:Property ;
    rdfs:isDefinedBy <http://rdaregistry.info/Elements/u/> ;
    rdfs:label "has details of illustrative content"@en ;
    skos:definition "Relates a resource to details of content intended to illustrate the primary content of a resource."@en .

<http://rdaregistry.info/Elements/u/P60805>
    reg:lexicalAlias <http://rdaregistry.info/Elements/u/subject.en> ;
    reg:name "subject"@en ;
    reg:status <http://metadataregistry.org/uri/RegStatus/1001> ;
    a rdf:Property ;
    rdfs:isDefinedBy <http://rdaregistry.info/Elements/u/> ;
    rdfs:label "has subject"@en ;
    owl:inverseOf <http://rdaregistry.info/Elements/u/P60806> ;
    skos:definition "Relates a resource to the subject of a resource; i.e., an indication of what the resource is about."@en .

<http://rdaregistry.info/Elements/u/P60806>
    reg:lexicalAlias <http://rdaregistry.info/Elements/u/subjectOf.en> ;
    reg:name "subjectOf"@en ;
    reg:status <http://metadataregistry.org/uri/RegStatus/1001> ;
    a rdf:Property ;
    rdfs:isDefinedBy <http://rdaregistry.info/Elements/u/> ;
    rdfs:label "is subject of"@en ;
    owl:inverseOf <http://rdaregistry.info/Elements/u/P60805> ;
    skos:definition "Relates a resource to a resource that is about the resource."@en .

<http://rdaregistry.info/Elements/u/P60807>
    reg:lexicalAlias <http://rdaregistry.info/Elements/u/graduate.en> ;
    reg:name "graduate"@en ;
    reg:status <http://metadataregistry.org/uri/RegStatus/1001> ;
    a rdf:Property ;
    rdfs:isDefinedBy <http://rdaregistry.info/Elements/u/> ;
    rdfs:label "has graduate"@en ;
    owl:inverseOf <http://rdaregistry.info/Elements/u/P60808> ;
    skos:definition "Relates an agent to an agent who receives an academic degree from the granting institution or faculty."@en .

<http://rdaregistry.info/Elements/u/P60808>
    reg:lexicalAlias <http://rdaregistry.info/Elements/u/graduateOf.en> ;
    reg:name "graduateOf"@en ;
    reg:status <http://metadataregistry.org/uri/RegStatus/1001> ;
    a rdf:Property ;
    rdfs:isDefinedBy <http://rdaregistry.info/Elements/u/> ;
    rdfs:label "is graduate of"@en ;
    owl:inverseOf <http://rdaregistry.info/Elements/u/P60807> ;
    skos:definition "Relates an agent to an institution or faculty that granted an academic degree to the agent."@en .

<http://rdaregistry.info/Elements/u/P60809>
    reg:lexicalAlias <http://rdaregistry.info/Elements/u/writerOfForeword.en> ;
    reg:name "writerOfForeword"@en ;
    reg:status <http://metadataregistry.org/uri/RegStatus/1001> ;
    a rdf:Property ;
    rdfs:isDefinedBy <http://rdaregistry.info/Elements/u/> ;
    rdfs:label "has writer of foreword"@en ;
    rdfs:subPropertyOf <http://rdaregistry.info/Elements/u/P60398> ;
    owl:inverseOf <http://rdaregistry.info/Elements/u/P60810> ;
    skos:definition "Relates a resource to an agent contributing to a resource by providing a foreword to the original resource."@en .

<http://rdaregistry.info/Elements/u/P60810>
    reg:lexicalAlias <http://rdaregistry.info/Elements/u/writerOfForewordOf.en> ;
    reg:name "writerOfForewordOf"@en ;
    reg:status <http://metadataregistry.org/uri/RegStatus/1001> ;
    a rdf:Property ;
    rdfs:isDefinedBy <http://rdaregistry.info/Elements/u/> ;
    rdfs:label "is writer of foreword of"@en ;
    rdfs:subPropertyOf <http://rdaregistry.info/Elements/u/P60626> ;
    owl:inverseOf <http://rdaregistry.info/Elements/u/P60809> ;
    skos:definition "Relates an agent contributing to a resource by providing a foreword to the original resource to the resource."@en .

<http://rdaregistry.info/Elements/u/P60811>
    reg:lexicalAlias <http://rdaregistry.info/Elements/u/soundDesigner.en> ;
    reg:name "soundDesigner"@en ;
    reg:status <http://metadataregistry.org/uri/RegStatus/1001> ;
    a rdf:Property ;
    rdfs:isDefinedBy <http://rdaregistry.info/Elements/u/> ;
    rdfs:label "has sound designer"@en ;
    rdfs:subPropertyOf <http://rdaregistry.info/Elements/u/P60398> ;
    owl:inverseOf <http://rdaregistry.info/Elements/u/P60812> ;
    skos:definition "Relates a resource to an agent contributing to a resource by designing and creating audio/sound components."@en .

<http://rdaregistry.info/Elements/u/P60812>
    reg:lexicalAlias <http://rdaregistry.info/Elements/u/soundDesignerOf.en> ;
    reg:name "soundDesignerOf"@en ;
    reg:status <http://metadataregistry.org/uri/RegStatus/1001> ;
    a rdf:Property ;
    rdfs:isDefinedBy <http://rdaregistry.info/Elements/u/> ;
    rdfs:label "is sound designer of"@en ;
    rdfs:subPropertyOf <http://rdaregistry.info/Elements/u/P60626> ;
    owl:inverseOf <http://rdaregistry.info/Elements/u/P60811> ;
    skos:definition "Relates an agent contributing to a resource by designing and creating audio/sound components to the resource."@en .

<http://rdaregistry.info/Elements/u/P60813>
    reg:lexicalAlias <http://rdaregistry.info/Elements/u/lightingDesigner.en> ;
    reg:name "lightingDesigner"@en ;
    reg:status <http://metadataregistry.org/uri/RegStatus/1001> ;
    a rdf:Property ;
    rdfs:isDefinedBy <http://rdaregistry.info/Elements/u/> ;
    rdfs:label "has lighting designer"@en ;
    rdfs:subPropertyOf <http://rdaregistry.info/Elements/u/P60398> ;
    owl:inverseOf <http://rdaregistry.info/Elements/u/P60814> ;
    skos:definition "Relates a resource to an agent contributing to a resource by designing and creating lighting components."@en .

<http://rdaregistry.info/Elements/u/P60814>
    reg:lexicalAlias <http://rdaregistry.info/Elements/u/lightingDesignerOf.en> ;
    reg:name "lightingDesignerOf"@en ;
    reg:status <http://metadataregistry.org/uri/RegStatus/1001> ;
    a rdf:Property ;
    rdfs:isDefinedBy <http://rdaregistry.info/Elements/u/> ;
    rdfs:label "is lighting designer of"@en ;
    rdfs:subPropertyOf <http://rdaregistry.info/Elements/u/P60626> ;
    owl:inverseOf <http://rdaregistry.info/Elements/u/P60813> ;
    skos:definition "Relates an agent contributing to a resource by designing and creating lighting components to the resource."@en .

<http://rdaregistry.info/Elements/u/P60815>
    reg:lexicalAlias <http://rdaregistry.info/Elements/u/degreeCommitteeMember.en> ;
    reg:name "degreeCommitteeMember"@en ;
    reg:status <http://metadataregistry.org/uri/RegStatus/1001> ;
    a rdf:Property ;
    rdfs:isDefinedBy <http://rdaregistry.info/Elements/u/> ;
    rdfs:label "has degree committee member"@en ;
    rdfs:subPropertyOf <http://rdaregistry.info/Elements/u/P60374> ;
    owl:inverseOf <http://rdaregistry.info/Elements/u/P60816> ;
    skos:definition "Relates a resource to an agent serving on a committee that supervises a student’s thesis or dissertation."@en .

<http://rdaregistry.info/Elements/u/P60816>
    reg:lexicalAlias <http://rdaregistry.info/Elements/u/degreeCommitteeMemberOf.en> ;
    reg:name "degreeCommitteeMemberOf"@en ;
    reg:status <http://metadataregistry.org/uri/RegStatus/1001> ;
    a rdf:Property ;
    rdfs:isDefinedBy <http://rdaregistry.info/Elements/u/> ;
    rdfs:label "is degree committee member of"@en ;
    rdfs:subPropertyOf <http://rdaregistry.info/Elements/u/P60602> ;
    owl:inverseOf <http://rdaregistry.info/Elements/u/P60815> ;
    skos:definition "Relates an agent serving on a committee that supervises a student’s thesis or dissertation to the resource."@en .

<http://rdaregistry.info/Elements/u/P60817>
    reg:lexicalAlias <http://rdaregistry.info/Elements/u/producerOfAnUnpublishedResourceOf.en> ;
    reg:name "producerOfAnUnpublishedResourceOf"@en ;
    reg:status <http://metadataregistry.org/uri/RegStatus/1001> ;
    a rdf:Property ;
    rdfs:isDefinedBy <http://rdaregistry.info/Elements/u/> ;
    rdfs:label "is producer of an unpublished resource of"@en ;
    skos:definition "Relates an agent responsible for inscribing, fabricating, constructing, etc. to the resource."@en .

<http://rdaregistry.info/Elements/u/P60818>
    reg:lexicalAlias <http://rdaregistry.info/Elements/u/alternativeChronologicalDesignationOfFirstIssueOrPartOfSequence.en> ;
    reg:name "alternativeChronologicalDesignationOfFirstIssueOrPartOfSequence"@en ;
    reg:status <http://metadataregistry.org/uri/RegStatus/1001> ;
    a rdf:Property ;
    rdfs:isDefinedBy <http://rdaregistry.info/Elements/u/> ;
    rdfs:label "has alternative chronological designation of first issue or part of sequence"@en ;
    rdfs:subPropertyOf <http://rdaregistry.info/Elements/u/P60533> ;
    skos:definition "Relates a resource to a second or subsequent system of numbering presented in the form of a date (e.g., a year; year and month; month, day, and year) on the first issue or part of a sequence of numbering for a serial."@en .

<http://rdaregistry.info/Elements/u/P60819>
    reg:lexicalAlias <http://rdaregistry.info/Elements/u/alternativeChronologicalDesignationOfLastIssueOrPartOfSequence.en> ;
    reg:name "alternativeChronologicalDesignationOfLastIssueOrPartOfSequence"@en ;
    reg:status <http://metadataregistry.org/uri/RegStatus/1001> ;
    a rdf:Property ;
    rdfs:isDefinedBy <http://rdaregistry.info/Elements/u/> ;
    rdfs:label "has alternative chronological designation of last issue or part of sequence"@en ;
    rdfs:subPropertyOf <http://rdaregistry.info/Elements/u/P60533> ;
    skos:definition "Relates a resource to a second or subsequent system of numbering presented in the form of a date (e.g., a year; year and month; month, day, and year) on the last issue or part of a sequence of numbering for a serial."@en .

<http://rdaregistry.info/Elements/u/P60820>
    reg:lexicalAlias <http://rdaregistry.info/Elements/u/alternativeNumericAndOrAlphabeticDesignationOfFirstIssueOrPartOfSequence.en> ;
    reg:name "alternativeNumericAndOrAlphabeticDesignationOfFirstIssueOrPartOfSequence"@en ;
    reg:status <http://metadataregistry.org/uri/RegStatus/1001> ;
    a rdf:Property ;
    rdfs:isDefinedBy <http://rdaregistry.info/Elements/u/> ;
    rdfs:label "has alternative numeric and/or alphabetic designation of first issue or part of sequence"@en ;
    rdfs:subPropertyOf <http://rdaregistry.info/Elements/u/P60533> ;
    skos:definition "Relates a resource to a second or subsequent system of numbering presented in numeric and/or alphabetic form on the first issue or part of a sequence of numbering for a serial."@en .

<http://rdaregistry.info/Elements/u/P60821>
    reg:lexicalAlias <http://rdaregistry.info/Elements/u/alternativeNumericAndOrAlphabeticDesignationOfLastIssueOrPartOfSequence.en> ;
    reg:name "alternativeNumericAndOrAlphabeticDesignationOfLastIssueOrPartOfSequence"@en ;
    reg:status <http://metadataregistry.org/uri/RegStatus/1001> ;
    a rdf:Property ;
    rdfs:isDefinedBy <http://rdaregistry.info/Elements/u/> ;
    rdfs:label "has alternative numeric and/or alphabetic designation of last issue or part of sequence"@en ;
    rdfs:subPropertyOf <http://rdaregistry.info/Elements/u/P60533> ;
    skos:definition "Relates a resource to a second or subsequent system of numbering presented in numeric and/or alphabetic form on the last issue or part of a sequence of numbering for a serial."@en .

<http://rdaregistry.info/Elements/u/P60822>
    reg:lexicalAlias <http://rdaregistry.info/Elements/u/scopeOfUsage.en> ;
    reg:name "scopeOfUsage"@en ;
    reg:status <http://metadataregistry.org/uri/RegStatus/1001> ;
    a rdf:Property ;
    rdfs:isDefinedBy <http://rdaregistry.info/Elements/u/> ;
    rdfs:label "has scope of usage"@en ;
    skos:definition "Relates a name to the type or form of resource associated with the name chosen as the preferred name for an agent."@en .

<http://rdaregistry.info/Elements/u/P60823>
    reg:lexicalAlias <http://rdaregistry.info/Elements/u/detailsOfDuration.en> ;
    reg:name "detailsOfDuration"@en ;
    reg:status <http://metadataregistry.org/uri/RegStatus/1001> ;
    a rdf:Property ;
    rdfs:isDefinedBy <http://rdaregistry.info/Elements/u/> ;
    rdfs:label "has details of duration"@en ;
    skos:definition "Relates a resource to details of the playing time, running time, performance time, etc., of the content of a resource."@en .

<http://rdaregistry.info/Elements/u/P60824>
    reg:hasSubproperty <http://rdaregistry.info/Elements/e/P20279> ;
    reg:lexicalAlias <http://rdaregistry.info/Elements/u/onScreenParticipant.en> ;
    reg:name "onScreenParticipant"@en ;
    reg:status <http://metadataregistry.org/uri/RegStatus/1001> ;
    a rdf:Property ;
    rdfs:isDefinedBy <http://rdaregistry.info/Elements/u/> ;
    rdfs:label "has on-screen participant"@en ;
    rdfs:subPropertyOf <http://rdaregistry.info/Elements/u/P60398> ;
    owl:inverseOf <http://rdaregistry.info/Elements/u/P60825> ;
    skos:definition "Relates a resource to an agent contributing to a nonfiction moving image resource by taking an active role as a participant."@en .

<http://rdaregistry.info/Elements/u/P60825>
    reg:hasSubproperty <http://rdaregistry.info/Elements/a/P50261> ;
    reg:lexicalAlias <http://rdaregistry.info/Elements/u/onScreenParticipantOf.en> ;
    reg:name "onScreenParticipantOf"@en ;
    reg:status <http://metadataregistry.org/uri/RegStatus/1001> ;
    a rdf:Property ;
    rdfs:isDefinedBy <http://rdaregistry.info/Elements/u/> ;
    rdfs:label "is on-screen participant of"@en ;
    rdfs:subPropertyOf <http://rdaregistry.info/Elements/u/P60626> ;
    owl:inverseOf <http://rdaregistry.info/Elements/u/P60824> ;
    skos:definition "Relates an agent contributing to a nonfiction moving image resource by taking an active role as a participant to the resource."@en .

<http://rdaregistry.info/Elements/u/P60826>
    reg:lexicalAlias <http://rdaregistry.info/Elements/u/commissioningBody.en> ;
    reg:name "commissioningBody"@en ;
    reg:status <http://metadataregistry.org/uri/RegStatus/1001> ;
    a rdf:Property ;
    rdfs:isDefinedBy <http://rdaregistry.info/Elements/u/> ;
    rdfs:label "has commissioning body"@en ;
    rdfs:subPropertyOf <http://rdaregistry.info/Elements/u/P60447> ;
    owl:inverseOf <http://rdaregistry.info/Elements/u/P60827> ;
    skos:definition "Relates a resource to an agent responsible for commissioning a resource."@en .

<http://rdaregistry.info/Elements/u/P60827>
    reg:hasSubproperty <http://rdaregistry.info/Elements/a/P50262> ;
    reg:lexicalAlias <http://rdaregistry.info/Elements/u/commissioningBodyOf.en> ;
    reg:name "commissioningBodyOf"@en ;
    reg:status <http://metadataregistry.org/uri/RegStatus/1001> ;
    a rdf:Property ;
    rdfs:isDefinedBy <http://rdaregistry.info/Elements/u/> ;
    rdfs:label "is commissioning body of"@en ;
    rdfs:subPropertyOf <http://rdaregistry.info/Elements/u/P60672> ;
    owl:inverseOf <http://rdaregistry.info/Elements/u/P60826> ;
    skos:definition "Relates an agent responsible for commissioning a resource to the resource."@en .

<http://rdaregistry.info/Elements/u/P60828>
    reg:hasSubproperty <http://rdaregistry.info/Elements/e/P20280> ;
    reg:lexicalAlias <http://rdaregistry.info/Elements/u/softwareDeveloper.en> ;
    reg:name "softwareDeveloper"@en ;
    reg:status <http://metadataregistry.org/uri/RegStatus/1001> ;
    a rdf:Property ;
    rdfs:isDefinedBy <http://rdaregistry.info/Elements/u/> ;
    rdfs:label "has software developer"@en ;
    rdfs:subPropertyOf <http://rdaregistry.info/Elements/u/P60398> ;
    owl:inverseOf <http://rdaregistry.info/Elements/u/P60829> ;
    skos:definition "Relates a resource to an agent contributing to a resource by researching, designing, implementing, or testing the software."@en .

<http://rdaregistry.info/Elements/u/P60829>
    reg:hasSubproperty <http://rdaregistry.info/Elements/a/P50263> ;
    reg:lexicalAlias <http://rdaregistry.info/Elements/u/softwareDeveloperOf.en> ;
    reg:name "softwareDeveloperOf"@en ;
    reg:status <http://metadataregistry.org/uri/RegStatus/1001> ;
    a rdf:Property ;
    rdfs:isDefinedBy <http://rdaregistry.info/Elements/u/> ;
    rdfs:label "is software developer of"@en ;
    rdfs:subPropertyOf <http://rdaregistry.info/Elements/u/P60626> ;
    owl:inverseOf <http://rdaregistry.info/Elements/u/P60828> ;
    skos:definition "Relates an agent contributing to a resource by researching, designing, implementing, or testing the software to the resource."@en .

<http://rdaregistry.info/Elements/u/P60830>
    reg:hasSubproperty <http://rdaregistry.info/Elements/e/P20281> ;
    reg:lexicalAlias <http://rdaregistry.info/Elements/u/oratorioAdaptationOf.en> ;
    reg:name "oratorioAdaptationOf"@en ;
    reg:status <http://metadataregistry.org/uri/RegStatus/1001> ;
    a rdf:Property ;
    rdfs:isDefinedBy <http://rdaregistry.info/Elements/u/> ;
    rdfs:label "is oratorio adaptation of"@en ;
    rdfs:subPropertyOf <http://rdaregistry.info/Elements/u/P60305> ;
    owl:inverseOf <http://rdaregistry.info/Elements/u/P60831> ;
    skos:definition "Relates a resource to a resource that has been adapted as an oratorio."@en .

<http://rdaregistry.info/Elements/u/P60831>
    reg:hasSubproperty <http://rdaregistry.info/Elements/e/P20282> ;
    reg:lexicalAlias <http://rdaregistry.info/Elements/u/adaptedAsOratorio.en> ;
    reg:name "adaptedAsOratorio"@en ;
    reg:status <http://metadataregistry.org/uri/RegStatus/1001> ;
    a rdf:Property ;
    rdfs:isDefinedBy <http://rdaregistry.info/Elements/u/> ;
    rdfs:label "is adapted as oratorio"@en ;
    rdfs:subPropertyOf <http://rdaregistry.info/Elements/u/P60250> ;
    owl:inverseOf <http://rdaregistry.info/Elements/u/P60830> ;
    skos:definition "Relates a resource to an oratorio based on the source resource."@en .

<http://rdaregistry.info/Elements/u/P60832>
    reg:lexicalAlias <http://rdaregistry.info/Elements/u/inspiredBy.en> ;
    reg:name "inspiredBy"@en ;
    reg:status <http://metadataregistry.org/uri/RegStatus/1001> ;
    a rdf:Property ;
    rdfs:isDefinedBy <http://rdaregistry.info/Elements/u/> ;
    rdfs:label "is inspired by"@en ;
    rdfs:subPropertyOf <http://rdaregistry.info/Elements/u/P60305> ;
    owl:inverseOf <http://rdaregistry.info/Elements/u/P60833> ;
    skos:definition "Relates a resource to a resource which serves as the inspiration for another resource."@en .

<http://rdaregistry.info/Elements/u/P60833>
    reg:lexicalAlias <http://rdaregistry.info/Elements/u/inspirationFor.en> ;
    reg:name "inspirationFor"@en ;
    reg:status <http://metadataregistry.org/uri/RegStatus/1001> ;
    a rdf:Property ;
    rdfs:isDefinedBy <http://rdaregistry.info/Elements/u/> ;
    rdfs:label "is inspiration for"@en ;
    rdfs:subPropertyOf <http://rdaregistry.info/Elements/u/P60250> ;
    owl:inverseOf <http://rdaregistry.info/Elements/u/P60832> ;
    skos:definition "Relates a resource to a resource which was inspired by another resource."@en .

<http://rdaregistry.info/Elements/u/P60834>
    reg:lexicalAlias <http://rdaregistry.info/Elements/u/participantInATreaty.en> ;
    reg:name "participantInATreaty"@en ;
    reg:status <http://metadataregistry.org/uri/RegStatus/1001> ;
    a rdf:Property ;
    rdfs:isDefinedBy <http://rdaregistry.info/Elements/u/> ;
    rdfs:label "has participant in a treaty"@en ;
    rdfs:subPropertyOf <http://rdaregistry.info/Elements/u/P60374> ;
    owl:inverseOf <http://rdaregistry.info/Elements/u/P60835> ;
    skos:definition "Relates a resource to a government, international intergovernmental body, or other agent that has signed, ratified, or acceded to a treaty."@en .

<http://rdaregistry.info/Elements/u/P60835>
    reg:hasSubproperty <http://rdaregistry.info/Elements/a/P50264> ;
    reg:lexicalAlias <http://rdaregistry.info/Elements/u/participantInATreatyOf.en> ;
    reg:name "participantInATreatyOf"@en ;
    reg:status <http://metadataregistry.org/uri/RegStatus/1001> ;
    a rdf:Property ;
    rdfs:isDefinedBy <http://rdaregistry.info/Elements/u/> ;
    rdfs:label "is participant in a treaty of"@en ;
    rdfs:subPropertyOf <http://rdaregistry.info/Elements/u/P60602> ;
    owl:inverseOf <http://rdaregistry.info/Elements/u/P60834> ;
    skos:definition "Relates a government, international intergovernmental body, or other agent that has signed, ratified, or acceded to a treaty to the resource."@en .

<http://rdaregistry.info/Elements/u/P60836>
    reg:lexicalAlias <http://rdaregistry.info/Elements/u/researcher.en> ;
    reg:name "researcher"@en ;
    reg:status <http://metadataregistry.org/uri/RegStatus/1001> ;
    a rdf:Property ;
    rdfs:isDefinedBy <http://rdaregistry.info/Elements/u/> ;
    rdfs:label "has researcher"@en ;
    rdfs:subPropertyOf <http://rdaregistry.info/Elements/u/P60374> ;
    owl:inverseOf <http://rdaregistry.info/Elements/u/P60837> ;
    skos:definition "Relates a resource to an agent who does research in support of the creation of a resource."@en .

<http://rdaregistry.info/Elements/u/P60837>
    reg:hasSubproperty <http://rdaregistry.info/Elements/a/P50265> ;
    reg:lexicalAlias <http://rdaregistry.info/Elements/u/researchOf.en> ;
    reg:name "researcherOf"@en ;
    reg:status <http://metadataregistry.org/uri/RegStatus/1001> ;
    a rdf:Property ;
    rdfs:isDefinedBy <http://rdaregistry.info/Elements/u/> ;
    rdfs:label "is researcher of"@en ;
    rdfs:subPropertyOf <http://rdaregistry.info/Elements/u/P60602> ;
    owl:inverseOf <http://rdaregistry.info/Elements/u/P60836> ;
    skos:definition "Relates an agent who does research in support of the creation of a resource to the resource."@en .

<http://rdaregistry.info/Elements/u/P60838>
    reg:hasSubproperty <http://rdaregistry.info/Elements/e/P20283> ;
    reg:lexicalAlias <http://rdaregistry.info/Elements/u/colourist.en> ;
    reg:name "colourist"@en ;
    reg:status <http://metadataregistry.org/uri/RegStatus/1001> ;
    a rdf:Property ;
    rdfs:isDefinedBy <http://rdaregistry.info/Elements/u/> ;
    rdfs:label "has colourist"@en ;
    rdfs:subPropertyOf <http://rdaregistry.info/Elements/u/P60398> ;
    owl:inverseOf <http://rdaregistry.info/Elements/u/P60839> ;
    skos:definition "Relates a resource to an agent contributing to a resource by applying colour to drawings, prints, photographs, maps, moving images, etc."@en .

<http://rdaregistry.info/Elements/u/P60839>
    reg:hasSubproperty <http://rdaregistry.info/Elements/a/P50266> ;
    reg:lexicalAlias <http://rdaregistry.info/Elements/u/colouristOf.en> ;
    reg:name "colouristOf"@en ;
    reg:status <http://metadataregistry.org/uri/RegStatus/1001> ;
    a rdf:Property ;
    rdfs:isDefinedBy <http://rdaregistry.info/Elements/u/> ;
    rdfs:label "is colourist of"@en ;
    rdfs:subPropertyOf <http://rdaregistry.info/Elements/u/P60626> ;
    owl:inverseOf <http://rdaregistry.info/Elements/u/P60838> ;
    skos:definition "Relates an agent contributing to a resource by applying colour to drawings, prints, photographs, maps, moving images, etc. to the resource."@en .

<http://rdaregistry.info/Elements/u/P60840>
    reg:hasSubproperty <http://rdaregistry.info/Elements/e/P20284> ;
    reg:lexicalAlias <http://rdaregistry.info/Elements/u/makeUpArtist.en> ;
    reg:name "makeUpArtist"@en ;
    reg:status <http://metadataregistry.org/uri/RegStatus/1001> ;
    a rdf:Property ;
    rdfs:isDefinedBy <http://rdaregistry.info/Elements/u/> ;
    rdfs:label "has make-up artist"@en ;
    rdfs:subPropertyOf <http://rdaregistry.info/Elements/u/P60398> ;
    owl:inverseOf <http://rdaregistry.info/Elements/u/P60841> ;
    skos:definition "Relates a resource to an agent contributing to a resource by applying make-up and prosthetics for a moving image production or for a musical or dramatic presentation or entertainment."@en .

<http://rdaregistry.info/Elements/u/P60841>
    reg:hasSubproperty <http://rdaregistry.info/Elements/a/P50267> ;
    reg:lexicalAlias <http://rdaregistry.info/Elements/u/makeUpArtistOf.en> ;
    reg:name "makeUpArtistOf"@en ;
    reg:status <http://metadataregistry.org/uri/RegStatus/1001> ;
    a rdf:Property ;
    rdfs:isDefinedBy <http://rdaregistry.info/Elements/u/> ;
    rdfs:label "is make-up artist of"@en ;
    rdfs:subPropertyOf <http://rdaregistry.info/Elements/u/P60626> ;
    owl:inverseOf <http://rdaregistry.info/Elements/u/P60840> ;
    skos:definition "Relates an agent contributing to a resource by applying make-up and prosthetics for a moving image production or for a musical or dramatic presentation or entertainment to the resource."@en .

<http://rdaregistry.info/Elements/u/P60842>
    reg:hasSubproperty <http://rdaregistry.info/Elements/e/P20285> ;
    reg:lexicalAlias <http://rdaregistry.info/Elements/u/choralConductor.en> ;
    reg:name "choralConductor"@en ;
    reg:status <http://metadataregistry.org/uri/RegStatus/1001> ;
    a rdf:Property ;
    rdfs:isDefinedBy <http://rdaregistry.info/Elements/u/> ;
    rdfs:label "has choral conductor"@en ;
    rdfs:subPropertyOf <http://rdaregistry.info/Elements/u/P60141> ;
    owl:inverseOf <http://rdaregistry.info/Elements/u/P60843> ;
    skos:definition "Relates a resource to a conductor contributing to a musical resource by leading a choral performing group in a musical or dramatic presentation, etc."@en .

<http://rdaregistry.info/Elements/u/P60843>
    reg:hasSubproperty <http://rdaregistry.info/Elements/a/P50268> ;
    reg:lexicalAlias <http://rdaregistry.info/Elements/u/choralConductorOf.en> ;
    reg:name "choralConductorOf"@en ;
    reg:status <http://metadataregistry.org/uri/RegStatus/1001> ;
    a rdf:Property ;
    rdfs:isDefinedBy <http://rdaregistry.info/Elements/u/> ;
    rdfs:label "is choral conductor of"@en ;
    rdfs:subPropertyOf <http://rdaregistry.info/Elements/u/P60016> ;
    owl:inverseOf <http://rdaregistry.info/Elements/u/P60842> ;
    skos:definition "Relates a conductor contributing to a musical resource by leading a choral performing group in a musical or dramatic presentation, etc. to the resource."@en .

<http://rdaregistry.info/Elements/u/P60844>
    reg:hasSubproperty <http://rdaregistry.info/Elements/e/P20286> ;
    reg:lexicalAlias <http://rdaregistry.info/Elements/u/instrumentalConductor.en> ;
    reg:name "instrumentalConductor"@en ;
    reg:status <http://metadataregistry.org/uri/RegStatus/1001> ;
    a rdf:Property ;
    rdfs:isDefinedBy <http://rdaregistry.info/Elements/u/> ;
    rdfs:label "has instrumental conductor"@en ;
    rdfs:subPropertyOf <http://rdaregistry.info/Elements/u/P60141> ;
    owl:inverseOf <http://rdaregistry.info/Elements/u/P60845> ;
    skos:definition "Relates a resource to a conductor contributing to a musical resource by leading an instrumental performing group in a musical or dramatic presentation, etc."@en .

<http://rdaregistry.info/Elements/u/P60845>
    reg:hasSubproperty <http://rdaregistry.info/Elements/a/P50269> ;
    reg:lexicalAlias <http://rdaregistry.info/Elements/u/instrumentalConductorOf.en> ;
    reg:name "instrumentalConductorOf"@en ;
    reg:status <http://metadataregistry.org/uri/RegStatus/1001> ;
    a rdf:Property ;
    rdfs:isDefinedBy <http://rdaregistry.info/Elements/u/> ;
    rdfs:label "is instrumental conductor of"@en ;
    rdfs:subPropertyOf <http://rdaregistry.info/Elements/u/P60016> ;
    owl:inverseOf <http://rdaregistry.info/Elements/u/P60844> ;
    skos:definition "Relates a conductor contributing to a musical resource by leading an instrumental performing group in a musical or dramatic presentation, etc. to the resource"@en .

<http://rdaregistry.info/Elements/u/P60846>
    reg:lexicalAlias <http://rdaregistry.info/Elements/u/commemoration.en> ;
    reg:name "commemoration"@en ;
    reg:status <http://metadataregistry.org/uri/RegStatus/1001> ;
    a rdf:Property ;
    rdfs:isDefinedBy <http://rdaregistry.info/Elements/u/> ;
    rdfs:label "has commemoration"@en ;
    rdfs:subPropertyOf <http://rdaregistry.info/Elements/u/P60848> ;
    owl:inverseOf <http://rdaregistry.info/Elements/u/P60847> ;
    skos:definition "Relates a resource to a resource created to commemorate the earlier resource."@en .

<http://rdaregistry.info/Elements/u/P60847>
    reg:lexicalAlias <http://rdaregistry.info/Elements/u/commemorationOf.en> ;
    reg:name "commemorationOf"@en ;
    reg:status <http://metadataregistry.org/uri/RegStatus/1001> ;
    a rdf:Property ;
    rdfs:isDefinedBy <http://rdaregistry.info/Elements/u/> ;
    rdfs:label "is commemoration of"@en ;
    rdfs:subPropertyOf <http://rdaregistry.info/Elements/u/P60848> ;
    owl:inverseOf <http://rdaregistry.info/Elements/u/P60846> ;
    skos:definition "Relates a resource to a resource commemorated in the later resource."@en .

<http://rdaregistry.info/Elements/u/P60848>
    reg:hasSubproperty <http://rdaregistry.info/Elements/u/P60846>, <http://rdaregistry.info/Elements/u/P60847> ;
    reg:lexicalAlias <http://rdaregistry.info/Elements/u/referentialResourceRelationship.en> ;
    reg:name "referentialResourceRelationship"@en ;
    reg:status <http://metadataregistry.org/uri/RegStatus/1001> ;
    a rdf:Property ;
    rdfs:isDefinedBy <http://rdaregistry.info/Elements/u/> ;
    rdfs:label "has referential resource relationship with"@en ;
    owl:inverseOf <http://rdaregistry.info/Elements/u/P60848> ;
    skos:definition "Relates a resource to a resource that references the resource."@en .

<http://rdaregistry.info/Elements/u/P60849>
    reg:hasSubproperty <http://rdaregistry.info/Elements/w/P10297> ;
    reg:lexicalAlias <http://rdaregistry.info/Elements/u/organizer.en> ;
    reg:name "organizer"@en ;
    reg:status <http://metadataregistry.org/uri/RegStatus/1001> ;
    a rdf:Property ;
    rdfs:isDefinedBy <http://rdaregistry.info/Elements/u/> ;
    rdfs:label "has organizer"@en ;
    rdfs:subPropertyOf <http://rdaregistry.info/Elements/u/P60374> ;
    owl:inverseOf <http://rdaregistry.info/Elements/u/P60850> ;
    skos:definition "Relates a resource to an agent organizing the exhibit, event, conference, course, program, etc., which gave rise to a resource."@en .

<http://rdaregistry.info/Elements/u/P60850>
    reg:hasSubproperty <http://rdaregistry.info/Elements/a/P50270> ;
    reg:lexicalAlias <http://rdaregistry.info/Elements/u/organizerOf.en> ;
    reg:name "organizerOf"@en ;
    reg:status <http://metadataregistry.org/uri/RegStatus/1001> ;
    a rdf:Property ;
    rdfs:isDefinedBy <http://rdaregistry.info/Elements/u/> ;
    rdfs:label "is organizer of"@en ;
    rdfs:subPropertyOf <http://rdaregistry.info/Elements/u/P60602> ;
    owl:inverseOf <http://rdaregistry.info/Elements/u/P60849> ;
    skos:definition "Relates an agent organizing the exhibit, event, conference, course, program, etc., which gave rise to a resource to the resource."@en .

<http://rdaregistry.info/Elements/u/P60851>
    reg:hasSubproperty <http://rdaregistry.info/Elements/e/P20287> ;
    reg:lexicalAlias <http://rdaregistry.info/Elements/u/censor.en> ;
    reg:name "censor"@en ;
    reg:status <http://metadataregistry.org/uri/RegStatus/1001> ;
    a rdf:Property ;
    rdfs:isDefinedBy <http://rdaregistry.info/Elements/u/> ;
    rdfs:label "has censor"@en ;
    rdfs:subPropertyOf <http://rdaregistry.info/Elements/u/P60398> ;
    owl:inverseOf <http://rdaregistry.info/Elements/u/P60852> ;
    skos:definition "Relates a resource to an agent contributing to a resource by revising the content for the purpose of suppressing parts deemed objectionable on moral, political, military, or other grounds, but leaving the nature and content of the original resource substantially unchanged."@en .

<http://rdaregistry.info/Elements/u/P60852>
    reg:hasSubproperty <http://rdaregistry.info/Elements/a/P50271> ;
    reg:lexicalAlias <http://rdaregistry.info/Elements/u/censorOf.en> ;
    reg:name "censorOf"@en ;
    reg:status <http://metadataregistry.org/uri/RegStatus/1001> ;
    a rdf:Property ;
    rdfs:isDefinedBy <http://rdaregistry.info/Elements/u/> ;
    rdfs:label "is censor of"@en ;
    rdfs:subPropertyOf <http://rdaregistry.info/Elements/u/P60626> ;
    owl:inverseOf <http://rdaregistry.info/Elements/u/P60851> ;
    skos:definition "Relates an agent contributing to a resource by revising the content for the purpose of suppressing parts deemed objectionable on moral, political, military, or other grounds, but leaving the nature and content of the original resource substantially unchanged to the resource."@en .

<http://rdaregistry.info/Elements/u/P60853>
    reg:hasSubproperty <http://rdaregistry.info/Elements/a/P50274>, <http://rdaregistry.info/Elements/u/P60857>, <http://rdaregistry.info/Elements/u/P60858>, <http://rdaregistry.info/Elements/u/P60859>, <http://rdaregistry.info/Elements/u/P60860> ;
    reg:lexicalAlias <http://rdaregistry.info/Elements/u/colleague.en> ;
    reg:name "colleague"@en ;
    reg:status <http://metadataregistry.org/uri/RegStatus/1001> ;
    a rdf:Property ;
    rdfs:isDefinedBy <http://rdaregistry.info/Elements/u/> ;
    rdfs:label "has colleague"@en ;
    rdfs:subPropertyOf <http://rdaregistry.info/Elements/u/P60454> ;
    owl:inverseOf <http://rdaregistry.info/Elements/u/P60853> ;
    skos:definition "Relates an agent to a fellow member of a profession, staff, or academic faculty."@en .

<http://rdaregistry.info/Elements/u/P60854>
    reg:hasSubproperty <http://rdaregistry.info/Elements/a/P50280> ;
    reg:lexicalAlias <http://rdaregistry.info/Elements/u/friend.en> ;
    reg:name "friend"@en ;
    reg:status <http://metadataregistry.org/uri/RegStatus/1001> ;
    a rdf:Property ;
    rdfs:isDefinedBy <http://rdaregistry.info/Elements/u/> ;
    rdfs:label "has friend"@en ;
    rdfs:subPropertyOf <http://rdaregistry.info/Elements/u/P60454> ;
    owl:inverseOf <http://rdaregistry.info/Elements/u/P60854> ;
    skos:definition "Relates an agent to an agent who shares a bond of mutual affection or regard with the other agent."@en .

<http://rdaregistry.info/Elements/u/P60855>
    reg:hasSubproperty <http://rdaregistry.info/Elements/a/P50283> ;
    reg:lexicalAlias <http://rdaregistry.info/Elements/u/enrolledStudent.en> ;
    reg:name "enrolledStudent"@en ;
    reg:status <http://metadataregistry.org/uri/RegStatus/1001> ;
    a rdf:Property ;
    rdfs:isDefinedBy <http://rdaregistry.info/Elements/u/> ;
    rdfs:label "has enrolled student"@en ;
    rdfs:subPropertyOf <http://rdaregistry.info/Elements/u/P60454> ;
    owl:inverseOf <http://rdaregistry.info/Elements/u/P60856> ;
    skos:definition "Relates an agent to an agent who receives instruction at the educational institution."@en .

<http://rdaregistry.info/Elements/u/P60856>
    reg:hasSubproperty <http://rdaregistry.info/Elements/a/P50288> ;
    reg:lexicalAlias <http://rdaregistry.info/Elements/u/studentAt.en> ;
    reg:name "studentAt"@en ;
    reg:status <http://metadataregistry.org/uri/RegStatus/1001> ;
    a rdf:Property ;
    rdfs:isDefinedBy <http://rdaregistry.info/Elements/u/> ;
    rdfs:label "is student at"@en ;
    rdfs:subPropertyOf <http://rdaregistry.info/Elements/u/P60454> ;
    owl:inverseOf <http://rdaregistry.info/Elements/u/P60855> ;
    skos:definition "Relates an agent to an educational institution that provides instruction to the agent."@en .

<http://rdaregistry.info/Elements/u/P60857>
    reg:hasSubproperty <http://rdaregistry.info/Elements/a/P50275> ;
    reg:lexicalAlias <http://rdaregistry.info/Elements/u/assistant.en> ;
    reg:name "assistant"@en ;
    reg:status <http://metadataregistry.org/uri/RegStatus/1001> ;
    a rdf:Property ;
    rdfs:isDefinedBy <http://rdaregistry.info/Elements/u/> ;
    rdfs:label "has assistant"@en ;
    rdfs:subPropertyOf <http://rdaregistry.info/Elements/u/P60853> ;
    owl:inverseOf <http://rdaregistry.info/Elements/u/P60588> ;
    skos:definition "Relates an agent to a colleague who helps the other agent."@en .

<http://rdaregistry.info/Elements/u/P60858>
    reg:hasSubproperty <http://rdaregistry.info/Elements/a/P50276> ;
    reg:lexicalAlias <http://rdaregistry.info/Elements/u/assistantTo.en> ;
    reg:name "assistantTo"@en ;
    reg:status <http://metadataregistry.org/uri/RegStatus/1001> ;
    a rdf:Property ;
    rdfs:isDefinedBy <http://rdaregistry.info/Elements/u/> ;
    rdfs:label "is assistant to"@en ;
    rdfs:subPropertyOf <http://rdaregistry.info/Elements/u/P60853> ;
    owl:inverseOf <http://rdaregistry.info/Elements/u/P60587> ;
    skos:definition "Relates an agent to a colleague who is helped by the other agent."@en .

<http://rdaregistry.info/Elements/u/P60859>
    reg:hasSubproperty <http://rdaregistry.info/Elements/a/P50277> ;
    reg:lexicalAlias <http://rdaregistry.info/Elements/u/coworker.en> ;
    reg:name "coworker"@en ;
    reg:status <http://metadataregistry.org/uri/RegStatus/1001> ;
    a rdf:Property ;
    rdfs:isDefinedBy <http://rdaregistry.info/Elements/u/> ;
    rdfs:label "has co-worker"@en ;
    rdfs:subPropertyOf <http://rdaregistry.info/Elements/u/P60853> ;
    owl:inverseOf <http://rdaregistry.info/Elements/u/P60859> ;
    skos:definition "Relates an agent to a colleague who works with or shares a task with the other agent."@en .

<http://rdaregistry.info/Elements/u/P60860>
    reg:hasSubproperty <http://rdaregistry.info/Elements/a/P50278> ;
    reg:lexicalAlias <http://rdaregistry.info/Elements/u/partner.en> ;
    reg:name "partner"@en ;
    reg:status <http://metadataregistry.org/uri/RegStatus/1001> ;
    a rdf:Property ;
    rdfs:isDefinedBy <http://rdaregistry.info/Elements/u/> ;
    rdfs:label "has partner"@en ;
    rdfs:subPropertyOf <http://rdaregistry.info/Elements/u/P60853> ;
    owl:inverseOf <http://rdaregistry.info/Elements/u/P60860> ;
    skos:definition "Relates an agent to a colleague working with the other agent in an activity of common interest, most often a business partnership."@en .

<http://rdaregistry.info/Elements/u/P60861>
    reg:hasSubproperty <http://rdaregistry.info/Elements/a/P50279> ;
    reg:lexicalAlias <http://rdaregistry.info/Elements/u/fellowStudent.en> ;
    reg:name "fellowStudent"@en ;
    reg:status <http://metadataregistry.org/uri/RegStatus/1001> ;
    a rdf:Property ;
    rdfs:isDefinedBy <http://rdaregistry.info/Elements/u/> ;
    rdfs:label "has fellow student"@en ;
    rdfs:subPropertyOf <http://rdaregistry.info/Elements/u/P60454> ;
    owl:inverseOf <http://rdaregistry.info/Elements/u/P60861> ;
    skos:definition "Relates an agent to an associate of the other student who is also formally engaged in learning."@en .

<http://rdaregistry.info/Elements/u/P60862>
    reg:hasSubproperty <http://rdaregistry.info/Elements/a/P50281> ;
    reg:lexicalAlias <http://rdaregistry.info/Elements/u/student.en> ;
    reg:name "student"@en ;
    reg:status <http://metadataregistry.org/uri/RegStatus/1001> ;
    a rdf:Property ;
    rdfs:isDefinedBy <http://rdaregistry.info/Elements/u/> ;
    rdfs:label "has student"@en ;
    rdfs:subPropertyOf <http://rdaregistry.info/Elements/u/P60454> ;
    owl:inverseOf <http://rdaregistry.info/Elements/u/P60863> ;
    skos:definition "Relates an agent to an agent who receives instruction from the other agent."@en .

<http://rdaregistry.info/Elements/u/P60863>
    reg:hasSubproperty <http://rdaregistry.info/Elements/a/P50282> ;
    reg:lexicalAlias <http://rdaregistry.info/Elements/u/teacher.en> ;
    reg:name "teacher"@en ;
    reg:status <http://metadataregistry.org/uri/RegStatus/1001> ;
    a rdf:Property ;
    rdfs:isDefinedBy <http://rdaregistry.info/Elements/u/> ;
    rdfs:label "has teacher"@en ;
    rdfs:subPropertyOf <http://rdaregistry.info/Elements/u/P60454> ;
    owl:inverseOf <http://rdaregistry.info/Elements/u/P60862> ;
    skos:definition "Relates an agent to an agent who instructs the other agent."@en .

<http://rdaregistry.info/Elements/u/P60864>
    reg:hasSubproperty <http://rdaregistry.info/Elements/a/P50284> ;
    reg:lexicalAlias <http://rdaregistry.info/Elements/u/chiefExecutive.en> ;
    reg:name "chiefExecutive"@en ;
    reg:status <http://metadataregistry.org/uri/RegStatus/1001> ;
    a rdf:Property ;
    rdfs:isDefinedBy <http://rdaregistry.info/Elements/u/> ;
    rdfs:label "has chief executive"@en ;
    rdfs:subPropertyOf <http://rdaregistry.info/Elements/u/P60633> ;
    owl:inverseOf <http://rdaregistry.info/Elements/u/P60865> ;
    skos:definition "Relates an agent to an officer who is the top ranking official of the agent."@en .

<http://rdaregistry.info/Elements/u/P60865>
    reg:hasSubproperty <http://rdaregistry.info/Elements/a/P50286> ;
    reg:lexicalAlias <http://rdaregistry.info/Elements/u/chiefExecutiveOf.en> ;
    reg:name "chiefExecutiveOf"@en ;
    reg:status <http://metadataregistry.org/uri/RegStatus/1001> ;
    a rdf:Property ;
    rdfs:isDefinedBy <http://rdaregistry.info/Elements/u/> ;
    rdfs:label "is chief executive of"@en ;
    rdfs:subPropertyOf <http://rdaregistry.info/Elements/u/P60737> ;
    owl:inverseOf <http://rdaregistry.info/Elements/u/P60864> ;
    skos:definition "Relates an agent to an agent in which the officer is the top ranking official."@en .

<http://rdaregistry.info/Elements/u/P60866>
    reg:hasSubproperty <http://rdaregistry.info/Elements/a/P50285> ;
    reg:lexicalAlias <http://rdaregistry.info/Elements/u/trustee.en> ;
    reg:name "trustee"@en ;
    reg:status <http://metadataregistry.org/uri/RegStatus/1001> ;
    a rdf:Property ;
    rdfs:isDefinedBy <http://rdaregistry.info/Elements/u/> ;
    rdfs:label "has trustee"@en ;
    rdfs:subPropertyOf <http://rdaregistry.info/Elements/u/P60633> ;
    owl:inverseOf <http://rdaregistry.info/Elements/u/P60867> ;
    skos:definition "Relates an agent to an officer granted the powers of administration in the agent in order to act for its benefit."@en .

<http://rdaregistry.info/Elements/u/P60867>
    reg:hasSubproperty <http://rdaregistry.info/Elements/a/P50287> ;
    reg:lexicalAlias <http://rdaregistry.info/Elements/u/trusteeOf.en> ;
    reg:name "trusteeOf"@en ;
    reg:status <http://metadataregistry.org/uri/RegStatus/1001> ;
    a rdf:Property ;
    rdfs:isDefinedBy <http://rdaregistry.info/Elements/u/> ;
    rdfs:label "is trustee of"@en ;
    rdfs:subPropertyOf <http://rdaregistry.info/Elements/u/P60737> ;
    owl:inverseOf <http://rdaregistry.info/Elements/u/P60866> ;
    skos:definition "Relates an agent to an agent that grants the powers of administration to the officer in order to act for its benefit."@en .

<http://rdaregistry.info/Elements/u/P60868>
    reg:lexicalAlias <http://rdaregistry.info/Elements/u/noteOnIdentifierForTheResource.en> ;
    reg:name "noteOnIdentifierForTheResource"@en ;
    reg:status <http://metadataregistry.org/uri/RegStatus/1001> ;
    a rdf:Property ;
    rdfs:isDefinedBy <http://rdaregistry.info/Elements/u/> ;
    rdfs:label "has note on identifier for the resource"@en ;
    rdfs:subPropertyOf <http://rdaregistry.info/Elements/u/P60470> ;
    skos:definition "Relates a resource to a note providing information on identifiers for the resource not recorded as part of the identifier for the resource element."@en .

<http://rdaregistry.info/Elements/u/P60869>
    reg:hasSubproperty <http://rdaregistry.info/Elements/w/P10298> ;
    reg:lexicalAlias <http://rdaregistry.info/Elements/u/editorialDirector.en> ;
    reg:name "editorialDirector"@en ;
    reg:status <http://metadataregistry.org/uri/RegStatus/1001> ;
    a rdf:Property ;
    rdfs:isDefinedBy <http://rdaregistry.info/Elements/u/> ;
    rdfs:label "has editorial director"@en ;
    rdfs:subPropertyOf <http://rdaregistry.info/Elements/u/P60374> ;
    owl:inverseOf <http://rdaregistry.info/Elements/u/P60870> ;
    skos:definition "Relates a resource to an agent having legal and/or intellectual responsibility (other than creation) for the content of a serial, integrating resource, or multipart monographic resource."@en .

<http://rdaregistry.info/Elements/u/P60870>
    reg:lexicalAlias <http://rdaregistry.info/Elements/u/editorialDirectorOf.en> ;
    reg:name "editorialDirectorOf"@en ;
    reg:status <http://metadataregistry.org/uri/RegStatus/1001> ;
    a rdf:Property ;
    rdfs:isDefinedBy <http://rdaregistry.info/Elements/u/> ;
    rdfs:label "is editorial director of"@en ;
    rdfs:subPropertyOf <http://rdaregistry.info/Elements/u/P60602> ;
    owl:inverseOf <http://rdaregistry.info/Elements/u/P60869> ;
    skos:definition "Relates an agent responsible for the legal and/or intellectual responsibility (other than creation) for the content of a serial, integrating resource, or multipart monographic resource to the resource."@en .

<http://rdaregistry.info/Elements/u/P60871>
    reg:hasSubproperty <http://rdaregistry.info/Elements/w/P10299> ;
    reg:lexicalAlias <http://rdaregistry.info/Elements/u/founderOfResource.en> ;
    reg:name "founderOfResource"@en ;
    reg:status <http://metadataregistry.org/uri/RegStatus/1001> ;
    a rdf:Property ;
    rdfs:isDefinedBy <http://rdaregistry.info/Elements/u/> ;
    rdfs:label "has founder of resource"@en ;
    rdfs:subPropertyOf <http://rdaregistry.info/Elements/u/P60374> ;
    owl:inverseOf <http://rdaregistry.info/Elements/u/P60872> ;
    skos:definition "Relates a resource to an agent responsible for establishing a serial, integrating resource, or multipart monographic resource."@en .

<http://rdaregistry.info/Elements/u/P60872>
    reg:lexicalAlias <http://rdaregistry.info/Elements/u/founderOfResourceOf.en> ;
    reg:name "founderOfResourceOf"@en ;
    reg:status <http://metadataregistry.org/uri/RegStatus/1001> ;
    a rdf:Property ;
    rdfs:isDefinedBy <http://rdaregistry.info/Elements/u/> ;
    rdfs:label "is founder of resource of"@en ;
    rdfs:subPropertyOf <http://rdaregistry.info/Elements/u/P60602> ;
    owl:inverseOf <http://rdaregistry.info/Elements/u/P60871> ;
    skos:definition "Relates an agent responsible for establishing a serial, integrating resource, or multipart monograph to the resource."@en .

